@prefix owl:    <http://www.w3.org/2002/07/owl#> .
@prefix rdf:    <http://www.w3.org/1999/02/22-rdf-syntax-ns#> .
@prefix rdfs:   <http://www.w3.org/2000/01/rdf-schema#> .
@prefix xsd:    <http://www.w3.org/2001/XMLSchema#> .
@prefix dct:    <http://purl.org/dc/terms/> .
@prefix skos:   <http://www.w3.org/2004/02/skos/core#> .
@prefix vann:   <http://purl.org/vocab/vann/> .
@prefix void:   <http://rdfs.org/ns/void#> .
@prefix olo:    <http://purl.org/ontology/olo/core#> .
@prefix vs:     <http://www.w3.org/2003/06/sw-vocab-status/ns#> .
@prefix doap:   <http://usefulinc.com/ns/doap#> .
@prefix schema: <http://schema.org/> .
@prefix scor:   <http://purl.org/eis/vocab/scor#> .

scor:
    rdf:type owl:Ontology ;
    rdfs:comment "A vocabulary which represents the Supply Chain Operations Reference (SCOR) standard."@en ;
    rdfs:label "SCORVoc"@en;
    doap:maintainer <http://eis.iai.uni-bonn.de/NiklasPetersen> ;
    dct:creator <http://eis.iai.uni-bonn.de/Irlan>, <http://eis.iai.uni-bonn.de/NiklasPetersen>, <http://sebastian.tramp.name> ;
    dct:publisher <http://dbpedia.org/resource/University_of_Bonn>, <https://ns.eccenca.com/eccenca-GmbH> ;
    dct:license <http://www.opendatacommons.org/licenses/pddl/1.0/> ;
    dct:created "2015-03-01"^^xsd:date ;
    dct:modified "2015-11-05"^^xsd:date ;
  #  owl:imports skos: , dct: ;
    owl:versionInfo "SNAPSHOT" ;
    void:vocabulary
        <http://purl.org/dc/terms/> ,
        <http://www.w3.org/2004/02/skos/core#> ,
        <http://purl.org/vocab/vann/> ,
        <http://rdfs.org/ns/void#> ,
        <http://purl.org/ontology/olo/core#> ,
        <http://www.w3.org/2003/06/sw-vocab-status/ns#> ,
        <http://usefulinc.com/ns/doap#> ,
        <http://schema.org/> ;
    vann:preferredNamespacePrefix "scor" ;
    vann:preferredNamespaceUri "http://purl.org/eis/vocab/scor#" ;
    doap:homepage <https://github.com/vocol/scor> ;
    doap:implements <http://www.apics.org/sites/apics-supply-chain-council/frameworks/scor> ;
    doap:bug-database <https://github.com/vocol/scor/issues> ;
    doap:download-page <https://github.com/vocol/scor/releases> ;
    doap:wiki <https://github.com/vocol/scor/wiki> ;
    doap:repository <https://github.com/vocol/scor.git> ;
    rdfs:isDefinedBy scor: ;
 .

<https://github.com/vocol/scor.git>
    rdf:type doap:GitRepository ;
    rdfs:label "SCORVoc GitHub Repository" ;
.

<http://eis.iai.uni-bonn.de/Irlan>
    rdf:type schema:Person;
    rdfs:label "Irlán Grangel-González";
    schema:affiliation <http://dbpedia.org/resource/University_of_Bonn>;
.

<http://eis.iai.uni-bonn.de/NiklasPetersen>
    rdf:type schema:Person;
    rdfs:label "Niklas Petersen";
    schema:affiliation <http://dbpedia.org/resource/University_of_Bonn>;
.

<http://sebastian.tramp.name>
    rdf:type schema:Person;
    rdfs:label "Sebastian Tramp";
    owl:sameAs <http://aksw.org/SebastianTramp>, <https://ns.eccenca.com/stramp> ;
    schema:affiliation <https://ns.eccenca.com/eccenca-GmbH> ;
.

<http://dbpedia.org/resource/University_of_Bonn>
    rdf:type schema:CollegeOrUniversity;
    rdfs:label "University of Bonn"@en, "Rheinische Friedrich-Wilhelms-Universität Bonn"@de;
.

<https://ns.eccenca.com/eccenca-GmbH>
    rdf:type schema:Corporation;
    rdfs:label "eccenca GmbH";
.

<http://www.opendatacommons.org/licenses/pddl/1.0/>
    rdfs:label "ODC Public Domain Dedication and Licence (PDDL) 1.0"@en ;
.

# Level 0

[]
    rdf:type owl:AllDisjointClasses ;
    owl:members (
        scor:Aptitude scor:Competency scor:Experience scor:Skill
        scor:Training scor:Practice scor:Process
        schema:Person
    ) .

scor:Aptitude
    rdf:type owl:Class ;
    rdfs:comment "A natural, acquired, learned or developed ability to perform a certain kind of work at a"@en  ;
    rdfs:label "Aptitude"@en  ;
    rdfs:isDefinedBy scor: ;
    vs:term_status "stable" ;
    dct:modified "2015-11-05"^^xsd:date ;
 .

scor:Competency
    rdf:type owl:Class ;
    rdfs:comment "Describes the level or state of qualification to perform a certain role or tasks"@en  ;
    rdfs:label "Competency"@en  ;
    rdfs:isDefinedBy scor: ;
    vs:term_status "stable" ;
    dct:modified "2015-11-05"^^xsd:date ;
 .

scor:Experience
    rdf:type owl:Class ;
    rdfs:comment " the knowledge or ability acquired by observation or active participation. "@en  ;
    rdfs:label "Experience"@en  ;
    rdfs:isDefinedBy scor: ;
    vs:term_status "stable" ;
    dct:modified "2015-11-05"^^xsd:date ;
 .

scor:Skill
    rdf:type owl:Class ;
    rdfs:comment "The capacity to deliver pre-determined results with minimal input of time and energy"@en  ;
    rdfs:label "Skill"@en  ;
    rdfs:isDefinedBy scor: ;
    vs:term_status "stable" ;
    dct:modified "2015-11-05"^^xsd:date ;
 .

scor:Training
    rdf:type owl:Class ;
    rdfs:comment "Develops a skill or type of behavior through instruction"@en  ;
    rdfs:label "Training"@en  ;
    rdfs:isDefinedBy scor: ;
    vs:term_status "stable" ;
    dct:modified "2015-11-05"^^xsd:date ;
 .

scor:Practice
    rdf:type owl:Class ;
    rdfs:comment "A practice is a unique way to configure a process or a set of processes"@en ;
    rdfs:label "Practice"@en ;
    rdfs:isDefinedBy scor: ;
    vs:term_status "stable" ;
    dct:modified "2015-11-05"^^xsd:date ;
 .

scor:Process
    rdf:type owl:Class ;
    rdfs:comment "A process is a unique activity performed to meet predefined outcomes"@en ;
    rdfs:label "Process"@en ;
    rdfs:isDefinedBy scor: ;
    vs:term_status "stable" ;
    dct:modified "2015-11-05"^^xsd:date ;
 .

# Level 1 Practice

[]
    rdf:type owl:AllDisjointClasses ;
    owl:members (
        scor:BestPractice scor:EmergingPractice scor:StandardPractice
    ) .

scor:BestPractice
    rdf:type owl:Class ;
    rdfs:comment "Best practices are 'current', 'structured' and 'repeatable' practices that have had a proved and positive impact on supply chain performance"@en ;
    rdfs:label "Best Practice"@en ;
    rdfs:subClassOf scor:Practice ;
    skos:notation "BP.B" ;
    rdfs:isDefinedBy scor: ;
    vs:term_status "stable" ;
    dct:modified "2015-11-05"^^xsd:date ;
 .

scor:EmergingPractice
    rdf:type owl:Class ;
    rdfs:comment "Introduce new technology, knowledge or radically different ways of organizing processes"@en ;
    rdfs:label "Emerging Practice"@en ;
    rdfs:subClassOf scor:Practice ;
    skos:notation "BP.E" ;
    rdfs:isDefinedBy scor: ;
    vs:term_status "stable" ;
    dct:modified "2015-11-05"^^xsd:date ;
 .

scor:StandardPractice
    rdf:type owl:Class ;
    rdfs:comment "How a wide range of companies have historically done business by default or happenstance"@en ;
    rdfs:label "Standard Practice"@en ;
    rdfs:subClassOf scor:Practice ;
    skos:notation "BP.S" ;
    rdfs:isDefinedBy scor: ;
    vs:term_status "stable" ;
    dct:modified "2015-11-05"^^xsd:date ;
 .

# Level 1 Processes

[]
    rdf:type owl:AllDisjointClasses ;
    owl:members (
        scor:Plan scor:Source scor:Make scor:Deliver scor:Return scor:Enable
    ) .

scor:Plan
    rdf:type owl:Class ;
    rdfs:subClassOf scor:Process ;
    rdfs:comment "Describes the planning activities associated with operating a supply chain. This includes gathering customer requirements, collecting information on available resources, and balancing requirements and resources to determine planned capabilities and resource gaps. This is followed by identifying the actions required to correct any gaps."@en ;
    rdfs:label "Plan"@en ;
    rdfs:subClassOf scor:Process ;
    skos:notation "sP" ;
    rdfs:isDefinedBy scor: ;
    vs:term_status "stable" ;
    dct:modified "2015-11-05"^^xsd:date ;
 .

scor:Source
    rdf:type owl:Class ;
    rdfs:subClassOf scor:Process ;
    rdfs:comment "Order, deliver, receipt and transfer of raw material items, subassemblies, product and/or services"@en ;
    rdfs:label "Source"@en ;
    rdfs:subClassOf scor:Process ;
    skos:notation "sS" ;
    rdfs:isDefinedBy scor: ;
    vs:term_status "stable" ;
    dct:modified "2015-11-05"^^xsd:date ;
 .

scor:Make
    rdf:type owl:Class ;
    rdfs:subClassOf scor:Process ;
    rdfs:comment "Adds value to products through mixing, separating, forming, machining, and chemical processes"@en ;
    rdfs:label "Make"@en ;
    rdfs:subClassOf scor:Process ;
    skos:notation "sM" ;
    rdfs:isDefinedBy scor: ;
    vs:term_status "stable" ;
    dct:modified "2015-11-05"^^xsd:date ;
 .

scor:Deliver
    rdf:type owl:Class ;
    rdfs:subClassOf scor:Process ;
    rdfs:comment "Performs customer-facing order management and order fulfillment activities"@en ;
    rdfs:label "Deliver"@en ;
    rdfs:subClassOf scor:Process ;
    skos:notation "sD" ;
    rdfs:isDefinedBy scor: ;
    vs:term_status "stable" ;
    dct:modified "2015-11-05"^^xsd:date ;
 .

scor:Return
    rdf:type owl:Class ;
    rdfs:subClassOf scor:Process ;
    rdfs:comment "Moves material from a customer back through the supply chain to address defects in product, ordering, or manufacturing, or to perform upkeep activities"@en ;
    rdfs:label "Return"@en ;
    rdfs:subClassOf scor:Process ;
    skos:notation "sR" ;
    rdfs:isDefinedBy scor: ;
    vs:term_status "stable" ;
    dct:modified "2015-11-05"^^xsd:date ;
 .

scor:Enable
    rdf:type owl:Class ;
    rdfs:subClassOf scor:Process ;
    rdfs:comment "Establishing, maintaining and monitoring information, relationships, resources, assets, business rules, compliance and contracts required to operate the supply chain"@en ;
    rdfs:label "Enable"@en ;
    rdfs:subClassOf scor:Process ;
    skos:notation "sE" ;
    rdfs:isDefinedBy scor: ;
    vs:term_status "stable" ;
    dct:modified "2015-11-05"^^xsd:date ;
 .

# Level 2 Processes

# Plan

[]
    rdf:type owl:AllDisjointClasses ;
    owl:members (
        scor:PlanSupplyChain scor:PlanSource scor:PlanMake scor:PlanDeliver scor:PlanReturn
    ) .

scor:PlanSupplyChain
    rdf:type owl:Class ;
    rdfs:subClassOf scor:Plan ;
    rdfs:comment "The development and establishment of courses of action over specified time periods that represent a projected appropriation of supply chain resources to meet supply chain requirements for the longest time fence constraints of supply resources"@en ;
    rdfs:label "Plan Supply Chain"@en ;
    rdfs:subClassOf scor:Plan ;
    skos:notation "sP1" ;
    scor:hasDefaultSteps scor:PlanSupplyChainStepList;
    rdfs:isDefinedBy scor: ;
    vs:term_status "stable" ;
    dct:modified "2015-11-05"^^xsd:date ;
 .

scor:PlanSource
    rdf:type owl:Class ;
    rdfs:subClassOf scor:Plan ;
    rdfs:comment "The development and establishment of courses of action over specified time periods that represent a projected appropriation of material resources to meet supply chain requirements"@en ;
    rdfs:label "Plan Source"@en ;
    rdfs:subClassOf scor:Plan ;
    skos:notation "sP2" ;
    scor:hasDefaultSteps scor:PlanSourceStepList;
    rdfs:isDefinedBy scor: ;
    vs:term_status "stable" ;
    dct:modified "2015-11-05"^^xsd:date ;
 .

scor:PlanMake
    rdf:type owl:Class ;
    rdfs:subClassOf scor:Plan ;
    rdfs:comment "The development and establishment of courses of action over specified time periods that represent a projected appropriation of production resources to meet production requirements"@en ;
    rdfs:label "Plan Make"@en ;
    rdfs:subClassOf scor:Plan ;
    scor:hasDefaultSteps scor:PlanMakeStepList;
    skos:notation "sP3" ;
    rdfs:isDefinedBy scor: ;
    vs:term_status "stable" ;
    dct:modified "2015-11-05"^^xsd:date ;
 .

scor:PlanDeliver
    rdf:type owl:Class ;
    rdfs:subClassOf scor:Plan ;
    rdfs:comment "The development and establishment of courses of action over specified time periods that represent a projected appropriation of delivery resources to meet delivery requirements"@en ;
    rdfs:label "Plan Deliver"@en ;
    rdfs:subClassOf scor:Plan ;
    skos:notation "sP4" ;
    scor:hasDefaultSteps scor:PlanDeliverStepList;
    rdfs:isDefinedBy scor: ;
    vs:term_status "stable" ;
    dct:modified "2015-11-05"^^xsd:date ;
 .

scor:PlanReturn
    rdf:type owl:Class ;
    rdfs:subClassOf scor:Plan ;
    rdfs:comment "establish and adjust courses of action or tasks over specified time periods that represent a projected appropriation of return resources and assets to meet anticipated as well as unanticipated return requirements"@en ;
    rdfs:label "Plan Return"@en ;
    rdfs:subClassOf scor:Plan ;
    skos:notation "sP5" ;
    scor:hasDefaultSteps scor:PlanReturnStepList;
    rdfs:isDefinedBy scor: ;
    vs:term_status "stable" ;
    dct:modified "2015-11-05"^^xsd:date ;
 .

# Source

[]
    rdf:type owl:AllDisjointClasses ;
    owl:members (
        scor:SourceStockedProduct scor:SourceMakeToOrderProduct scor:SourceEngineerToOrderProduct
    ) .

scor:SourceStockedProduct
    rdf:type owl:Class ;
    rdfs:subClassOf scor:Source ;
    rdfs:comment "The process of ordering, receiving and transferring raw material items, sub-assemblies, product and or services based on aggregated demand requirements."@en;
    rdfs:label "Source Stocked Product"@en ;
    skos:notation "sS1" ;
    scor:hasDefaultSteps scor:SourceStockedProductStepList;
    rdfs:isDefinedBy scor: ;
    vs:term_status "stable" ;
    dct:modified "2015-11-05"^^xsd:date ;
 .

scor:SourceMakeToOrderProduct
    rdf:type owl:Class ;
    rdfs:subClassOf scor:Source ;
    rdfs:comment "The processes of ordering and receiving product or material that is ordered (and may be configured) only when required by a specific customer order."@en ;
    rdfs:label "Source Make-to-Order Product"@en ;
    skos:notation "sS2" ;
    scor:hasDefaultSteps scor:SourceMakeToOrderProductStepList;
    rdfs:isDefinedBy scor: ;
    vs:term_status "stable" ;
    dct:modified "2015-11-05"^^xsd:date ;
 .

scor:SourceEngineerToOrderProduct
    rdf:type owl:Class ;
    rdfs:subClassOf scor:Source ;
    rdfs:comment "The processes of identifying and selecting sources of supply, negotiating, validating, scheduling, ordering and receiving parts, assemblies or specialized products or services that are designed, ordered and/or built based on the requirements or specifications of a specific customer order."@en ;
    rdfs:label "Source Engineer-to-Order Product"@en ;
    skos:notation "sS3" ;
    scor:hasDefaultSteps scor:SourceEngineerToOrderProductStepList;
    rdfs:isDefinedBy scor: ;
    vs:term_status "stable" ;
    dct:modified "2015-11-05"^^xsd:date ;
 .

# Make

[]
    rdf:type owl:AllDisjointClasses ;
    owl:members (
        scor:MakeToStock scor:MakeToOrder scor:MakeEngineerToOrder
    ) .

scor:MakeToStock
    rdf:type owl:Class ;
    rdfs:subClassOf scor:Make ;
    rdfs:comment "The process of manufacturing in a make-to-stock environment adds value to products through mixing, separating, forming, machining, and chemical processes."@en ;
    rdfs:label "Make-to-Stock"@en ;
    skos:notation "sM1" ;
    scor:hasDefaultSteps scor:MakeToStockStepList;
    rdfs:isDefinedBy scor: ;
    vs:term_status "stable" ;
    dct:modified "2015-11-05"^^xsd:date ;
 .

scor:MakeToOrder
    rdf:type owl:Class ;
    rdfs:subClassOf scor:Make ;
    rdfs:comment "The process of manufacturing in a make-to-order environment adds value to products through mixing, separating, forming, machining, and chemical processes for a specific customer order."@en ;
    rdfs:label "Make-to-Order"@en ;
    skos:notation "sM2" ;
    scor:hasDefaultSteps scor:MakeToOrderStepList;
    rdfs:isDefinedBy scor: ;
    vs:term_status "stable" ;
    dct:modified "2015-11-05"^^xsd:date ;
 .

scor:MakeEngineerToOrder
    rdf:type owl:Class ;
    rdfs:subClassOf scor:Make ;
    rdfs:comment "The process of developing, designing, validating, and ultimately using a manufacturing process to produce products or services based on the requirements of a specific customer."@en;
    rdfs:label "Engineer-to-Order"@en ;
    scor:hasDefaultSteps scor:EngineerToOrderStepList;
    skos:notation "sM3" ;
    rdfs:isDefinedBy scor: ;
    vs:term_status "stable" ;
    dct:modified "2015-11-05"^^xsd:date ;
 .

# Deliver

[]
    rdf:type owl:AllDisjointClasses ;
    owl:members (
        scor:DeliverStockedProduct scor:DeliverMakeToOrderProduct
        scor:DeliverEngineerToOrderProduct scor:DeliverRetailProduct
    ) .

scor:DeliverStockedProduct
    rdf:type owl:Class ;
    rdfs:subClassOf scor:Deliver ;
    rdfs:comment "Delivers product that is sourced or made based on aggregated customer orders, projected orders/demand and inventory re-ordering parameters"@en ;
    rdfs:label "Deliver Stocked Product"@en ;
    skos:notation "sD1" ;
    scor:hasDefaultSteps scor:DeliverStockedProductStepList;
    rdfs:isDefinedBy scor: ;
    vs:term_status "stable" ;
    dct:modified "2015-11-05"^^xsd:date ;
 .

scor:DeliverMakeToOrderProduct
    rdf:type owl:Class ;
    rdfs:subClassOf scor:Deliver ;
    rdfs:comment "Delivers product that is sourced, configured, manufactured, and/or assembled from standard raw materials, parts, ingredients or sub-assemblies, in response to a specific firm customer order"@en ;
    rdfs:label "Deliver Make-to-Order Product"@en ;
    skos:notation "sD2" ;
    scor:hasDefaultSteps scor:DeliverMakeToOrderProductStepList;
    rdfs:isDefinedBy scor: ;
    vs:term_status "stable" ;
    dct:modified "2015-11-05"^^xsd:date ;
 .

scor:DeliverEngineerToOrderProduct
    rdf:type owl:Class ;
    rdfs:subClassOf scor:Deliver ;
    rdfs:comment "Obtaining, responding to, and allocating resources for a customer order that has unique requirements or specifications and delivering a product that is partially or fully designed, redesigned, manufactured, and/or assembled from a bill of materials or recipe that includes one or more custom parts or ingredients"@en ;
    rdfs:label "Deliver Engineer-to-Order Product"@en ;
    skos:notation "sD3" ;
    scor:hasDefaultSteps scor:DeliverEngineerToProductStepList;
    rdfs:isDefinedBy scor: ;
    vs:term_status "stable" ;
    dct:modified "2015-11-05"^^xsd:date ;
 .

scor:DeliverRetailProduct
    rdf:type owl:Class ;
    rdfs:subClassOf scor:Deliver ;
    rdfs:comment "To acquire, merchandise, and sell finished goods at a retail store"@en ;
    rdfs:label "Deliver Retail Product"@en ;
    skos:notation "sD4" ;
    scor:hasDefaultSteps scor:DeliverRetailProductStepList;
    rdfs:isDefinedBy scor: ;
    vs:term_status "stable" ;
    dct:modified "2015-11-05"^^xsd:date ;
 .

# Return

[]
    rdf:type owl:AllDisjointClasses ;
    owl:members (
        scor:DeliverReturnDefectiveProduct scor:DeliverReturnMROProduct
        scor:DeliverReturnExcessProduct scor:SourceReturnMROProduct
        scor:SourceReturnDefectiveProduct scor:SourceReturnExcessProduct
    ) .

scor:DeliverReturnDefectiveProduct
    rdf:type owl:Class ;
    rdfs:subClassOf scor:Return ;
    rdfs:comment "The receipt and disposition determination of defective products as defined by the warranty claims, product recall, non-conforming product and/or other similar policies including appropriate replacement"@en ;
    rdfs:label "Deliver Return Defective Product"@en ;
    skos:notation "sDR1" ;
    scor:hasDefaultSteps scor:DeliverReturnDefectiveProduct;
    rdfs:isDefinedBy scor: ;
    vs:term_status "stable" ;
    dct:modified "2015-11-05"^^xsd:date ;
 .

scor:DeliverReturnMROProduct
    rdf:type owl:Class ;
    rdfs:subClassOf scor:Return ;
    rdfs:comment "The receipt of Maintenance, Repair and Overhaul (MRO) products or company assets for the purpose of servicing, repairing or upgrading it, as defined by Maintenance Plans or the occurrence or anticipation of risk of failure"@en ;
    rdfs:label "Deliver Return MRO Product"@en ;
    scor:hasDefaultSteps scor:DRMROProductStepList;
    skos:notation "sDR2" ;
    rdfs:isDefinedBy scor: ;
    vs:term_status "stable" ;
    dct:modified "2015-11-05"^^xsd:date ;
 .

scor:DeliverReturnExcessProduct
    rdf:type owl:Class ;
    rdfs:subClassOf scor:Return ;
    rdfs:comment "The receipt of excess or aging inventory or obsolete products as defined by the terms and conditions of a customer/supplier contract"@en ;
    rdfs:label "Deliver Return Excess Product"@en ;
    skos:notation "sDR3" ;
    scor:hasDefaultSteps scor:DRExcessProductStepList;
    rdfs:isDefinedBy scor: ;
    vs:term_status "stable" ;
    dct:modified "2015-11-05"^^xsd:date ;
 .

scor:SourceReturnMROProduct
    rdf:type owl:Class ;
    rdfs:subClassOf scor:Return ;
    rdfs:comment "The return of Maintenance, Repair and Overhaul (MRO) products or company assets for the purpose of servicing, repairing or upgrading it, as defined by Maintenance Plans or the occurrence or anticipation of risk of failure"@en ;
    rdfs:label "Source Return MRO Product"@en ;
    skos:notation "sSR2" ;
    scor:hasDefaultSteps scor:SRMROProductStepList;
    rdfs:isDefinedBy scor: ;
    vs:term_status "stable" ;
    dct:modified "2015-11-05"^^xsd:date ;
 .

scor:SourceReturnDefectiveProduct
    rdf:type owl:Class ;
    rdfs:subClassOf scor:Return ;
    rdfs:comment "The return and disposition determination of defective products as defined by the warranty claims, product recall, non-conforming product and/or other similar policies including appropriate replacement"@en ;
    rdfs:label "Source Return Defective Product"@en ;
    skos:notation "sSR1" ;
    scor:hasDefaultSteps scor:SRDefectiveProductStepList;
    rdfs:isDefinedBy scor: ;
    vs:term_status "stable" ;
    dct:modified "2015-11-05"^^xsd:date ;
 .

scor:SourceReturnExcessProduct
    rdf:type owl:Class ;
    rdfs:subClassOf scor:Return ;
    rdfs:comment "The return of excess or aging inventory or obsolete products as defined by the terms and conditions of a customer/supplier contract"@en ;
    rdfs:label "Source Return Excess Product"@en ;
    skos:notation "sSR3" ;
    scor:hasDefaultSteps scor:SRExcessProductStepList;
    rdfs:isDefinedBy scor: ;
    vs:term_status "stable" ;
    dct:modified "2015-11-05"^^xsd:date ;
 .

# Enable

[]
    rdf:type owl:AllDisjointClasses ;
    owl:members (
        scor:ManagePerformance scor:ManageSupplyChainBusinessRules
        scor:ManageDataAndInformation scor:ManageSupplyChainHumanResources
        scor:ManageSupplyChainAssets scor:ManageSupplyChainContracts
        scor:ManageSupplyChainNetworks scor:ManageRegulatoryCompliance
        scor:ManageSupplyChainRisk
    ) .

scor:ManageSupplyChainBusinessRules
    rdf:type owl:Class ;
    rdfs:subClassOf scor:Enable ;
    rdfs:comment "Establishing, documenting, communicating and publishing supply chain business rules"@en ;
    rdfs:label "Manage Supply Chain Business Rules"@en ;
    skos:notation "sE1" ;
    scor:hasDefaultSteps scor:ManageSCBusinessRulesStepList;
    rdfs:isDefinedBy scor: ;
    vs:term_status "stable" ;
    dct:modified "2015-11-05"^^xsd:date ;
 .

scor:ManagePerformance
    rdf:type owl:Class ;
    rdfs:subClassOf scor:Enable ;
    rdfs:comment "Reporting performance, identifying gaps in performance, performing root cause analysis, and developing and launching corrective actions to close gaps in performance"@en ;
    rdfs:label "Manage Performance"@en ;
    skos:notation "sE2" ;
    scor:hasDefaultSteps scor:ManageSCPerformanceStepList;
    rdfs:isDefinedBy scor: ;
    vs:term_status "stable" ;
    dct:modified "2015-11-05"^^xsd:date ;
 .

scor:ManageDataAndInformation
    rdf:type owl:Class ;
    rdfs:subClassOf scor:Enable ;
    rdfs:comment "Collecting, maintaining and publishing data and information required to plan, operate, measure and manage the supply chain"@en ;
    rdfs:label "Manage Data and Information"@en ;
    skos:notation "sE3" ;
    scor:hasDefaultSteps scor:ManageSCDataAndInformationStepList;
    rdfs:isDefinedBy scor: ;
    vs:term_status "stable" ;
    dct:modified "2015-11-05"^^xsd:date ;
 .

scor:ManageSupplyChainHumanResources
    rdf:type owl:Class ;
    rdfs:subClassOf scor:Enable ;
    rdfs:comment "Developing, governing and maintaining an organization of permanent, temporary and outsourced staff, with the right qualifications, in support of the business objects and supply chain goals"@en ;
    rdfs:label "Manage Supply Chain Human Resources"@en ;
    skos:notation "sE4" ;
    scor:hasDefaultSteps scor:ManageSupplyChainHumanResources;
    rdfs:isDefinedBy scor: ;
    vs:term_status "stable" ;
    dct:modified "2015-11-05"^^xsd:date ;
 .

scor:ManageSupplyChainAssets
    rdf:type owl:Class ;
    rdfs:subClassOf scor:Enable ;
    rdfs:comment "Scheduling, maintaining and dispositioning of supply chain assets that operate supply chain processes"@en ;
    rdfs:label "Manage Supply Chain Assets"@en ;
    skos:notation "sE5" ;
    scor:hasDefaultSteps scor:ManageSCAssetsStepList;
    rdfs:isDefinedBy scor: ;
    vs:term_status "stable" ;
    dct:modified "2015-11-05"^^xsd:date ;
 .

scor:ManageSupplyChainContracts
    rdf:type owl:Class ;
    rdfs:subClassOf scor:Enable ;
    rdfs:comment "The management and communication of contractual agreements in support of business objectives and supply chain goals"@en ;
    rdfs:label "Manage Supply Chain Contracts"@en ;
    skos:notation "sE6" ;
    scor:hasDefaultSteps scor:ManageSCContractsStepList;
    rdfs:isDefinedBy scor: ;
    vs:term_status "stable" ;
    dct:modified "2015-11-05"^^xsd:date ;
 .

scor:ManageSupplyChainNetworks
    rdf:type owl:Class ;
    rdfs:subClassOf scor:Enable ;
    rdfs:comment "Developing, governing and maintaining a network of supply chain assets"@en ;
    rdfs:label "Manage Supply Chain Networks"@en ;
    skos:notation "sE7" ;
    scor:hasDefaultSteps scor:ManageSCNetworkStepList;
    rdfs:isDefinedBy scor: ;
    vs:term_status "stable" ;
    dct:modified "2015-11-05"^^xsd:date ;
 .

scor:ManageRegulatoryCompliance
    rdf:type owl:Class ;
    rdfs:subClassOf scor:Enable ;
    rdfs:comment "Identifying, collecting, assessing and integrating regulatory compliance requirements in standard supply chain processes, policies and business rules"@en ;
    rdfs:label "Manage Regulatory Compliance"@en ;
    skos:notation "sE8" ;
    scor:hasDefaultSteps scor:ManageSCRegulatoryComplianceStepList;
    rdfs:isDefinedBy scor: ;
    vs:term_status "stable" ;
    dct:modified "2015-11-05"^^xsd:date ;
 .

scor:ManageSupplyChainRisk
    rdf:type owl:Class ;
    rdfs:subClassOf scor:Enable ;
    rdfs:comment "Identification and assessment of potential disruptions (risks) in the supply chain and developing a plan to mitigate these threats to operating the supply chain"@en ;
    rdfs:label "Manage Supply Chain Risk"@en ;
    skos:notation "sE9" ;
    scor:hasDefaultSteps scor:ManageSCRiskStepList;
    rdfs:isDefinedBy scor: ;
    vs:term_status "stable" ;
    dct:modified "2015-11-05"^^xsd:date ;
 .

# Step definition

scor:Step
    rdf:type owl:Class ;
    rdfs:comment "Steps are all level 3 processe to be executed to accomplish a level 2 process."@en ;
    rdfs:label "Step"@en ;
    rdfs:isDefinedBy scor: ;
    vs:term_status "stable" ;
    dct:modified "2015-11-05"^^xsd:date ;
 .

scor:PlanStep
    rdf:type owl:Class ;
    rdfs:subClassOf scor:Step ;
    rdfs:comment "Plan Steps ."@en ;
    rdfs:label "Plan Step"@en ;
    rdfs:isDefinedBy scor: ;
    vs:term_status "stable" ;
    dct:modified "2015-11-05"^^xsd:date ;
 .

scor:SourceReturnStep
    rdf:type owl:Class ;
    rdfs:subClassOf scor:Step ;
    rdfs:comment "Source Return Steps to be exectued for a Source Return level 2 process."@en ;
    rdfs:label "Source Return Step"@en ;
    rdfs:isDefinedBy scor: ;
    vs:term_status "stable" ;
    dct:modified "2015-11-05"^^xsd:date ;
 .

scor:SourceStep
    rdf:type owl:Class ;
    rdfs:subClassOf scor:Step ;
    rdfs:comment "Source Steps to be exectued for a Source level 2 process."@en ;
    rdfs:label "Source Step"@en ;
    rdfs:isDefinedBy scor: ;
    vs:term_status "stable" ;
    dct:modified "2015-11-05"^^xsd:date ;
 .

scor:MakeStep
    rdf:type owl:Class ;
    rdfs:subClassOf scor:Step ;
    rdfs:comment "Make Steps to be exectued for a Make level 2 process."@en ;
    rdfs:label "Make Step"@en ;
    rdfs:isDefinedBy scor: ;
    vs:term_status "stable" ;
    dct:modified "2015-11-05"^^xsd:date ;
 .

scor:EnableStep
    rdf:type owl:Class ;
    rdfs:subClassOf scor:Step ;
    rdfs:comment "Enable Steps to be exectued for a Enable level 2 process."@en ;
    rdfs:label "Enable Step"@en ;
    rdfs:isDefinedBy scor: ;
    vs:term_status "stable" ;
    dct:modified "2015-11-05"^^xsd:date ;
 .

scor:DeliverStep
    rdf:type owl:Class ;
    rdfs:subClassOf scor:Step ;
    rdfs:comment "Deliver Steps to be exectued for a Deliver level 2 process."@en ;
    rdfs:label "Deliver Step"@en ;
    rdfs:isDefinedBy scor: ;
    vs:term_status "stable" ;
    dct:modified "2015-11-05"^^xsd:date ;
 .

 ################################

 scor:PlanSupplyChainStep
    rdf:type owl:Class ;
    rdfs:subClassOf scor:PlanStep ;
    rdfs:comment "Steps to be exectued for a Plan Supply Chain process."@en ;
    rdfs:label "Plan Supply Chain Step"@en ;
    rdfs:isDefinedBy scor: ;
    vs:term_status "stable" ;
    dct:modified "2015-11-05"^^xsd:date ;
 .

 scor:PlanSourceStep
    rdf:type owl:Class ;
    rdfs:subClassOf scor:PlanStep ;
    rdfs:comment "Steps to be exectued for a Plan Source process."@en ;
    rdfs:label "Plan Source Step"@en ;
    rdfs:isDefinedBy scor: ;
    vs:term_status "stable" ;
    dct:modified "2015-11-05"^^xsd:date ;
 .

  scor:PlanMakeStep
    rdf:type owl:Class ;
    rdfs:subClassOf scor:PlanStep ;
    rdfs:comment "Steps to be exectued for a Plan Make process."@en ;
    rdfs:label "Plan Make Step"@en ;
    rdfs:isDefinedBy scor: ;
    vs:term_status "stable" ;
    dct:modified "2015-11-05"^^xsd:date ;
 .

  scor:PlanDeliverStep
    rdf:type owl:Class ;
    rdfs:subClassOf scor:PlanStep ;
    rdfs:comment "Steps to be exectued for a Plan Deliver process."@en ;
    rdfs:label "Plan Deliver Step"@en ;
    rdfs:isDefinedBy scor: ;
    vs:term_status "stable" ;
    dct:modified "2015-11-05"^^xsd:date ;
 .
  scor:PlanReturnStep
    rdf:type owl:Class ;
    rdfs:subClassOf scor:PlanStep ;
    rdfs:comment "Steps to be exectued for a Plan Return process."@en ;
    rdfs:label "Plan Return Step"@en ;
    rdfs:isDefinedBy scor: ;
    vs:term_status "stable" ;
    dct:modified "2015-11-05"^^xsd:date ;
 .

 ################################

scor:SourceReturnDefectiveProductStep
    rdf:type owl:Class ;
    rdfs:subClassOf scor:SourceReturnStep ;
    rdfs:comment "Steps to be exectued for a Source Return Defective Product process."@en ;
    rdfs:label "Source Return Defective Product Step"@en ;
    rdfs:isDefinedBy scor: ;
    vs:term_status "stable" ;
    dct:modified "2015-11-05"^^xsd:date ;
 .


scor:SourceReturnMROProductStep
    rdf:type owl:Class ;
    rdfs:subClassOf scor:SourceReturnStep ;
    rdfs:comment "Steps to be exectued for a Source Return MRO Product process."@en ;
    rdfs:label "Source Return MRO Product Step"@en ;
    rdfs:isDefinedBy scor: ;
    vs:term_status "stable" ;
    dct:modified "2015-11-05"^^xsd:date ;
 .

scor:SourceReturnExcessProductStep
    rdf:type owl:Class ;
    rdfs:subClassOf scor:SourceReturnStep ;
    rdfs:comment "Steps to be exectued for a Source Return MRO Product process."@en ;
    rdfs:label "Source Return MRO Product Step"@en ;
    rdfs:isDefinedBy scor: ;
    vs:term_status "stable" ;
    dct:modified "2015-11-05"^^xsd:date ;
 .

scor:DeliverReturnDefectiveProductStep
    rdf:type owl:Class ;
    rdfs:subClassOf scor:SourceReturnStep ;
    rdfs:comment "Steps to be exectued for a Deliver Return Defective Product process."@en ;
    rdfs:label "Deliver Return Defective Product Step"@en ;
    rdfs:isDefinedBy scor: ;
    vs:term_status "stable" ;
    dct:modified "2015-11-05"^^xsd:date ;
 .


scor:DeliverReturnExcessProductStep
    rdf:type owl:Class ;
    rdfs:subClassOf scor:SourceReturnStep ;
    rdfs:comment "Steps to be exectued for a Deliver Return Excess Product process."@en ;
    rdfs:label "Deliver Return Excess Product Step"@en ;
    rdfs:isDefinedBy scor: ;
    vs:term_status "stable" ;
    dct:modified "2015-11-05"^^xsd:date ;
 .

 scor:DeliverReturnMROProductStep
    rdf:type owl:Class ;
    rdfs:subClassOf scor:SourceReturnStep ;
    rdfs:comment "Steps to be exectued for a Source Return MRO Product process."@en ;
    rdfs:label "Deliver Return MRO Product Step"@en ;
    rdfs:isDefinedBy scor: ;
    vs:term_status "stable" ;
    dct:modified "2015-11-05"^^xsd:date ;
 .


 ################################

 scor:SourceStockedProductStep
    rdf:type owl:Class ;
    rdfs:subClassOf scor:SourceStep ;
    rdfs:comment "Steps to be exectued for a Source Stocked Product process."@en ;
    rdfs:label "Source Stocked Product Step"@en ;
    rdfs:isDefinedBy scor: ;
    vs:term_status "stable" ;
    dct:modified "2015-11-05"^^xsd:date ;
 .

scor:SourceMakeToOrderProductStep
    rdf:type owl:Class ;
    rdfs:subClassOf scor:SourceStep ;
    rdfs:comment "Steps to be exectued for a Source Stocked Product process."@en ;
    rdfs:label "Source Stocked Product Step"@en ;
    rdfs:isDefinedBy scor: ;
    vs:term_status "stable" ;
    dct:modified "2015-11-05"^^xsd:date ;
 .

scor:SourceEngineerToOrderProductStep
    rdf:type owl:Class ;
    rdfs:subClassOf scor:SourceStep ;
    rdfs:comment "Steps to be exectued for a Source Stocked Product process."@en ;
    rdfs:label "Source Stocked Product Step"@en ;
    rdfs:isDefinedBy scor: ;
    vs:term_status "stable" ;
    dct:modified "2015-11-05"^^xsd:date ;
 .


 ################################

scor:MakeToStockStep
    rdf:type owl:Class ;
    rdfs:subClassOf scor:MakeStep ;
    rdfs:comment "Steps to be exectued for a Make to Stock process."@en ;
    rdfs:label "Make to Stock Step"@en ;
    rdfs:isDefinedBy scor: ;
    vs:term_status "stable" ;
    dct:modified "2015-11-05"^^xsd:date ;
 .

scor:MakeToOrderStep
    rdf:type owl:Class ;
    rdfs:subClassOf scor:MakeStep ;
    rdfs:comment "Steps to be exectued for a Make to Order process."@en ;
    rdfs:label "Make to Order Step"@en ;
    rdfs:isDefinedBy scor: ;
    vs:term_status "stable" ;
    dct:modified "2015-11-05"^^xsd:date ;
 .

scor:MakeToEngineerStep
    rdf:type owl:Class ;
    rdfs:subClassOf scor:MakeStep ;
    rdfs:comment "Steps to be exectued for a Make to Engineer process."@en ;
    rdfs:label "Make to Engineer Step"@en ;
    rdfs:isDefinedBy scor: ;
    vs:term_status "stable" ;
    dct:modified "2015-11-05"^^xsd:date ;
 .


 ################################

scor:ManageSupplyChainBusinessRulesStep
    rdf:type owl:Class ;
    rdfs:subClassOf scor:EnableStep ;
    rdfs:comment "Steps to be exectued for a Manage SC Business Rules process."@en ;
    rdfs:label "Manage Supply Chain Business Rules Step"@en ;
    rdfs:isDefinedBy scor: ;
    vs:term_status "stable" ;
    dct:modified "2015-11-05"^^xsd:date ;
 .

scor:ManageSupplyChainPerformanceStep
    rdf:type owl:Class ;
    rdfs:subClassOf scor:EnableStep ;
    rdfs:comment "Steps to be exectued for a Manage SC Performance process."@en ;
    rdfs:label "Manage Supply Chain Performance Step"@en ;
    rdfs:isDefinedBy scor: ;
    vs:term_status "stable" ;
    dct:modified "2015-11-05"^^xsd:date ;
 .

 scor:ManageSupplyChainDataAndInformationStep
    rdf:type owl:Class ;
    rdfs:subClassOf scor:EnableStep ;
    rdfs:comment "Steps to be exectued for a Manage SC Data and Information process."@en ;
    rdfs:label "Manage Supply Chain Data and Information Step"@en ;
    rdfs:isDefinedBy scor: ;
    vs:term_status "stable" ;
    dct:modified "2015-11-05"^^xsd:date ;
 .

scor:ManageSupplyChainHumanResourceStep
    rdf:type owl:Class ;
    rdfs:subClassOf scor:EnableStep ;
    rdfs:comment "Steps to be exectued for a Manage SC Human Resource process."@en ;
    rdfs:label "Manage Supply Chain Human Resources Step"@en ;
    rdfs:isDefinedBy scor: ;
    vs:term_status "stable" ;
    dct:modified "2015-11-05"^^xsd:date ;
 .

scor:ManageSupplyChainAssetsStep
    rdf:type owl:Class ;
    rdfs:subClassOf scor:EnableStep ;
    rdfs:comment "Steps to be exectued for a Manage SC Assets process."@en ;
    rdfs:label "Manage Supply Chain Assets Step"@en ;
    rdfs:isDefinedBy scor: ;
    vs:term_status "stable" ;
    dct:modified "2015-11-05"^^xsd:date ;
 .


scor:ManageSupplyChainContractsStep
    rdf:type owl:Class ;
    rdfs:subClassOf scor:EnableStep ;
    rdfs:comment "Steps to be exectued for a Manage SC Contracts process."@en ;
    rdfs:label "Manage Supply Chain Contracts Step"@en ;
    rdfs:isDefinedBy scor: ;
    vs:term_status "stable" ;
    dct:modified "2015-11-05"^^xsd:date ;
 .

scor:ManageSupplyChainNetworkStep
    rdf:type owl:Class ;
    rdfs:subClassOf scor:EnableStep ;
    rdfs:comment "Steps to be exectued for a Manage SC Network process."@en ;
    rdfs:label "Manage Supply Chain Network Step"@en ;
    rdfs:isDefinedBy scor: ;
    vs:term_status "stable" ;
    dct:modified "2015-11-05"^^xsd:date ;
 .

scor:ManageSupplyChainRegulatoryComplianceStep
    rdf:type owl:Class ;
    rdfs:subClassOf scor:EnableStep ;
    rdfs:comment "Steps to be exectued for a Manage SC Regulatory Compliance process."@en ;
    rdfs:label "Manage Supply Chain Regulatory Compliance Step"@en ;
    rdfs:isDefinedBy scor: ;
    vs:term_status "stable" ;
    dct:modified "2015-11-05"^^xsd:date ;
 .

scor:ManageSupplyChainRiskStep
    rdf:type owl:Class ;
    rdfs:subClassOf scor:EnableStep ;
    rdfs:comment "Steps to be exectued for a Manage SC Risk process."@en ;
    rdfs:label "Manage Supply Chain Risk Step"@en ;
    rdfs:isDefinedBy scor: ;
    vs:term_status "stable" ;
    dct:modified "2015-11-05"^^xsd:date ;
 .

 ################################

scor:DeliverStockedProductStep
    rdf:type owl:Class ;
    rdfs:subClassOf scor:DeliverStep ;
    rdfs:comment "Steps to be exectued for a Deliver Stocked Product process."@en ;
    rdfs:label "Deliver Stocked Product Step"@en ;
    rdfs:isDefinedBy scor: ;
    vs:term_status "stable" ;
    dct:modified "2015-11-05"^^xsd:date ;
 .

 scor:DeliverMakeToOrderProductStep
    rdf:type owl:Class ;
    rdfs:subClassOf scor:DeliverStep ;
    rdfs:comment "Steps to be exectued for a Deliver Make to Order Product process."@en ;
    rdfs:label "Deliver Make to Order Product Step"@en ;
    rdfs:isDefinedBy scor: ;
    vs:term_status "stable" ;
    dct:modified "2015-11-05"^^xsd:date ;
 .

scor:DeliverEngineerToOrderProductStep
    rdf:type owl:Class ;
    rdfs:subClassOf scor:DeliverStep ;
    rdfs:comment "Steps to be exectued for a Deliver Engineer to Order Product process."@en ;
    rdfs:label "Deliver Engineer to Order Product Step"@en ;
    rdfs:isDefinedBy scor: ;
    vs:term_status "stable" ;
    dct:modified "2015-11-05"^^xsd:date ;
 .

scor:DeliverRetailProductStep
    rdf:type owl:Class ;
    rdfs:subClassOf scor:DeliverStep ;
    rdfs:comment "Steps to be exectued for a Deliver Retail Product process."@en ;
    rdfs:label "Deliver Retail Product Step"@en ;
    rdfs:isDefinedBy scor: ;
    vs:term_status "stable" ;
    dct:modified "2015-11-05"^^xsd:date ;
 .


######################
# level 3 processes (steps) start

# Plan SC
scor:PSCIdentifyPrioritizeAggregateSCRequirements
    rdf:type owl:Class ;
    rdfs:subClassOf scor:PlanSupplyChainStep ;
    rdfs:comment "The process of identifying, aggregating, and prioritizing, all sources of demand for the integrated supply chain of a product or service at the appropriate level, horizon and interval."@en ;
    rdfs:label "Identify, Prioritize Aggregate Supply Chain Requirements"@en ;
    scor:isStepOf scor:PlanSupplyChain ;
    skos:notation "sP1.1" ;
    rdfs:isDefinedBy scor: ;
    vs:term_status "stable" ;
    dct:modified "2015-11-05"^^xsd:date ;
 .

scor:IdentifyPrioritizeAggregateSCResources
    rdf:type owl:Class ;
    rdfs:comment "The process of identifying, prioritizing, and aggregating, as a whole with constituent parts, all sources of supply that are required and add value in the supply chain of a product or service at the appropriate level, horizon and interval."@en ;
    rdfs:label "Identify, Prioritize Aggregate Supply Chain Resources"@en ;
    scor:isStepOf scor:PlanSupplyChain ;
    rdfs:subClassOf scor:PlanSupplyChainStep ;
    skos:notation "sP1.2" ;
    rdfs:isDefinedBy scor: ;
    vs:term_status "stable" ;
    dct:modified "2015-11-05"^^xsd:date ;
 .

scor:BalanceSCResourcesWithSCRequirements
    rdf:type owl:Class ;
    rdfs:comment "The process of identifying and measuring the gaps and imbalances between demand and resources in order to determine how to best resolve the variances through marketing, pricing, packaging, warehousing, outsource plans or some other action that will optimize service, flexibility, costs, assets, (or other supply chain inconsistencies) in an iterative and collaborative environment."@en ;
    rdfs:label "Balance Supply Chain Resources with SC Requirements"@en ;
    scor:isStepOf scor:PlanSupplyChain ;
    rdfs:subClassOf scor:PlanSupplyChainStep ;
    skos:notation "sP1.3" ;
    rdfs:isDefinedBy scor: ;
    vs:term_status "stable" ;
    dct:modified "2015-11-05"^^xsd:date ;
 .

scor:EstablishCommunicateSCPlans
    rdf:type owl:Class ;
    rdfs:comment "The establishment and communication of courses of action over the appropriate time-defined (long-term, annual, monthly, weekly) planning horizon and interval, representing a projected appropriation of supply-chain resources to meet supply chain requirements."@en ;
    rdfs:label "Establish and Communicate Supply Chain Plans"@en ;
    scor:isStepOf scor:PlanSupplyChain ;
    rdfs:subClassOf scor:PlanSupplyChainStep ;
    skos:notation "sP1.4" ;
    rdfs:isDefinedBy scor: ;
    vs:term_status "stable" ;
    dct:modified "2015-11-05"^^xsd:date ;
 .

# Plan Source

scor:IdentifyPrioritizeAggregateProductRequirements
    rdf:type owl:Class ;
    rdfs:comment "The process of identifying, prioritizing, and considering, as a whole with constituent parts, all sources of demand for a product or service in the supply chain."@en ;
    rdfs:label "Identify, Prioritize and Aggregate Product Requirements"@en ;
    scor:isStepOf scor:PlanSource ;
    rdfs:subClassOf scor:PlanSourceStep ;
    skos:notation "sP2.1" ;
    rdfs:isDefinedBy scor: ;
    vs:term_status "stable" ;
    dct:modified "2015-11-05"^^xsd:date ;
 .

scor:IdentifyAssessAggregateProductResources
    rdf:type owl:Class ;
    rdfs:subClassOf scor:PlanSourceStep ;
    rdfs:comment "The process of identifying, evaluating, and considering, as a whole with constituent parts, all material and other resources used to add value in the supply chain for a product or services."@en ;
    rdfs:label "Identify, Assess and Aggregate Product Resources"@en ;
    scor:isStepOf scor:PlanSource ;
    skos:notation "sP2.2" ;
    rdfs:isDefinedBy scor: ;
    vs:term_status "stable" ;
    dct:modified "2015-11-05"^^xsd:date ;
 .

scor:BalanceProductResourcesWithProductRequirements
    rdf:type owl:Class ;
    rdfs:subClassOf scor:PlanSourceStep ;
    rdfs:comment "The process of developing a time-phased course of action that commits resources to meet requirements."@en ;
    rdfs:label "Balance Product Resources with Product Requirements"@en ;
    scor:isStepOf scor:PlanSource ;
    skos:notation "sP2.3" ;
    rdfs:isDefinedBy scor: ;
    vs:term_status "stable" ;
    dct:modified "2015-11-05"^^xsd:date ;
 .

scor:EstablishSourcingPlans
    rdf:type owl:Class ;
    rdfs:subClassOf scor:PlanSourceStep ;
    rdfs:comment "The establishment of courses of action over specified time periods that represent a projected appropriation of supply resources to meet sourcing plan requirements."@en ;
    rdfs:label "Establish Sourcing Plans"@en ;
    scor:isStepOf scor:PlanSource ;
    skos:notation "sP2.4" ;
    rdfs:isDefinedBy scor: ;
    vs:term_status "stable" ;
    dct:modified "2015-11-05"^^xsd:date ;
 .

# Plan Make

scor:IdentifyPrioritizeAggregateProductionRequirements
    rdf:type owl:Class ;
    rdfs:subClassOf scor:PlanMakeStep ;
    rdfs:comment "The process of identifying, prioritizing, and considering as a whole with constituent parts, all sources of demand in the creation of a product or service."@en ;
    rdfs:label "Identify, Prioritize and Aggregate Production Requirements"@en ;
    scor:isStepOf scor:PlanMake ;
    skos:notation "sP3.1" ;
    rdfs:isDefinedBy scor: ;
    vs:term_status "stable" ;
    dct:modified "2015-11-05"^^xsd:date ;
 .

scor:IdentifyAssessAggregateProductionResources
    rdf:type owl:Class ;
    rdfs:subClassOf scor:PlanMakeStep ;
    rdfs:comment "The process of identifying, evaluating, and considering, as a whole with constituent parts, all things that add value in the creation of a product or performance of a service."@en ;
    rdfs:label "Identify, Assess and Aggregate Production Resources"@en ;
    scor:isStepOf scor:PlanMake ;
    skos:notation "sP3.2" ;
    rdfs:isDefinedBy scor: ;
    vs:term_status "stable" ;
    dct:modified "2015-11-05"^^xsd:date ;
 .

scor:BalanceProductionResourcesWithProductionRequirements
    rdf:type owl:Class ;
    rdfs:subClassOf scor:PlanMakeStep ;
    rdfs:comment "The process of developing a time-phased course of action that commits creation and operation resources to meet creation and operation requirements."@en ;
    rdfs:label "Balance Production Resources with Production Requirements"@en ;
    scor:isStepOf scor:PlanMake ;
    skos:notation "sP3.3" ;
    rdfs:isDefinedBy scor: ;
    vs:term_status "stable" ;
    dct:modified "2015-11-05"^^xsd:date ;
 .

scor:EstablishProductionPlans
    rdf:type owl:Class ;
    rdfs:subClassOf scor:PlanMakeStep ;
    rdfs:comment "The establishment of courses of action over specified time periods that represent a projected appropriation of supply resources to meet production and operating plan requirements."@en ;
    rdfs:label "Establish Production Plans"@en ;
    scor:isStepOf scor:PlanMake ;
    skos:notation "sP3.4" ;
    rdfs:isDefinedBy scor: ;
    vs:term_status "stable" ;
    dct:modified "2015-11-05"^^xsd:date ;
 .

# Plan Deliver

scor:IdentifyPrioritizeAggregateDeliveryRequirements
    rdf:type owl:Class ;
    rdfs:subClassOf scor:PlanDeliverStep ;
    rdfs:comment "The process of identifying, prioritizing, and considering, as a whole with constituent parts, all sources of demand in the delivery of a product or service."@en ;
    rdfs:label "Identify, Prioritize and Aggregate Delivery Requirements"@en ;
    scor:isStepOf scor:PlanDeliver ;
    skos:notation "sP4.1" ;
    rdfs:isDefinedBy scor: ;
    vs:term_status "stable" ;
    dct:modified "2015-11-05"^^xsd:date ;
 .

scor:IdentifyAssessAggregateDeliveryResources
    rdf:type owl:Class ;
    rdfs:subClassOf scor:PlanDeliverStep ;
    rdfs:comment "The process of identifying, evaluating, and considering, as a whole with constituent parts, all things that add value in the delivery of a product or service."@en ;
    rdfs:label "Identify, Assess and Aggregate Delivery Resources"@en ;
    scor:isStepOf scor:PlanDeliver ;
    skos:notation "sP4.2" ;
    rdfs:isDefinedBy scor: ;
    vs:term_status "stable" ;
    dct:modified "2015-11-05"^^xsd:date ;
 .

scor:BalanceDeliveryResourcesCapabilitiesWithDeliveryRequirements
    rdf:type owl:Class ;
    rdfs:subClassOf scor:PlanDeliverStep ;
    rdfs:comment "The process of developing a time-phased course of action that commits delivery resources to meet delivery requirements."@en ;
    rdfs:label "Balance Delivery Resources and Capabilities with Delivery Requirements"@en ;
    scor:isStepOf scor:PlanDeliver ;
    skos:notation "sP4.3" ;
    rdfs:isDefinedBy scor: ;
    vs:term_status "stable" ;
    dct:modified "2015-11-05"^^xsd:date ;
 .

scor:EstablishDeliveryPlans
    rdf:type owl:Class ;
    rdfs:subClassOf scor:PlanDeliverStep ;
    rdfs:comment "The establishment of courses of action over specified time periods that represent a projected appropriation of delivery resources to meet delivery requirements."@en ;
    rdfs:label "Establish Delivery Plans"@en ;
    scor:isStepOf scor:PlanDeliver ;
    skos:notation "sP4.4" ;
    rdfs:isDefinedBy scor: ;
    vs:term_status "stable" ;
    dct:modified "2015-11-05"^^xsd:date ;
 .

# Plan Return

scor:AssessAggregateReturnRequirements
    rdf:type owl:Class ;
    rdfs:subClassOf scor:PlanReturnStep ;
    rdfs:comment "The process of identifying, evaluating, and considering, as a whole with constituent parts, all sources of demand for the return of a product."@en ;
    rdfs:label "Assess and Aggregate Return Requirements"@en ;
    scor:isStepOf scor:PlanReturn ;
    skos:notation "sP5.1" ;
    rdfs:isDefinedBy scor: ;
    vs:term_status "stable" ;
    dct:modified "2015-11-05"^^xsd:date ;
 .

scor:IdentifyAssessAggregateReturnResources
    rdf:type owl:Class ;
    rdfs:subClassOf scor:PlanReturnStep ;
    rdfs:comment "The process of identifying, evaluating, and consideration for all resources that add value to, execute, or constrain the processes for the return of a product.."@en ;
    rdfs:label "Identify, Assess and Aggregate Return Resources"@en ;
    scor:isStepOf scor:PlanReturn ;
    skos:notation "sP5.2" ;
    rdfs:isDefinedBy scor: ;
    vs:term_status "stable" ;
    dct:modified "2015-11-05"^^xsd:date ;
 .

scor:BalanceReturnResourcesWithReturnRequirements
    rdf:type owl:Class ;
    rdfs:subClassOf scor:PlanReturnStep ;
    rdfs:comment "The process of developing courses of action that make feasible the commitment the appropriate return resources and or assets to satisfy return requirements."@en ;
    rdfs:label "Balance Return Resources with Return Requirements"@en ;
    scor:isStepOf scor:PlanReturn ;
    skos:notation "sP5.3" ;
    rdfs:isDefinedBy scor: ;
    vs:term_status "stable" ;
    dct:modified "2015-11-05"^^xsd:date ;
 .

scor:EstablishCommunicateReturnPlans
    rdf:type owl:Class ;
    rdfs:subClassOf scor:PlanReturnStep ;
    rdfs:comment "The establishment and communication of courses of action over specified time periods that represent a projected appropriation of required return resources and or assets to meet return process requirements."@en ;
    rdfs:label "Establish and Communicate Return Plans"@en ;
    scor:isStepOf scor:PlanReturn ;
    skos:notation "sP5.4" ;
    rdfs:isDefinedBy scor: ;
    vs:term_status "stable" ;
    dct:modified "2015-11-05"^^xsd:date ;
 .

# Source Stocked Product

scor:SSPScheduleProductDeliveries
    rdf:type owl:Class ;
    rdfs:subClassOf scor:SourceStockedProductStep ;
    rdfs:comment "Scheduling and managing the execution of the individual deliveries of product against an existing contract or purchase order."@en ;
    rdfs:label "Schedule Product Deliveries (Source Stocked Product)"@en ;
    scor:isStepOf scor:SourceStockedProduct ;
    skos:notation "sS1.1" ;
    rdfs:isDefinedBy scor: ;
    vs:term_status "stable" ;
    dct:modified "2015-11-05"^^xsd:date ;
 .

scor:SSPReceiveProduct
    rdf:type owl:Class ;
    rdfs:subClassOf scor:SourceStockedProductStep ;
    rdfs:comment "The process and associated activities of receiving product to contract requirements."@en ;
    rdfs:label "Receive Product (Source Stocked Product)"@en ;
    scor:isStepOf scor:SourceStockedProduct ;
    skos:notation "sS1.2" ;
    rdfs:isDefinedBy scor: ;
    vs:term_status "stable" ;
    dct:modified "2015-11-05"^^xsd:date ;
 .

scor:SSPVerifyProduct
    rdf:type owl:Class ;
    rdfs:subClassOf scor:SourceStockedProductStep ;
    rdfs:comment "The process and associated activities of receiving product to contract requirements."@en ;
    rdfs:label "Verify Product (Source Stocked Product)"@en ;
    scor:isStepOf scor:SourceStockedProduct ;
    skos:notation "sS1.3" ;
    rdfs:isDefinedBy scor: ;
    vs:term_status "stable" ;
    dct:modified "2015-11-05"^^xsd:date ;
 .

scor:SSPTransferProduct
    rdf:type owl:Class ;
    rdfs:subClassOf scor:SourceStockedProductStep ;
    rdfs:comment "The transfer of accepted product to the appropriate stocking location within the supply chain."@en ;
    rdfs:label "Transfer Product (Source Stocked Product)"@en ;
    scor:isStepOf scor:SourceStockedProduct ;
    skos:notation "sS1.4" ;
    rdfs:isDefinedBy scor: ;
    vs:term_status "stable" ;
    dct:modified "2015-11-05"^^xsd:date ;
 .

scor:AuthorizeSupplierPayment
    rdf:type owl:Class ;
    rdfs:subClassOf scor:SourceStockedProductStep ;
    rdfs:comment "The process of authorizing payments and paying suppliers for product or services."@en ;
    rdfs:label "Authorize Supplier Payment (Source Stocked Product)"@en ;
    scor:isStepOf scor:SourceStockedProduct ;
    skos:notation "sS1.5" ;
    rdfs:isDefinedBy scor: ;
    vs:term_status "stable" ;
    dct:modified "2015-11-05"^^xsd:date ;
 .

# Source MakeToOrderProduct

scor:SMOPScheduleProductDeliveries
    rdf:type owl:Class ;
    rdfs:subClassOf scor:SourceMakeToOrderProductStep ;
    rdfs:comment "Scheduling and managing the execution of the individual deliveries of product against the contract."@en ;
    rdfs:label "Schedule Product Deliveries (Source Make To Order Product)"@en ;
    scor:isStepOf scor:SourceMakeToOrderProduct ;
    skos:notation "sS2.1" ;
    rdfs:isDefinedBy scor: ;
    vs:term_status "stable" ;
    dct:modified "2015-11-05"^^xsd:date ;
 .

scor:SMOPReceiveProduct
    rdf:type owl:Class ;
    rdfs:subClassOf scor:SourceMakeToOrderProductStep ;
    rdfs:comment "The process and associated activities of receiving product to contract requirements."@en ;
    rdfs:label "Receive Product (Source Make To Order Product)"@en ;
    scor:isStepOf scor:SourceMakeToOrderProduct ;
    skos:notation "sS2.2" ;
    rdfs:isDefinedBy scor: ;
    vs:term_status "stable" ;
    dct:modified "2015-11-05"^^xsd:date ;
 .

scor:SMOPVerifyProduct
    rdf:type owl:Class ;
    rdfs:subClassOf scor:SourceMakeToOrderProductStep ;
    rdfs:comment "The process and actions required determining product conformance to requirements and criteria."@en ;
    rdfs:label "Verify Product (Source Make To Order Product)"@en ;
    scor:isStepOf scor:SourceMakeToOrderProduct ;
    skos:notation "sS2.3" ;
    rdfs:isDefinedBy scor: ;
    vs:term_status "stable" ;
    dct:modified "2015-11-05"^^xsd:date ;
 .

scor:SMOPTransferProduct
    rdf:type owl:Class ;
    rdfs:subClassOf scor:SourceMakeToOrderProductStep ;
    rdfs:comment "The transfer of accepted product to the appropriate stocking location within the supply chain."@en ;
    rdfs:label "Transfer Product (Source Make To Order Product)"@en ;
    scor:isStepOf scor:SourceMakeToOrderProduct ;
    skos:notation "sS2.4" ;
    rdfs:isDefinedBy scor: ;
    vs:term_status "stable" ;
    dct:modified "2015-11-05"^^xsd:date ;
 .

scor:SMOPAuthorizeSupplierPayment
    rdf:type owl:Class ;
    rdfs:subClassOf scor:SourceMakeToOrderProductStep ;
    rdfs:comment "The process of authorizing payments and paying suppliers for product or services."@en ;
    rdfs:label "Supplier Payment (Source Make To Order Product)"@en ;
    scor:isStepOf scor:SourceMakeToOrderProduct ;
    skos:notation "sS2.5" ;
    rdfs:isDefinedBy scor: ;
    vs:term_status "stable" ;
    dct:modified "2015-11-05"^^xsd:date ;
 .

# SourceEngineerToOrderProduct

scor:IdentifySourcesOfSupply
    rdf:type owl:Class ;
    rdfs:subClassOf scor:SourceEngineerToOrderProductStep ;
    rdfs:comment "The identification and qualification of potential suppliers capable of designing and delivering product that will meet all of the required product specifications."@en ;
    rdfs:label "Identify Sources of Supply"@en ;
    scor:isStepOf scor:SourceEngineerToOrderProduct ;
    skos:notation "sS3.1" ;
    rdfs:isDefinedBy scor: ;
    vs:term_status "stable" ;
    dct:modified "2015-11-05"^^xsd:date ;
 .

scor:SelectFinalSupplierNegotiate
    rdf:type owl:Class ;
    rdfs:subClassOf scor:SourceEngineerToOrderProductStep ;
    rdfs:comment "The identification of the final supplier(s) based on the evaluation of RFQs, supplier qualifications and the generation of a contract defining the costs and terms and conditions of product availability."@en ;
    rdfs:label "Select Final Supplier and Negotiate"@en ;
    scor:isStepOf scor:SourceEngineerToOrderProduct ;
    skos:notation "sS3.2" ;
    rdfs:isDefinedBy scor: ;
    vs:term_status "stable" ;
    dct:modified "2015-11-05"^^xsd:date ;
 .

scor:SEOPScheduleProductDeliveries
    rdf:type owl:Class ;
    rdfs:subClassOf scor:SourceEngineerToOrderProductStep ;
    rdfs:comment "Scheduling and managing the execution of the individual deliveries of product against the contract."@en ;
    rdfs:label "Schedule Product Deliveries (Source Engineer To Order Product)"@en ;
    scor:isStepOf scor:SourceEngineerToOrderProduct ;
    skos:notation "sS3.3" ;
    rdfs:isDefinedBy scor: ;
    vs:term_status "stable" ;
    dct:modified "2015-11-05"^^xsd:date ;
 .

scor:SEOPReceiveProduct
    rdf:type owl:Class ;
    rdfs:subClassOf scor:SourceEngineerToOrderProductStep ;
    rdfs:comment "The process and associated activities of receiving product to contract requirements."@en ;
    rdfs:label "Receive Product (Source Engineer To Order Product)"@en ;
    scor:isStepOf scor:SourceEngineerToOrderProduct ;
    skos:notation "sS3.4" ;
    rdfs:isDefinedBy scor: ;
    vs:term_status "stable" ;
    dct:modified "2015-11-05"^^xsd:date ;
 .

scor:SEOPVerifyProduct
    rdf:type owl:Class ;
    rdfs:subClassOf scor:SourceEngineerToOrderProductStep ;
    rdfs:comment "The process and actions required determining product conformance to requirements and criteria."@en ;
    rdfs:label "Verify Product (Source Engineer To Order Product)"@en ;
    scor:isStepOf scor:SourceEngineerToOrderProduct ;
    skos:notation "sS3.5" ;
    rdfs:isDefinedBy scor: ;
    vs:term_status "stable" ;
    dct:modified "2015-11-05"^^xsd:date ;
 .

scor:SEOPTransferProduct
    rdf:type owl:Class ;
    rdfs:subClassOf scor:SourceEngineerToOrderProductStep ;
    rdfs:comment "The transfer of accepted product to the appropriate stocking location within the supply chain."@en ;
    rdfs:label "Transfer Product (Source Engineer To Order Product)"@en ;
    scor:isStepOf scor:SourceEngineerToOrderProduct ;
    skos:notation "sS3.6" ;
    rdfs:isDefinedBy scor: ;
    vs:term_status "stable" ;
    dct:modified "2015-11-05"^^xsd:date ;
 .

scor:SEOPAuthorizeSupplierPayment
    rdf:type owl:Class ;
    rdfs:subClassOf scor:SourceEngineerToOrderProductStep ;
    rdfs:comment "The process of authorizing payments and paying suppliers for product or services. This process includes invoice collection, invoice matching and the issuance of checks."@en ;
    rdfs:label "Authorize Supplier Payment (Source Engineer To Order Product)"@en ;
    scor:isStepOf scor:SourceEngineerToOrderProduct ;
    skos:notation "sS3.7" ;
    rdfs:isDefinedBy scor: ;
    vs:term_status "stable" ;
    dct:modified "2015-11-05"^^xsd:date ;
 .

# Make MakeToStock

scor:MSScheduleProductionActivities
    rdf:type owl:Class ;
    rdfs:subClassOf scor:MakeToStockStep ;
    rdfs:comment "Given plans for the production of specific parts, products, or formulations in specified quantities and planned availability of required sourced products, the scheduling of the operations to be performed in accordance with these plans."@en ;
    rdfs:label "Schedule Production Activities (Make To Stock)"@en ;
    scor:isStepOf scor:MakeToStock ;
    skos:notation "sM1.1" ;
    rdfs:isDefinedBy scor: ;
    vs:term_status "stable" ;
    dct:modified "2015-11-05"^^xsd:date ;
 .

scor:IssueMaterial
    rdf:type owl:Class ;
    rdfs:subClassOf scor:MakeToStockStep ;
    rdfs:comment "The selection and physical movement of sourced/in-process product (e.g., raw materials, fabricated components, subassemblies, required ingredients or intermediate formulations) from a stocking location (e.g., stockroom, a location on the production floor, a supplier) to a specific point of use location."@en ;
    rdfs:label "Issue Material"@en ;
    scor:isStepOf scor:MakeToStock ;
    skos:notation "sM1.2" ;
    rdfs:isDefinedBy scor: ;
    vs:term_status "stable" ;
    dct:modified "2015-11-05"^^xsd:date ;
 .

scor:MSProduceTest
    rdf:type owl:Class ;
    rdfs:subClassOf scor:MakeToStockStep ;
    rdfs:comment "The series of activities performed upon sourced/in-process product to convert it from the raw or semi-finished state to a state of completion and greater value."@en ;
    rdfs:label "Produce and Test (Make To Stock)"@en ;
    scor:isStepOf scor:MakeToStock ;
    skos:notation "sM1.3" ;
    rdfs:isDefinedBy scor: ;
    vs:term_status "stable" ;
    dct:modified "2015-11-05"^^xsd:date ;
 .

scor:MSPackage
    rdf:type owl:Class ;
    rdfs:subClassOf scor:MakeToStockStep ;
    rdfs:comment "The series of activities that containerize completed products for storage or sale to end-users."@en ;
    rdfs:label "Package (Make To Stock)"@en ;
    scor:isStepOf scor:MakeToStock ;
    skos:notation "sM1.4" ;
    rdfs:isDefinedBy scor: ;
    vs:term_status "stable" ;
    dct:modified "2015-11-05"^^xsd:date ;
 .

scor:StageProduct
    rdf:type owl:Class ;
    rdfs:subClassOf scor:MakeToStockStep ;
    rdfs:comment "The movement of packaged products into a temporary holding location to await movement to a finished goods location."@en ;
    rdfs:label "Stage Product"@en ;
    scor:isStepOf scor:MakeToStock ;
    skos:notation "sM1.5" ;
    rdfs:isDefinedBy scor: ;
    vs:term_status "stable" ;
    dct:modified "2015-11-05"^^xsd:date ;
 .

scor:ReleaseProductToDeliver
    rdf:type owl:Class ;
    rdfs:subClassOf scor:MakeToStockStep ;
    rdfs:comment "Activities associated with post-production documentation, stable, or certification required prior to delivery of finished product to customer."@en ;
    rdfs:label "Release Product to Deliver (Make To Stock)"@en ;
    scor:isStepOf scor:MakeToStock ;
    skos:notation "sM1.6" ;
    rdfs:isDefinedBy scor: ;
    vs:term_status "stable" ;
    dct:modified "2015-11-05"^^xsd:date ;
 .

scor:MSWasteDisposal
    rdf:type owl:Class ;
    rdfs:subClassOf scor:MakeToStockStep ;
    rdfs:comment "Activities associated with collecting and managing waste produced during the produce and test process including scrap material and non-conforming product."@en ;
    rdfs:label "Waste Disposal (Make To Stock)"@en ;
    scor:isStepOf scor:MakeToStock ;
    skos:notation "sM1.7" ;
    rdfs:isDefinedBy scor: ;
    vs:term_status "stable" ;
    dct:modified "2015-11-05"^^xsd:date ;
 .

# Make MakeToOrder

scor:MOScheduleProductionActivities
    rdf:type owl:Class ;
    rdfs:subClassOf scor:MakeToOrderStep ;
    rdfs:comment "Given plans for the production of specific parts, products, or formulations in specific quantities and planned availability of required sourced products, the scheduling of the operations to be preformed in accordance with these plans."@en ;
    rdfs:label "Schedule Production Activities (Make To Order)"@en ;
    scor:isStepOf scor:MakeToOrder ;
    skos:notation "sM2.1" ;
    rdfs:isDefinedBy scor: ;
    vs:term_status "stable" ;
    dct:modified "2015-11-05"^^xsd:date ;
 .

scor:IssueSourcedInProcessProduct
    rdf:type owl:Class ;
    rdfs:subClassOf scor:MakeToOrderStep ;
    rdfs:comment "The selection and physical movement of sourced/in-process products (e.g., raw materials, fabricated components, subassemblies, required ingredients or intermediate formulations) from a stocking location (e.g., stockroom, a location on the production floor, a supplier) to a specific point of use location."@en ;
    rdfs:label "Issue Sourced In-Process Product (Make To Order)"@en ;
    scor:isStepOf scor:MakeToOrder ;
    skos:notation "sM2.2" ;
    rdfs:isDefinedBy scor: ;
    vs:term_status "stable" ;
    dct:modified "2015-11-05"^^xsd:date ;
 .

scor:MOProduceTest
    rdf:type owl:Class ;
    rdfs:subClassOf scor:MakeToOrderStep ;
    rdfs:comment "The series of activities performed upon sourced/in-process product to convert it from the raw or semi-finished state to a state of completion and greater value."@en ;
    rdfs:label "Produce and Test (Make to Order)"@en ;
    scor:isStepOf scor:MakeToOrder ;
    skos:notation "sM2.3" ;
    rdfs:isDefinedBy scor: ;
    vs:term_status "stable" ;
    dct:modified "2015-11-05"^^xsd:date ;
 .

scor:MOPackage
    rdf:type owl:Class ;
    rdfs:subClassOf scor:MakeToOrderStep ;
    rdfs:comment "The series of activities that containerize completed products for storage or sale to end-users."@en ;
    rdfs:label "Package (Make To Order)"@en ;
    scor:isStepOf scor:MakeToOrder ;
    skos:notation "sM2.4" ;
    rdfs:isDefinedBy scor: ;
    vs:term_status "stable" ;
    dct:modified "2015-11-05"^^xsd:date ;
 .

scor:StageFinishedProduct
    rdf:type owl:Class ;
    rdfs:subClassOf scor:MakeToOrderStep ;
    rdfs:comment "The movement of packaged products into a temporary holding location to await movement to a finished goods location."@en ;
    rdfs:label "Stage Finished Product (Make To Order)"@en ;
    scor:isStepOf scor:MakeToOrder ;
    skos:notation "sM2.5" ;
    rdfs:isDefinedBy scor: ;
    vs:term_status "stable" ;
    dct:modified "2015-11-05"^^xsd:date ;
 .

scor:ReleaseFinishedProductToDeliver
    rdf:type owl:Class ;
    rdfs:subClassOf scor:MakeToOrderStep ;
    rdfs:comment "Activities associated with post-production documentation, stable, or certification required prior to delivery of finished product to customer."@en ;
    rdfs:label "Release Finished Product to Deliver"@en ;
    scor:isStepOf scor:MakeToOrder ;
    skos:notation "sM2.6" ;
    rdfs:isDefinedBy scor: ;
    vs:term_status "stable" ;
    dct:modified "2015-11-05"^^xsd:date ;
 .

scor:MOWasteDisposal
    rdf:type owl:Class ;
    rdfs:subClassOf scor:MakeToOrderStep ;
    rdfs:comment "Activities associated with collecting and managing waste produced during the produce and test process including scrap material and non-conforming product."@en ;
    rdfs:label "Waste Disposal (Make To Order)"@en ;
    scor:isStepOf scor:MakeToOrder ;
    skos:notation "sM2.7" ;
    rdfs:isDefinedBy scor: ;
    vs:term_status "stable" ;
    dct:modified "2015-11-05"^^xsd:date ;
 .

# Make Engineer to Order

scor:FinalizeProductionEngineering
    rdf:type owl:Class ;
    rdfs:subClassOf scor:MakeToEngineerStep ;
    rdfs:comment "Engineering activities required after acceptance of order, but before product can be produced. May include generation and delivery of final drawings, specifications, formulas, part programs, etc."@en ;
    rdfs:label "Finalize Production Engineering"@en ;
    scor:isStepOf scor:MakeEngineerToOrder ;
    skos:notation "sM3.1" ;
    rdfs:isDefinedBy scor: ;
    vs:term_status "stable" ;
    dct:modified "2015-11-05"^^xsd:date ;
 .

scor:MEOScheduleProductionActivities
    rdf:type owl:Class ;
    rdfs:subClassOf scor:MakeToEngineerStep ;
    rdfs:comment "Given plans for the production of specific parts, products, or formulations in specified quantities and planned availability of required sourced products, the scheduling of the operations to be performed in accordance with these plans"@en ;
    rdfs:label "Schedule Production Activities (Engineer To Order)"@en ;
    scor:isStepOf scor:MakeEngineerToOrder ;
    skos:notation "sM3.2" ;
    rdfs:isDefinedBy scor: ;
    vs:term_status "stable" ;
    dct:modified "2015-11-05"^^xsd:date ;
 .

scor:MEOSourcedInProcessProduct
    rdf:type owl:Class ;
    rdfs:subClassOf scor:MakeToEngineerStep ;
    rdfs:comment "The selection and physical movement of sourced/in-process products (e.g., raw materials, fabricated components, subassemblies, required ingredients or intermediate formulations) from a stocking location (e.g., stockroom, a location on the production floor, a supplier) to a specific point of use location"@en ;
    rdfs:label "Issue Sourced In-Process Product (Engineer To Order)"@en ;
    scor:isStepOf scor:MakeEngineerToOrder ;
    skos:notation "sM3.3" ;
    rdfs:isDefinedBy scor: ;
    vs:term_status "stable" ;
    dct:modified "2015-11-05"^^xsd:date ;
 .

scor:MEOProduceTest
    rdf:type owl:Class ;
    rdfs:subClassOf scor:MakeToEngineerStep ;
    rdfs:comment "The series of activities performed upon sourced/in-process product to convert it from the raw or semi-finished state to a state of completion and greater value"@en ;
    rdfs:label "Produce and Test (Engineer to Order)"@en ;
    scor:isStepOf scor:MakeEngineerToOrder ;
    skos:notation "sM3.4" ;
    rdfs:isDefinedBy scor: ;
    vs:term_status "stable" ;
    dct:modified "2015-11-05"^^xsd:date ;
 .

scor:MEOPackage
    rdf:type owl:Class ;
    rdfs:subClassOf scor:MakeToEngineerStep ;
    rdfs:comment "The series of activities that containerize completed products for storage or sale to end-users."@en ;
    rdfs:label "Package (Engineer To Order)"@en ;
    scor:isStepOf scor:MakeEngineerToOrder ;
    skos:notation "sM3.5" ;
    rdfs:isDefinedBy scor: ;
    vs:term_status "stable" ;
    dct:modified "2015-11-05"^^xsd:date ;
 .

scor:MEOStageFinishedProduct
    rdf:type owl:Class ;
    rdfs:subClassOf scor:MakeToEngineerStep ;
    rdfs:comment "The movement of packaged products into a temporary holding location to await movement to a finished goods location."@en ;
    rdfs:label "Stage Finished Product (Engineer To Order)"@en ;
    scor:isStepOf scor:MakeEngineerToOrder ;
    skos:notation "sM3.6" ;
    rdfs:isDefinedBy scor: ;
    vs:term_status "stable" ;
    dct:modified "2015-11-05"^^xsd:date ;
 .

scor:MEOReleaseProductToDeliver
    rdf:type owl:Class ;
    rdfs:subClassOf scor:MakeToEngineerStep ;
    rdfs:comment "Activities associated with post-production documentation, stable, or certification required prior to delivery of finished product to customer."@en ;
    rdfs:label "Release Product to Deliver (Engineer To Order)"@en ;
    scor:isStepOf scor:MakeEngineerToOrder ;
    skos:notation "sM3.7" ;
    rdfs:isDefinedBy scor: ;
    vs:term_status "stable" ;
    dct:modified "2015-11-05"^^xsd:date ;
 .

scor:MEOWasteDisposal
    rdf:type owl:Class ;
    rdfs:subClassOf scor:MakeToEngineerStep ;   
    rdfs:comment "Activities associated with collecting and managing waste produced during the produce and test process including scrap material and non-conforming product."@en ;
    rdfs:label "Waste Disposal (Engineer To Order)"@en ;
    scor:isStepOf scor:MakeEngineerToOrder ;
    skos:notation "sM3.8" ;
    rdfs:isDefinedBy scor: ;
    vs:term_status "stable" ;
    dct:modified "2015-11-05"^^xsd:date ;
 .

# Deliver Stocked Product

scor:ProcessInquiryQuote
    rdf:type owl:Class ;
    rdfs:subClassOf scor:DeliverStockedProductStep ;   
    rdfs:comment "Receive and respond to general customer inquiries and requests for quotes."@en ;
    rdfs:label "Process Inquiry and Quote (Deliver Stocked Product)"@en ;
    scor:isStepOf scor:DeliverStockedProduct ;
    skos:notation "sD1.1" ;
    rdfs:isDefinedBy scor: ;
    vs:term_status "stable" ;
    dct:modified "2015-11-05"^^xsd:date ;
 .

scor:ReceiveEnterValidateOrder
    rdf:type owl:Class ;
    rdfs:subClassOf scor:DeliverStockedProductStep ;   
    rdfs:comment "Receive orders from the customer and enter them into a company's order processing system."@en ;
    rdfs:label "Receive, Enter, and Validate Order"@en ;
    scor:isStepOf scor:DeliverStockedProduct ;
    skos:notation "sD1.2" ;
    rdfs:isDefinedBy scor: ;
    vs:term_status "stable" ;
    dct:modified "2015-11-05"^^xsd:date ;
 .

scor:DSPReserveInventoryDetermineDeliveryDate
    rdf:type owl:Class ;
    rdfs:subClassOf scor:DeliverStockedProductStep ;   
    rdfs:comment "Inventory (both on hand and scheduled) is identified and reserved for specific orders and a delivery date is committed and scheduled."@en ;
    rdfs:label "Reserve Inventory and Determine Delivery Date (Deliver Stocked Product)"@en ;
    scor:isStepOf scor:DeliverStockedProduct ;
    skos:notation "sD1.3" ;
    rdfs:isDefinedBy scor: ;
    vs:term_status "stable" ;
    dct:modified "2015-11-05"^^xsd:date ;
 .

scor:DSPConsolidateOrders
    rdf:type owl:Class ;
    rdfs:subClassOf scor:DeliverStockedProductStep ;   
    rdfs:comment "The process of analyzing orders to determine the groupings that result in least cost/best service fulfillment and transportation."@en ;
    rdfs:label "Consolidate Orders (Deliver Stocked Product)"@en ;
    scor:isStepOf scor:DeliverStockedProduct ;
    skos:notation "sD1.4" ;
    rdfs:isDefinedBy scor: ;
    vs:term_status "stable" ;
    dct:modified "2015-11-05"^^xsd:date ;
 .

scor:DSPBuildLoads
    rdf:type owl:Class ;
    rdfs:subClassOf scor:DeliverStockedProductStep ;   
    rdfs:comment "Transportation modes are selected and efficient loads are built."@en ;
    rdfs:label "Build Loads (Deliver Stocked Product)"@en ;
    scor:isStepOf scor:DeliverStockedProduct ;
    skos:notation "sD1.5" ;
    rdfs:isDefinedBy scor: ;
    vs:term_status "stable" ;
    dct:modified "2015-11-05"^^xsd:date ;
 .

scor:DSPRouteShipments
    rdf:type owl:Class ;
    rdfs:subClassOf scor:DeliverStockedProductStep ;   
    rdfs:comment "Loads are consolidated and routed by mode, lane and location."@en ;
    rdfs:label "Route Shipments (Deliver Stocked Product)"@en ;
    scor:isStepOf scor:DeliverStockedProduct ;
    skos:notation "sD1.6" ;
    rdfs:isDefinedBy scor: ;
    vs:term_status "stable" ;
    dct:modified "2015-11-05"^^xsd:date ;
 .

scor:DSPSelectCarriersRateShipments
    rdf:type owl:Class ;
    rdfs:subClassOf scor:DeliverStockedProductStep ;   
    rdfs:comment "Specific carriers are selected by lowest cost per route and shipments are rated and tendered."@en ;
    rdfs:label "Select Carriers and Rate Shipments (Deliver Stocked Product)"@en ;
    scor:isStepOf scor:DeliverStockedProduct ;
    skos:notation "sD1.7" ;
    rdfs:isDefinedBy scor: ;
    vs:term_status "stable" ;
    dct:modified "2015-11-05"^^xsd:date ;
 .

scor:DSPReceiveProductFromSourceMake
    rdf:type owl:Class ;
    rdfs:subClassOf scor:DeliverStockedProductStep ;   
    rdfs:comment "The activities such as receiving product, verifying, recording product receipt, determining put-away location, putting away and recording location that a company performs at its own warehouses."@en ;
    rdfs:label "Receive Product from Source or Make (Deliver Stocked Product)"@en ;
    scor:isStepOf scor:DeliverStockedProduct ;
    skos:notation "sD1.8" ;
    rdfs:isDefinedBy scor: ;
    vs:term_status "stable" ;
    dct:modified "2015-11-05"^^xsd:date ;
 .

scor:DSPPickProduct
    rdf:type owl:Class ;
    rdfs:subClassOf scor:DeliverStockedProductStep ;   
    rdfs:comment "The series of activities including retrieving orders to pick, determining inventory availability, building the pick wave, picking the product, recording the pick and delivering product to shipping in response to an order."@en ;
    rdfs:label "Pick Product (Deliver Stocked Product)"@en ;
    scor:isStepOf scor:DeliverStockedProduct ;
    skos:notation "sD1.9" ;
    rdfs:isDefinedBy scor: ;
    vs:term_status "stable" ;
    dct:modified "2015-11-05"^^xsd:date ;
 .

scor:DSPPackProduct
    rdf:type owl:Class ;
    rdfs:subClassOf scor:DeliverStockedProductStep ;   
    rdfs:comment "The activities such as sorting / combining the products, packing / kitting the products, paste labels, barcodes etc. and delivering the products to the shipping area for loading."@en ;
    rdfs:label "Pack Product (Deliver Stocked Product)"@en ;
    scor:isStepOf scor:DeliverStockedProduct ;
    skos:notation "sD1.10" ;
    rdfs:isDefinedBy scor: ;
    vs:term_status "stable" ;
    dct:modified "2015-11-05"^^xsd:date ;
 .

scor:LoadVehicleGenerateShippingDocuments
    rdf:type owl:Class ;
    rdfs:subClassOf scor:DeliverStockedProductStep ;   
    rdfs:comment "The series of tasks including placing/loading product onto modes of transportation, and generating the documentation necessary to meet internal, customer, carrier and government needs."@en ;
    rdfs:label "Load Vehicle and Generate Shipping Documents"@en ;
    scor:isStepOf scor:DeliverStockedProduct ;
    skos:notation "sD1.11" ;
    rdfs:isDefinedBy scor: ;
    vs:term_status "stable" ;
    dct:modified "2015-11-05"^^xsd:date ;
 .

scor:DSPShipProduct
    rdf:type owl:Class ;
    rdfs:subClassOf scor:DeliverStockedProductStep ;   
    rdfs:comment "The process of shipping the product to the customer site."@en ;
    rdfs:label "Ship Product (Deliver Stocked Product)"@en ;
    scor:isStepOf scor:DeliverStockedProduct ;
    skos:notation "sD1.12" ;
    rdfs:isDefinedBy scor: ;
    vs:term_status "stable" ;
    dct:modified "2015-11-05"^^xsd:date ;
 .

scor:DSPReceiveVerifyProductByCustomer
    rdf:type owl:Class ;
    rdfs:subClassOf scor:DeliverStockedProductStep ;   
    rdfs:comment "The process of receiving the shipment by the customer (either at customer site or at shipping area in case of self-collection) and verifying that the order was shipped complete and that the product meets delivery terms."@en ;
    rdfs:label "Receive and verify Product by Customer (Deliver Stocked Product)"@en ;
    scor:isStepOf scor:DeliverStockedProduct ;
    skos:notation "sD1.13" ;
    rdfs:isDefinedBy scor: ;
    vs:term_status "stable" ;
    dct:modified "2015-11-05"^^xsd:date ;
 .

scor:DSPInstallProduct
    rdf:type owl:Class ;
    rdfs:subClassOf scor:DeliverStockedProductStep ;   
    rdfs:comment "the process of preparing, stable and installing the product at the customer site. The product is fully functional upon completion."@en ;
    rdfs:label "Install Product (Deliver Stocked Product)"@en ;
    scor:isStepOf scor:DeliverStockedProduct ;
    skos:notation "sD1.14" ;
    rdfs:isDefinedBy scor: ;
    vs:term_status "stable" ;
    dct:modified "2015-11-05"^^xsd:date ;
 .

scor:DSPInvoice
    rdf:type owl:Class ;
    rdfs:subClassOf scor:DeliverStockedProductStep ;   
    rdfs:comment "A signal is sent to the financial organization that the order has been shipped and that the billing process should begin and payment be received or be closed out if payment has already been received."@en ;
    rdfs:label "Invoice (Deliver Stocked Product)"@en ;
    scor:isStepOf scor:DeliverStockedProduct ;
    skos:notation "sD1.15" ;
    rdfs:isDefinedBy scor: ;
    vs:term_status "stable" ;
    dct:modified "2015-11-05"^^xsd:date ;
 .

# Deliver Make-to-Order Product

scor:DMOPInquiryQuote
    rdf:type owl:Class ;
    rdfs:subClassOf scor:DeliverMakeToOrderProductStep ;   
    rdfs:comment "Receive and respond to general customer inquiries and requests for quotes."@en ;
    rdfs:label "Process Inquiry and Quote (Deliver Make To Order Product)"@en ;
    scor:isStepOf scor:DeliverMakeToOrderProduct ;
    skos:notation "sD2.1" ;
    rdfs:isDefinedBy scor: ;
    vs:term_status "stable" ;
    dct:modified "2015-11-05"^^xsd:date ;
 .

scor:ReceiveConfigureEnterValidateOrder
    rdf:type owl:Class ;
    rdfs:subClassOf scor:DeliverMakeToOrderProductStep ;  
    rdfs:comment "Receive orders from the customer and enter them into a company's order processing system."@en ;
    rdfs:label "Receive, Configure, Enter and Validate Order"@en ;
    scor:isStepOf scor:DeliverMakeToOrderProduct ;
    skos:notation "sD2.2" ;
    rdfs:isDefinedBy scor: ;
    vs:term_status "stable" ;
    dct:modified "2015-11-05"^^xsd:date ;
 .

scor:DMOPReserveInventoryDetermineDeliveryDate
    rdf:type owl:Class ;
    rdfs:subClassOf scor:DeliverMakeToOrderProductStep ;  
    rdfs:comment "Inventory and/or planned capacity is identified and reserved for specific orders, and a delivery date is committed and scheduled."@en ;
    rdfs:label "Reserve Inventory and Determine Delivery Date (Deliver Make To Order Product)"@en ;
    scor:isStepOf scor:DeliverMakeToOrderProduct ;
    skos:notation "sD2.3" ;
    rdfs:isDefinedBy scor: ;
    vs:term_status "stable" ;
    dct:modified "2015-11-05"^^xsd:date ;
 .

scor:DMOPConsolidateOrders
    rdf:type owl:Class ;
    rdfs:subClassOf scor:DeliverMakeToOrderProductStep ;  
    rdfs:comment "The process of analyzing orders to determine the groupings that result in least cost/best service fulfillment and transportation."@en ;
    rdfs:label "Consolidate Orders (Deliver Make To Order Product)"@en ;
    scor:isStepOf scor:DeliverMakeToOrderProduct ;
    skos:notation "sD2.4" ;
    rdfs:isDefinedBy scor: ;
    vs:term_status "stable" ;
    dct:modified "2015-11-05"^^xsd:date ;
 .

scor:DMOPBuildLoads
    rdf:type owl:Class ;
    rdfs:subClassOf scor:DeliverMakeToOrderProductStep ;  
    rdfs:comment "Transportation modes are selected and efficient loads are built."@en ;
    rdfs:label "Build Loads (Deliver Make To Order Product)"@en ;
    scor:isStepOf scor:DeliverMakeToOrderProduct ;
    skos:notation "sD2.5" ;
    rdfs:isDefinedBy scor: ;
    vs:term_status "stable" ;
    dct:modified "2015-11-05"^^xsd:date ;
 .

scor:DMOPRouteShipments
    rdf:type owl:Class ;
    rdfs:subClassOf scor:DeliverMakeToOrderProductStep ;  
    rdfs:comment "Loads are consolidated and routed by mode, lane, and location."@en ;
    rdfs:label "Route Shipments (Deliver Make To Order Product)"@en ;
    scor:isStepOf scor:DeliverMakeToOrderProduct ;
    skos:notation "sD2.6" ;
    rdfs:isDefinedBy scor: ;
    vs:term_status "stable" ;
    dct:modified "2015-11-05"^^xsd:date ;
 .

scor:DMOPSelectCarriersRateShipments
    rdf:type owl:Class ;
    rdfs:subClassOf scor:DeliverMakeToOrderProductStep ;  
    rdfs:comment "Specific carriers are selected by lowest cost per route and shipments are rated and tendered."@en ;
    rdfs:label "Select Carriers and Rate Shipments (Deliver Make To Order Product)"@en ;
    scor:isStepOf scor:DeliverMakeToOrderProduct ;
    skos:notation "sD2.7" ;
    rdfs:isDefinedBy scor: ;
    vs:term_status "stable" ;
    dct:modified "2015-11-05"^^xsd:date ;
 .

scor:DMOPReceiveProductFromSourceMake
    rdf:type owl:Class ;
    rdfs:subClassOf scor:DeliverMakeToOrderProductStep ;  
    rdfs:comment "The activities such as receiving product, verifying, recording product receipt, determining put-away location, putting away and recording location for goods received from either Make or Source."@en ;
    rdfs:label "Receive Product from Source or Make (Deliver Make To Order Product)"@en ;
    scor:isStepOf scor:DMOPPickProduct ;
    skos:notation "sD2.8" ;
    rdfs:isDefinedBy scor: ;
    vs:term_status "stable" ;
    dct:modified "2015-11-05"^^xsd:date ;
 .

scor:DMOPPickProduct
    rdf:type owl:Class ;
    rdfs:subClassOf scor:DeliverMakeToOrderProductStep ;  
    rdfs:comment "The series of activities including retrieving orders to pick, verifying inventory availability, building the pick wave, picking the product, recording the pick and delivering product to packing area in response to an order."@en ;
    rdfs:label "Pick Product (Deliver Make To Order Product)"@en ;
    scor:isStepOf scor:DeliverMakeToOrderProduct ;
    skos:notation "sD2.9" ;
    rdfs:isDefinedBy scor: ;
    vs:term_status "stable" ;
    dct:modified "2015-11-05"^^xsd:date ;
 .

scor:DMOPPackProduct
    rdf:type owl:Class ;
    rdfs:subClassOf scor:DeliverMakeToOrderProductStep ;  
    rdfs:comment "The activities such as sorting / combining the products, packing / kitting the products, paste labels, barcodes etc. and delivering the products to the shipping area for loading."@en ;
    rdfs:label "Pack Product (Make To Order Product)"@en ;
    scor:isStepOf scor:DeliverMakeToOrderProduct ;
    skos:notation "sD2.10" ;
    rdfs:isDefinedBy scor: ;
    vs:term_status "stable" ;
    dct:modified "2015-11-05"^^xsd:date ;
 .

scor:DMOPLoadProductGenerateShippingDocs
    rdf:type owl:Class ;
    rdfs:subClassOf scor:DeliverMakeToOrderProductStep ;  
    rdfs:comment "The series of tasks including placing/loading product onto modes of transportation, and generating the documentation necessary to meet internal, customer, carrier and government needs."@en ;
    rdfs:label "Load Product Generate Shipping Docs"@en ;
    scor:isStepOf scor:DeliverMakeToOrderProduct ;
    skos:notation "sD2.11" ;
    rdfs:isDefinedBy scor: ;
    vs:term_status "stable" ;
    dct:modified "2015-11-05"^^xsd:date ;
 .

scor:DMOPShipProduct
    rdf:type owl:Class ;
    rdfs:subClassOf scor:DeliverMakeToOrderProductStep ;  
    rdfs:comment "The process of shipping the product to the customer site."@en ;
    rdfs:label "Ship Product (Deliver Make To Order Product)"@en ;
    scor:isStepOf scor:DeliverMakeToOrderProduct ;
    skos:notation "sD2.12" ;
    rdfs:isDefinedBy scor: ;
    vs:term_status "stable" ;
    dct:modified "2015-11-05"^^xsd:date ;
 .

scor:DMOPReceiveVerifyProductByCustomer
    rdf:type owl:Class ;
    rdfs:subClassOf scor:DeliverMakeToOrderProductStep ;  
    rdfs:comment "The process of receiving the shipment at the customer (either at customer site or at shipping area in case of self-collection) and verifying that the order was shipped complete and that the product meets delivery terms."@en ;
    rdfs:label "Receive and verify Product by Customer (Deliver Make To Order Product)"@en ;
    scor:isStepOf scor:DeliverMakeToOrderProduct ;
    skos:notation "sD2.13" ;
    rdfs:isDefinedBy scor: ;
    vs:term_status "stable" ;
    dct:modified "2015-11-05"^^xsd:date ;
 .

scor:DMOPInstallProduct
    rdf:type owl:Class ;
    rdfs:subClassOf scor:DeliverMakeToOrderProductStep ;  
    rdfs:comment "the process of preparing, stable and installing the product at the customer site."@en ;
    rdfs:label "Install Product (Deliver Make To Order Product)"@en ;
    scor:isStepOf scor:DeliverMakeToOrderProduct ;
    skos:notation "sD2.14" ;
    rdfs:isDefinedBy scor: ;
    vs:term_status "stable" ;
    dct:modified "2015-11-05"^^xsd:date ;
 .

scor:DMOPInvoice
    rdf:type owl:Class ;
    rdfs:subClassOf scor:DeliverMakeToOrderProductStep ;  
    rdfs:comment "A signal is sent to the financial organization that the order has been shipped and that the billing process should begin and payment be received or be closed out if payment has already been received."@en ;
    rdfs:label "Invoice (Deliver Make To Order Product)"@en ;
    scor:isStepOf scor:DeliverMakeToOrderProduct ;
    skos:notation "sD2.15" ;
    rdfs:isDefinedBy scor: ;
    vs:term_status "stable" ;
    dct:modified "2015-11-05"^^xsd:date ;
 .

# Deliver Engineer-to-Order Product

scor:ObtainRespondToRFPRFQ
    rdf:type owl:Class ;
    rdfs:subClassOf scor:DeliverEngineerToOrderProductStep ;  
    rdfs:comment "The process of receiving a request for proposal or request for quote, evaluating the request (estimating the schedule, developing costs estimates, establishing price), and responding to the potential customer."@en ;
    rdfs:label "Obtain and Respond to RFP-RFQ"@en ;
    scor:isStepOf scor:DeliverEngineerToOrderProduct ;
    skos:notation "sD3.1" ;
    rdfs:isDefinedBy scor: ;
    vs:term_status "stable" ;
    dct:modified "2015-11-05"^^xsd:date ;
 .

scor:NegotiateReceiveContract
    rdf:type owl:Class ;
    rdfs:subClassOf scor:DeliverEngineerToOrderProductStep ;  
    rdfs:comment "The process of negotiating order details with customer (e.g., price, schedule, product performance) and finalizing the contract."@en ;
    rdfs:label "Negotiate and Receive Contract"@en ;
    scor:isStepOf scor:DeliverEngineerToOrderProduct ;
    skos:notation "sD3.2" ;
    rdfs:isDefinedBy scor: ;
    vs:term_status "stable" ;
    dct:modified "2015-11-05"^^xsd:date ;
 .

scor:EnterOrderCommitResourcesLaunchProgram
    rdf:type owl:Class ;
    rdfs:subClassOf scor:DeliverEngineerToOrderProductStep ;  
    rdfs:comment "The process of entering/finalizing the customers order, approving the planned resources (e.g., engineering, manufacturing, etc.) and officially launching the program."@en ;
    rdfs:label "Enter Order, Commit Resources Launch Program"@en ;
    scor:isStepOf scor:DeliverEngineerToOrderProduct ;
    skos:notation "sD3.3" ;
    rdfs:isDefinedBy scor: ;
    vs:term_status "stable" ;
    dct:modified "2015-11-05"^^xsd:date ;
 .

scor:ScheduleInstallation
    rdf:type owl:Class ;
    rdfs:subClassOf scor:DeliverEngineerToOrderProductStep ;  
    rdfs:comment "The process of evaluating the design and build schedules relative to customer requested installation date to determine installation schedule."@en ;
    rdfs:label "Schedule Installation"@en ;
    scor:isStepOf scor:DeliverEngineerToOrderProduct ;
    skos:notation "sD3.4" ;
    rdfs:isDefinedBy scor: ;
    vs:term_status "stable" ;
    dct:modified "2015-11-05"^^xsd:date ;
 .

scor:DEOPBuildLoads
    rdf:type owl:Class ;
    rdfs:subClassOf scor:DeliverEngineerToOrderProductStep ;  
    rdfs:comment "The process of evaluating the design and build schedules relative to customer requested installation date to determine installation schedule."@en ;
    rdfs:label "Build Loads (Deliver Engineer To Order Product)"@en ;
    scor:isStepOf scor:DeliverEngineerToOrderProduct ;
    skos:notation "sD3.5" ;
    rdfs:isDefinedBy scor: ;
    vs:term_status "stable" ;
    dct:modified "2015-11-05"^^xsd:date ;
 .

scor:DEOPRouteShipments
    rdf:type owl:Class ;
    rdfs:subClassOf scor:DeliverEngineerToOrderProductStep ;  
    rdfs:comment "Loads are consolidated and routed by mode, lane, and location."@en ;
    rdfs:label "Route Shipments (Deliver Engineer To Order Product)"@en ;
    scor:isStepOf scor:DeliverEngineerToOrderProduct ;
    skos:notation "sD3.6" ;
    rdfs:isDefinedBy scor: ;
    vs:term_status "stable" ;
    dct:modified "2015-11-05"^^xsd:date ;
 .

scor:DEOPSelectCarriersRateShipments
    rdf:type owl:Class ;
    rdfs:subClassOf scor:DeliverEngineerToOrderProductStep ;  
    rdfs:comment "Specific carriers are selected by lowest cost per route and shipments are rated and tendered."@en ;
    rdfs:label "Select Carriers Rate Shipments"@en ;
    scor:isStepOf scor:DeliverEngineerToOrderProduct ;
    skos:notation "sD3.7" ;
    rdfs:isDefinedBy scor: ;
    vs:term_status "stable" ;
    dct:modified "2015-11-05"^^xsd:date ;
 .

scor:DEOPReceiveProductFromSourceMake
    rdf:type owl:Class ;
    rdfs:subClassOf scor:DeliverEngineerToOrderProductStep ;  
    rdfs:comment "The activities such as receiving product, verifying, recording product receipt, determining put-away location, putting away and recording location for goods received from either Make or Source."@en ;
    rdfs:label "Receive Product from Source or Make (Deliver Engineer To Order Product)"@en ;
    scor:isStepOf scor:DeliverEngineerToOrderProduct ;
    skos:notation "sD3.8" ;
    rdfs:isDefinedBy scor: ;
    vs:term_status "stable" ;
    dct:modified "2015-11-05"^^xsd:date ;
 .

scor:DEOPPickProduct
    rdf:type owl:Class ;
    rdfs:subClassOf scor:DeliverEngineerToOrderProductStep ;  
    rdfs:comment "The series of activities including retrieving orders to pick, verifying inventory availability, building the pick wave, picking the product, recording the pick and delivering product to packing area in response to an order."@en ;
    rdfs:label "Pick Product (Deliver Engineer To Order Product)"@en ;
    scor:isStepOf scor:DeliverEngineerToOrderProduct ;
    skos:notation "sD3.9" ;
    rdfs:isDefinedBy scor: ;
    vs:term_status "stable" ;
    dct:modified "2015-11-05"^^xsd:date ;
 .

scor:DEOPPackProduct
    rdf:type owl:Class ;
    rdfs:subClassOf scor:DeliverEngineerToOrderProductStep ;  
    rdfs:comment "The activities such as sorting / combining the products, packing / kitting the products, paste labels, barcodes etc. and delivering the products to the shipping area for loading."@en ;
    rdfs:label "Pack Product (Deliver Engineer To Order Product)"@en ;
    scor:isStepOf scor:DeliverEngineerToOrderProduct ;
    skos:notation "sD3.10" ;
    rdfs:isDefinedBy scor: ;
    vs:term_status "stable" ;
    dct:modified "2015-11-05"^^xsd:date ;
 .

scor:DEOPLoadProductGenerateShippingDocs
    rdf:type owl:Class ;
    rdfs:subClassOf scor:DeliverEngineerToOrderProductStep ;  
    rdfs:comment "The series of tasks including placing/loading product onto modes of transportation, and generating the documentation necessary to meet internal, customer, carrier and government needs."@en ;
    rdfs:label "Load Product & Generate Shipping Docs"@en ;
    scor:isStepOf scor:DeliverEngineerToOrderProduct ;
    skos:notation "sD3.11" ;
    rdfs:isDefinedBy scor: ;
    vs:term_status "stable" ;
    dct:modified "2015-11-05"^^xsd:date ;
 .

scor:DEOPShipProduct
    rdf:type owl:Class ;
    rdfs:subClassOf scor:DeliverEngineerToOrderProductStep ;  
    rdfs:comment "The process of shipping the product to the customer site."@en ;
    rdfs:label "Ship Product"@en ;
    scor:isStepOf scor:DeliverEngineerToOrderProduct ;
    skos:notation "sD3.12" ;
    rdfs:isDefinedBy scor: ;
    vs:term_status "stable" ;
    dct:modified "2015-11-05"^^xsd:date ;
 .

scor:DEOPReceiveVerifyProductByCustomer
    rdf:type owl:Class ;
    rdfs:subClassOf scor:DeliverEngineerToOrderProductStep ;  
    rdfs:comment "The process of receiving the shipment (either at customer site or at shipping area in case of self-collection) and verifying that the order was shipped complete and that the product meets delivery terms."@en ;
    rdfs:label "Receive and verify Product by Customer (Deliver Engineer To Order Product)"@en ;
    scor:isStepOf scor:DeliverEngineerToOrderProduct ;
    skos:notation "sD3.13" ;
    rdfs:isDefinedBy scor: ;
    vs:term_status "stable" ;
    dct:modified "2015-11-05"^^xsd:date ;
 .

scor:DEOPInstallProduct
    rdf:type owl:Class ;
    rdfs:subClassOf scor:DeliverEngineerToOrderProductStep ;  
    rdfs:comment "The process of preparing, stable and installing the product at the customer site. The product is fully functional upon completion."@en ;
    rdfs:label "Install Product (Deliver Engineer To Order Product)"@en ;
    scor:isStepOf scor:DeliverEngineerToOrderProduct ;
    skos:notation "sD3.14" ;
    rdfs:isDefinedBy scor: ;
    vs:term_status "stable" ;
    dct:modified "2015-11-05"^^xsd:date ;
 .

scor:DEOPInvoice
    rdf:type owl:Class ;
    rdfs:subClassOf scor:DeliverEngineerToOrderProductStep ;  
    rdfs:comment "A signal is sent to the financial organization that the order has been shipped and that the billing process should begin and payment be received or be closed out if payment has already been received."@en ;
    rdfs:label "Invoice (Deliver Engineer To Order Product)"@en ;
    scor:isStepOf scor:DeliverEngineerToOrderProduct ;
    skos:notation "sD3.15" ;
    rdfs:isDefinedBy scor: ;
    vs:term_status "stable" ;
    dct:modified "2015-11-05"^^xsd:date ;
 .

# DeliverRetailProduct

scor:GenerateStockingSchedule
    rdf:type owl:Class ;
    rdfs:subClassOf scor:DeliverRetailProductStep ;  
    rdfs:comment "The process of scheduling resources to support item-stocking requirements."@en ;
    rdfs:label "Generate Stocking Schedule"@en ;
    scor:isStepOf scor:DeliverRetailProduct ;
    skos:notation "sD4.1" ;
    rdfs:isDefinedBy scor: ;
    vs:term_status "stable" ;
    dct:modified "2015-11-05"^^xsd:date ;
 .

scor:ReceiveProductAtStore
    rdf:type owl:Class ;
    rdfs:subClassOf scor:DeliverRetailProductStep ;  
    rdfs:comment "The activities such as receiving product, verifying, recording product receipt, determining put-away location, putting away and recording location that a company performs at its own stores."@en ;
    rdfs:label "Receive Product at Store"@en ;
    scor:isStepOf scor:DeliverRetailProduct ;
    skos:notation "sD4.2" ;
    rdfs:isDefinedBy scor: ;
    vs:term_status "stable" ;
    dct:modified "2015-11-05"^^xsd:date ;
 .

scor:PickProductFromBackroom
    rdf:type owl:Class ;
    rdfs:subClassOf scor:DeliverRetailProductStep ;  
    rdfs:comment "The process of retrieving restocking orders to pick, determining inventory availability, building a pick wave, picking item and quantity from a designated backroom warehouse location, recording the resulting inventory transaction, and delivering the product to point of stock."@en ;
    rdfs:label "Pick Product from backroom"@en ;
    scor:isStepOf scor:DeliverRetailProduct ;
    skos:notation "sD4.3" ;
    rdfs:isDefinedBy scor: ;
    vs:term_status "stable" ;
    dct:modified "2015-11-05"^^xsd:date ;
 .

scor:StockShelf
    rdf:type owl:Class ;
    rdfs:subClassOf scor:DeliverRetailProductStep ;  
    rdfs:comment "For restocks, the tasks associated with identifying the item location, stocking the shelf according to merchandise plans, and recording the appropriate inventory transaction."@en ;
    rdfs:label "Stock Shelf"@en ;
    scor:isStepOf scor:DeliverRetailProduct ;
    skos:notation "sD4.4" ;
    rdfs:isDefinedBy scor: ;
    vs:term_status "stable" ;
    dct:modified "2015-11-05"^^xsd:date ;
 .

scor:FillShoppingCart
    rdf:type owl:Class ;
    rdfs:subClassOf scor:DeliverRetailProductStep ;  
    rdfs:comment "Typical set of tasks associated with product selection, storage and movement through to checkout."@en ;
    rdfs:label "Fill Shopping Cart"@en ;
    scor:isStepOf scor:DeliverRetailProduct ;
    skos:notation "sD4.5" ;
    rdfs:isDefinedBy scor: ;
    vs:term_status "stable" ;
    dct:modified "2015-11-05"^^xsd:date ;
 .

scor:Checkout
    rdf:type owl:Class ;
    rdfs:subClassOf scor:DeliverRetailProductStep ;  
    rdfs:comment "The processes and tasks associated with product checkout including scanning, method of payment, credit application and approval, service agreement, order confirmation, and/or invoice or receipt."@en ;
    rdfs:label "Checkout"@en ;
    scor:isStepOf scor:DeliverRetailProduct ;
    skos:notation "sD4.6" ;
    rdfs:isDefinedBy scor: ;
    vs:term_status "stable" ;
    dct:modified "2015-11-05"^^xsd:date ;
 .

scor:DeliverInstall
    rdf:type owl:Class ;
    rdfs:subClassOf scor:DeliverRetailProductStep ;  
    rdfs:comment "The process of preparing and installing the product at the customer site. The product is fully functional upon completion."@en ;
    rdfs:label "Deliver and/or install"@en ;
    scor:isStepOf scor:DeliverRetailProduct ;
    skos:notation "sD4.7" ;
    rdfs:isDefinedBy scor: ;
    vs:term_status "stable" ;
    dct:modified "2015-11-05"^^xsd:date ;
 .

# Source Return Defective Product

scor:IdentifyDefectiveProductCondition
    rdf:type owl:Class ;
    rdfs:subClassOf scor:SourceReturnDefectiveProductStep ;
    rdfs:comment "The process where the customer utilizes planned policies, business rules and product operating conditions inspection as criteria to identify and confirm that material is excess to requirements defective."@en ;
    rdfs:label "Identify Defective Product Condition"@en ;
    scor:isStepOf scor:SourceReturnDefectiveProduct ;
    skos:notation "sSR1.1" ;
    rdfs:isDefinedBy scor: ;
    vs:term_status "stable" ;
    dct:modified "2015-11-05"^^xsd:date ;
.

scor:DispositionDefectiveProduct
    rdf:type owl:Class ;
    rdfs:subClassOf scor:SourceReturnDefectiveProductStep ;
    rdfs:comment "The process of the customer determining whether to return the defective item and the appropriate source contact for a return authorization."@en ;
    rdfs:label "Disposition Defective Product"@en ;
    scor:isStepOf scor:SourceReturnDefectiveProduct ;
    skos:notation "sSR1.2" ;
    rdfs:isDefinedBy scor: ;
    vs:term_status "stable" ;
    dct:modified "2015-11-05"^^xsd:date ;
.

scor:RequestDefectiveProductReturnAuthorization
    rdf:type owl:Class ;
    rdfs:subClassOf scor:SourceReturnDefectiveProductStep ;
    rdfs:comment "The process of a customer requesting and obtaining authorization, from last known holder or designated return center, for the return of defective product. Additionally, the customer and last known holder or designated return center would discuss enabling conditions such as return replacement or credit, packaging, handling, transportation and import / export requirements to facilitate the efficient return of the defective product."@en ;
    rdfs:label "Request Defective Product Return Authorization"@en ;
    scor:isStepOf scor:SourceReturnDefectiveProduct ;
    skos:notation "sSR1.3" ;
    rdfs:isDefinedBy scor: ;
    vs:term_status "stable" ;
    dct:modified "2015-11-05"^^xsd:date ;
.

scor:ScheduleDefectiveProductShipment
    rdf:type owl:Class ;
    rdfs:subClassOf scor:SourceReturnDefectiveProductStep ;
    rdfs:comment "The process where the customer develops the schedule for a carrier to pick-up for delivery of the defective product. Activities include selecting the carrier and rates, preparing the item for transfer, preparing scheduling documentation and managing overall scheduling administration."@en ;
    rdfs:label "Schedule Defective Product Shipment"@en ;
    scor:isStepOf scor:SourceReturnDefectiveProduct ;
    skos:notation "sSR1.4" ;
    rdfs:isDefinedBy scor: ;
    vs:term_status "stable" ;
    dct:modified "2015-11-05"^^xsd:date ;
.

scor:ReturnDefectiveProduct
    rdf:type owl:Class ;
    rdfs:subClassOf scor:SourceReturnDefectiveProductStep ;
    rdfs:comment "The process where the customer packages, and handles the defective product in preparation for shipping in accord with pre-determined conditions. The product is then provided by the customer to the carrier who physically transports the product and its associated documentation to the last known holder or designated return center."@en ;
    rdfs:label "Return Defective Product"@en ;
    scor:isStepOf scor:SourceReturnDefectiveProduct ;
    skos:notation "sSR1.5" ;
    rdfs:isDefinedBy scor: ;
    vs:term_status "stable" ;
    dct:modified "2015-11-05"^^xsd:date ;
.
# Deliver Return Defective Product

scor:AuthorizeDefectiveProductReturn
    rdf:type owl:Class ;
    rdfs:subClassOf scor:DeliverReturnDefectiveProductStep ;
    rdfs:comment "The process where the last known holder or designated return center receives a defective product return authorization request from a customer, determines if the item can be accepted and communicates decision to the customer. Accepting the request would include negotiating the conditions of the return with the customer, including authorizing return replacement or credit. Rejecting the request would include providing a reason for the rejection to the customer."@en ;
    rdfs:label "Authorize Defective Product Return"@en ;
    scor:isStepOf scor:DeliverReturnDefectiveProduct ;
    skos:notation "sDR1.1" ;
    rdfs:isDefinedBy scor: ;
    vs:term_status "stable" ;
    dct:modified "2015-11-05"^^xsd:date ;
.

scor:ScheduleDefectiveReturnReceipt
    rdf:type owl:Class ;
    rdfs:subClassOf scor:DeliverReturnDefectiveProductStep ;
    rdfs:comment "The process where the last known holder or designated return center evaluates the defective product handling requirements including negotiated conditions and develops a schedule that tells the Customer when to ship the product. The scheduling activity would also inform Receiving when to expect the shipment and where to send the product, for disposition, upon receipt."@en ;
    rdfs:label "Schedule Defective Return Receipt"@en ;
    scor:isStepOf scor:DeliverReturnDefectiveProduct ;
    skos:notation "sDR1.2" ;
    rdfs:isDefinedBy scor: ;
    vs:term_status "stable" ;
    dct:modified "2015-11-05"^^xsd:date ;
.

scor:ReceiveDefectiveProduct
    rdf:type owl:Class ;
    rdfs:subClassOf scor:DeliverReturnDefectiveProductStep ;
    rdfs:comment "The process where the last known holder or designated return center receives and verifies the returned defective product against the return authorization and other documentation and prepares the item for transfer."@en ;
    rdfs:label "Receive Defective Product"@en ;
    scor:isStepOf scor:DeliverReturnDefectiveProduct ;
    skos:notation "sDR1.3" ;
    rdfs:isDefinedBy scor: ;
    vs:term_status "stable" ;
    dct:modified "2015-11-05"^^xsd:date ;
.

scor:TransferDefectiveProduct
    rdf:type owl:Class ;
    rdfs:subClassOf scor:DeliverReturnDefectiveProductStep ;
    rdfs:comment "The process where the last known holder or designated return center transfers the defective product to the appropriate process to implement the disposition decision."@en ;
    rdfs:label "Transfer Defective Product"@en ;
    scor:isStepOf scor:DeliverReturnDefectiveProduct ;
    skos:notation "sDR1.4" ;
    rdfs:isDefinedBy scor: ;
    vs:term_status "stable" ;
    dct:modified "2015-11-05"^^xsd:date ;
.


# Return MRO Product

scor:IdentifyMROProductCondition
    rdf:type owl:Class ;
    rdfs:subClassOf scor:SourceReturnMROProductStep ;
    rdfs:comment "The process where the customer utilizes pre-determined MRO policies, business rules and product operating conditions as criteria to identify and confirm that an item requires maintenance, repair, overhaul or disposal. Includes operating failures and planned maintenance requirements."@en ;
    rdfs:label "Identify MRO Product Condition"@en ;
    scor:isStepOf scor:SourceReturnMROProduct ;
    skos:notation "sSR2.1" ;
    rdfs:isDefinedBy scor: ;
    vs:term_status "stable" ;
    dct:modified "2015-11-05"^^xsd:date ;
.

scor:DispositionMROProduct
    rdf:type owl:Class ;
    rdfs:subClassOf scor:SourceReturnMROProductStep ;
    rdfs:comment "The process of the customer determining whether to service the item, what service is required, and who the appropriate service provider would be to service the item. Outputs include a decision to: (1) send a return authorization request to a service provider, (2) send the product back into service without requiring a return authorization request, or (3) discard the item."@en ;
    rdfs:label "Disposition MRO Product"@en ;
    scor:isStepOf scor:SourceReturnMROProduct ;
    skos:notation "sSR2.2" ;
    rdfs:isDefinedBy scor: ;
    vs:term_status "stable" ;
    dct:modified "2015-11-05"^^xsd:date ;
.

scor:RequestMROReturnAuthorization
    rdf:type owl:Class ;
    rdfs:subClassOf scor:SourceReturnMROProductStep ;
    rdfs:comment "The process of a customer requesting and obtaining authorization, from a service provider, for the return of an MRO product. In addition to discussing the MRO issue, the customer and service provider would discuss enabling conditions such as return replacement or credit, packaging, handling, transportation and import / export requirements to facilitate the efficient return of the MRO product to the service provider. The customer may need to go through several return authorization iterations with multiple service providers before authorization is received."@en ;
    rdfs:label "Request MRO Return Authorization"@en ;
    scor:isStepOf scor:SourceReturnMROProduct ;
    skos:notation "sSR2.3" ;
    rdfs:isDefinedBy scor: ;
    vs:term_status "stable" ;
    dct:modified "2015-11-05"^^xsd:date ;
.

scor:ScheduleMROShipment
    rdf:type owl:Class ;
    rdfs:subClassOf scor:SourceReturnMROProductStep ;
    rdfs:comment "The process where the customer develops the schedule for a carrier to pick-up and deliver the MRO product. Activities include selecting the carrier and rates, preparing the item for transfer, preparing scheduling documentation and managing overall scheduling administration."@en ;
    rdfs:label "Schedule MRO Shipment"@en ;
    scor:isStepOf scor:SourceReturnMROProduct ;
    skos:notation "sSR2.4" ;
    rdfs:isDefinedBy scor: ;
    vs:term_status "stable" ;
    dct:modified "2015-11-05"^^xsd:date ;
.

scor:ReturnMROPRoduct
    rdf:type owl:Class ;
    rdfs:subClassOf scor:SourceReturnMROProductStep ;
    rdfs:comment "The process where the customer packages, and handles the MRO product in preparation for shipping in accord with pre-determined conditions. The product is then provided by the customer to the carrier who physically transports the product and its associated documentation to the service provider."@en ;
    rdfs:label "Return MRO Shipment"@en ;
    scor:isStepOf scor:SourceReturnMROProduct ;
    skos:notation "sSR2.5" ;
    rdfs:isDefinedBy scor: ;
    vs:term_status "stable" ;
    dct:modified "2015-11-05"^^xsd:date ;
.


# Deliver Return MRO Product

 scor:AuthorizeMROProductReturn
    rdf:type owl:Class ;
    rdfs:subClassOf scor:DeliverReturnMROProductStep ;
    rdfs:comment "The process where a service provider receives an MRO product return authorization request from a customer, determines if the item can be accepted for MRO and communicates their decision to the customer. Accepting the request would include negotiating the conditions of the return with the customer, including authorizing return replacement or credit. Rejecting the request would include providing a reason for the rejection to the customer."@en ;
    rdfs:label "Authorize MRO Product Return"@en ;
    scor:isStepOf scor:DeliverReturnMROProduct ;
    skos:notation "sDR2.1" ;
    rdfs:isDefinedBy scor: ;
    vs:term_status "stable" ;
    dct:modified "2015-11-05"^^xsd:date ;
.

 scor:ScheduleMROReturnReceipt
    rdf:type owl:Class ;
    rdfs:subClassOf scor:DeliverReturnMROProductStep ;
    rdfs:comment "The process where the service provider evaluates the MRO service requirements including negotiated conditions and develops a schedule that tells the Customer when to ship the part. The scheduling activity would also inform Receiving when to expect the shipment and where to send the part, for induction or storage, upon receipt."@en ;
    rdfs:label "Schedule MRO Return Receipt"@en ;
    scor:isStepOf scor:DeliverReturnMROProduct ;
    skos:notation "sDR2.2" ;
    rdfs:isDefinedBy scor: ;
    vs:term_status "stable" ;
    dct:modified "2015-11-05"^^xsd:date ;
.

 scor:ReceiveMROProduct
    rdf:type owl:Class ;
    rdfs:subClassOf scor:DeliverReturnMROProductStep ;
    rdfs:comment "The process where the service provider receives and verifies the returned MRO item against the return authorization and other documentation and prepares the item for transfer."@en ;
    rdfs:label "Receive MRO Product"@en ;
    scor:isStepOf scor:DeliverReturnMROProduct ;
    skos:notation "sDR2.3" ;
    rdfs:isDefinedBy scor: ;
    vs:term_status "stable" ;
    dct:modified "2015-11-05"^^xsd:date ;
.

 scor:TransferMROProduct
    rdf:type owl:Class ;
    rdfs:subClassOf scor:DeliverReturnMROProductStep ;
    rdfs:comment "The process where the service provider transfers the MRO product to the appropriate process to implement the disposition decision."@en ;
    rdfs:label "Transfer MRO Product"@en ;
    scor:isStepOf scor:DeliverReturnMROProduct ;
    skos:notation "sDR2.4" ;
    rdfs:isDefinedBy scor: ;
    vs:term_status "stable" ;
    dct:modified "2015-11-05"^^xsd:date ;
.


# Source Return Excess Product

 scor:IdentifyExcessProductCondition
    rdf:type owl:Class ;
    rdfs:subClassOf scor:SourceReturnExcessProductStep ;
    rdfs:comment "The process where the customer utilizes planned policies, business rules and product inspection as criteria to identify and confirm that material is in excess of the current requirements."@en ;
    rdfs:label "Identify Excess Product Condition"@en ;
    scor:isStepOf scor:SourceReturnExcessProduct ;
    skos:notation "sSR3.1" ;
    rdfs:isDefinedBy scor: ;
    vs:term_status "stable" ;
    dct:modified "2015-11-05"^^xsd:date ;
.

 scor:DispositionExcessProduct
    rdf:type owl:Class ;
    rdfs:subClassOf scor:SourceReturnExcessProductStep ;
    rdfs:comment "The process of the customer determining whether to return the excess material and identification of a designated return center a return authorization."@en ;
    rdfs:label "Disposition Excess Product"@en ;
    scor:isStepOf scor:SourceReturnExcessProduct ;
    skos:notation "sSR3.2" ;
    rdfs:isDefinedBy scor: ;
    vs:term_status "stable" ;
    dct:modified "2015-11-05"^^xsd:date ;
.

 scor:RequestExcessProductReturnAuthorization
    rdf:type owl:Class ;
    rdfs:subClassOf scor:SourceReturnExcessProductStep ;
    rdfs:comment "The process of a customer requesting and obtaining authorization, from the designated return center, for the return of excess product. Additionally, the customer and designated return center would negotiate enabling conditions such as return credit or cash discount, packaging, handling, transportation and import / export requirements to facilitate the efficient return of the excess product."@en ;
    rdfs:label "Request Excess Product Return Authorization"@en ;
    scor:isStepOf scor:SourceReturnExcessProduct ;
    skos:notation "sSR3.3" ;
    rdfs:isDefinedBy scor: ;
    vs:term_status "stable" ;
    dct:modified "2015-11-05"^^xsd:date ;
.

 scor:ScheduleExcessProductShipment
    rdf:type owl:Class ;
    rdfs:subClassOf scor:SourceReturnExcessProductStep ;
    rdfs:comment "The process where the customer develops the schedule for a carrier to pick-up the excess product. Activities include selecting the carrier and rates, preparing the item for transfer, preparing scheduling documentation and managing overall scheduling administration."@en ;
    rdfs:label "Schedule Excess Product Shipment"@en ;
    scor:isStepOf scor:SourceReturnExcessProduct ;
    skos:notation "sSR3.4" ;
    rdfs:isDefinedBy scor: ;
    vs:term_status "stable" ;
    dct:modified "2015-11-05"^^xsd:date ;
.

 scor:ReturnExcessProduct
    rdf:type owl:Class ;
    rdfs:subClassOf scor:SourceReturnExcessProductStep ;
    rdfs:comment "The process where the customer packages, and handles the excess product in preparation for shipping in accord with pre-determined conditions. The product is then provided by the customer to the carrier who physically transports the product and its associated documentation to the last known holder or designated return center."@en ;
    rdfs:label "Return Excess Product"@en ;
    scor:isStepOf scor:SourceReturnExcessProduct ;
    skos:notation "sSR3.5" ;
    rdfs:isDefinedBy scor: ;
    vs:term_status "stable" ;
    dct:modified "2015-11-05"^^xsd:date ;
.

# Deliver Return Excess Product

 scor:AuthorizeExcessProductReturn
    rdf:type owl:Class ;
    rdfs:subClassOf scor:DeliverReturnExcessProductStep ;
    rdfs:comment "The process where the designated return center receives an excess product return authorization request from a customer, determines if the item can be accepted and communicates their decision to the customer. Accepting the request would include negotiating the conditions of the return with the customer, including authorizing credit or cash discount. Rejecting the request would include providing a reason for the rejection to the customer."@en ;
    rdfs:label "Authorize Excess Product Return"@en ;
    scor:isStepOf scor:DeliverReturnExcessProduct ;
    skos:notation "sDR3.1" ;
    rdfs:isDefinedBy scor: ;
    vs:term_status "stable" ;
    dct:modified "2015-11-05"^^xsd:date ;
.

 scor:ScheduleExcessReturnReceipt
    rdf:type owl:Class ;
    rdfs:subClassOf scor:DeliverReturnExcessProductStep ;
    rdfs:comment "The process where the l designated return center evaluates an authorized excess material return toolsdetermine packaging and handling requirements. This assessment will lead to the development of a return disposition decision and a return schedule with terms and conditions that will tell the Customer how and when to ship the product. The scheduling activity would also inform the Return Center?s Receiving department when to expect the shipment and where to send the product, for disposition, upon receipt."@en ;
    rdfs:label "Schedule Excess Return Receipt"@en ;
    scor:isStepOf scor:DeliverReturnExcessProduct ;
    skos:notation "sDR3.2" ;
    rdfs:isDefinedBy scor: ;
    vs:term_status "stable" ;
    dct:modified "2015-11-05"^^xsd:date ;
.

 scor:ReceiveExcessProduct
    rdf:type owl:Class ;
    rdfs:subClassOf scor:DeliverReturnExcessProductStep ;
    rdfs:comment "The process where the designated return center receives and verifies the returned excess product and associated documentation against the return authorization and other documentation and prepares the item for transfer. Administrate any discrepancies that arise."@en ;
    rdfs:label "Receive Excess Product"@en ;
    scor:isStepOf scor:DeliverReturnExcessProduct ;
    skos:notation "sDR3.3" ;
    rdfs:isDefinedBy scor: ;
    vs:term_status "stable" ;
    dct:modified "2015-11-05"^^xsd:date ;
.

scor:TransferExcessProduct
    rdf:type owl:Class ;
    rdfs:subClassOf scor:DeliverReturnExcessProductStep ;
    rdfs:comment "The process where the designated return center transfers the excess product to the appropriate process to implement the disposition decision."@en ;
    rdfs:label "Transfer Excess Product"@en ;
    scor:isStepOf scor:DeliverReturnExcessProduct ;
    skos:notation "sDR3.4" ;
    rdfs:isDefinedBy scor: ;
    vs:term_status "stable" ;
    dct:modified "2015-11-05"^^xsd:date ;
.

# Manage Supply Chain Business Rule Steps

scor:GatherBusinessRuleRequirements
    rdf:type owl:Class ;
    rdfs:subClassOf scor:ManageSupplyChainBusinessRulesStep ;  
    rdfs:comment "The process of collecting, organizing, prioritizing and scheduling policies and directives requiring new supply chain business rules, changes to business rules or discontinuation of business rules. This may include scheduling and assigning activities to responsible individuals, groups or organizations."@en ;
    rdfs:label "Gather Business Rule Requirements"@en ;
    scor:isStepOf scor:ManageSupplyChainBusinessRules;
    skos:notation "sE1.1" ;
    rdfs:isDefinedBy scor: ;
    vs:term_status "stable" ;
    dct:modified "2015-11-05"^^xsd:date ;
.

scor:InterpretBusinessRuleRequirement
    rdf:type owl:Class ;
    rdfs:subClassOf scor:ManageSupplyChainBusinessRulesStep ;  
    rdfs:comment "The process of determining how the policy or directive impacts supply chain processes, technology and business rules. This includes reviewing existing business rules and determining the need to add, change or delete business rules. The outcome is one or more of the following: (1) Request to Add a Business Rule (2) Request to Change a Business Rule (3) Request to Delete or Archive a Business Rule. The purpose of this step is to identify the type of activities required and routing the request if required."@en ;
    rdfs:label "Interpret Business Rule Requirement"@en ;
    scor:isStepOf scor:ManageSupplyChainBusinessRules;
    skos:notation "sE1.2" ;
    rdfs:isDefinedBy scor: ;
    vs:term_status "stable" ;
    dct:modified "2015-11-05"^^xsd:date ;
.

scor:DocumentBusinessRule
    rdf:type owl:Class ;
    rdfs:subClassOf scor:ManageSupplyChainBusinessRulesStep ;  
    rdfs:comment "The process of writing the business rule in the appropriate system of record. This includes adding, editing and deleting policy and process documentation. A business rule includes a directive or policy, scope and effective date. Updates to existing business rules may include discontinuation information. The final activity of Document Business Rule is obtaining formal approval. The output of this process step is a fully documented business rule that is signed off by the responsible function."@en ;
    rdfs:label "Document Business Rules"@en ;
    scor:isStepOf scor:ManageSupplyChainBusinessRules;
    skos:notation "sE1.3" ;
    rdfs:isDefinedBy scor: ;
    vs:term_status "stable" ;
    dct:modified "2015-11-05"^^xsd:date ;
.

scor:CommunicateBusinessRule
    rdf:type owl:Class ;
    rdfs:subClassOf scor:ManageSupplyChainBusinessRulesStep ;  
    rdfs:comment "The process of creating awareness in the relevant organization and/or staff of the upcoming changes. This may include communications, training and education programs. For small or incremental changes a notice maybe sufficient."@en;     
    rdfs:label "Communicate Business Rules"@en ;
    scor:isStepOf scor:ManageSupplyChainBusinessRules;
    skos:notation "sE1.4" ;
    rdfs:isDefinedBy scor: ;
    vs:term_status "stable" ;
    dct:modified "2015-11-05"^^xsd:date ;
.

scor:ReleaseAndPublishBusinessRule
    rdf:type owl:Class ;
    rdfs:subClassOf scor:ManageSupplyChainBusinessRulesStep ;  
    rdfs:comment "The process of activating the business rule. Business rules release may be time-phased --e.g. Bill of Materials release for newer revisions. This may include activiation of a business rule in a software algorithm and starting to use a new or updated standard operating procedure. For large impact business rule changes this may include updating external websites, formal announcements, etc."@en;     
    rdfs:label "Release and Publish Business Rule"@en ;
    scor:isStepOf scor:ManageSupplyChainBusinessRules;
    skos:notation "sE1.5" ;
    rdfs:isDefinedBy scor: ;
    vs:term_status "stable" ;
    dct:modified "2015-11-05"^^xsd:date ;
.

scor:RetireBusinessRule
    rdf:type owl:Class ;
    rdfs:subClassOf scor:ManageSupplyChainBusinessRulesStep ;  
    rdfs:comment "The process of de-activating the business rule. Business rules retirement may be time-phased --e.g. Bill of Materials replaced by newer revisions. This may include archiving the business rule in the associated software to avoid users from inadvertently using it or in order to comply to regulatory requirements or policies."@en;
    rdfs:label "Retire Business Rule"@en ;
    scor:isStepOf scor:ManageSupplyChainBusinessRules;
    skos:notation "sE1.6" ;
    rdfs:isDefinedBy scor: ;
    vs:term_status "stable" ;
    dct:modified "2015-11-05"^^xsd:date ;
.
# Manage Supply Chain Steps

scor:InitiateReporting
    rdf:type owl:Class ;
    rdfs:subClassOf scor:ManageSupplyChainPerformanceStep ;  
    rdfs:comment "The process of scheduling, running reports, collecting and aggregating perfomance data. This includes running standard (pre-defined) reports as well as adhoc reporting. Ad hoc reporting includes developing a data collection plan and organizing data collection through: (1) Inspections (2) Measurement (e.g. stopwatch to measure duration of activities) (3) Sampling (4) Self assessements (e.g. Baldridge Self Assessment). Note: Today reports may be delivered (pushed) to the user by electronic media. This process step represents the delivery of reports to the user in such scenarios.";
    rdfs:label "Initiate Reporting"@en ;
    scor:isStepOf scor:ManagePerformance;
    skos:notation "sE2.1" ;
    rdfs:isDefinedBy scor: ;
    vs:term_status "stable" ;
    dct:modified "2015-11-05"^^xsd:date ;
.

scor:AnalyzeReports
    rdf:type owl:Class ;
    rdfs:subClassOf scor:ManageSupplyChainPerformanceStep ;  
    rdfs:comment "The process of reviewing the reported performance. This includes comparing actual performance and trends to targets set for each metric. Identify metrics that require root cause analysis and notification/scheduling of process owners or 'root cause analysis' resources.";    #
    rdfs:label "Analyze Reports"@en ;
    scor:isStepOf scor:ManagePerformance;
    skos:notation "sE2.2" ;
    rdfs:isDefinedBy scor: ;
    vs:term_status "stable" ;
    dct:modified "2015-11-05"^^xsd:date ;
.

scor:FindRootCauses
    rdf:type owl:Class ;
    rdfs:subClassOf scor:ManageSupplyChainPerformanceStep ;  
    rdfs:comment "The process of analyzing the gaps in performance. Example root cause finding methods and techniques include: (1) Adding commentary to reported data (2) Metrics decomposition using diagnostic relationships of (SCOR) metrics (3) Time studies, sampling, audits, cycle counting (4) 5-Whys/Cause & Effect analysis (5) Statistical Analysis Techniques: e.g. Histogram, Scatter Plots, ANOVA. All root causes are documented and quantified. Quantification is the calculation or estimation of the relative contribution to the gap in performance."@en;
    rdfs:label "Find Root Causes"@en ;
    scor:isStepOf scor:ManagePerformance;
    skos:notation "sE2.3" ;
    rdfs:isDefinedBy scor: ;
    vs:term_status "stable" ;
    dct:modified "2015-11-05"^^xsd:date ;
.

scor:PrioritizeRootCauses
    rdf:type owl:Class ;
    rdfs:subClassOf scor:ManageSupplyChainPerformanceStep ;  
    rdfs:comment "The process of sorting root causes by relative contribution and prioritizing root causes. This includes assigning root causes to resources and scheduling development of corrective actions."@en;
    rdfs:label "Prioritize Root Causes"@en ;
    scor:isStepOf scor:ManagePerformance;
    skos:notation "sE2.4" ;
    rdfs:isDefinedBy scor: ;
    vs:term_status "stable" ;
    dct:modified "2015-11-05"^^xsd:date ;
.

scor:DevelopeCorrectiveActions
    rdf:type owl:Class ;
    rdfs:subClassOf scor:ManageSupplyChainPerformanceStep ;  
    rdfs:comment "The process of identifying, documenting and stable corrective actions to address the root cause in order to close the performance gap. Corrections actions include: (1) Organizational changes (hiring, redeployment) (2) Policy changes (business rules) (3) Process improvements (work instructions, training) (4) Production equipment repairs/calibration (5) Supply chain network reconfiguration (6) Software algorithm changes (e.g. planning or scheduling logic) (7) Technology introduction (new equipment, tools, software). Note: This list of corrective actions is a general characterization for example purposes only. Different root causes may require different corrective actions."@en;
    rdfs:label "Develope Corrective Actions"@en ;
    scor:isStepOf scor:ManagePerformance;
    skos:notation "sE2.5" ;
    rdfs:isDefinedBy scor: ;
    vs:term_status "stable" ;
    dct:modified "2015-11-05"^^xsd:date ;
.

scor:ApproveAndLaunch
    rdf:type owl:Class ;
    rdfs:subClassOf scor:ManageSupplyChainPerformanceStep ;  
    rdfs:comment "The process of obtaining approvals, prioritizing, communicating and launching the corrective actions."@en;
    rdfs:label "Approve And Launch"@en ;
    scor:isStepOf scor:ManagePerformance;
    skos:notation "sE2.6" ;
    rdfs:isDefinedBy scor: ;
    vs:term_status "stable" ;
    dct:modified "2015-11-05"^^xsd:date ;
.

# Manage Data and Information steps

scor:ReceiveMaintainanceRequest
    rdf:type owl:Class ;
    rdfs:subClassOf scor:ManageSupplyChainDataAndInformationStep ;  
    rdfs:comment "The process of receiving, validating and logging the request for information, configuration or system functionality maintenance. Maintenance request types: (1) Add data - creation of new record/document (includes duplicating existing records/documents) (2) Change data - modification of an existing record/document (3) Delete data - deletion of an existing record (includes archiving and unpublishing existing records/documents) (4) Change configuration (includes creating and maintaining user access) (5) Add code - (includes installing software updates and security updates) (6) Change code (modification of software code) (7) Delete code. This process may include assigning a ticket, tracking or order number and routing the request to the appropriate resource."@en;
    rdfs:label "Manage Data and Information"@en ;
    scor:isStepOf scor:ManageDataAndInformation;
    skos:notation "sE3.1" ;
    rdfs:isDefinedBy scor: ;
    vs:term_status "stable" ;
    dct:modified "2015-11-05"^^xsd:date ;
.

scor:DetermineAndScopeWork
    rdf:type owl:Class ;
    rdfs:subClassOf scor:ManageSupplyChainDataAndInformationStep ; 
    rdfs:comment "The activities associated with determining the activities required to perform the requested maintenance. The requestor may be contacted for additinal information. Complex requests may be setup as projects with appropriate work breakdown structure, milestones, acceptance criteria and deliverable schedules. This process may include routing the request to the appropriate resource."@en;
    rdfs:label "Determine/Scope Work"@en ;
    scor:isStepOf scor:ManageDataAndInformation;
    skos:notation "sE3.2" ;
    rdfs:isDefinedBy scor: ;
    vs:term_status "stable" ;
    dct:modified "2015-11-05"^^xsd:date ;
.

scor:MaintainContentAndCode
    rdf:type owl:Class ;
    rdfs:subClassOf scor:ManageSupplyChainDataAndInformationStep ; 
    rdfs:comment "The process of formatting, entering, loading, editing or deleting the information, software updates and code changes requested. This includes verification of changes as needed (unit and integration stable). Typical changes included are: (1) Data record maintenance (such as bills-of-materials, shipping routes) (2) Configuration (system parameter) changes (such as activating and disabling system functionality) (3) Loading/installing software updates (e.g. code changes from vendors or development groups) (4) Loading/installing security updates. This process is not a placeholder for complex software engineering processes. Such processes would lay outside of the SCOR process framework."@en;    
    rdfs:label "Maintain Content/Code"@en ;
    scor:isStepOf scor:ManageDataAndInformation;
    skos:notation "sE3.3" ;
    rdfs:isDefinedBy scor: ;
    vs:term_status "stable" ;
    dct:modified "2015-11-05"^^xsd:date ;
.

scor:MaintainAccess
    rdf:type owl:Class ;
    rdfs:subClassOf scor:ManageSupplyChainDataAndInformationStep ; 
    rdfs:comment "The process of establishing, changing or removing access rights for users."@en;
    rdfs:label "Maintain Access"@en ;
    scor:isStepOf scor:ManageDataAndInformation;
    skos:notation "sE3.4" ;
    rdfs:isDefinedBy scor: ;
    vs:term_status "stable" ;
    dct:modified "2015-11-05"^^xsd:date ;
.

scor:PublishInformation
    rdf:type owl:Class ;
    rdfs:subClassOf scor:ManageSupplyChainDataAndInformationStep ; 
    rdfs:comment "The process of activating the changes to information, configuration and/or code and populating the information to dependent systems, where applicable. For data record maintenance this is the activation of the new data and populating dependent systems with the new data. For example activating a bill-of-materials (BOM) in the system-of-record* and populating the BOM to dependent systems that require a copy of this data. This process may be manual, automated or a combination. *system-of-record = the information storage system, which is the authoritative data source for a given data element or piece of information."@en;    
    rdfs:label "Publish Information"@en ;
    scor:isStepOf scor:ManageDataAndInformation;
    skos:notation "sE3.5" ;
    rdfs:isDefinedBy scor: ;
    vs:term_status "stable" ;
    dct:modified "2015-11-05"^^xsd:date ;
.

scor:VerfyInformation
    rdf:type owl:Class ;
    rdfs:subClassOf scor:ManageSupplyChainDataAndInformationStep ; 
    rdfs:comment "The process of verifying the information is properly recorded in the system of record and populated to dependent systems. This includes verifying information is accessible to users."@en;    
    rdfs:label "Verfy Information"@en ;
    scor:isStepOf scor:ManageDataAndInformation;
    skos:notation "sE3.6" ;
    rdfs:isDefinedBy scor: ;
    vs:term_status "stable" ;
    dct:modified "2015-11-05"^^xsd:date ;
.

#Manage Supply Chain Human Resources steps 


scor:VerifyInformation
    rdf:type owl:Class ;
    rdfs:subClassOf scor:ManageSupplyChainHumanResourceStep ; 
    rdfs:comment "The activities associated with the collection of the required skills to operate (part of) the supply chain. Examples of this process are planning meetings, periodic performance reviews, reorganizations. The data collected should list the required skills and/or number of resources and is generally organized by entity (supply chain node, department, function or a combination of these)."@en;    
    rdfs:label "Identify Skills and Resource Requirement"@en ;
    scor:isStepOf scor:ManageSupplyChainHumanResources;
    skos:notation "sE4.1" ;
    rdfs:isDefinedBy scor: ;
    vs:term_status "stable" ;
    dct:modified "2015-11-05"^^xsd:date ;
.

scor:IdentifyAvailableSkillsAndResources
    rdf:type owl:Class ;
    rdfs:subClassOf scor:ManageSupplyChainHumanResourceStep ; 
    rdfs:comment "The activities associated with the collection of skills/resources currently available in the supply chain. Generally this information is collected and organized by entity (supply chain node, department, function or a combination of these). Examples of this process include data collection for standard headcount reports, but should include temporary staff and outsourced resources."@en;
    rdfs:label "Identify available Skills and Resource Requirement"@en ;
    scor:isStepOf scor:ManageSupplyChainHumanResources;
    skos:notation "sE4.2" ;
    rdfs:isDefinedBy scor: ;
    vs:term_status "stable" ;
    dct:modified "2015-11-05"^^xsd:date ;
.

scor:MatchSkillsAndResources
    rdf:type owl:Class ;
    rdfs:subClassOf scor:ManageSupplyChainHumanResourceStep ; 
    rdfs:comment "The activities associated with the matching of skills or resource demand with the available skills/ resources. The purpose of this process is to determine which skill/resource requirements (demand) can be met using existing resources, determine which skill/resource requirements are not supported by current available skills/resources (gap) and determine the skills/resources for which no demand exists (excess) For each skill/resource gap or excess, one or more actions need to be identified to close the gap or address the excess: (1) Training/Cross-training (add skills to existing resources) (2) Hiring (add resources with existing skills) (3) Redeployment (moving staff to different organizations or layoff. It is important to consider the lead-time of these actions, scarce skills may have longer leadtimes for example. Hiring includes temporary workers and all types of outsourced staff."@en;
    rdfs:label "Match Skills/Resources"@en ;
    scor:isStepOf scor:ManageSupplyChainHumanResources;
    skos:notation "sE4.3" ;
    rdfs:isDefinedBy scor: ;
    vs:term_status "stable" ;
    dct:modified "2015-11-05"^^xsd:date ;
.

scor:DetermineHiringAndRedeployment
    rdf:type owl:Class ;
    rdfs:subClassOf scor:ManageSupplyChainHumanResourceStep ; 
    rdfs:comment "The activities associated with identification of sources of new hires or sources/destinations for redeployment. The purpose of this process step includes assessing the feasibility of hiring the required skills/resources within the required time period, assessing the feasibility of redeploying the excess employees (resources) and assessing the feasibility and impact of possible layoff of employees. Note: At this stage this is a planning activity. The actual hiring process is not documented in SCOR as this is a Human Resources Management (HR) process. Employee in this context includes temporary workers and employees of service providers."@en;
    rdfs:label "Determine Hiring/Redeployment"@en ;
    scor:isStepOf scor:ManageSupplyChainHumanResources;
    skos:notation "sE4.4" ;
    rdfs:isDefinedBy scor:DetermineTrainingAndEducation ;
    vs:term_status "stable" ;
    dct:modified "2015-11-05"^^xsd:date ;
.

scor:DetermineTrainingAndEducation
    rdf:type owl:Class ;
    rdfs:subClassOf scor:ManageSupplyChainHumanResourceStep ; 
    rdfs:comment "The activities associated with the identification of training and education programs to ensure existing (and newly hired) employees will have the appropriate skills to perform the work allocated to each individual employee. Employee in this definition may include temporary workers and employees of service providers."@en;  
    rdfs:label "Determine Training/Education"@en ;
    scor:isStepOf scor:ManageSupplyChainHumanResources;
    skos:notation "sE4.5" ;
    rdfs:isDefinedBy scor: ;
    vs:term_status "stable" ;
    dct:modified "2015-11-05"^^xsd:date ;
.

scor:ApprovePrioritizeAndLaunch
    rdf:type owl:Class ;
    rdfs:subClassOf scor:ManageSupplyChainHumanResourceStep ; 
    rdfs:comment "The activities associated with obtaining approvals for hiring, redeployment, training and education plans, prioritizing and executing these plans. Additional resources and skills will become available over time, adjusting the labor component of capacity in Plan, Source, Make, Deliver, Return and/or Enable processes."@en;    
    rdfs:label "Approve, Prioritize and Launch"@en ;
    scor:isStepOf scor:ManageSupplyChainHumanResources;
    skos:notation "sE4.6" ;
    rdfs:isDefinedBy scor: ;
    vs:term_status "stable" ;
    dct:modified "2015-11-05"^^xsd:date ;
.

# Manage Supply Chain Assets Steps

scor:ScheduleAssetManagementActivities
    rdf:type owl:Class ;
    rdfs:subClassOf scor:ManageSupplyChainAssetsStep ; 
    rdfs:comment "The activities associated with receiving maintenance requests, receiving repair/replacement/installation requests, maintaining preventive/regular maintenance tasks, scheduling individual mainentance tasks and assigning resources to individual maintenance tasks. Scheduling may include incorporating production and delivery plans and schedules and communication of maintenance schedules to production and delivery planning and scheduling processes."@en;
    rdfs:label "Schedule Assets Management Activities"@en ;
    scor:isStepOf scor:ManageSupplyChainAssets;
    skos:notation "sE5.1" ;
    rdfs:isDefinedBy scor: ;
    vs:term_status "stable" ;
    dct:modified "2015-11-05"^^xsd:date ;
.

scor:TakeAssetOffline
    rdf:type owl:Class ;
    rdfs:subClassOf scor:ManageSupplyChainAssetsStep ; 
    rdfs:comment "The activities associated with the preparation of the maintenance tasks. In general terms this mean the asset or equipment needs to be stopped or put into maintenance mode. Safety precautions need to be made to ensure the equipment cannot be restarted during mainentance without active approval of the maintenance operators/engineers. This may include installing safety barriers, transporting the asset/equipment to a location where the maintenance will take place, removing deposits/materials from production equipment (cleaning), unloading transportation equipment and backing up data from the equipment and associated automation systems."@en;    
    rdfs:label "Take Asset Off-line"@en ;
    scor:isStepOf scor:ManageSupplyChainAssets;
    skos:notation "sE5.2" ;
    rdfs:isDefinedBy scor: ;
    vs:term_status "stable" ;
    dct:modified "2015-11-05"^^xsd:date ;
.

scor:InspectAndTroubleshoot
    rdf:type owl:Class ;
    rdfs:subClassOf scor:ManageSupplyChainAssetsStep ; 
    rdfs:comment "The activities associated with assessing the overall status of the equipment, performing standard inspection and detailed troublshooting if required. This includes identification of repairs, upgrades and maintenance tasks in order to bring the asset/equipment in optimal or acceptable working condition. This process may be the identification of readiness for installing new hardware or software and preparing (documenting) the steps of decommissioning and dispositioning for equipment/assets installation or de-installation and disposal."@en;    
    rdfs:label "Inspect and Troubleshoot"@en ;
    scor:isStepOf scor:ManageSupplyChainAssets;
    skos:notation "sE5.3" ;
    rdfs:isDefinedBy scor: ;
    vs:term_status "stable" ;
    dct:modified "2015-11-05"^^xsd:date ;
.

scor:InstallAndConfigure
    rdf:type owl:Class ;
    rdfs:subClassOf scor:ManageSupplyChainAssetsStep ; 
    rdfs:comment "The activities associated with the installation of new hardware, software or functionality (equipment/ assets). This includes installation and initial stable of the new hardware, software or functionality. The general purpose of installation is to increase capacity or add/improve capabilities. Note: This process step may trigger a separate supply chain (depending on the scale of the installation) building and installing new supply chain assets."@en;
    rdfs:label "Install and Configure"@en ;
    scor:isStepOf scor:ManageSupplyChainAssets;
    skos:notation "sE5.4" ;
    rdfs:isDefinedBy scor: ;
    vs:term_status "stable" ;
    dct:modified "2015-11-05"^^xsd:date ;
.

scor:CleanMaintainAndRepair
    rdf:type owl:Class ;
    rdfs:subClassOf scor:ManageSupplyChainAssetsStep ; 
    rdfs:comment "The activities associated with the cleaning, replacement of parts, reconditioning of the equipment/ asset. (The general purpose of this process step is to bring the equipment/asset back in optimal/ acceptable operating condition). This may include measuring and stable of the equipment. Note: This is a Make process for the function performing the maintenance/repair activities."@en;    
    rdfs:label "Clean, Maintain and Repair"@en ;
    scor:isStepOf scor:ManageSupplyChainAssets;
    skos:notation "sE5.5" ;
    rdfs:isDefinedBy scor: ;
    vs:term_status "stable" ;
    dct:modified "2015-11-05"^^xsd:date ;
.

scor:DecomissionAndDispose
    rdf:type owl:Class ;
    rdfs:subClassOf scor:ManageSupplyChainAssetsStep ; 
    rdfs:comment "The activities associated with the de-installation and disposal of existing hardware, software or functionality (equipment/assets). This includes physical removal from the original point of use. The general purpose of installation is to replace capacity or remove outdated capabilities."@en;    
    rdfs:label "Decommission and Dispose"@en ;
    scor:isStepOf scor:ManageSupplyChainAssets;
    skos:notation "sE5.6" ;
    rdfs:isDefinedBy scor: ;
    vs:term_status "stable" ;
    dct:modified "2015-11-05"^^xsd:date ;
.

scor:InspectMaintenance
    rdf:type owl:Class ;
    rdfs:subClassOf scor:ManageSupplyChainAssetsStep ; 
    rdfs:comment "The activities associated with the inspection of the maintenance work performed. This may include performing test runs to assess whether new capacity or functionality is meeting expectations. This includes documentation of any inspection data, recording any inspection errors and obtaining approvals. The purpose of Inspect Mainentance is to verify the effectiveness/success of the maintenance activities."@en ;  
    rdfs:label "Inspect Maintenance"@en ;
    scor:isStepOf scor:ManageSupplyChainAssets;
    skos:notation "sE5.7" ;
    rdfs:isDefinedBy scor: ;
    vs:term_status "stable" ;
    dct:modified "2015-11-05"^^xsd:date ;
.

scor:ReinstateAsset
    rdf:type owl:Class ;
    rdfs:subClassOf scor:ManageSupplyChainAssetsStep ; 
    rdfs:comment "The activities associated with completion of the maintenance work and preparing the equipment/ asset to be brought 'on-line'. The general purpose of this process step is to make the asset available for 'production' (add to capacity). This includes closing work orders and receiving and approving payment of invoices for work performed by external resources. Upon completion of this process step the asset is expected to be in full working condition."@en;    
    rdfs:label "Reinstate Asset"@en ;
    scor:isStepOf scor:ManageSupplyChainAssets;
    skos:notation "sE5.8" ;
    rdfs:isDefinedBy scor: ;
    vs:term_status "stable" ;
    dct:modified "2015-11-05"^^xsd:date ;
.

# Manage Supply Chain Contracts

scor:ReceiveContractUpdates
    rdf:type owl:Class ;
    rdfs:subClassOf scor:ManageSupplyChainContractsStep ; 
    rdfs:comment "The activities associated with receiving new contracts or changes to existing contracts. These contract updates may originate in Sales & Support processes (customer contracts) or in Product and Process Design processes (for material supplier or services providers such as transportation services, equipment maintenance services, IT services). This includes validation of contracts against criteria (business rules). A contract needs to include information such as effective date and duration, customer or supplier address and payment terms and may not be in conflict with business rules (and regulatory requirements).";    
    rdfs:label "Receive Contract Updates"@en ;
    scor:isStepOf scor:ManageSupplyChainContracts;
    skos:notation "sE6.1" ;
    rdfs:isDefinedBy scor: ;
    vs:term_status "stable" ;
    dct:modified "2015-11-05"^^xsd:date ;
.

scor:EnterAndDistirbuteContract
    rdf:type owl:Class ;
    rdfs:subClassOf scor:ManageSupplyChainContractsStep ; 
    rdfs:comment "The activities associated with entering contractual information in document management systems and ERP systems. This includes the 'translation' of contractual language/information into a format that the system can comprehend. A final step in this process is to distribute the contract or updates to an existing contract to the appropriate processes/functions."@en;    
    rdfs:label "Enter and Distribute Contract"@en ;
    scor:isStepOf scor:ManageSupplyChainContracts;
    skos:notation "sE6.2" ;
    rdfs:isDefinedBy scor: ;
    vs:term_status "stable" ;
    dct:modified "2015-11-05"^^xsd:date ;
.

scor:ActiviateOrArchiveContract
    rdf:type owl:Class ;
    rdfs:subClassOf scor:ManageSupplyChainContractsStep ; 
    rdfs:comment "The activities associated with activation or de-activation and archiving the contract. This may include updating statuses of information in document management systems or ERP systems. This activity may be triggered and performed by the document management system or ERP system based on parameters entered as part of sE6.2 Enter and Distribute Contract"@en;
    rdfs:label "Activate or Archive Contract"@en ;
    scor:isStepOf scor:ManageSupplyChainContracts;
    skos:notation "sE6.3" ;
    rdfs:isDefinedBy scor: ;
    vs:term_status "stable" ;
    dct:modified "2015-11-05"^^xsd:date ;
.

scor:ReviewContractualPerformance
    rdf:type owl:Class ;
    rdfs:subClassOf scor:ManageSupplyChainContractsStep ; 
    rdfs:comment "The activities associated with reviewing the performance of contractual parties (both supplier and customer). This includes comparing the contractual service level agreements with the actual service levels. This process may be triggered by a calendar event - such as annual or quarterly quality reviews or actual performance issues identified in daily supply chain processes."@en;    
    rdfs:label "Review Contractual Performance"@en ;
    scor:isStepOf scor:ManageSupplyChainContracts;
    skos:notation "sE6.4" ;
    rdfs:isDefinedBy scor: ;
    vs:term_status "stable" ;
    dct:modified "2015-11-05"^^xsd:date ;
.

scor:IdentifyPerformanceIssuesAndOpportunities
    rdf:type owl:Class ;
    rdfs:subClassOf scor:ManageSupplyChainContractsStep ; 
    rdfs:comment "The activities associated with identifying and prioritization of key performance issues or areas of ongoing process improvement. This includes notifying contractual partners of non-conformance to contractual agreements or agreed service level agreements. This process addresses both the non-compliance issues (severe) as well as areas of continuous improvement (non-severe, common interest)."@en;    
    rdfs:label "Identify Performance Issues/Opportunities"@en ;
    scor:isStepOf scor:ManageSupplyChainContracts;
    skos:notation "sE6.5" ;
    rdfs:isDefinedBy scor: ;
    vs:term_status "stable" ;
    dct:modified "2015-11-05"^^xsd:date ;
.

scor:IdentifyResolutionsAndImprovements
    rdf:type owl:Class ;
    rdfs:subClassOf scor:ManageSupplyChainContractsStep ; 
    rdfs:comment "The activities associated with identifying ways to address the non-compliance or how to implement performance improvements. For non-compliance this process may have one or a combination of outcomes: (1) Terminate the contract (2) Pay/Collect Penalties (3) Update contract (service levels, quality levels, terms and conditions) (4) Continue as-is (internal process, policy or business rule changes). Litigation or mediation may be considered in this process. Litigation or mediation is not part of supply chain processes."@en;   
    rdfs:label "Identify Resolutions/Improvements"@en ;
    scor:isStepOf scor:ManageSupplyChainContracts;
    skos:notation "sE6.6" ;
    rdfs:isDefinedBy scor: ;
    vs:term_status "stable" ;
    dct:modified "2015-11-05"^^xsd:date ;
.

scor:SelectPrioritizeAndDistributeResolutions
    rdf:type owl:Class ;
    rdfs:subClassOf scor:ManageSupplyChainContractsStep ; 
    rdfs:comment "The activities associated with selecting, obtaining approvals and prioritizing the appropriate issue resolution and distributing the resolution to the appropriate processes/functions. Litigation or mediation may be the result of decisions made in this process. Litigation or mediation is not part of supply chain processes."@en;    
    rdfs:label "Select, Prioritize and Distribute Resolutions"@en ;
    scor:isStepOf scor:ManageSupplyChainContracts;
    skos:notation "sE6.7" ;
    rdfs:isDefinedBy scor: ;
    vs:term_status "stable" ;
    dct:modified "2015-11-05"^^xsd:date ;
.

# Manage Supply Chain Networks Steps

scor:SelectScopeAndOrganization
    rdf:type owl:Class ;
    rdfs:subClassOf scor:ManageSupplyChainNetworkStep ; 
    rdfs:comment "The activities associated with determining what part of the supply chain network will be assessed (the scope). Organizations that manage the supply chain network as a project structure will need to establish a project organization. Organization selection includes identification and securing availability of sponsor, stakeholders and data/information providers as well as selecting project team members."@en;
    rdfs:label "Select Scope and Organization"@en ;
    scor:isStepOf scor:ManageSupplyChainNetworks;
    skos:notation "sE7.1" ;
    rdfs:isDefinedBy scor: ;
    vs:term_status "stable" ;
    dct:modified "2015-11-05"^^xsd:date ;
.

scor:GatherInputAndData
    rdf:type owl:Class ;
    rdfs:subClassOf scor:ManageSupplyChainNetworkStep ; 
    rdfs:comment "The activities associated with identification of the objective of the supply chain ('what strategy does the supply chain need to support') and collection of data required to describe (model) the supply chain at the required level. Data collected includes: facilities costs, capacity and locations, transportation cost, capacity and lead times, customer volumes, order frequency and size and customer locations."@en;    
    rdfs:label "Gather Input and Data"@en ;
    scor:isStepOf scor:ManageSupplyChainNetworks;
    skos:notation "sE7.2" ;
    rdfs:isDefinedBy scor: ;
    vs:term_status "stable" ;
    dct:modified "2015-11-05"^^xsd:date ;
.

scor:DevelopeScenarios
    rdf:type owl:Class ;
    rdfs:subClassOf scor:ManageSupplyChainNetworkStep ; 
    rdfs:comment "The activities associated with the development of scenarios (what-if) in support of different strategies and projections. Scenarios may be developed for different detailed strategies, requirements and potential internal/external changes. Activities include management interview, external transportation and warehousing studies. Initial review of developed scenarios may result in rejection of the scenario or proceeding to simulation."@en;   
    rdfs:label "Develope Scenarios"@en ;
    scor:isStepOf scor:ManageSupplyChainNetworks;
    skos:notation "sE7.3" ;
    rdfs:isDefinedBy scor: ;
    vs:term_status "stable" ;
    dct:modified "2015-11-05"^^xsd:date ;
.

scor:ModelAndSimulateScenarios
    rdf:type owl:Class ;
    rdfs:subClassOf scor:ManageSupplyChainNetworkStep ; 
    rdfs:comment "The activities associated with the development of models and/or simulation models to run 'what-if' scenarios through a validation process. Simulation models may use automation, but conference room pilots or walk-throughs may also serve this purpose. The purpose of simulation is to validat feasibility of each scenario and find possible network/process design flaws. Automated simulation tools may also predict the performance of the new network/processes by simulating the processing of large numbers of orders."@en;
    rdfs:label "Model/Simulate Scenarios"@en ;
    scor:isStepOf scor:ManageSupplyChainNetworks;
    skos:notation "sE7.4" ;
    rdfs:isDefinedBy scor: ;
    vs:term_status "stable" ;
    dct:modified "2015-11-05"^^xsd:date ;
.

scor:ProjectImpact
    rdf:type owl:Class ;
    rdfs:subClassOf scor:ManageSupplyChainNetworkStep ; 
    rdfs:comment "The activities associated with estimating the effort, risks, results of implementing the scenario. effort includes the estimating the risks and duration and the funding, staffing and skills required for implementing the scenario. Risks includes estimating the impact on the Value-at-Risk for the supply chain. Results includes determining the changes to the performance of the supply chain on all relevant metrics."@en;    
    rdfs:label "Project Impact"@en ;
    scor:isStepOf scor:ManageSupplyChainNetworks;
    skos:notation "sE7.5" ;
    rdfs:isDefinedBy scor: ;
    vs:term_status "stable" ;
    dct:modified "2015-11-05"^^xsd:date ;
.

scor:SelectAndApprove
    rdf:type owl:Class ;
    rdfs:subClassOf scor:ManageSupplyChainNetworkStep ; 
    rdfs:comment "The activities associated with recommending and obtaining approvals for proposed supply chain network/configuration changes. This includes reviewing the 'what-if' scenarios and impact/benefit results with key stakeholders. The objective of this process is to identify the optimal solution and present this recommendation to sponsor and stakeholders and obtain approval to develop network change program."@en;    
    rdfs:label "Select and Approve"@en ;
    scor:isStepOf scor:ManageSupplyChainNetworks;
    skos:notation "sE7.6" ;
    rdfs:isDefinedBy scor: ;
    vs:term_status "stable" ;
    dct:modified "2015-11-05"^^xsd:date ;
.

scor:DevelopChangeProgram
    rdf:type owl:Class ;
    rdfs:subClassOf scor:ManageSupplyChainNetworkStep ; 
    rdfs:comment "The activities associated with developing the roadmap for change. This includes identifying the steps (or projects) required to implement changes to facilities, contracted parties, staffing, automation an process. Specific changes are assigned to unique owners. This includes reviewing the specific change/projects with key stakeholders. The objective of this process is to obtain approval to launch change projects."@en;    
    rdfs:label "Develop Change Program"@en ;
    scor:isStepOf scor:ManageSupplyChainNetworks;
    skos:notation "sE7.7" ;
    rdfs:isDefinedBy scor: ;
    vs:term_status "stable" ;
    dct:modified "2015-11-05"^^xsd:date ;
.

scor:LaunchChangeProgram
    rdf:type owl:Class ;
    rdfs:subClassOf scor:ManageSupplyChainNetworkStep ; 
    rdfs:comment "The activities associated with coordinating, starting and monitoring the inidividual change projects. This includes support the establishment of change projects, coordinate launch dates and communicate reporting requirements. Steps may include archiving the supply chain network/ configuration project documentation for future reference and dissolving the project team. Dissolving the project team requires transfer of responsibilities to monitor progress to appropriate organizations."@en;
    rdfs:label "Launch Change Program"@en ;
    scor:isStepOf scor:ManageSupplyChainNetworks;
    skos:notation "sE7.8" ;
    rdfs:isDefinedBy scor: ;
    vs:term_status "stable" ;
    dct:modified "2015-11-05"^^xsd:date ;
.

# Manage Regulatory Compliance

scor:MonitorRegulatoryEntities
    rdf:type owl:Class ;
    rdfs:subClassOf scor:ManageSupplyChainRegulatoryComplianceStep ; 
    rdfs:comment "The activities associated with identification regulatory publications, subscribing to publications, receiving and registering publications of relevant regulatory entities (e.g. goverment agencies)."@en;
    rdfs:label "Monitor Regulatory Entities"@en ;
    scor:isStepOf scor:ManageRegulatoryCompliance;
    skos:notation "sE8.1" ;
    rdfs:isDefinedBy scor: ;
    vs:term_status "stable" ;
    dct:modified "2015-11-05"^^xsd:date ;
.

scor:AssessRegulatoryPublications
    rdf:type owl:Class ;
    rdfs:subClassOf scor:ManageSupplyChainRegulatoryComplianceStep ; 
    rdfs:comment "The activities associated with reading, interpreting and researching policies, laws, rules and regulations. This includes determining if and how these regulatory requirements apply to the supply chain."@en;    
    rdfs:label "Assess Regulatory Publications"@en ;
    scor:isStepOf scor:ManageRegulatoryCompliance;
    skos:notation "sE8.2" ;
    rdfs:isDefinedBy scor: ;
    vs:term_status "stable" ;
    dct:modified "2015-11-05"^^xsd:date ;
.

scor:IdentifyRegulatoryDeficiencies
    rdf:type owl:Class ;
    rdfs:subClassOf scor:ManageSupplyChainRegulatoryComplianceStep ; 
    rdfs:comment "The activities associated with identification of past, current and future regulatory requirements that are not or can not be met using existing processes, business rules and policies. This includes notification of deficiency status to impacted organizations."@en;    
    rdfs:label "Identify Regulatory Deficiencies"@en ;
    scor:isStepOf scor:ManageRegulatoryCompliance;
    skos:notation "sE8.3" ;
    rdfs:isDefinedBy scor: ;
    vs:term_status "stable" ;
    dct:modified "2015-11-05"^^xsd:date ;
.

scor:DefineRemediation
    rdf:type owl:Class ;
    rdfs:subClassOf scor:ManageSupplyChainRegulatoryComplianceStep ; 
    rdfs:comment "The activities associated with identification remediation alternatives, selecting and documenting processes, policies and business rules and setting documentation requirements to remediate a deficiency."@en;    
    rdfs:label "Define Remediation"@en ;
    scor:isStepOf scor:ManageRegulatoryCompliance;
    skos:notation "sE8.4" ;
    rdfs:isDefinedBy scor: ;
    vs:term_status "stable" ;
    dct:modified "2015-11-05"^^xsd:date ;
.

scor:VerifyAndObtainLicense
    rdf:type owl:Class ;
    rdfs:subClassOf scor:ManageSupplyChainRegulatoryComplianceStep ; 
    rdfs:comment "The activities asscoiated with verification of the remediation strategy with controlling entities and/or obtaining a license certifying compliance by the controlling entity."@en;    
    rdfs:label "Verify/Obtain License"@en ;
    scor:isStepOf scor:ManageRegulatoryCompliance;
    skos:notation "sE8.5" ;
    rdfs:isDefinedBy scor: ;
    vs:term_status "stable" ;
    dct:modified "2015-11-05"^^xsd:date ;
.

scor:PublishRemediation
    rdf:type owl:Class ;
    rdfs:subClassOf scor:ManageSupplyChainRegulatoryComplianceStep ; 
    rdfs:comment "The activities asscoiated with approving and implementing changes to processes, policies and business rules. This may include distributing certification documentation to relevant organizations in the supply chain."@en;    
    rdfs:label "Publish Remediation"@en ;
    scor:isStepOf scor:ManageRegulatoryCompliance;
    skos:notation "sE8.6" ;
    rdfs:isDefinedBy scor: ;
    vs:term_status "stable" ;
    dct:modified "2015-11-05"^^xsd:date ;
.

# Manage Supply Chain Risk Steps

scor:EstablishContext
    rdf:type owl:Class ;
    rdfs:subClassOf scor:ManageSupplyChainRiskStep ; 
    rdfs:comment "The process of defining and documenting the objectives and scope (internal and external) for managing risk. This includes developing/maintaining understanding of the internal and external relationships, internal and external factors that influence the supply chain's ability to achieve it's objectives, and defining and maintaining a risk management organization -- stakeholders, governance structure, procedures and schedule"@en;
    rdfs:label "Establish Context"@en ;
    scor:isStepOf scor:ManageSupplyChainRisk;
    skos:notation "sE9.1" ;
    rdfs:isDefinedBy scor: ;
    vs:term_status "stable" ;
    dct:modified "2015-11-05"^^xsd:date ;
.

scor:IdentifyRiskEvents
    rdf:type owl:Class ;
    rdfs:subClassOf scor:ManageSupplyChainRiskStep ; 
    rdfs:comment "The process of identifying, collecting and documenting all potential risk events that may impact the organization from meeting its goals. This includes identification of sources of risks, identification and discovery of risk events. This process generates a comprehensive list of all risks that may disrupt the supply chain, including information which processes in the supply chain will be directly and indirectly impacted by the occurance of the risk event. A broad classification of risk types includes: (1) Disruptions in demand - e.g. customers going out of business (2) Disruptions in supply - e.g. suppliers going out of business, supplier quality/performance issues (3) Environmental disruptions - e.g. weather, flooding, earthquakes (4) Financial disruptions - e.g. availability of credit, investors (5) Fraud, theft and mismanagement - lack of risk mitigation (6) Labor disruption - e.g. employee strikes, availability of qualified staff (7) Terrorism and cyber attacks. The number of risks within these types may differ by industry."@en;    
    rdfs:label "Identify Risk Events"@en ;
    scor:isStepOf scor:ManageSupplyChainRisk;
    skos:notation "sE9.2" ;
    rdfs:isDefinedBy scor: ;
    vs:term_status "stable" ;
    dct:modified "2015-11-05"^^xsd:date ;
.

scor:QuantifyRisks
    rdf:type owl:Class ;
    rdfs:subClassOf scor:ManageSupplyChainRiskStep ; 
    rdfs:comment "The process of collecting and documenting for each potential risk the causes, probability and consequences. The standard metric for quantification of risk is Value at Risk (VaR): VaR = Probability of Occurance x Monetary Impact of Occurance This process generates a comprehensive list of the monetary impact for all risks that may disrupt th supply chain. For certain types of risk events probability information may be available through government agencies, insurance companies or research firms. The monetary impact is determined based on the projected monetary impact for each supply chain for each risk event. For example: (1) For a single sourced material the supplier going out of business means the product manufactured using this material can not be produced until a new supplier has been identified, qualified and integrated in the supply chain. The manetary impact would be the loss of the projected revenue for these products during the qualification and integration process of a new supplier. (2) For a dual sourced material one of the two suppliers going out of business means the product manufactured using this material can only be produced for the percentage the remaining supplier may be able to support until a new supplier has been identified, qualified and integrated or until the remaining supplier can support 100% of the project revenue. Different risk events may have different monetary impacts: reduction of revenue vs. increase of cost."@en;
    rdfs:label "Quantify Risks"@en ;
    scor:isStepOf scor:ManageSupplyChainRisk;
    skos:notation "sE9.3" ;
    rdfs:isDefinedBy scor: ;
    vs:term_status "stable" ;
    dct:modified "2015-11-05"^^xsd:date ;
.

scor:EvaluateRisks
    rdf:type owl:Class ;
    rdfs:subClassOf scor:ManageSupplyChainRiskStep ; 
    rdfs:comment "The process of prioritizing risk events by VaR and determining for each risk whether mitigation actions are required or the risk is acceptable ('risk of doing business')."@en;
    rdfs:label "Evaluate Risks"@en ;
    scor:isStepOf scor:ManageSupplyChainRisk;
    skos:notation "sE9.4" ;
    rdfs:isDefinedBy scor: ;
    vs:term_status "stable" ;
    dct:modified "2015-11-05"^^xsd:date ;
.

scor:MitigateRisk
    rdf:type owl:Class ;
    rdfs:subClassOf scor:ManageSupplyChainRiskStep ; 
    rdfs:comment "The process of determining the actions required to eliminate, reduce or accept and monitor the risks - creating, approving, communicating and launching the 'Risk Mitigation Plan'."@en;     
    rdfs:label "Mitigate Risk"@en ;
    scor:isStepOf scor:ManageSupplyChainRisk;
    skos:notation "sE9.5" ;
    rdfs:isDefinedBy scor: ;
    vs:term_status "stable" ;
    dct:modified "2015-11-05"^^xsd:date ;
.

#############################################################################################
#############################################################################################
#############################################################################################
#### Default Step Configuration

scor:PlanSupplyChainStepList a olo:OrderedList ;
   dct:title "Default Plan Supply Chain Steps"^^xsd:string ;
   dct:description "An ordered list of all process steps involved in the Plan Supply Chain process."^^xsd:string ;
      olo:length 4 ;
      olo:slot [   
         olo:index 1 ;
         olo:item scor:PSCIdentifyPrioritizeAggregateSCRequirements
      ] ;
      olo:slot [
         olo:index 2 ;
         olo:item scor:IdentifyPrioritizeAggregateSCResources
      ] ;
      olo:slot [   
         olo:index 3 ;
         olo:item scor:BalanceSCResourcesWithSCRequirements
      ] ;
      olo:slot [
         olo:index 4 ;
         olo:item scor:EstablishCommunicateSCPlans
      ] ;
.


scor:PlanSourceStepList a olo:OrderedList ;
   dct:title "Default Plan Source Steps"^^xsd:string ;
   dct:description "An ordered list of all process steps involved in the Plan Source process."^^xsd:string ;
      olo:length 4 ;
      olo:slot [   
         olo:index 1 ;
         olo:item scor:IdentifyPrioritizeAggregateProductRequirements
      ] ;
      olo:slot [
         olo:index 2 ;
         olo:item scor:IdentifyAssessAggregateProductResources
      ] ;
      olo:slot [   
         olo:index 3 ;
         olo:item scor:BalanceProductResourcesWithProductRequirements
      ] ;
      olo:slot [
         olo:index 4 ;
         olo:item scor:EstablishSourcingPlans
      ] ;
.

scor:PlanMakeStepList a olo:OrderedList ;
   dct:title "Default Plan Make Steps"^^xsd:string ;
   dct:description "An ordered list of all process steps involved in the Plan Make process."^^xsd:string ;
      olo:length 4 ;
      olo:slot [   
         olo:index 1 ;
         olo:item scor:IdentifyPrioritizeAggregateProductionRequirements
      ] ;
      olo:slot [
         olo:index 2 ;
         olo:item scor:IdentifyAssessAggregateProductionResources
      ] ;
      olo:slot [   
         olo:index 3 ;
         olo:item scor:BalanceProductionResourcesWithProductionRequirements
      ] ;
      olo:slot [
         olo:index 4 ;
         olo:item scor:EstablishProductionPlans
      ] ;
.

scor:PlanDeliverStepList a olo:OrderedList ;
   dct:title "Default Plan Deliver Steps"^^xsd:string ;
   dct:description "An ordered list of all process steps involved in the Plan Deliver process."^^xsd:string ;
      olo:length 4 ;
      olo:slot [   
         olo:index 1 ;
         olo:item scor:IdentifyPrioritizeAggregateDeliveryRequirements
      ] ;
      olo:slot [
         olo:index 2 ;
         olo:item scor:IdentifyAssessAggregateDeliveryResources
      ] ;
      olo:slot [   
         olo:index 3 ;
         olo:item scor:BalanceDeliveryResourcesCapabilitiesWithDeliveryRequirements
      ] ;
      olo:slot [
         olo:index 4 ;
         olo:item scor:EstablishDeliveryPlans
      ] ;
.

scor:PlanReturnStepList a olo:OrderedList ;
   dct:title "Default Plan Return Steps"^^xsd:string ;
   dct:description "An ordered list of all process steps involved in the Plan Return process."^^xsd:string ;
      olo:length 4 ;
      olo:slot [   
         olo:index 1 ;
         olo:item scor:AssessAggregateReturnRequirements
      ] ;
      olo:slot [
         olo:index 2 ;
         olo:item scor:IdentifyAssessAggregateReturnResources
      ] ;
      olo:slot [   
         olo:index 3 ;
         olo:item scor:BalanceReturnResourcesWithReturnRequirements
      ] ;
      olo:slot [
         olo:index 4 ;
         olo:item scor:EstablishCommunicateReturnPlans
      ] ;
.

scor:SRDefectiveProductStepList a olo:OrderedList ;
   dct:title "Source Return Defective Product Steps"^^xsd:string ;
   dct:description "An ordered list of all process steps involved in the Source Return Defective Product process."^^xsd:string ;
      olo:length 5 ;
      olo:slot [   
         olo:index 1 ;
         olo:item scor:IdentifyDefectiveProductCondition
      ] ;
      olo:slot [
         olo:index 2 ;
         olo:item scor:DispositionDefectiveProduct
      ] ;
      olo:slot [   
         olo:index 3 ;
         olo:item scor:RequestDefectiveProductReturnAuthorization
      ] ;
      olo:slot [
         olo:index 4 ;
         olo:item scor:ScheduleDefectiveProductShipment
      ] ;
      olo:slot [
         olo:index 5 ;
         olo:item scor:ReturnDefectiveProduct
      ] ;
.

scor:SRMROProductStepList a olo:OrderedList ;
   dct:title "Source Return MRO Product Steps"^^xsd:string ;
   dct:description "An ordered list of all process steps involved in the Source Return MRO Product process."^^xsd:string ;
      olo:length 5 ;
      olo:slot [   
         olo:index 1 ;
         olo:item scor:IdentifyMROProductCondition
      ] ;
      olo:slot [
         olo:index 2 ;
         olo:item scor:DispositionMROProduct
      ] ;
      olo:slot [   
         olo:index 3 ;
         olo:item scor:RequestMROReturnAuthorization
      ] ;
      olo:slot [
         olo:index 4 ;
         olo:item scor:ScheduleMROShipment
      ] ;
      olo:slot [
         olo:index 5 ;
         olo:item scor:ReturnMROPRoduct
      ] ;
.

scor:SRExcessProductStepList a olo:OrderedList ;
   dct:title "Source Return Excess Product Steps"^^xsd:string ;
   dct:description "An ordered list of all process steps involved in the Source Return Excess Product process."^^xsd:string ;
      olo:length 5 ;
      olo:slot [   
         olo:index 1 ;
         olo:item scor:IdentifyExcessProductCondition
      ] ;
      olo:slot [
         olo:index 2 ;
         olo:item scor:DispositionExcessProduct
      ] ;
      olo:slot [   
         olo:index 3 ;
         olo:item scor:BalanceProductionResourcesWithProductionRequirements
      ] ;
      olo:slot [
         olo:index 4 ;
         olo:item scor:ScheduleExcessProductShipment
      ] ;
      olo:slot [
         olo:index 5 ;
         olo:item scor:ReturnExcessProduct
      ] ;
.

scor:DRDefectiveProductStepList a olo:OrderedList ;
   dct:title "Deliver Return Defective Product Steps"^^xsd:string ;
   dct:description "An ordered list of all process steps involved in the Deliver Return Defective Product process."^^xsd:string ;
      olo:length 4 ;
      olo:slot [   
         olo:index 1 ;
         olo:item scor:AuthorizeDefectiveProductReturn
      ] ;
      olo:slot [
         olo:index 2 ;
         olo:item scor:ScheduleDefectiveReturnReceipt
      ] ;
      olo:slot [   
         olo:index 3 ;
         olo:item scor:ReceiveDefectiveProduct
      ] ;
      olo:slot [
         olo:index 4 ;
         olo:item scor:TransferExcessProduct
      ] ;
.

scor:DRMROProductStepList a olo:OrderedList ;
   dct:title "Deliver Return MRO Product Steps"^^xsd:string ;
   dct:description "An ordered list of all process steps involved in the Deliver Return MRO Product process."^^xsd:string ;
      olo:length 4 ;
      olo:slot [   
         olo:index 1 ;
         olo:item scor:AuthorizeMROProductReturn
      ] ;
      olo:slot [
         olo:index 2 ;
         olo:item scor:ScheduleMROReturnReceipt
      ] ;
      olo:slot [   
         olo:index 3 ;
         olo:item scor:ReceiveMROProduct
      ] ;
      olo:slot [
         olo:index 4 ;
         olo:item scor:TransferMROProduct
      ] ;
.


scor:DRExcessProductStepList a olo:OrderedList ;
   dct:title "Deliver Return Excess Product Steps"^^xsd:string ;
   dct:description "An ordered list of all process steps involved in the Deliver Return Excess Product process."^^xsd:string ;
      olo:length 4 ;
      olo:slot [   
         olo:index 1 ;
         olo:item scor:AuthorizeExcessProductReturn
      ] ;
      olo:slot [
         olo:index 2 ;
         olo:item scor:ScheduleExcessReturnReceipt
      ] ;
      olo:slot [   
         olo:index 3 ;
         olo:item scor:ReceiveExcessProduct
      ] ;
      olo:slot [
         olo:index 4 ;
         olo:item scor:TransferExcessProduct
      ] ;
.

scor:SourceStockedProductStepList a olo:OrderedList ;
   dct:title "Source Stocked Product Steps"^^xsd:string ;
   dct:description "An ordered list of all process steps involved in the Source Stocked Product process."^^xsd:string ;
      olo:length 5 ;
      olo:slot [   
         olo:index 1 ;
         olo:item scor:SSPScheduleProductDeliveries
      ] ;
      olo:slot [
         olo:index 2 ;
         olo:item scor:SSPReceiveProduct
      ] ;
      olo:slot [   
         olo:index 3 ;
         olo:item scor:SSPVerifyProduct
      ] ;
      olo:slot [
         olo:index 4 ;
         olo:item scor:SSPTransferProduct
      ] ;
      olo:slot [
         olo:index 5 ;
         olo:item scor:AuthorizeSupplierPayment
      ] ;
.

scor:SourceMakeToOrderProductStepList a olo:OrderedList ;
   dct:title "Source Make-to-Order Product Steps"^^xsd:string ;
   dct:description "An ordered list of all process steps involved in the Source Make-to-Order process."^^xsd:string ;
      olo:length 5 ;
      olo:slot [   
         olo:index 1 ;
         olo:item scor:SMOPScheduleProductDeliveries
      ] ;
      olo:slot [
         olo:index 2 ;
         olo:item scor:SMOPReceiveProduct
      ] ;
      olo:slot [   
         olo:index 3 ;
         olo:item scor:SMOPVerifyProduct
      ] ;
      olo:slot [
         olo:index 4 ;
         olo:item scor:SMOPTransferProduct
      ] ;
      olo:slot [
         olo:index 5 ;
         olo:item scor:SMOPAuthorizeSupplierPayment
      ] ;
.

scor:SourceEngineerToOrderProductStepList a olo:OrderedList ;
   dct:title "Source Engineer-to-Order Product Steps"^^xsd:string ;
   dct:description "An ordered list of all process steps involved in the Source Engineer-to-Order process."^^xsd:string ;
      olo:length 7 ;
      olo:slot [   
         olo:index 1 ;
         olo:item scor:IdentifySourcesOfSupply
      ] ;
      olo:slot [
         olo:index 2 ;
         olo:item scor:SelectFinalSupplierNegotiate
      ] ;
      olo:slot [   
         olo:index 3 ;
         olo:item scor:SEOPScheduleProductDeliveries
      ] ;
      olo:slot [
         olo:index 4 ;
         olo:item scor:SEOPReceiveProduct
      ] ;
      olo:slot [
         olo:index 5 ;
         olo:item scor:SEOPVerifyProduct
      ] ;
      olo:slot [
         olo:index 6 ;
         olo:item scor:SEOPTransferProduct
      ] ;
      olo:slot [
         olo:index 7 ;
         olo:item scor:SEOPAuthorizeSupplierPayment
      ] ;
.

scor:MakeToStockStepList a olo:OrderedList ;
   dct:title "Make-to-Stock Product Steps"^^xsd:string ;
   dct:description "An ordered list of all process steps involved in the Make-to-Stock process."^^xsd:string ;
      olo:length 7 ;
      olo:slot [   
         olo:index 1 ;
         olo:item scor:MSScheduleProductionActivities
      ] ;
      olo:slot [
         olo:index 2 ;
         olo:item scor:IssueMaterial
      ] ;
      olo:slot [   
         olo:index 3 ;
         olo:item scor:MSProduceTest
      ] ;
      olo:slot [
         olo:index 4 ;
         olo:item scor:MSPackage
      ] ;
      olo:slot [
         olo:index 5 ;
         olo:item scor:StageProduct
      ] ;
      olo:slot [
         olo:index 6 ;
         olo:item scor:ReleaseProductToDeliver
      ] ;
      olo:slot [
         olo:index 7 ;
         olo:item scor:MSWasteDisposal
      ] ;
.

scor:MakeToOrderStepList a olo:OrderedList ;
   dct:title "Make-to-Order Product Steps"^^xsd:string ;
   dct:description "An ordered list of all process steps involved in the Make-to-Order process."^^xsd:string ;
      olo:length 7 ;
      olo:slot [   
         olo:index 1 ;
         olo:item scor:MOScheduleProductionActivities
      ] ;
      olo:slot [
         olo:index 2 ;
         olo:item scor:IssueSourcedInProcessProduct
      ] ;
      olo:slot [   
         olo:index 3 ;
         olo:item scor:MOProduceTest
      ] ;
      olo:slot [
         olo:index 4 ;
         olo:item scor:MOPackage
      ] ;
      olo:slot [
         olo:index 5 ;
         olo:item scor:StageFinishedProduct
      ] ;
      olo:slot [
         olo:index 6 ;
         olo:item scor:ReleaseFinishedProductToDeliver
      ] ;
      olo:slot [
         olo:index 7 ;
         olo:item scor:MOWasteDisposal
      ] ;
.

scor:EngineerToOrderStepList a olo:OrderedList ;
   dct:title "Engineer-to-Order Product Steps"^^xsd:string ;
   dct:description "An ordered list of all process steps involved in the Engineer-to-Order process."^^xsd:string ;
      olo:length 8 ;
      olo:slot [   
         olo:index 1 ;
         olo:item scor:FinalizeProductionEngineering
      ] ;
      olo:slot [
         olo:index 2 ;
         olo:item scor:MEOScheduleProductionActivities
      ] ;
      olo:slot [   
         olo:index 3 ;
         olo:item scor:MEOSourcedInProcessProduct
      ] ;
      olo:slot [
         olo:index 4 ;
         olo:item scor:MEOProduceTest
      ] ;
      olo:slot [
         olo:index 5 ;
         olo:item scor:MEOPackage
      ] ;
      olo:slot [
         olo:index 6 ;
         olo:item scor:MEOStageFinishedProduct
      ] ;
      olo:slot [
         olo:index 7 ;
         olo:item scor:MEOReleaseProductToDeliver
      ] ;
      olo:slot [
         olo:index 8 ;
         olo:item scor:MEOWasteDisposal
      ] ;
.

scor:ManageSCBusinessRulesStepList a olo:OrderedList ;
   dct:title "Manage Supply Chain Business Rules Steps"^^xsd:string ;
   dct:description "An ordered list of all process steps involved in the Manage Supply Chain Business Rules process."^^xsd:string ;
      olo:length 6 ;
      olo:slot [   
         olo:index 1 ;
         olo:item scor:GatherBusinessRuleRequirements
      ] ;
      olo:slot [
         olo:index 2 ;
         olo:item scor:InterpretBusinessRuleRequirement
      ] ;
      olo:slot [   
         olo:index 3 ;
         olo:item scor:DocumentBusinessRule
      ] ;
      olo:slot [
         olo:index 4 ;
         olo:item scor:CommunicateBusinessRule
      ] ;
      olo:slot [
         olo:index 5 ;
         olo:item scor:ReleaseAndPublishBusinessRule
      ] ;
      olo:slot [
         olo:index 6 ;
         olo:item scor:RetireBusinessRule
      ] ;
.

scor:ManageSCPerformanceStepList a olo:OrderedList ;
   dct:title "Manage Supply Chain Performance Steps"^^xsd:string ;
   dct:description "An ordered list of all process steps involved in the Manage Supply Chain Performance process."^^xsd:string ;
      olo:length 6 ;
      olo:slot [   
         olo:index 1 ;
         olo:item scor:InitiateReporting
      ] ;
      olo:slot [
         olo:index 2 ;
         olo:item scor:AnalyzeReports
      ] ;
      olo:slot [   
         olo:index 3 ;
         olo:item scor:PrioritizeRootCauses
      ] ;
      olo:slot [
         olo:index 4 ;
         olo:item scor:DevelopeCorrectiveActions
      ] ;
      olo:slot [
         olo:index 5 ;
         olo:item scor:DevelopeCorrectiveActions
      ] ;
      olo:slot [
         olo:index 6 ;
         olo:item scor:ApproveAndLaunch
      ] ;
.

scor:ManageSCDataAndInformationStepList a olo:OrderedList ;
   dct:title "Manage Supply Chain Data and Information Steps"^^xsd:string ;
   dct:description "An ordered list of all process steps involved in the Manage Supply Chain Data and Information process."^^xsd:string ;
      olo:length 6 ;
      olo:slot [   
         olo:index 1 ;
         olo:item scor:DetermineAndScopeWork
      ] ;
      olo:slot [
         olo:index 2 ;
         olo:item scor:DetermineAndScopeWork
      ] ;
      olo:slot [   
         olo:index 3 ;
         olo:item scor:MaintainContentAndCode
      ] ;
      olo:slot [
         olo:index 4 ;
         olo:item scor:MaintainAccess
      ] ;
      olo:slot [
         olo:index 5 ;
         olo:item scor:PublishInformation
      ] ;
      olo:slot [
         olo:index 6 ;
         olo:item scor:VerfyInformation
      ] ;
.

scor:ManageSCHumanResourcesStepList a olo:OrderedList ;
   dct:title "Manage Supply Chain Human Resources Steps"^^xsd:string ;
   dct:description "An ordered list of all process steps involved in the Manage Supply Chain Human Resources process."^^xsd:string ;
      olo:length 6 ;
      olo:slot [   
         olo:index 1 ;
         olo:item scor:VerifyInformation
      ] ;
      olo:slot [
         olo:index 2 ;
         olo:item scor:IdentifyAvailableSkillsAndResources
      ] ;
      olo:slot [   
         olo:index 3 ;
         olo:item scor:MatchSkillsAndResources
      ] ;
      olo:slot [
         olo:index 4 ;
         olo:item scor:DetermineHiringAndRedeployment
      ] ;
      olo:slot [
         olo:index 5 ;
         olo:item scor:DetermineTrainingAndEducation
      ] ;
      olo:slot [
         olo:index 6 ;
         olo:item scor:ApprovePrioritizeAndLaunch
      ] ;
.

scor:ManageSCAssetsStepList a olo:OrderedList ;
   dct:title "Manage Supply Chain Assets Steps"^^xsd:string ;
   dct:description "An ordered list of all process steps involved in the Manage Supply Chain Assets process."^^xsd:string ;
      olo:length 8 ;
      olo:slot [   
         olo:index 1 ;
         olo:item scor:ScheduleAssetManagementActivities
      ] ;
      olo:slot [
         olo:index 2 ;
         olo:item scor:TakeAssetOffline
      ] ;
      olo:slot [   
         olo:index 3 ;
         olo:item scor:InspectAndTroubleshoot
      ] ;
      olo:slot [
         olo:index 4 ;
         olo:item scor:InstallAndConfigure
      ] ;
      olo:slot [
         olo:index 5 ;
         olo:item scor:CleanMaintainAndRepair
      ] ;
      olo:slot [
         olo:index 6 ;
         olo:item scor:DecomissionAndDispose
      ] ;
      olo:slot [
         olo:index 7 ;
         olo:item scor:InspectMaintenance
      ] ;
      olo:slot [
         olo:index 8 ;
         olo:item scor:ReinstateAsset
      ] ;
.


scor:ManageSCContractsStepList a olo:OrderedList ;
   dct:title "Manage Supply Chain Contracts Steps"^^xsd:string ;
   dct:description "An ordered list of all process steps involved in the Manage Supply Chain Contracts process."^^xsd:string ;
      olo:length 7 ;
      olo:slot [   
         olo:index 1 ;
         olo:item scor:ReceiveContractUpdates
      ] ;
      olo:slot [
         olo:index 2 ;
         olo:item scor:EnterAndDistirbuteContract
      ] ;
      olo:slot [   
         olo:index 3 ;
         olo:item scor:ActiviateOrArchiveContract
      ] ;
      olo:slot [
         olo:index 4 ;
         olo:item scor:ReviewContractualPerformance
      ] ;
      olo:slot [
         olo:index 5 ;
         olo:item scor:IdentifyPerformanceIssuesAndOpportunities
      ] ;
      olo:slot [
         olo:index 6 ;
         olo:item scor:IdentifyResolutionsAndImprovements
      ] ;
      olo:slot [
         olo:index 7 ;
         olo:item scor:SelectPrioritizeAndDistributeResolutions
      ] ;
.

scor:ManageSCNetworkStepList a olo:OrderedList ;
   dct:title "Manage Supply Chain Network Steps"^^xsd:string ;
   dct:description "An ordered list of all process steps involved in the Manage Supply Chain Networks process."^^xsd:string ;
      olo:length 8 ;
      olo:slot [   
         olo:index 1 ;
         olo:item scor:SelectScopeAndOrganization
      ] ;
      olo:slot [
         olo:index 2 ;
         olo:item scor:GatherInputAndData
      ] ;
      olo:slot [   
         olo:index 3 ;
         olo:item scor:DevelopeScenarios
      ] ;
      olo:slot [
         olo:index 4 ;
         olo:item scor:ModelAndSimulateScenarios
      ] ;
      olo:slot [
         olo:index 5 ;
         olo:item scor:ProjectImpact
      ] ;
      olo:slot [
         olo:index 6 ;
         olo:item scor:SelectAndApprove
      ] ;
      olo:slot [
         olo:index 7 ;
         olo:item scor:DevelopChangeProgram
      ] ;
      olo:slot [
         olo:index 8 ;
         olo:item scor:LaunchChangeProgram
      ] ;
.

scor:ManageSCRegulatoryComplianceStepList a olo:OrderedList ;
   dct:title "Manage Supply Chain Regulatory Compliance Steps"^^xsd:string ;
   dct:description "An ordered list of all process steps involved in the Manage Supply Chain Regulatory Compliance process."^^xsd:string ;
      olo:length 7 ;
      olo:slot [   
         olo:index 1 ;
         olo:item scor:MonitorRegulatoryEntities
      ] ;
      olo:slot [
         olo:index 2 ;
         olo:item scor:AssessRegulatoryPublications
      ] ;
      olo:slot [   
         olo:index 3 ;
         olo:item scor:IdentifyRegulatoryDeficiencies
      ] ;
      olo:slot [
         olo:index 4 ;
         olo:item scor:DefineRemediation
      ] ;
      olo:slot [
         olo:index 5 ;
         olo:item scor:VerifyAndObtainLicense
      ] ;
      olo:slot [
         olo:index 6 ;
         olo:item scor:VerifyAndObtainLicense
      ] ;
      olo:slot [
         olo:index 7 ;
         olo:item scor:PublishRemediation
      ] ;
.

scor:ManageSCRiskStepList a olo:OrderedList ;
   dct:title "Manage Supply Chain Risk Steps"^^xsd:string ;
   dct:description "An ordered list of all process steps involved in the Manage Supply Chain Risk process."^^xsd:string ;
      olo:length 5 ;
      olo:slot [   
         olo:index 1 ;
         olo:item scor:EstablishContext
      ] ;
      olo:slot [
         olo:index 2 ;
         olo:item scor:IdentifyRiskEvents
      ] ;
      olo:slot [   
         olo:index 3 ;
         olo:item scor:QuantifyRisks
      ] ;
      olo:slot [
         olo:index 4 ;
         olo:item scor:EvaluateRisks
      ] ;
      olo:slot [
         olo:index 5 ;
         olo:item scor:MitigateRisk
      ] ;
.

scor:DeliverStockedProductStepList a olo:OrderedList ;
   dct:title "Deliver Stocked Product Steps"^^xsd:string ;
   dct:description "An ordered list of all process steps involved in the Deliver Stocked Product process."^^xsd:string ;
      olo:length 15 ;
      olo:slot [   
         olo:index 1 ;
         olo:item scor:ProcessInquiryQuote
      ] ;
      olo:slot [
         olo:index 2 ;
         olo:item scor:ReceiveEnterValidateOrder
      ] ;
      olo:slot [   
         olo:index 3 ;
         olo:item scor:DSPReserveInventoryDetermineDeliveryDate
      ] ;
      olo:slot [
         olo:index 4 ;
         olo:item scor:DSPConsolidateOrders
      ] ;
      olo:slot [
         olo:index 5 ;
         olo:item scor:DSPBuildLoads
      ] ;
      olo:slot [   
         olo:index 6 ;
         olo:item scor:DSPRouteShipments
      ] ;
      olo:slot [
         olo:index 7 ;
         olo:item scor:DSPSelectCarriersRateShipments
      ] ;
      olo:slot [   
         olo:index 8 ;
         olo:item scor:DSPReceiveProductFromSourceMake
      ] ;
      olo:slot [
         olo:index 9 ;
         olo:item scor:DSPPickProduct
      ] ;
      olo:slot [
         olo:index 10 ;
         olo:item scor:DSPPackProduct
      ] ;
      olo:slot [   
         olo:index 11 ;
         olo:item scor:LoadVehicleGenerateShippingDocuments
      ] ;
      olo:slot [
         olo:index 12 ;
         olo:item scor:DSPShipProduct
      ] ;
      olo:slot [   
         olo:index 13 ;
         olo:item scor:DSPReceiveVerifyProductByCustomer
      ] ;
      olo:slot [
         olo:index 14 ;
         olo:item scor:DSPInstallProduct
      ] ;
      olo:slot [
         olo:index 15 ;
         olo:item scor:DSPInvoice
      ] ;
.

scor:DeliverMakeToOrderProductStepList a olo:OrderedList ;
   dct:title "Deliver Make-to-Order Product Steps"^^xsd:string ;
   dct:description "An ordered list of all process steps involved in the Deliver Make-to-Order Product process."^^xsd:string ;
      olo:length 15 ;
      olo:slot [   
         olo:index 1 ;
         olo:item scor:DMOPInquiryQuote
      ] ;
      olo:slot [
         olo:index 2 ;
         olo:item scor:ReceiveConfigureEnterValidateOrder
      ] ;
      olo:slot [   
         olo:index 3 ;
         olo:item scor:DMOPReserveInventoryDetermineDeliveryDate
      ] ;
      olo:slot [
         olo:index 4 ;
         olo:item scor:DMOPConsolidateOrders
      ] ;
      olo:slot [
         olo:index 5 ;
         olo:item scor:DMOPBuildLoads
      ] ;
      olo:slot [   
         olo:index 6 ;
         olo:item scor:DMOPRouteShipments
      ] ;
      olo:slot [
         olo:index 7 ;
         olo:item scor:DMOPSelectCarriersRateShipments
      ] ;
      olo:slot [   
         olo:index 8 ;
         olo:item scor:DMOPReceiveProductFromSourceMake
      ] ;
      olo:slot [
         olo:index 9 ;
         olo:item scor:DMOPPickProduct
      ] ;
      olo:slot [
         olo:index 10 ;
         olo:item scor:DMOPPackProduct
      ] ;
      olo:slot [   
         olo:index 11 ;
         olo:item scor:DMOPLoadProductGenerateShippingDocs
      ] ;
      olo:slot [
         olo:index 12 ;
         olo:item scor:DMOPShipProduct
      ] ;
      olo:slot [   
         olo:index 13 ;
         olo:item scor:DMOPReceiveVerifyProductByCustomer
      ] ;
      olo:slot [
         olo:index 14 ;
         olo:item scor:DMOPInstallProduct
      ] ;
      olo:slot [
         olo:index 15 ;
         olo:item scor:DMOPInvoice
      ] ;
.

scor:DeliverEngineerToProductStepList a olo:OrderedList ;
   dct:title "Deliver Engineer-to-Order Product Steps"^^xsd:string ;
   dct:description "An ordered list of all process steps involved in the Deliver Stocked Product process."^^xsd:string ;
      olo:length 15 ;
      olo:slot [   
         olo:index 1 ;
         olo:item scor:ObtainRespondToRFPRFQ
      ] ;
      olo:slot [
         olo:index 2 ;
         olo:item scor:NegotiateReceiveContract
      ] ;
      olo:slot [   
         olo:index 3 ;
         olo:item scor:EnterOrderCommitResourcesLaunchProgram
      ] ;
      olo:slot [
         olo:index 4 ;
         olo:item scor:ScheduleInstallation
      ] ;
      olo:slot [
         olo:index 5 ;
         olo:item scor:DEOPBuildLoads
      ] ;
      olo:slot [   
         olo:index 6 ;
         olo:item scor:DEOPRouteShipments
      ] ;
      olo:slot [
         olo:index 7 ;
         olo:item scor:DEOPSelectCarriersRateShipments
      ] ;
      olo:slot [   
         olo:index 8 ;
         olo:item scor:DEOPReceiveProductFromSourceMake
      ] ;
      olo:slot [
         olo:index 9 ;
         olo:item scor:DEOPPickProduct
      ] ;
      olo:slot [
         olo:index 10 ;
         olo:item scor:DEOPPackProduct
      ] ;
      olo:slot [   
         olo:index 11 ;
         olo:item scor:DEOPLoadProductGenerateShippingDocs
      ] ;
      olo:slot [
         olo:index 12 ;
         olo:item scor:DEOPShipProduct
      ] ;
      olo:slot [   
         olo:index 13 ;
         olo:item scor:DEOPReceiveVerifyProductByCustomer
      ] ;
      olo:slot [
         olo:index 14 ;
         olo:item scor:DEOPInstallProduct
      ] ;
      olo:slot [
         olo:index 15 ;
         olo:item scor:DEOPInvoice
      ] ;
.

scor:DeliverRetailProductStepList a olo:OrderedList ;
   dct:title "Deliver Retail Product Steps"^^xsd:string ;
   dct:description "An ordered list of all process steps involved in the Deliver Retail Product process."^^xsd:string ;
      olo:length 7 ;
      olo:slot [   
         olo:index 1 ;
         olo:item scor:GenerateStockingSchedule
      ] ;
      olo:slot [
         olo:index 2 ;
         olo:item scor:ReceiveProductAtStore
      ] ;
      olo:slot [   
         olo:index 3 ;
         olo:item scor:PickProductFromBackroom
      ] ;
      olo:slot [
         olo:index 4 ;
         olo:item scor:StockShelf
      ] ;
      olo:slot [
         olo:index 5 ;
         olo:item scor:FillShoppingCart
      ] ;
      olo:slot [   
         olo:index 6 ;
         olo:item scor:Checkout
      ] ;
      olo:slot [
         olo:index 7 ;
         olo:item scor:DeliverInstall
      ] ;
.


#############################################################################################
#############################################################################################
#############################################################################################
#### Properties

scor:isStepOf
    rdf:type owl:ObjectProperty ;
    rdfs:label "is Step of"@en ;
    rdfs:domain scor:Process ;
    rdfs:range  scor:Process ;
    rdfs:comment "Steps which are part of a certain process"@en  ;
    rdfs:isDefinedBy scor: ;
    vs:term_status "stable" ;
    dct:modified "2015-11-05"^^xsd:date ;
 .

scor:hasDefaultSteps
    rdf:type owl:AnnotationProperty;
    rdfs:label "has default steps"@en;
    rdfs:domain owl:Class;
    rdfs:range olo:OrderedList;
    rdfs:isDefinedBy scor: ;
	rdfs:comment "A list of default steps for a specific class of processes. A particular instance of the class can override this by using scor:hasSteps."@en  ;
    vs:term_status "stable" ;
    dct:modified "2015-11-16"^^xsd:date .
	
scor:hasSteps
    rdf:type owl:ObjectProperty;
    rdfs:label "has Step List"@en ;
    rdfs:domain scor:Process ;
    rdfs:range  olo:OrderedList;
    rdfs:comment "A list of steps for certain processes"@en  ;
    rdfs:isDefinedBy scor: ;
    vs:term_status "stable" ;
    dct:modified "2015-11-05"^^xsd:date ;
 .

scor:hasAptitude
    rdf:type rdf:Property ;
    rdfs:domain scor:Skill ;
    rdfs:range scor:Aptitude ;
    rdfs:comment "An aptitude required for certain skills"@en  ;
    rdfs:label "has Aptitude"@en  ;
    rdfs:isDefinedBy scor: ;
    vs:term_status "stable" ;
    dct:modified "2015-11-05"^^xsd:date ;
 .

scor:hasExperience
    rdf:type rdf:Property ;
    rdfs:domain scor:Skill ;
    rdfs:range scor:Experience ;
    rdfs:label "has Experience"@en  ;
    rdfs:comment "An Experience required for certain skills"@en  ;
    rdfs:isDefinedBy scor: ;
    vs:term_status "stable" ;
    dct:modified "2015-11-05"^^xsd:date ;
 .

scor:hasSkill
    rdf:type rdf:Property ;
    rdfs:domain schema:Person ;
    rdfs:label "has Skill"@en  ;
    rdfs:comment "A Skill of a Person"@en  ;
    rdfs:range scor:Skill ;
    rdfs:isDefinedBy scor: ;
    vs:term_status "stable" ;
    dct:modified "2015-11-05"^^xsd:date ;
 .

scor:hasTraining
    rdf:type rdf:Property ;
    rdfs:domain scor:Skill ;
    rdfs:label "has Training"@en  ;
    rdfs:comment "A Training required to gain a skill"@en  ;
    rdfs:range scor:Training ;
    rdfs:isDefinedBy scor: ;
    vs:term_status "stable" ;
    dct:modified "2015-11-05"^^xsd:date ;
 .

##########################################################################################
#### Metric Properties

scor:hasMetric
    rdf:type owl:DatatypeProperty ;
    rdfs:range xsd:decimal ;
    rdfs:isDefinedBy scor: ;
    rdfs:comment "A Meric related to Processes"@en ;
    rdfs:label "has Metric"@en;
    vs:term_status "stable" ;
    dct:modified "2015-11-05"^^xsd:date ;
 .

scor:hasReliabilityMetric
    rdf:type owl:DatatypeProperty ;
    rdfs:subPropertyOf scor:hasMetric ;
    rdfs:range xsd:decimal ;
    rdfs:isDefinedBy scor: ;
    rdfs:comment "A reliability metric related to Processes"@en ;
    rdfs:label "has reliability metric"@en;
    vs:term_status "stable" ;
    dct:modified "2015-11-05"^^xsd:date ;
 .

 scor:hasResponsivenessMetric
    rdf:type owl:DatatypeProperty ;
    rdfs:subPropertyOf scor:hasMetric ;
    rdfs:range xsd:decimal ;
    rdfs:isDefinedBy scor: ;
    rdfs:comment "A responsiveness metric related to Processes"@en ;
    rdfs:label "has responsiveness metric"@en;
    vs:term_status "stable" ;
    dct:modified "2015-11-05"^^xsd:date ;
 .

 scor:hasAgilityMetric
    rdf:type owl:DatatypeProperty ;
    rdfs:subPropertyOf scor:hasMetric ;
    rdfs:range xsd:decimal ;
    rdfs:isDefinedBy scor: ;
    rdfs:comment "A agility metric related to Processes"@en ;
    rdfs:label "has agility metric"@en;
    vs:term_status "stable" ;
    dct:modified "2015-11-05"^^xsd:date ;
 .

  scor:hasCostMetric
    rdf:type owl:DatatypeProperty ;
    rdfs:subPropertyOf scor:hasMetric ;
    rdfs:range xsd:decimal ;
    rdfs:isDefinedBy scor: ;
    rdfs:comment "A cost metric related to Processes"@en ;
    rdfs:label "has cost metric"@en;
    vs:term_status "stable" ;
    dct:modified "2015-11-05"^^xsd:date ;
 .

scor:hasAssetManagemenEfficiencyMetric 
    rdf:type owl:DatatypeProperty ;
    rdfs:subPropertyOf scor:hasMetric ;
    rdfs:range xsd:decimal ;
    rdfs:isDefinedBy scor: ;
    rdfs:comment "An asset management efficiency metric related to Processes"@en ;
    rdfs:label "has asset management efficiency metric"@en;
    vs:term_status "stable" ;
    dct:modified "2015-11-05"^^xsd:date ;
 .


######### Reliability Metrics

scor:hasMetricRL_1
    rdfs:subPropertyOf scor:hasReliabilityMetric ;
    rdf:type owl:DatatypeProperty ;
    rdfs:domain scor:ReleaseProductToDeliver ;
    rdfs:label "# of complaints regarding missing environmental documentation"@en;
    rdfs:comment "The number of products released without proper environmental documentation as a percent of total products released"@en ;
    rdfs:isDefinedBy scor: ;
    vs:term_status "stable" ;
    dct:modified "2015-11-05"^^xsd:date ;
 .

scor:hasMetricRL_2
    rdfs:subPropertyOf scor:hasReliabilityMetric ;
    rdf:type owl:DatatypeProperty ;
    rdfs:domain scor:ReleaseProductToDeliver ;
    rdfs:label "# of recordkeeping related NOVs"@en;
    rdfs:comment "The number of recordkeeping related regulatory violations received per year"@en;
    rdfs:isDefinedBy scor: ;
    vs:term_status "stable" ;
    dct:modified "2015-11-05"^^xsd:date ;
 .

#3 seems to be deprecated #


scor:hasMetricRL_4
    rdfs:subPropertyOf scor:hasReliabilityMetric ;
    rdf:type owl:DatatypeProperty ;
    rdfs:domain [rdf:type owl:Class ;
        owl:unionOf (
        scor:DSPPackProduct
        scor:DMOPPickProduct
        scor:SSPReceiveProduct
        )] ;
    rdfs:label "% correct material documentation"@en;
    rdfs:comment "The percent of total shipments that include the correct environmental documentation"@en;
    rdfs:isDefinedBy scor: ;
    vs:term_status "stable" ;
    dct:modified "2015-11-05"^^xsd:date ;
 .

scor:hasMetricRL_5
    rdfs:subPropertyOf scor:hasReliabilityMetric ;
    rdf:type owl:DatatypeProperty ;
    rdfs:domain [rdf:type owl:Class ;
        owl:unionOf (
        scor:ReturnDefectiveProduct
        scor:ReturnMROPRoduct
        scor:ReturnExcessProduct
        )] ;
    rdfs:label "% Error-freeReturns Shipped"@en;
    rdfs:comment "Percentage of Error-free Returns Shipped"@en;
    rdfs:isDefinedBy scor: ;
    vs:term_status "stable" ;
    dct:modified "2015-11-05"^^xsd:date ;
 .

scor:hasMetricRL_6
    rdfs:subPropertyOf scor:hasReliabilityMetric ;
    rdf:type owl:DatatypeProperty ;
    rdfs:domain scor:DispositionMROProduct ;
    rdfs:label "% Identified MROProducts ReturnedTo Service"@en;
    rdfs:comment "Percentage Identified MROProducts ReturnedTo Service"@en;
    rdfs:isDefinedBy scor: ;
    vs:term_status "stable" ;
    dct:modified "2015-11-05"^^xsd:date ;
 .

scor:hasMetricRL_7
    rdfs:subPropertyOf scor:hasReliabilityMetric ;
    rdf:type owl:DatatypeProperty ;
    rdfs:domain scor:FillShoppingCart;
    rdfs:label "Item Location Accuracy"@en;
    rdfs:comment "Percentage of items delivered at the correct Location"@en;
    rdfs:isDefinedBy scor: ;
    vs:term_status "stable" ;
    dct:modified "2015-11-05"^^xsd:date ;
 .

#8 seems to be deprecated

#9 seems to be deprecated

scor:hasMetricRL_10
    rdfs:subPropertyOf scor:hasReliabilityMetric ;
    rdf:type owl:DatatypeProperty ;
    rdfs:domain [rdf:type owl:Class ;
        owl:unionOf (
        scor:SourceReturnExcessProduct
        scor:DeliverReturnExcessProduct
        )] ;
    rdfs:label "% of Excess Product Returns Delivered Complete to the Designated Return Center"@en;
    rdfs:comment "Correct destination, according to the schedule, with the correct part and documentation"@en;
    rdfs:isDefinedBy scor: ;
    vs:term_status "stable" ;
    dct:modified "2015-11-05"^^xsd:date ;
 .

scor:hasMetricRL_11
    rdfs:subPropertyOf scor:hasReliabilityMetric ;
    rdf:type owl:DatatypeProperty ;
    rdfs:domain [rdf:type owl:Class ;
        owl:unionOf (
        scor:DSPInvoice
        scor:DMOPInvoice
        scor:DEOPInvoice
        )] ;
    rdfs:label "% of Faultless Invoices"@en;
    rdfs:comment "The number of invoices processed without issues and or errors divided by the total number of invoices. Examples of potential invoice defects are: Change from customer purchase order without proper customer involvement Wrong Customer Information (e.g., name, address, telephone number) Wrong Product Information (e.g., part number, product description) Wrong Price (e.g., discounts not applied) Wrong Quantity or Wrong Terms or Wrong Date"@en;
    rdfs:isDefinedBy scor: ;
    vs:term_status "stable" ;
    dct:modified "2015-11-05"^^xsd:date ;
 .

scor:hasMetricRL_12
    rdfs:subPropertyOf scor:hasReliabilityMetric ;
    rdf:type owl:DatatypeProperty ;
    rdfs:domain scor:DSPInstallProduct ;
    rdfs:label "% Of Faultless Installations"@en;
    rdfs:comment "Number of Faultless Installations divided by Total Number of Units Installed."@en;
    rdfs:isDefinedBy scor: ;
    vs:term_status "stable" ;
    dct:modified "2015-11-05"^^xsd:date ;
 .

scor:hasMetricRL_13
    rdfs:subPropertyOf scor:hasReliabilityMetric ;
    rdf:type owl:DatatypeProperty ;
    rdfs:domain scor:DeliverReturnMROProduct ;
    rdfs:label "% of MRO returnsdelivered to the correct service provider location"@en;
    rdfs:comment "% of MRO returns delivered to the correct service provider location, within schedule, with the correct part and documentation"@en;
    rdfs:isDefinedBy scor: ;
    vs:term_status "stable" ;
    dct:modified "2015-11-05"^^xsd:date ;
 .

scor:hasMetricRL_14
    rdfs:subPropertyOf scor:hasReliabilityMetric ;
    rdf:type owl:DatatypeProperty ;
    rdfs:domain scor:ReleaseFinishedProductToDeliver ;
    rdfs:label "% of products meeting specified environmental performance requirements"@en;
    rdfs:comment "The number of products that meet desired environmental performance specifications as a percent of total products produced"@en;
    rdfs:isDefinedBy scor: ;
    vs:term_status "stable" ;
    dct:modified "2015-11-05"^^xsd:date ;
 .

scor:hasMetricRL_15
    rdfs:subPropertyOf scor:hasReliabilityMetric ;
    rdf:type owl:DatatypeProperty;
    rdfs:domain scor:ReleaseFinishedProductToDeliver ;
    rdfs:label "% of products with proper environmental labeling (if required)"@en;
    rdfs:comment "The number of products with proper environmental labels in place as a per cent of total products produced"@en;
    rdfs:isDefinedBy scor: ;
    vs:term_status "stable" ;
    dct:modified "2015-11-05"^^xsd:date ;
 .

scor:hasMetricRL_16
    rdfs:subPropertyOf scor:hasReliabilityMetric ;
    rdf:type owl:DatatypeProperty ;
    rdfs:domain [rdf:type owl:Class ;
        owl:unionOf (
        scor:DSPSelectCarriersRateShipments
        scor:DMOPSelectCarriersRateShipments
        )] ;
    rdfs:label "% of suppliers meeting environmental metrics/ criteria"@en;
    rdfs:comment "Number of suppliers that completely meet agreement environmental criteria divided by the total number of suppliers used."@en;
    rdfs:isDefinedBy scor: ;
    vs:term_status "stable" ;
    dct:modified "2015-11-05"^^xsd:date ;
 .

scor:hasMetricRL_17
    rdfs:subPropertyOf scor:hasReliabilityMetric ;
    rdf:type owl:DatatypeProperty ;
    rdfs:domain scor:SelectFinalSupplierNegotiate ;
    rdfs:label "% of suppliers with an EMS or ISO 14001 certification"@en;
    rdfs:comment "Percent of suppliers used that have a validated Environmental Management System or ISO 14000 certification"@en;
    rdfs:isDefinedBy scor: ;
    vs:term_status "stable" ;
    dct:modified "2015-11-05"^^xsd:date ;
 .

scor:hasMetricRL_18
    rdfs:subPropertyOf scor:hasReliabilityMetric ;
    rdf:type owl:DatatypeProperty ;
    rdfs:domain [rdf:type owl:Class ;
        owl:unionOf (
        scor:SSPReceiveProduct
        scor:SMOPReceiveProduct
        scor:SEOPReceiveProduct
        )] ;
    rdfs:label "% Orders/ Lines Processed Complete"@en;
    rdfs:comment "The number of orders / lines that are processed complete divided by the total orders / lines processed within the measurement period"@en;
    rdfs:isDefinedBy scor: ;
    vs:term_status "stable" ;
    dct:modified "2015-11-05"^^xsd:date ;
 .

scor:hasMetricRL_19
    rdfs:subPropertyOf scor:hasReliabilityMetric ;
    rdf:type owl:DatatypeProperty ;
    rdfs:domain [rdf:type owl:Class ;
        owl:unionOf (
        scor:SSPVerifyProduct
        scor:SMOPVerifyProduct
        scor:SEOPVerifyProduct
        )] ;
    rdfs:label "% Orders/ Lines Received Defect Free"@en;
    rdfs:comment "The number of orders / lines that are received defect free divided by the total orders / lines processed in the measurement period."@en;
    rdfs:isDefinedBy scor: ;
    vs:term_status "stable" ;
    dct:modified "2015-11-05"^^xsd:date ;
 .

scor:hasMetricRL_20
    rdfs:subPropertyOf scor:hasReliabilityMetric ;
    rdf:type owl:DatatypeProperty ;
    rdfs:domain [rdf:type owl:Class ;
        owl:unionOf (
        scor:SSPReceiveProduct
        scor:SMOPReceiveProduct
        scor:SEOPReceiveProduct
        )] ;
    rdfs:label "% Orders/ Lines Received On-Time To Demand Requirement"@en;
    rdfs:comment "The number of orders / lines that are received on- time to the demand requirements divided by the total orders / lines for the demand requirements in the measurement period"@en;
    rdfs:isDefinedBy scor: ;
    vs:term_status "stable" ;
    dct:modified "2015-11-05"^^xsd:date ;
 .

scor:hasMetricRL_21
    rdfs:subPropertyOf scor:hasReliabilityMetric ;
    rdf:type owl:DatatypeProperty ;
    rdfs:domain [rdf:type owl:Class ;
        owl:unionOf (
        scor:SSPVerifyProduct
        scor:SMOPVerifyProduct
        scor:SEOPVerifyProduct
        )] ;
    rdfs:label "% Orders/ lines received with correct content"@en;
    rdfs:comment "Percent of orders or lines received that have the correct material content as specified in the product design specs and supplier agreements."@en;
    rdfs:isDefinedBy scor: ;
    vs:term_status "stable" ;
    dct:modified "2015-11-05"^^xsd:date ;
 .

 scor:hasMetricRL_22
    rdfs:subPropertyOf scor:hasReliabilityMetric ;
    rdf:type owl:DatatypeProperty ;
    rdfs:domain [rdf:type owl:Class ;
        owl:unionOf (
        scor:SSPReceiveProduct
        scor:SMOPReceiveProduct
        scor:SEOPReceiveProduct
        )] ;
    rdfs:label "% Orders/ lines received with correct packaging"@en;
    rdfs:comment "Percent of orders or lines received that are packaged correctly with the right type and quantity of packaging material."@en;
    rdfs:isDefinedBy scor: ;
    vs:term_status "stable" ;
    dct:modified "2015-11-05"^^xsd:date ;
 .

scor:hasMetricRL_23
    rdfs:subPropertyOf scor:hasReliabilityMetric ;
    rdf:type owl:DatatypeProperty ;
    rdfs:domain [rdf:type owl:Class ;
        owl:unionOf (
        scor:SSPReceiveProduct
        scor:SMOPReceiveProduct
        scor:SEOPReceiveProduct
        )] ;
    rdfs:label "% Orders/ Lines Received with Correct Shipping Documents"@en;
    rdfs:comment "The number of orders / lines that are received on- time with correct shipping documents divided by the total orders / lines processed in the measurement period"@en;
    rdfs:isDefinedBy scor: ;
    vs:term_status "stable" ;
    dct:modified "2015-11-05"^^xsd:date ;
 .

scor:hasMetricRL_24
    rdfs:subPropertyOf scor:hasReliabilityMetric ;
    rdf:type owl:DatatypeProperty ;
    rdfs:domain [rdf:type owl:Class ;
        owl:unionOf (
        scor:SSPVerifyProduct
        scor:SMOPVerifyProduct
        scor:SEOPVerifyProduct
        )] ;
    rdfs:label "% Orders/lines received damage free"@en;
    rdfs:comment "The number of orders / lines that are processed damage free divided by the total orders / Lines processed in the measurement period"@en;
    rdfs:isDefinedBy scor: ;
    vs:term_status "stable" ;
    dct:modified "2015-11-05"^^xsd:date ;
 .

scor:hasMetricRL_25
    rdfs:subPropertyOf scor:hasReliabilityMetric ;
    rdf:type owl:DatatypeProperty ;
    rdfs:domain [rdf:type owl:Class ;
        owl:unionOf (
        scor:SSPTransferProduct
        scor:SMOPTransferProduct
        scor:SEOPTransferProduct
        )] ;
    rdfs:label "% Product Transferred On-Time to Demand Requirement"@en;
    rdfs:comment "The number of product orders / lines that are transferred on-time to demand requirements divided by the total orders / lines transferred in the measurement period"@en;
    rdfs:isDefinedBy scor: ;
    vs:term_status "stable" ;
    dct:modified "2015-11-05"^^xsd:date ;
 .

scor:hasMetricRL_26 
    rdfs:subPropertyOf scor:hasReliabilityMetric ;
    rdf:type owl:DatatypeProperty ;
    rdfs:domain [rdf:type owl:Class ;
        owl:unionOf (
        scor:SSPTransferProduct
        scor:SMOPTransferProduct
        scor:SEOPTransferProduct
        )] ;
    rdfs:label "% Product Transferred without Transaction Errors"@en;
    rdfs:comment "The number of transactions processed without error divided by the total transactions processed in the measurement period."@en;
    rdfs:isDefinedBy scor: ;
    vs:term_status "stable" ;
    dct:modified "2015-11-05"^^xsd:date ;
 .

scor:hasMetricRL_27
    rdfs:subPropertyOf scor:hasReliabilityMetric ;
    rdf:type owl:DatatypeProperty ;
    rdfs:domain [rdf:type owl:Class ;
        owl:unionOf (
        scor:SSPScheduleProductDeliveries
        scor:SMOPScheduleProductDeliveries
        scor:SEOPScheduleProductDeliveries
        )] ;
    rdfs:label "% Schedules Changed within Supplier's Lead Time"@en;
    rdfs:comment "The number of schedules that are changed within the suppliers lead-time divided by the total number Deliveries of schedules generated within the measurement period"@en;
    rdfs:isDefinedBy scor: ;
    vs:term_status "stable" ;
    dct:modified "2015-11-05"^^xsd:date ;
 .

scor:hasMetricRL_28
    rdfs:subPropertyOf scor:hasReliabilityMetric ;
    rdf:type owl:DatatypeProperty ;
    rdfs:domain [rdf:type owl:Class ;
        owl:unionOf (
        scor:ScheduleDefectiveProductShipment
        scor:ScheduleMROShipment
        scor:ScheduleExcessProductShipment
        )] ;
    rdfs:label "% Shipping Schedules that Support Customer Required Return by Date"@en;
    rdfs:comment "Percentage Shipping Schedules that Support Customer Required Return by Date"@en;
    rdfs:isDefinedBy scor: ;
    vs:term_status "stable" ;
    dct:modified "2015-11-05"^^xsd:date ;
 .

#29 seems to be deprecated

#30 seems to be deprecated

scor:hasMetricRL_31
    rdfs:subPropertyOf scor:hasReliabilityMetric ;
    rdf:type owl:DatatypeProperty ;
    rdfs:domain [rdf:type owl:Class ;
        owl:unionOf (
        scor:MSPackage
        scor:MOPackage
        scor:MEOPackage
        scor:LoadVehicleGenerateShippingDocuments
        scor:DMOPLoadProductGenerateShippingDocs
        scor:DEOPLoadProductGenerateShippingDocs
        )] ;
    rdfs:label "Compliance Documentation Accuracy"@en;
    rdfs:comment "Percentage of compliance documentations are complete, correct, and readily available when and  how expected by customer, Government and other supply chain regulatory entities. Compliance documentation includes material safety data sheets."@en;
    rdfs:isDefinedBy scor: ;
    vs:term_status "stable" ;
    dct:modified "2015-11-05"^^xsd:date ;
 .

scor:hasMetricRL_32
    rdfs:subPropertyOf scor:hasReliabilityMetric ;
    rdf:type owl:DatatypeProperty ;
    rdfs:domain [rdf:type owl:Class ;
        owl:unionOf (
        scor:DSPReceiveVerifyProductByCustomer
        scor:DMOPReceiveVerifyProductByCustomer
        scor:DEOPReceiveVerifyProductByCustomer
        )] ;
    rdfs:label "Customer Commit Date Achievement Time"@en;
    rdfs:comment "Percentage of orders which is received on time as defined by the custome"@en;
    rdfs:isDefinedBy scor: ;
    vs:term_status "stable" ;
    dct:modified "2015-11-05"^^xsd:date ;
 .

scor:hasMetricRL_33
    rdfs:subPropertyOf scor:hasReliabilityMetric ;
    rdf:type owl:DatatypeProperty ;
    rdfs:domain [rdf:type owl:Class ;
        owl:unionOf (
        scor:ReceiveEnterValidateOrder
        scor:DSPConsolidateOrders
        scor:LoadVehicleGenerateShippingDocuments
        scor:DSPShipProduct
        scor:DSPReceiveVerifyProductByCustomer
        scor:ReceiveConfigureEnterValidateOrder
        scor:DMOPConsolidateOrders
        scor:DMOPLoadProductGenerateShippingDocs
        scor:DMOPShipProduct
        scor:DMOPReceiveVerifyProductByCustomer
        scor:EnterOrderCommitResourcesLaunchProgram
        scor:DEOPRouteShipments
        scor:DEOPLoadProductGenerateShippingDocs
        scor:DEOPShipProduct
        scor:DMOPReceiveVerifyProductByCustomer
        )] ;
    rdfs:label "Delivery Item Accuracy"@en;
    rdfs:comment "Percentage of orders in which all items ordered are the items actually provided, and no extra items are provided"@en;
    rdfs:isDefinedBy scor: ;
    vs:term_status "stable" ;
    dct:modified "2015-11-05"^^xsd:date ;
 .

scor:hasMetricRL_34
    rdfs:subPropertyOf scor:hasReliabilityMetric ;
    rdf:type owl:DatatypeProperty ;
    rdfs:domain [rdf:type owl:Class ;
        owl:unionOf (
        scor:ReceiveEnterValidateOrder
        scor:DSPConsolidateOrders
        scor:LoadVehicleGenerateShippingDocuments
        scor:DSPShipProduct
        scor:DSPReceiveVerifyProductByCustomer
        scor:ReceiveConfigureEnterValidateOrder
        scor:DMOPConsolidateOrders
        scor:DMOPLoadProductGenerateShippingDocs
        scor:DMOPShipProduct
        scor:DSPReceiveVerifyProductByCustomer
        scor:EnterOrderCommitResourcesLaunchProgram
        scor:DEOPRouteShipments
        scor:DEOPLoadProductGenerateShippingDocs
        scor:DEOPShipProduct
        scor:DEOPReceiveVerifyProductByCustomer
        )] ;
    rdfs:label "Delivery Location Accuracy"@en;
    rdfs:comment "Percentage of orders which is delivered to the correct location and customer entity"@en;
    rdfs:isDefinedBy scor: ;
    vs:term_status "stable" ;
    dct:modified "2015-11-05"^^xsd:date ;
 .

scor:hasMetricRL_35
    rdfs:subPropertyOf scor:hasReliabilityMetric ;
    rdf:type owl:DatatypeProperty ;
    rdfs:domain [rdf:type owl:Class ;
        owl:unionOf (
        scor:ReceiveEnterValidateOrder
        scor:DSPConsolidateOrders
        scor:LoadVehicleGenerateShippingDocuments
        scor:DSPShipProduct
        scor:DSPReceiveVerifyProductByCustomer
        scor:ReceiveConfigureEnterValidateOrder
        scor:DMOPConsolidateOrders
        scor:DMOPLoadProductGenerateShippingDocs
        scor:DMOPShipProduct
        scor:DMOPReceiveVerifyProductByCustomer
        scor:EnterOrderCommitResourcesLaunchProgram
        scor:DEOPRouteShipments
        scor:DEOPLoadProductGenerateShippingDocs
        scor:DEOPShipProduct
        scor:DEOPReceiveVerifyProductByCustomer
        )] ;
    rdfs:label "Delivery Quantity Accuracy"@en;
    rdfs:comment "Percentage of orders in which all quantities received by the customer match the order quantities (within mutually agreed tolerances)"@en;
    rdfs:isDefinedBy scor: ;
    vs:term_status "stable" ;
    dct:modified "2015-11-05"^^xsd:date ;
 .

scor:hasMetricRL_36
    rdfs:subPropertyOf scor:hasReliabilityMetric ;
    rdf:type owl:DatatypeProperty ;
    rdfs:domain [rdf:type owl:Class ;
        owl:unionOf (
        scor:BalanceSCResourcesWithSCRequirements
        scor:EstablishDeliveryPlans
        scor:MSProduceTest
        scor:DSPReserveInventoryDetermineDeliveryDate
        scor:DSPPickProduct
        )] ;
    rdfs:label "Fill Rate"@en;
    rdfs:comment "The percentage of ship-from-stock orders shipped within 24 hours of order receipt. For services, this metric is the proportion for services that are filled so that the service is completed within 24 hours"@en;
    rdfs:isDefinedBy scor: ;
    vs:term_status "stable" ;
    dct:modified "2015-11-05"^^xsd:date ;
 .

scor:hasMetricRL_37
    rdfs:subPropertyOf scor:hasReliabilityMetric ;
    rdf:type owl:DatatypeProperty ;
    rdfs:domain [rdf:type owl:Class ;
        owl:unionOf (
        scor:PSCIdentifyPrioritizeAggregateSCRequirements
        scor:IdentifyPrioritizeAggregateProductRequirements
        scor:IdentifyPrioritizeAggregateProductionRequirements
        scor:IdentifyPrioritizeAggregateDeliveryRequirements
        scor:IdentifyAssessAggregateDeliveryResources
        scor:ManageSupplyChainHumanResources
        scor:ManageSupplyChainAssets
        scor:ManageSupplyChainContracts
        scor:ManageSupplyChainNetworks
        )] ;
    rdfs:label "Forecast Accuracy"@en;
    rdfs:comment "Forecast accuracy is calculated for products and/or families for markets/distribution channels, in unit measurement. Common calculation (Sum Actuals - Sum of Variance) / Sum Actuals to determine percentage error. *monitoring the delta of Forecast Accuracy over measured time periods can determine success rates."@en;
    rdfs:isDefinedBy scor: ;
    vs:term_status "stable" ;
    dct:modified "2015-11-05"^^xsd:date ;
 .

#38 seems to be deprecated

scor:hasMetricRL_39
    rdfs:subPropertyOf scor:hasReliabilityMetric ;
    rdf:type owl:DatatypeProperty ;
    rdfs:domain scor:DispositionExcessProduct;
    rdfs:label "# of occurrences of incorrect designated return center"@en;
    rdfs:comment "Number of occurrences of incorrect designated return center"@en;
    rdfs:isDefinedBy scor: ;
    vs:term_status "stable" ;
    dct:modified "2015-11-05"^^xsd:date ;
 .

scor:hasMetricRL_40
    rdfs:subPropertyOf scor:hasReliabilityMetric ;
    rdf:type owl:DatatypeProperty ;
    rdfs:domain scor:IdentifyExcessProductCondition ;
    rdfs:label "# occurrences where excessive inventory is returned and followed"@en;
    rdfs:comment "Number of occurrences where excessive inventory is returned and followed"@en;
    rdfs:isDefinedBy scor: ;
    vs:term_status "stable" ;
    dct:modified "2015-11-05"^^xsd:date ;
 .

scor:hasMetricRL_41
    rdfs:subPropertyOf scor:hasReliabilityMetric ;
    rdf:type owl:DatatypeProperty ;
    rdfs:domain [rdf:type owl:Class ;
        owl:unionOf (
        scor:DSPReceiveVerifyProductByCustomer
        scor:DMOPReceiveVerifyProductByCustomer
        scor:DEOPReceiveVerifyProductByCustomer
        )] ;
    rdfs:label "Orders Delivered Damage Free Conformance"@en;
    rdfs:comment "Percentage of orders which is delivered without damage."@en;
    rdfs:isDefinedBy scor: ;
    vs:term_status "stable" ;
    dct:modified "2015-11-05"^^xsd:date ;
 .

scor:hasMetricRL_42
    rdfs:subPropertyOf scor:hasReliabilityMetric ;
    rdf:type owl:DatatypeProperty ;
    rdfs:domain [rdf:type owl:Class ;
        owl:unionOf (
        scor:DSPReceiveVerifyProductByCustomer
        scor:DMOPReceiveVerifyProductByCustomer
        scor:DEOPReceiveVerifyProductByCustomer
        )] ;
    rdfs:label "Orders Delivered Defect Free Conformance"@en;
    rdfs:comment "Percentage of orders which is delivered without defect"@en;
    rdfs:isDefinedBy scor: ;
    vs:term_status "stable" ;
    dct:modified "2015-11-05"^^xsd:date ;
 .

scor:hasMetricRL_43
    rdfs:subPropertyOf scor:hasReliabilityMetric ;
    rdf:type owl:DatatypeProperty ;
    rdfs:domain [rdf:type owl:Class ;
        owl:unionOf (
        scor:LoadVehicleGenerateShippingDocuments
        scor:DMOPLoadProductGenerateShippingDocs
        scor:DEOPLoadProductGenerateShippingDocs
        )] ;
    rdfs:label "Other Required Documentation Accuracy"@en;
    rdfs:comment "Percentage of other required documentations (besides of compliance documentation, payment documentation and shipping documentation) are complete, correct, and readily available when and how expected by customer, Government and other supply chain regulatory entities. This kind of documentations includes quality certification"@en;
    rdfs:isDefinedBy scor: ;
    vs:term_status "stable" ;
    dct:modified "2015-11-05"^^xsd:date ;
 .

#44 seems to be deprecated

scor:hasMetricRL_45
    rdfs:subPropertyOf scor:hasReliabilityMetric ;
    rdf:type owl:DatatypeProperty ;
    rdfs:domain [rdf:type owl:Class ;
        owl:unionOf (
        scor:LoadVehicleGenerateShippingDocuments
        scor:DMOPLoadProductGenerateShippingDocs
        scor:DEOPLoadProductGenerateShippingDocs
        )] ;
    rdfs:label "Payment Documentation Accuracy"@en;
    rdfs:comment "Percentage of payment documentations are complete, correct, and readily available when and how expected by customer, Government and other supply chain regulatory entities. Payment documentations includes invoice, contractual outline agreement"@en;
    rdfs:isDefinedBy scor: ;
    vs:term_status "stable" ;
    dct:modified "2015-11-05"^^xsd:date ;
 .

#46 seems to be deprecated

scor:hasMetricRL_47
    rdfs:subPropertyOf scor:hasReliabilityMetric ;
    rdf:type owl:DatatypeProperty ;
    rdfs:domain [rdf:type owl:Class ;
        owl:unionOf (
        scor:ReturnDefectiveProduct
        scor:ReturnMROPRoduct
        scor:DEOPLoadProductGenerateShippingDocs
        )] ;
    rdfs:label "Return Shipments on Time"@en;
    rdfs:comment "Percentage of return shipments on Time"@en;
    rdfs:isDefinedBy scor: ;
    vs:term_status "stable" ;
    dct:modified "2015-11-05"^^xsd:date ;
 .

#48 seems to be deprecated

scor:hasMetricRL_49
    rdfs:subPropertyOf scor:hasReliabilityMetric ;
    rdf:type owl:DatatypeProperty ;
    rdfs:domain [rdf:type owl:Class ;
        owl:unionOf (
        scor:MSScheduleProductionActivities
        scor:MOScheduleProductionActivities
        scor:MEOScheduleProductionActivities
        )] ;
    rdfs:label "Schedule Achievement"@en;
    rdfs:comment "The percentage of time that a plant achieves its production schedule. This calculation is based on the number of scheduled end-items or total volume for a specific period. Note: over-shipments do not make up for under-shipments."@en;
    rdfs:isDefinedBy scor: ;
    vs:term_status "stable" ;
    dct:modified "2015-11-05"^^xsd:date ;
 .


scor:hasMetricRL_50
    rdfs:subPropertyOf scor:hasReliabilityMetric ;
    rdf:type owl:DatatypeProperty ;
    rdfs:domain [rdf:type owl:Class ;
        owl:unionOf (
        scor:LoadVehicleGenerateShippingDocuments
        scor:DMOPLoadProductGenerateShippingDocs
        scor:DEOPLoadProductGenerateShippingDocs
        )] ;
    rdfs:label "Shipping Documentation Accuracy"@en;
    rdfs:comment "Percentage of shipping documentations are complete, correct, and readily available when and how expected by customer, Government and other supply chain regulatory entities. Shipping documentations includes packing slips (customers), bill of lading (carriers) and government or customs documentation/forms"@en;
    rdfs:isDefinedBy scor: ;
    vs:term_status "stable" ;
    dct:modified "2015-11-05"^^xsd:date ;
 .



#51-54 seem to be deprecated

scor:hasMetricRL_55
    rdfs:subPropertyOf scor:hasReliabilityMetric ;
    rdf:type owl:DatatypeProperty ;
    rdfs:domain [rdf:type owl:Class ;
        owl:unionOf (
        scor:MSProduceTest
        scor:MSPackage
        )] ;
    rdfs:label "Warranty and Returns"@en;
    rdfs:comment "Warranty costs include materials, labor and problem diagnosis for product defects."@en;
    rdfs:isDefinedBy scor: ;
    vs:term_status "stable" ;
    dct:modified "2015-11-05"^^xsd:date ;
 .

scor:hasMetricRL_56
    rdfs:subPropertyOf scor:hasReliabilityMetric ;
    rdf:type owl:DatatypeProperty ;
    rdfs:domain [rdf:type owl:Class ;
        owl:unionOf (
        scor:MSProduceTest
        scor:MSPackage
        scor:MOProduceTest
        scor:MOPackage
        scor:MEOProduceTest
        scor:MEOPackage
        )] ;
    rdfs:label "Warranty Costs"@en;
    rdfs:comment "Warranty costs include materials, labor and problem diagnosis for product defects."@en;
    rdfs:isDefinedBy scor: ;
    vs:term_status "stable" ;
    dct:modified "2015-11-05"^^xsd:date ;
 .

scor:hasMetricRL_57
    rdfs:subPropertyOf scor:hasReliabilityMetric ;
    rdf:type owl:DatatypeProperty ;
    rdfs:domain [rdf:type owl:Class ;
        owl:unionOf (
        scor:MSWasteDisposal
        scor:MOWasteDisposal
        scor:MEOWasteDisposal
        )] ;
    rdfs:label "Waste Processing Errors"@en;
    rdfs:comment "Number of errors in waste transactions as percent of total waste transactions"@en;
    rdfs:isDefinedBy scor: ;
    vs:term_status "stable" ;
    dct:modified "2015-11-05"^^xsd:date ;
 .

scor:hasMetricRL_58
    rdfs:subPropertyOf scor:hasReliabilityMetric ;
    rdf:type owl:DatatypeProperty ;
    rdfs:domain [rdf:type owl:Class ;
        owl:unionOf (
        scor:MakeToStock
        scor:MSProduceTest
        scor:MSPackage
        scor:MakeToOrder
        scor:MOProduceTest
        scor:MOPackage
        scor:MakeEngineerToOrder
        scor:MEOProduceTest
        scor:MEOPackage
        )] ;
    rdfs:label "Yield"@en;
    rdfs:comment "The ratio of usable output from a process to its input."@en;
    rdfs:isDefinedBy scor: ;
    vs:term_status "stable" ;
    dct:modified "2015-11-05"^^xsd:date ;
 .

scor:hasMetricRL_59
    rdfs:subPropertyOf scor:hasReliabilityMetric ;
    rdf:type owl:DatatypeProperty ;
    rdfs:domain [rdf:type owl:Class ;
        owl:unionOf (
        scor:MSProduceTest
        scor:MOProduceTest
        scor:MEOProduceTest
        )] ;
    rdfs:label "Yield Availability"@en;
    rdfs:comment "The condition that occurs when the output of a process is not consistently repeatable either in quantity, quality, or combination of these."@en;
    rdfs:isDefinedBy scor: ;

    vs:term_status "stable" ;
    dct:modified "2015-11-05"^^xsd:date ;
 .


######### Responsiveness Metrics


#1 seems to be deprecated



scor:hasMetricRS_2
    rdf:type owl:DatatypeProperty ;
    rdfs:subPropertyOf scor:hasResponsivenessMetric ;
    rdfs:domain scor:ManagePerformance ;
    rdfs:label "Assess Delivery Performance Cycle Time"@en;
    rdfs:comment "The average time associated with assessing the performance of deliver processes."@en;
    rdfs:isDefinedBy scor: ;
    vs:term_status "stable" ;
    dct:modified "2015-11-05"^^xsd:date ;
 .

scor:hasMetricRS_3
    rdf:type owl:DatatypeProperty ;
    rdfs:subPropertyOf scor:hasResponsivenessMetric ;
    rdfs:domain scor:ManagePerformance ;
    rdfs:label "Assess Supplier Performance Cycle Time"@en;
    rdfs:comment "The average time associated with assessing the performance of deliver processes."@en;
    rdfs:isDefinedBy scor: ;
    vs:term_status "stable" ;
    dct:modified "2015-11-05"^^xsd:date ;
.

scor:hasMetricRS_4
    rdf:type owl:DatatypeProperty ;
    rdfs:subPropertyOf scor:hasResponsivenessMetric ;
    rdfs:domain [rdf:type owl:Class ;
        owl:unionOf (
        scor:MSProduceTest
        scor:MSPackage
        scor:MOProduceTest
        scor:MOPackage
        scor:MEOProduceTest
        scor:MEOPackage
        )] ;
    rdfs:label "Asset Turns"@en;
    rdfs:comment "Total gross product revenue / Total net assets."@en;
    rdfs:isDefinedBy scor: ;
    vs:term_status "stable" ;
    dct:modified "2015-11-05"^^xsd:date ;
.

scor:hasMetricRS_5
    rdf:type owl:DatatypeProperty ;
    rdfs:subPropertyOf scor:hasResponsivenessMetric ;
    rdfs:domain [rdf:type owl:Class ;
        owl:unionOf (
        scor:AuthorizeDefectiveProductReturn
        )] ;
    rdfs:label "Authorize Defective Product Return Cycle Time"@en;
    rdfs:comment "The average time associated with authorizing the return of defective product."@en;
    rdfs:isDefinedBy scor: ;
    vs:term_status "stable" ;
    dct:modified "2015-11-05"^^xsd:date ;
.

scor:hasMetricRS_6
    rdf:type owl:DatatypeProperty ;
    rdfs:subPropertyOf scor:hasResponsivenessMetric ;
    rdfs:domain [rdf:type owl:Class ;
        owl:unionOf (
        scor:
        )] ;
    rdfs:label "Authorize Excess Product Return Cycle Time"@en;
    rdfs:comment "The average time associated with authorizing the turn of excess product."@en;
    rdfs:isDefinedBy scor: ;
    vs:term_status "stable" ;
    dct:modified "2015-11-05"^^xsd:date ;
.

scor:hasMetricRS_7
    rdf:type owl:DatatypeProperty ;
    rdfs:subPropertyOf scor:hasResponsivenessMetric ;
    rdfs:domain [rdf:type owl:Class ;
        owl:unionOf (
        scor:AuthorizeMROProductReturn
        )] ;
    rdfs:label "Authorize MRO Product Return Cycle Time"@en;
    rdfs:comment "The average time associated with authorizing the turn of MRO product."@en;
    rdfs:isDefinedBy scor: ;
    vs:term_status "stable" ;
    dct:modified "2015-11-05"^^xsd:date ;
.

scor:hasMetricRS_8
    rdf:type owl:DatatypeProperty ;
    rdfs:subPropertyOf scor:hasResponsivenessMetric ;
    rdfs:domain [rdf:type owl:Class ;
        owl:unionOf (
        scor:AuthorizeSupplierPayment
        scor:SMOPAuthorizeSupplierPayment
        scor:SEOPAuthorizeSupplierPayment
        )] ;
    rdfs:label "Authorize Supplier Payment Cycle Time"@en;
    rdfs:comment "The average time associated with authorizing payment to suppliers."@en;
    rdfs:isDefinedBy scor: ;
    vs:term_status "stable" ;
    dct:modified "2015-11-05"^^xsd:date ;
.

scor:hasMetricRS_9
    rdf:type owl:DatatypeProperty ;
    rdfs:subPropertyOf scor:hasResponsivenessMetric ;
    rdfs:domain [rdf:type owl:Class ;
        owl:unionOf (
        scor:SSPScheduleProductDeliveries
        scor:SMOPScheduleProductDeliveries
        scor:SEOPScheduleProductDeliveries
        )] ;
    rdfs:label "Average Days per Engineering Change"@en;
    rdfs:comment "# of days each engineering change impacts the delivery date divided by the total # of changes."@en;
    rdfs:isDefinedBy scor: ;
    vs:term_status "stable" ;
    dct:modified "2015-11-05"^^xsd:date ;
.

scor:hasMetricRS_10
    rdf:type owl:DatatypeProperty ;
    rdfs:subPropertyOf scor:hasResponsivenessMetric ;
    rdfs:domain [rdf:type owl:Class ;
        owl:unionOf (
        scor:SSPScheduleProductDeliveries
        scor:SMOPScheduleProductDeliveries
        scor:SEOPScheduleProductDeliveries
        )] ;
    rdfs:label "Average Days per Schedule Change"@en;
    rdfs:comment "# of days each schedule change impacts the delivery date divided by the total # of changes."@en;
    rdfs:isDefinedBy scor: ;
    vs:term_status "stable" ;
    dct:modified "2015-11-05"^^xsd:date ;
.

scor:hasMetricRS_11
    rdf:type owl:DatatypeProperty ;
    rdfs:subPropertyOf scor:hasResponsivenessMetric ;
    rdfs:domain [rdf:type owl:Class ;
        owl:unionOf (
        scor:SSPScheduleProductDeliveries
        scor:SMOPScheduleProductDeliveries
        scor:SEOPScheduleProductDeliveries
        )] ;
    rdfs:label "Average Release Cycle of Changes"@en;
    rdfs:comment "Cycle time for implementing change notices divided by total number of changes."@en;
    rdfs:isDefinedBy scor: ;
    vs:term_status "stable" ;
    dct:modified "2015-11-05"^^xsd:date ;
.

scor:hasMetricRS_12
    rdf:type owl:DatatypeProperty ;
    rdfs:subPropertyOf scor:hasResponsivenessMetric ;
    rdfs:domain [rdf:type owl:Class ;
        owl:unionOf (
        scor:BalanceProductResourcesWithProductRequirements
        )] ;
    rdfs:label "Balance Product Resources with Product Requirements Cycle Time"@en;
    rdfs:comment "The average time associated with balancing the product resources and product requirements."@en;
    rdfs:isDefinedBy scor: ;
    vs:term_status "stable" ;
    dct:modified "2015-11-05"^^xsd:date ;
.

scor:hasMetricRS_13
    rdf:type owl:DatatypeProperty ;
    rdfs:subPropertyOf scor:hasResponsivenessMetric ;
    rdfs:domain [rdf:type owl:Class ;
        owl:unionOf (
        scor:BalanceProductionResourcesWithProductionRequirements
        )] ;
    rdfs:label "Balance Production Resources with Product Requirements Cycle Time"@en;
    rdfs:comment "The average time associated with identifying, prioritizing, and aggregating product requirements."@en;
    rdfs:isDefinedBy scor: ;
    vs:term_status "stable" ;
    dct:modified "2015-11-05"^^xsd:date ;
.

scor:hasMetricRS_14
    rdf:type owl:DatatypeProperty ;
    rdfs:subPropertyOf scor:hasResponsivenessMetric ;
    rdfs:domain [rdf:type owl:Class ;
        owl:unionOf (
        scor:BalanceReturnResourcesWithReturnRequirements
        )] ;
    rdfs:label "Balance Return Resources with Return Requirements Cycle Time"@en;
    rdfs:comment "The average time associated with balancing return resources and return requirements."@en;
    rdfs:isDefinedBy scor: ;
    vs:term_status "stable" ;
    dct:modified "2015-11-05"^^xsd:date ;
.

scor:hasMetricRS_15
    rdf:type owl:DatatypeProperty ;
    rdfs:subPropertyOf scor:hasResponsivenessMetric ;
    rdfs:domain [rdf:type owl:Class ;
        owl:unionOf (
        scor:BalanceSCResourcesWithSCRequirements
        )] ;
    rdfs:label "Balance Supply Chain Resources with SC Requirements"@en;
    rdfs:comment "The average time associated with balancing supply chain resources and supply chain requirements requirements."@en;
    rdfs:isDefinedBy scor: ;
    vs:term_status "stable" ;
    dct:modified "2015-11-05"^^xsd:date ;
.

scor:hasMetricRS_16
    rdf:type owl:DatatypeProperty ;
    rdfs:subPropertyOf scor:hasResponsivenessMetric ;
    rdfs:domain [rdf:type owl:Class ;
        owl:unionOf (
        scor:DSPBuildLoads
        scor:DMOPBuildLoads
        scor:DEOPBuildLoads
        )] ;
    rdfs:label "Build Loads Cycle Time"@en;
    rdfs:comment "The average time associated with building shipment loads."@en;
    rdfs:isDefinedBy scor: ;
    vs:term_status "stable" ;
    dct:modified "2015-11-05"^^xsd:date ;
.

scor:hasMetricRS_17
    rdf:type owl:DatatypeProperty ;
    rdfs:subPropertyOf scor:hasResponsivenessMetric ;
    rdfs:domain [rdf:type owl:Class ;
        owl:unionOf (
        scor:Checkout
        )] ;
    rdfs:label "Checkout Cycle Time"@en;
    rdfs:comment "The average time required for customer checkout."@en;
    rdfs:isDefinedBy scor: ;
    vs:term_status "stable" ;
    dct:modified "2015-11-05"^^xsd:date ;
.

scor:hasMetricRS_18
    rdf:type owl:DatatypeProperty ;
    rdfs:subPropertyOf scor:hasResponsivenessMetric ;
    rdfs:domain [rdf:type owl:Class ;
        owl:unionOf (
        scor:DSPConsolidateOrders
        )] ;
    rdfs:label "Consolidate Orders Cycle Time"@en;
    rdfs:comment "The average time required for customer order consolidation."@en;
    rdfs:isDefinedBy scor: ;
    vs:term_status "stable" ;
    dct:modified "2015-11-05"^^xsd:date ;
.

scor:hasMetricRS_19
    rdf:type owl:DatatypeProperty ;
    rdfs:subPropertyOf scor:hasResponsivenessMetric ;
    rdfs:domain [rdf:type owl:Class ;
        owl:unionOf (
        scor:
        scor:DeliverReturnMROProduct
        scor:DeliverReturnExcessProduct
        )] ;
    rdfs:label "Current customer return order cycle time"@en;
    rdfs:comment "Current return order cycle time, including customer return order processing cycle time, transit time, return processing and disposition cycle time, etc."@en;
    rdfs:isDefinedBy scor: ;
    vs:term_status "stable" ;
    dct:modified "2015-11-05"^^xsd:date ;
.

scor:hasMetricRS_20
    rdf:type owl:DatatypeProperty ;
    rdfs:subPropertyOf scor:hasResponsivenessMetric ;
    rdfs:domain [rdf:type owl:Class ;
        owl:unionOf (
        scor:DeliverStockedProduct
        scor:DeliverMakeToOrderProduct
        scor:DeliverEngineerToOrderProduct
        )] ;
    rdfs:label "Current logistics order cycle time"@en;
    rdfs:comment "Current logistics order cycle time, including customer order processing cycle time, dock-to-stock cycle time, pick-to-ship cycle, transit time, etc."@en;
    rdfs:isDefinedBy scor: ;
    vs:term_status "stable" ;
    dct:modified "2015-11-05"^^xsd:date ;
.

scor:hasMetricRS_21
    rdf:type owl:DatatypeProperty ;
    rdfs:subPropertyOf scor:hasResponsivenessMetric ;
    rdfs:domain [rdf:type owl:Class ;
        owl:unionOf (
        scor:MakeToStock
        scor:MakeToOrder
        scor:MakeEngineerToOrder
        )] ;
    rdfs:label "Current manufacturing order cycle time"@en;
    rdfs:comment "Current manufacturing cycle time"@en;
    rdfs:isDefinedBy scor: ;
    vs:term_status "stable" ;
    dct:modified "2015-11-05"^^xsd:date ;
.

scor:hasMetricRS_22
    rdf:type owl:DatatypeProperty ;
    rdfs:subPropertyOf scor:hasResponsivenessMetric ;
    rdfs:domain [rdf:type owl:Class ;
        owl:unionOf (
        scor:SourceReturnDefectiveProduct
        )] ;
    rdfs:label "Current supplier return order cycle time"@en;
    rdfs:comment "Current supplier return cycle time, including supplier return order processing cycle time, pick-to-shop time, transit time etc."@en;
    rdfs:isDefinedBy scor: ;
    vs:term_status "stable" ;
    dct:modified "2015-11-05"^^xsd:date ;
.

#23 seems to be deprecated

scor:hasMetricRS_24
    rdf:type owl:DatatypeProperty ;
    rdfs:subPropertyOf scor:hasResponsivenessMetric ;
    rdfs:domain [rdf:type owl:Class ;
        owl:unionOf (
        scor:DeliverInstall
        )] ;
    rdfs:label "Deliver and/or Install Cycle Time"@en;
    rdfs:comment "The average time required to deliver and install product."@en;
    rdfs:isDefinedBy scor: ;
    vs:term_status "stable" ;
    dct:modified "2015-11-05"^^xsd:date ;
.

scor:hasMetricRS_25
    rdf:type owl:DatatypeProperty ;
    rdfs:subPropertyOf scor:hasResponsivenessMetric ;
    rdfs:domain [rdf:type owl:Class ;
        owl:unionOf (
        scor:EnterOrderCommitResourcesLaunchProgram
        )] ;
    rdfs:label "Enter Order, Commmit Resources & Launch Program Cycle Time"@en;
    rdfs:comment "The average time associated with entering an order, committing resources and program launch."@en;
    rdfs:isDefinedBy scor: ;
    vs:term_status "stable" ;
    dct:modified "2015-11-05"^^xsd:date ;
.


scor:hasMetricRS_26
    rdf:type owl:DatatypeProperty ;
    rdfs:subPropertyOf scor:hasResponsivenessMetric ;
    rdfs:domain [rdf:type owl:Class ;
        owl:unionOf (
        scor:EstablishCommunicateReturnPlans
        )] ;
    rdfs:label "Establish and Communicate Return Plans Cycle Time"@en;
    rdfs:comment "The average time associated with entering an order, committing resources and program launch."@en;
    rdfs:isDefinedBy scor: ;
    vs:term_status "stable" ;
    dct:modified "2015-11-05"^^xsd:date ;
.

scor:hasMetricRS_27
    rdf:type owl:DatatypeProperty ;
    rdfs:subPropertyOf scor:hasResponsivenessMetric ;
    rdfs:domain [rdf:type owl:Class ;
        owl:unionOf (
        scor:EstablishDeliveryPlans
        )] ;
    rdfs:label "Establish Delivery Plans Cycle Time"@en;
    rdfs:comment "The average time associated with establish and communicating deliver plans"@en;
    rdfs:isDefinedBy scor: ;
    vs:term_status "stable" ;
    dct:modified "2015-11-05"^^xsd:date ;
.

scor:hasMetricRS_28
    rdf:type owl:DatatypeProperty ;
    rdfs:subPropertyOf scor:hasResponsivenessMetric ;
    rdfs:domain [rdf:type owl:Class ;
        owl:unionOf (
        scor:EstablishProductionPlans
        )] ;
    rdfs:label "Establish Production Plans Cycle Time"@en;
    rdfs:comment "The average time associated with establish and communicating production plans"@en;
    rdfs:isDefinedBy scor: ;
    vs:term_status "stable" ;
    dct:modified "2015-11-05"^^xsd:date ;
.

scor:hasMetricRS_29
    rdf:type owl:DatatypeProperty ;
    rdfs:subPropertyOf scor:hasResponsivenessMetric ;
    rdfs:domain [rdf:type owl:Class ;
        owl:unionOf (
        scor:EstablishSourcingPlans
        )] ;
    rdfs:label "Establish Sourcing Plans Cycle Time"@en;
    rdfs:comment "The average time associated with establishing and communicating source plans"@en;
    rdfs:isDefinedBy scor: ;
    vs:term_status "stable" ;
    dct:modified "2015-11-05"^^xsd:date ;
.

scor:hasMetricRS_30
    rdf:type owl:DatatypeProperty ;
    rdfs:subPropertyOf scor:hasResponsivenessMetric ;
    rdfs:domain [rdf:type owl:Class ;
        owl:unionOf (
        scor:EstablishCommunicateSCPlans
        )] ;
    rdfs:label "Establish Supply Chain Plans Cycle Time"@en;
    rdfs:comment "Five point annual average of the sum of all gross inventories (raw materials & WIP, plant FG, field FG, fiels samples, other) / (COGS / 365). Total gross value of iventory at standard cost before reservers for excess and obsolescence. Only includes inventory on company books, future liabilities should not be included"@en;
    rdfs:isDefinedBy scor: ;
    vs:term_status "stable" ;
    dct:modified "2015-11-05"^^xsd:date ;
.

#31 seems to be deprecated

scor:hasMetricRS_32
    rdf:type owl:DatatypeProperty ;
    rdfs:subPropertyOf scor:hasResponsivenessMetric ;
    rdfs:domain [rdf:type owl:Class ;
        owl:unionOf (
        scor:FillShoppingCart
        )] ;
    rdfs:label "Fill Shopping Cart Cycle Time"@en;
    rdfs:comment "The average time associated with 'filling the shopping cart'."@en;
    rdfs:isDefinedBy scor: ;
    vs:term_status "stable" ;
    dct:modified "2015-11-05"^^xsd:date ;
.

scor:hasMetricRS_33
    rdf:type owl:DatatypeProperty ;
    rdfs:subPropertyOf scor:hasResponsivenessMetric ;
    rdfs:domain [rdf:type owl:Class ;
        owl:unionOf (
        scor:FinalizeProductionEngineering
        )] ;
    rdfs:label "Finalize Production Engineering Cycle Time"@en;
    rdfs:comment "The average time associated with the finalization of production engineering."@en;
    rdfs:isDefinedBy scor: ;
    vs:term_status "stable" ;
    dct:modified "2015-11-05"^^xsd:date ;
.

scor:hasMetricRS_34
    rdf:type owl:DatatypeProperty ;
    rdfs:subPropertyOf scor:hasResponsivenessMetric ;
    rdfs:domain [rdf:type owl:Class ;
        owl:unionOf (
        scor:GenerateStockingSchedule
        )] ;
    rdfs:label "Generate Stocking Schedule Cycle Time"@en;
    rdfs:comment "The average time associated with the generation of the stocking schedlule."@en;
    rdfs:isDefinedBy scor: ;
    vs:term_status "stable" ;
    dct:modified "2015-11-05"^^xsd:date ;
.

scor:hasMetricRS_35
    rdf:type owl:DatatypeProperty ;
    rdfs:subPropertyOf scor:hasResponsivenessMetric ;
    rdfs:domain [rdf:type owl:Class ;
        owl:unionOf (
        scor:IdentifySourcesOfSupply
        )] ;
    rdfs:label "Identify Sources and Supply Cycle Time"@en;
    rdfs:comment "The average time associated with the generation of the stocking schedule."@en;
    rdfs:isDefinedBy scor: ;
    vs:term_status "stable" ;
    dct:modified "2015-11-05"^^xsd:date ;
.

scor:hasMetricRS_36
    rdf:type owl:DatatypeProperty ;
    rdfs:subPropertyOf scor:hasResponsivenessMetric ;
    rdfs:domain [rdf:type owl:Class ;
        owl:unionOf (
        scor:IdentifyAssessAggregateProductionResources
        )] ;
    rdfs:label "Identify, Assess and Aggregate Production"@en;
    rdfs:comment "The average time associated with the identifying, prioritizing and aggregating of product requirements."@en;
    rdfs:isDefinedBy scor: ;
    vs:term_status "stable" ;
    dct:modified "2015-11-05"^^xsd:date ;
.

scor:hasMetricRS_37
    rdf:type owl:DatatypeProperty ;
    rdfs:subPropertyOf scor:hasResponsivenessMetric ;
    rdfs:domain [rdf:type owl:Class ;
        owl:unionOf (
        scor:IdentifyAssessAggregateDeliveryResources
        )] ;
    rdfs:label "Identify, Assess and Aggregate Delivery Resources Cycle Time"@en;
    rdfs:comment "The average time associated with the identifying, prioritizing and aggregating delivery resource availability."@en;
    rdfs:isDefinedBy scor: ;
    vs:term_status "stable" ;
    dct:modified "2015-11-05"^^xsd:date ;
.

scor:hasMetricRS_38
    rdf:type owl:DatatypeProperty ;
    rdfs:subPropertyOf scor:hasResponsivenessMetric ;
    rdfs:domain [rdf:type owl:Class ;
        owl:unionOf (
        scor:IdentifyAssessAggregateProductResources
        )] ;
    rdfs:label "Identify, Assess and Aggregate Product Resources Cycle Time"@en;
    rdfs:comment "The average time associated with the identifying, prioritizing and aggregating product resource availability."@en;
    rdfs:isDefinedBy scor: ;
    vs:term_status "stable" ;
    dct:modified "2015-11-05"^^xsd:date ;
.

scor:hasMetricRS_39
    rdf:type owl:DatatypeProperty ;
    rdfs:subPropertyOf scor:hasResponsivenessMetric ;
    rdfs:domain [rdf:type owl:Class ;
        owl:unionOf (
        scor:IdentifyPrioritizeAggregateSCResources
        )] ;
    rdfs:label "Identify, Assess and Aggregate Supply Chain Cycle Time"@en;
    rdfs:comment "The average time associated with the identifying, prioritizing and aggregating supply chain resource availibity."@en;
    rdfs:isDefinedBy scor: ;
    vs:term_status "stable" ;
    dct:modified "2015-11-05"^^xsd:date ;
.


scor:hasMetricRS_40
    rdf:type owl:DatatypeProperty ;
    rdfs:subPropertyOf scor:hasResponsivenessMetric ;
    rdfs:domain [rdf:type owl:Class ;
        owl:unionOf (
        scor:IdentifyPrioritizeAggregateDeliveryRequirements
        )] ;
    rdfs:label "Identify, Assess and Aggregate Delivery Requirements Cycle Time"@en;
    rdfs:comment "The average time associated with the identifying, prioritizing and aggregating delivery requirements availibity."@en;
    rdfs:isDefinedBy scor: ;
    vs:term_status "stable" ;
    dct:modified "2015-11-05"^^xsd:date ;
.

scor:hasMetricRS_41
    rdf:type owl:DatatypeProperty ;
    rdfs:subPropertyOf scor:hasResponsivenessMetric ;
    rdfs:domain [rdf:type owl:Class ;
        owl:unionOf (
        scor:IdentifyPrioritizeAggregateProductRequirements
        )] ;
    rdfs:label "Identify, Assess and Aggregate Product Requirements Cycle Time"@en;
    rdfs:comment "The average time associated with the identifying, prioritizing and aggregating product requirements."@en;
    rdfs:isDefinedBy scor: ;
    vs:term_status "stable" ;
    dct:modified "2015-11-05"^^xsd:date ;
.

scor:hasMetricRS_42
    rdf:type owl:DatatypeProperty ;
    rdfs:subPropertyOf scor:hasResponsivenessMetric ;
    rdfs:domain [rdf:type owl:Class ;
        owl:unionOf (
        scor:IdentifyPrioritizeAggregateProductRequirements
        )] ;
    rdfs:label "Identify, Assess and Aggregate Product Requirements Cycle Time"@en;
    rdfs:comment "The average time associated with the identifying, prioritizing and aggregating product requirements."@en;
    rdfs:isDefinedBy scor: ;
    vs:term_status "stable" ;
    dct:modified "2015-11-05"^^xsd:date ;
.

scor:hasMetricRS_43
    rdf:type owl:DatatypeProperty ;
    rdfs:subPropertyOf scor:hasResponsivenessMetric ;
    rdfs:domain [rdf:type owl:Class ;
        owl:unionOf (
        scor:AssessAggregateReturnRequirements
        )] ;
    rdfs:label "Identify, Assess and Aggregate Return Requirements Cycle Time"@en;
    rdfs:comment "The average time associated with the identifying, prioritizing and aggregating return requirements."@en;
    rdfs:isDefinedBy scor: ;
    vs:term_status "stable" ;
    dct:modified "2015-11-05"^^xsd:date ;
.

scor:hasMetricRS_44
    rdf:type owl:DatatypeProperty ;
    rdfs:subPropertyOf scor:hasResponsivenessMetric ;
    rdfs:domain [rdf:type owl:Class ;
        owl:unionOf (
        scor:PSCIdentifyPrioritizeAggregateSCRequirements
        )] ;
    rdfs:label "Identify, Assess and Aggregate Supply Chain Requirements Cycle Time"@en;
    rdfs:comment "The average time associated with the identifying, prioritizing and aggregating supply chain requirements."@en;
    rdfs:isDefinedBy scor: ;
    vs:term_status "stable" ;
    dct:modified "2015-11-05"^^xsd:date ;
.
#45 seems to be deprecated

scor:hasMetricRS_46
    rdf:type owl:DatatypeProperty ;
    rdfs:subPropertyOf scor:hasResponsivenessMetric ;
    rdfs:domain [rdf:type owl:Class ;
        owl:unionOf (
        scor:DSPInstallProduct
        scor:DMOPInstallProduct
        scor:DEOPInstallProduct
        )] ;
    rdfs:label "Install Product Cycle Time"@en;
    rdfs:comment "The average time associated with product installation."@en;
    rdfs:isDefinedBy scor: ;
    vs:term_status "stable" ;
    dct:modified "2015-11-05"^^xsd:date ;
.

scor:hasMetricRS_47
    rdf:type owl:DatatypeProperty ;
    rdfs:subPropertyOf scor:hasResponsivenessMetric ;
    rdfs:domain [rdf:type owl:Class ;
        owl:unionOf (
        scor:StockShelf
        )] ;
    rdfs:label "In-stock %"@en;
    rdfs:comment "Percentage of materials, components, or finished goods that are there when needed."@en;
    rdfs:isDefinedBy scor: ;
    vs:term_status "stable" ;
    dct:modified "2015-11-05"^^xsd:date ;
.

scor:hasMetricRS_48
    rdf:type owl:DatatypeProperty ;
    rdfs:subPropertyOf scor:hasResponsivenessMetric ;
    rdfs:domain [rdf:type owl:Class ;
        owl:unionOf (
        scor:DSPInvoice
        )] ;
    rdfs:label "Invoice Cycle Time"@en;
    rdfs:comment "The average time associated with the generation and issuance of an invoice."@en;
    rdfs:isDefinedBy scor: ;
    vs:term_status "stable" ;
    dct:modified "2015-11-05"^^xsd:date ;
.

scor:hasMetricRS_49
    rdf:type owl:DatatypeProperty ;
    rdfs:subPropertyOf scor:hasResponsivenessMetric ;
    rdfs:domain [rdf:type owl:Class ;
        owl:unionOf (
        scor:IssueMaterial
        )] ;
    rdfs:label "Issue Material Cycle Time"@en;
    rdfs:comment "The average time associated with the issuance of material to production."@en;
    rdfs:isDefinedBy scor: ;
    vs:term_status "stable" ;
    dct:modified "2015-11-05"^^xsd:date ;
.

scor:hasMetricRS_50
    rdf:type owl:DatatypeProperty ;
    rdfs:subPropertyOf scor:hasResponsivenessMetric ;
    rdfs:domain [rdf:type owl:Class ;
        owl:unionOf (
        scor:IssueSourcedInProcessProduct
        )] ;
    rdfs:label "Issue Sourced/In-Process Product Cycle Time"@en;
    rdfs:comment "The average time associated with the issuance of material to production."@en;
    rdfs:isDefinedBy scor: ;
    vs:term_status "stable" ;
    dct:modified "2015-11-05"^^xsd:date ;
.

scor:hasMetricRS_51
    rdf:type owl:DatatypeProperty ;
    rdfs:subPropertyOf scor:hasResponsivenessMetric ;
    rdfs:domain [rdf:type owl:Class ;
        owl:unionOf (
        scor:LoadVehicleGenerateShippingDocuments
        scor:DMOPLoadProductGenerateShippingDocs
        scor:DEOPLoadProductGenerateShippingDocs
        )] ;
    rdfs:label "Load & Generate Shipping Documentation Cycle Time"@en;
    rdfs:comment "The average time associated with the product loading and the generation of shipping documentation."@en;
    rdfs:isDefinedBy scor: ;
    vs:term_status "stable" ;
    dct:modified "2015-11-05"^^xsd:date ;
.

#52 seems to be deprecated

scor:hasMetricRS_53
    rdf:type owl:DatatypeProperty ;
    rdfs:subPropertyOf scor:hasResponsivenessMetric ;
    rdfs:domain [rdf:type owl:Class ;
        owl:unionOf (
        scor:ManageDataAndInformation
        )] ;
    rdfs:label "Maintain Source Cycle Time"@en;
    rdfs:comment "The average time associated with with maintaining source data."@en;
    rdfs:isDefinedBy scor: ;
    vs:term_status "stable" ;
    dct:modified "2015-11-05"^^xsd:date ;
.

scor:hasMetricRS_54
    rdf:type owl:DatatypeProperty ;
    rdfs:subPropertyOf scor:hasResponsivenessMetric ;
    rdfs:domain [rdf:type owl:Class ;
        owl:unionOf (
        scor:ManageSupplyChainBusinessRules
        )] ;
    rdfs:label "Manage Business Rules for PLAN Processes Cycle Time"@en;
    rdfs:comment "The average time associated with managing plan business rules."@en;
    rdfs:isDefinedBy scor: ;
    vs:term_status "stable" ;
    dct:modified "2015-11-05"^^xsd:date ;
.

scor:hasMetricRS_55
    rdf:type owl:DatatypeProperty ;
    rdfs:subPropertyOf scor:hasResponsivenessMetric ;
    rdfs:domain [rdf:type owl:Class ;
        owl:unionOf (
        scor:ManageSupplyChainBusinessRules
        )] ;
    rdfs:label "Manage Business Rules for PLAN Processes Cycle Time"@en;
    rdfs:comment "The average time associated with managing plan business rules."@en;
    rdfs:isDefinedBy scor: ;
    vs:term_status "stable" ;
    dct:modified "2015-11-05"^^xsd:date ;
.

scor:hasMetricRS_56
    rdf:type owl:DatatypeProperty ;
    rdfs:subPropertyOf scor:hasResponsivenessMetric ;
    rdfs:domain [rdf:type owl:Class ;
        owl:unionOf (
        scor:ScheduleAssetManagementActivities
        scor:TakeAssetOffline
        scor:InspectAndTroubleshoot
        scor:InstallAndConfigure
        scor:CleanMaintainAndRepair
        scor:InspectAndTroubleshoot
        scor:ReinstateAsset
        )] ;
    rdfs:label "Manage Capital Assets Cycle Time"@en;
    rdfs:comment "The average time associated with managing capital assets."@en;
    rdfs:isDefinedBy scor: ;
    vs:term_status "stable" ;
    dct:modified "2015-11-05"^^xsd:date ;
.

scor:hasMetricRS_57
    rdf:type owl:DatatypeProperty ;
    rdfs:subPropertyOf scor:hasResponsivenessMetric ;
    rdfs:domain [rdf:type owl:Class ;
        owl:unionOf (
        scor:ManageSupplyChainBusinessRules
        )] ;
    rdfs:label "Manage Deliver Business Rules Cycle Time"@en;
    rdfs:comment "The average time associated with managing deliver business rules."@en;
    rdfs:isDefinedBy scor: ;
    vs:term_status "stable" ;
    dct:modified "2015-11-05"^^xsd:date ;
.

scor:hasMetricRS_58
    rdf:type owl:DatatypeProperty ;
    rdfs:subPropertyOf scor:hasResponsivenessMetric ;
    rdfs:domain [rdf:type owl:Class ;
        owl:unionOf (
        scor:ScheduleAssetManagementActivities
        scor:TakeAssetOffline
        scor:InspectAndTroubleshoot
        scor:InstallAndConfigure
        scor:CleanMaintainAndRepair
        scor:InspectAndTroubleshoot
        scor:ReinstateAsset
        )] ;
    rdfs:label "Manage Deliver Capital Assets Cycle Time"@en;
    rdfs:comment "The average time associated with managing deliver capital assets."@en;
    rdfs:isDefinedBy scor: ;
    vs:term_status "stable" ;
    dct:modified "2015-11-05"^^xsd:date ;
.

scor:hasMetricRS_59
    rdf:type owl:DatatypeProperty ;
    rdfs:subPropertyOf scor:hasResponsivenessMetric ;
    rdfs:domain [rdf:type owl:Class ;
        owl:unionOf (
        scor:ManageDataAndInformation
        )] ;
    rdfs:label "Manage Deliver Information Cycle Time"@en;
    rdfs:comment "The average time associated with managing deliver information."@en;
    rdfs:isDefinedBy scor: ;
    vs:term_status "stable" ;
    dct:modified "2015-11-05"^^xsd:date ;
.

#60 seems to be deprecated

scor:hasMetricRS_61
    rdf:type owl:DatatypeProperty ;
    rdfs:subPropertyOf scor:hasResponsivenessMetric ;
    rdfs:domain [rdf:type owl:Class ;
        owl:unionOf (
        scor:ManageRegulatoryCompliance
        )] ;
    rdfs:label "Manage Import/Export Requirements Cycle Time"@en;
    rdfs:comment "The average time associated with managing import/export requirements."@en;
    rdfs:isDefinedBy scor: ;
    vs:term_status "stable" ;
    dct:modified "2015-11-05"^^xsd:date ;
.

#61-62 seem to be deprecated

scor:hasMetricRS_64
    rdf:type owl:DatatypeProperty ;
    rdfs:subPropertyOf scor:hasResponsivenessMetric ;
    rdfs:domain [rdf:type owl:Class ;
        owl:unionOf (
        scor:ManageSupplyChainAssets
        scor:ScheduleAssetManagementActivities
        scor:TakeAssetOffline
        scor:InspectAndTroubleshoot
        scor:InstallAndConfigure
        scor:CleanMaintainAndRepair
        scor:InspectMaintenance
        scor:ReinstateAsset
        )] ;
    rdfs:label "Manage Integrated Supply Chain Capital Assets Cycle Time"@en;
    rdfs:comment "The average time associated with managing integrated supply chain capital assets."@en;
    rdfs:isDefinedBy scor: ;
    vs:term_status "stable" ;
    dct:modified "2015-11-05"^^xsd:date ;
.

scor:hasMetricRS_65
    rdf:type owl:DatatypeProperty ;
    rdfs:subPropertyOf scor:hasResponsivenessMetric ;
    rdfs:domain [rdf:type owl:Class ;
        owl:unionOf (
        scor:ManagePerformance
        )] ;
    rdfs:label "Manage Integrated Supply Chain Inventory Cycle Time"@en;
    rdfs:comment "The average time associated with managing integrated supply chain inventory."@en;
    rdfs:isDefinedBy scor: ;
    vs:term_status "stable" ;
    dct:modified "2015-11-05"^^xsd:date ;
.

scor:hasMetricRS_66
    rdf:type owl:DatatypeProperty ;
    rdfs:subPropertyOf scor:hasResponsivenessMetric ;
    rdfs:domain [rdf:type owl:Class ;
        owl:unionOf (
        scor:ManageSupplyChainNetworks
        )] ;
    rdfs:label "Manage Integrated Supply Chain Transportation Cycle Time"@en;
    rdfs:comment "The average time associated with managing integrated supply chain transportation."@en;
    rdfs:isDefinedBy scor: ;
    vs:term_status "stable" ;
    dct:modified "2015-11-05"^^xsd:date ;
.

scor:hasMetricRS_67
    rdf:type owl:DatatypeProperty ;
    rdfs:subPropertyOf scor:hasResponsivenessMetric ;
    rdfs:domain [rdf:type owl:Class ;
        owl:unionOf (
        scor:ScheduleAssetManagementActivities
        scor:TakeAssetOffline
        scor:InspectAndTroubleshoot
        scor:InstallAndConfigure
        scor:CleanMaintainAndRepair
        scor:InspectMaintenance
        scor:ReinstateAsset
        )] ;
    rdfs:label "Manage MAKE Equipment and Facilities Cycle Time"@en;
    rdfs:comment "The average time associated with managing production equipment and facilities."@en;
    rdfs:isDefinedBy scor: ;
    vs:term_status "stable" ;
    dct:modified "2015-11-05"^^xsd:date ;
.

scor:hasMetricRS_68
    rdf:type owl:DatatypeProperty ;
    rdfs:subPropertyOf scor:hasResponsivenessMetric ;
    rdfs:domain [rdf:type owl:Class ;
        owl:unionOf (
        scor:ManageDataAndInformation
        )] ;
    rdfs:label "Manage MAKE Information Cycle Time"@en;
    rdfs:comment "The average time associated with managing production information."@en;
    rdfs:isDefinedBy scor: ;
    vs:term_status "stable" ;
    dct:modified "2015-11-05"^^xsd:date ;
.

#70 seems to be deprecated

scor:hasMetricRS_70
    rdf:type owl:DatatypeProperty ;
    rdfs:subPropertyOf scor:hasResponsivenessMetric ;
    rdfs:domain [rdf:type owl:Class ;
        owl:unionOf (
        scor:ManagePerformance
        )] ;
    rdfs:label "Manage Performance of Return Cycle Time"@en;
    rdfs:comment "The average time associated with managing the performance of return activities."@en;
    rdfs:isDefinedBy scor: ;
    vs:term_status "stable" ;
    dct:modified "2015-11-05"^^xsd:date ;
.

scor:hasMetricRS_71
    rdf:type owl:DatatypeProperty ;
    rdfs:subPropertyOf scor:hasResponsivenessMetric ;
    rdfs:domain [rdf:type owl:Class ;
        owl:unionOf (
        scor:ManagePerformance
        )] ;
    rdfs:label "Manage Performance of Supply Chain Cycle Time"@en;
    rdfs:comment "The average time associated with managing the performance of supply chain activities."@en;
    rdfs:isDefinedBy scor: ;
    vs:term_status "stable" ;
    dct:modified "2015-11-05"^^xsd:date ;
.

scor:hasMetricRS_72
    rdf:type owl:DatatypeProperty ;
    rdfs:subPropertyOf scor:hasResponsivenessMetric ;
    rdfs:domain [rdf:type owl:Class ;
        owl:unionOf (
        scor:ManageDataAndInformation
        )] ;
    rdfs:label "Manage PLAN Data Collection Cycle Time"@en;
    rdfs:comment "The average time associated with collecting plan data"@en;
    rdfs:isDefinedBy scor: ;
    vs:term_status "stable" ;
    dct:modified "2015-11-05"^^xsd:date ;
.

#73 seems to be deprecated

scor:hasMetricRS_74
    rdf:type owl:DatatypeProperty ;
    rdfs:subPropertyOf scor:hasResponsivenessMetric ;
    rdfs:domain [rdf:type owl:Class ;
        owl:unionOf (
        scor:ManageSupplyChainNetworks
        )] ;
    rdfs:label "Manage Planning Configuration Cycle Time"@en;
    rdfs:comment "The average time associated with managing the planning of the supply chain configuration"@en;
    rdfs:isDefinedBy scor: ;
    vs:term_status "stable" ;
    dct:modified "2015-11-05"^^xsd:date ;
.

#75-76 seem to be deprecated

scor:hasMetricRS_77
    rdf:type owl:DatatypeProperty ;
    rdfs:subPropertyOf scor:hasResponsivenessMetric ;
    rdfs:domain [rdf:type owl:Class ;
        owl:unionOf (
        scor:ManageSupplyChainNetworks
        )] ;
    rdfs:label "Manage Production Network Cycle Time"@en;
    rdfs:comment "The average time associated with managing the production network."@en;
    rdfs:isDefinedBy scor: ;
    vs:term_status "stable" ;
    dct:modified "2015-11-05"^^xsd:date ;
.

scor:hasMetricRS_78
    rdf:type owl:DatatypeProperty ;
    rdfs:subPropertyOf scor:hasResponsivenessMetric ;
    rdfs:domain [rdf:type owl:Class ;
        owl:unionOf (
        scor:ManagePerformance
        )] ;
    rdfs:label "Manage Production Performance Cycle Time"@en;
    rdfs:comment "The average time associated with managing the production performance."@en;
    rdfs:isDefinedBy scor: ;
    vs:term_status "stable" ;
    dct:modified "2015-11-05"^^xsd:date ;
.

scor:hasMetricRS_79
    rdf:type owl:DatatypeProperty ;
    rdfs:subPropertyOf scor:hasResponsivenessMetric ;
    rdfs:domain [rdf:type owl:Class ;
        owl:unionOf (
        scor:ManageSupplyChainBusinessRules
        )] ;
    rdfs:label "Manage Production Rules Cycle Time"@en;
    rdfs:comment "The average time associated with managing the production rules."@en;
    rdfs:isDefinedBy scor: ;
    vs:term_status "stable" ;
    dct:modified "2015-11-05"^^xsd:date ;
.

scor:hasMetricRS_80
    rdf:type owl:DatatypeProperty ;
    rdfs:subPropertyOf scor:hasResponsivenessMetric ;
    rdfs:domain [rdf:type owl:Class ;
        owl:unionOf (
        scor:ScheduleAssetManagementActivities
        scor:TakeAssetOffline
        scor:InspectAndTroubleshoot
        scor:InstallAndConfigure
        scor:CleanMaintainAndRepair
        scor:InspectMaintenance
        scor:ReinstateAsset
        )] ;
    rdfs:label "Manage Return Capital Assets Cycle Time"@en;
    rdfs:comment "The average time associated with managing return capital assets."@en;
    rdfs:isDefinedBy scor: ;
    vs:term_status "stable" ;
    dct:modified "2015-11-05"^^xsd:date ;
.

scor:hasMetricRS_81
    rdf:type owl:DatatypeProperty ;
    rdfs:subPropertyOf scor:hasResponsivenessMetric ;
    rdfs:domain [rdf:type owl:Class ;
        owl:unionOf (
        scor:ManageDataAndInformation
        )] ;
    rdfs:label "Manage Return Data Collection Cycle Time"@en;
    rdfs:comment "The average time associated with managing the return data collection."@en;
    rdfs:isDefinedBy scor: ;
    vs:term_status "stable" ;
    dct:modified "2015-11-05"^^xsd:date ;
.

#82 seems to be deprecated

scor:hasMetricRS_83
    rdf:type owl:DatatypeProperty ;
    rdfs:subPropertyOf scor:hasResponsivenessMetric ;
    rdfs:domain [rdf:type owl:Class ;
        owl:unionOf (
        scor:ManageSupplyChainNetworks
        )] ;
    rdfs:label "Manage Return Network Configuration Cycle Time"@en;
    rdfs:comment "The average time associated with managing the return network configuration."@en;
    rdfs:isDefinedBy scor: ;
    vs:term_status "stable" ;
    dct:modified "2015-11-05"^^xsd:date ;
.

#84 seems to be deprecated

scor:hasMetricRS_85
    rdf:type owl:DatatypeProperty ;
    rdfs:subPropertyOf scor:hasResponsivenessMetric ;
    rdfs:domain [rdf:type owl:Class ;
        owl:unionOf (
        scor:ManageSupplyChainNetworks
        )] ;
    rdfs:label "Manage Return Transportation Cycle Time"@en;
    rdfs:comment "The average time associated with managing return transportation."@en;
    rdfs:isDefinedBy scor: ;
    vs:term_status "stable" ;
    dct:modified "2015-11-05"^^xsd:date ;
.

scor:hasMetricRS_86
    rdf:type owl:DatatypeProperty ;
    rdfs:subPropertyOf scor:hasResponsivenessMetric ;
    rdfs:domain [rdf:type owl:Class ;
        owl:unionOf (
        scor:ManageSupplyChainBusinessRules
        )] ;
    rdfs:label "Manage Sourcing Business Rules Cycle Time"@en;
    rdfs:comment "The average time associated with managing of source business rules."@en;
    rdfs:isDefinedBy scor: ;
    vs:term_status "stable" ;
    dct:modified "2015-11-05"^^xsd:date ;
.

scor:hasMetricRS_87
    rdf:type owl:DatatypeProperty ;
    rdfs:subPropertyOf scor:hasResponsivenessMetric ;
    rdfs:domain [rdf:type owl:Class ;
        owl:unionOf (
        scor:ManageSupplyChainContracts
        )] ;
    rdfs:label "Manage Supplier Agreements Cycle Time"@en;
    rdfs:comment "The average time associated with managing of supplier agreements."@en;
    rdfs:isDefinedBy scor: ;
    vs:term_status "stable" ;
    dct:modified "2015-11-05"^^xsd:date ;
.

scor:hasMetricRS_88
    rdf:type owl:DatatypeProperty ;
    rdfs:subPropertyOf scor:hasResponsivenessMetric ;
    rdfs:domain [rdf:type owl:Class ;
        owl:unionOf (
        scor:ManageSupplyChainNetworks
        )] ;
    rdfs:label "Manage Supplier Network Cycle Time"@en;
    rdfs:comment "The average time associated with managing of the supplier network."@en;
    rdfs:isDefinedBy scor: ;
    vs:term_status "stable" ;
    dct:modified "2015-11-05"^^xsd:date ;
.

scor:hasMetricRS_89
    rdf:type owl:DatatypeProperty ;
    rdfs:subPropertyOf scor:hasResponsivenessMetric ;
    rdfs:domain [rdf:type owl:Class ;
        owl:unionOf (
        scor:ManageSupplyChainNetworks
        )] ;
    rdfs:label "Manage Transportation (WIP) Cycle Time"@en;
    rdfs:comment "The average time associated with managing (WIP) transportation."@en;
    rdfs:isDefinedBy scor: ;
    vs:term_status "stable" ;
    dct:modified "2015-11-05"^^xsd:date ;
.

scor:hasMetricRS_90
    rdf:type owl:DatatypeProperty ;
    rdfs:subPropertyOf scor:hasResponsivenessMetric ;
    rdfs:domain [rdf:type owl:Class ;
        owl:unionOf (
        scor:ManageSupplyChainNetworks
        )] ;
    rdfs:label "Manage Transportation Cycle Time"@en;
    rdfs:comment "The average time associated with managing transportation."@en;
    rdfs:isDefinedBy scor: ;
    vs:term_status "stable" ;
    dct:modified "2015-11-05"^^xsd:date ;
.

#91 seems to be deprecated

scor:hasMetricRS_92
    rdf:type owl:DatatypeProperty ;
    rdfs:subPropertyOf scor:hasResponsivenessMetric ;
    rdfs:domain [rdf:type owl:Class ;
        owl:unionOf (
        scor:NegotiateReceiveContract
        )] ;
    rdfs:label "Negotiate & Receive Contract Cycle Time"@en;
    rdfs:comment "The average time associated with negotiating and receing contract."@en;
    rdfs:isDefinedBy scor: ;
    vs:term_status "stable" ;
    dct:modified "2015-11-05"^^xsd:date ;
.

scor:hasMetricRS_93
    rdf:type owl:DatatypeProperty ;
    rdfs:subPropertyOf scor:hasResponsivenessMetric ;
    rdfs:domain [rdf:type owl:Class ;
        owl:unionOf (
        scor:ObtainRespondToRFPRFQ
        )] ;
    rdfs:label "Obtain & Respond to Request for Quote (RFQ) / Request for Proposal (RFP) Cycle time"@en;
    rdfs:comment "The average time associated with obtaining and responding to RFQs/RFPs."@en;
    rdfs:isDefinedBy scor: ;
    vs:term_status "stable" ;
    dct:modified "2015-11-05"^^xsd:date ;
.

scor:hasMetricRS_94
    rdf:type owl:DatatypeProperty ;
    rdfs:subPropertyOf scor:hasResponsivenessMetric ;
    rdfs:domain [rdf:type owl:Class ;
        owl:unionOf (
        scor:ReceiveEnterValidateOrder
        scor:DSPReserveInventoryDetermineDeliveryDate
        scor:ReceiveConfigureEnterValidateOrder
        scor:DMOPReserveInventoryDetermineDeliveryDate
        scor:EnterOrderCommitResourcesLaunchProgram
        )] ;
    rdfs:label "Order Fulfillment Dwell Time"@en;
    rdfs:comment "Any lead time during the order fulfillment process where no activity takes place , which is imposed by customer requirements. Not that this dwell time is different from idle-time or non-value-add lead  time, which is cause by inefficiencies in the organizations processes and therefore ultimately under responsibility of the organization. This kind of idle time should not be deducted from Order Fulfillment Cycle Time."@en;
    rdfs:isDefinedBy scor: ;
    vs:term_status "stable" ;
    dct:modified "2015-11-05"^^xsd:date ;
.

scor:hasMetricRS_95
    rdf:type owl:DatatypeProperty ;
    rdfs:subPropertyOf scor:hasResponsivenessMetric ;
    rdfs:domain [rdf:type owl:Class ;
        owl:unionOf (
        scor:DSPPackProduct
        scor:DMOPPackProduct
        scor:DEOPPackProduct
        )] ;
    rdfs:label "Pack Product Cycle Time"@en;
    rdfs:comment "The average time associated with packing a product for shipment."@en;
    rdfs:isDefinedBy scor: ;
    vs:term_status "stable" ;
    dct:modified "2015-11-05"^^xsd:date ;
.

scor:hasMetricRS_96
    rdf:type owl:DatatypeProperty ;
    rdfs:subPropertyOf scor:hasResponsivenessMetric ;
    rdfs:domain [rdf:type owl:Class ;
        owl:unionOf (
        scor:DSPPickProduct
        scor:DMOPPickProduct
        scor:DEOPPickProduct
        )] ;
    rdfs:label "Pick Product Cycle Time"@en;
    rdfs:comment "The average time associated with product pick."@en;
    rdfs:isDefinedBy scor: ;
    vs:term_status "stable" ;
    dct:modified "2015-11-05"^^xsd:date ;
.

scor:hasMetricRS_97
    rdf:type owl:DatatypeProperty ;
    rdfs:subPropertyOf scor:hasResponsivenessMetric ;
    rdfs:domain [rdf:type owl:Class ;
        owl:unionOf (
        scor:PickProductFromBackroom
        )] ;
    rdfs:label "Pick Product from Backroom Cycle Time"@en;
    rdfs:comment "The average time associated with product pick from backroom."@en;
    rdfs:isDefinedBy scor: ;
    vs:term_status "stable" ;
    dct:modified "2015-11-05"^^xsd:date ;
.

scor:hasMetricRS_98
    rdf:type owl:DatatypeProperty ;
    rdfs:subPropertyOf scor:hasResponsivenessMetric ;
    rdfs:domain [rdf:type owl:Class ;
        owl:unionOf (
        scor:PlanSupplyChain
        )] ;
    rdfs:label "Plan Cycle Time"@en;
    rdfs:comment "The average time associated with Plan Processes"@en;
    rdfs:isDefinedBy scor: ;
    vs:term_status "stable" ;
    dct:modified "2015-11-05"^^xsd:date ;
.

scor:hasMetricRS_99
    rdf:type owl:DatatypeProperty ;
    rdfs:subPropertyOf scor:hasResponsivenessMetric ;
    rdfs:domain [rdf:type owl:Class ;
        owl:unionOf (
        scor:PlanSource
        )] ;
    rdfs:label "Plan Source Cycle Time"@en;
    rdfs:comment "The average time associated with planning source activities."@en;
    rdfs:isDefinedBy scor: ;
    vs:term_status "stable" ;
    dct:modified "2015-11-05"^^xsd:date ;
.

scor:hasMetricRS_100
    rdf:type owl:DatatypeProperty ;
    rdfs:subPropertyOf scor:hasResponsivenessMetric ;
    rdfs:domain [rdf:type owl:Class ;
        owl:unionOf (
        scor:ProcessInquiryQuote
        )] ;
    rdfs:label "Plan Inquiry & Quote Cycle Time"@en;
    rdfs:comment "The average time associated with processing inquiries and quotes."@en;
    rdfs:isDefinedBy scor: ;
    vs:term_status "stable" ;
    dct:modified "2015-11-05"^^xsd:date ;
.

scor:hasMetricRS_101
    rdf:type owl:DatatypeProperty ;
    rdfs:subPropertyOf scor:hasResponsivenessMetric ;
    rdfs:domain [rdf:type owl:Class ;
        owl:unionOf (
        scor:MSProduceTest
        scor:MOProduceTest
        scor:MEOProduceTest
        )] ;
    rdfs:label "Produce and Test Cycle Time"@en;
    rdfs:comment "The average time associated with production and test."@en;
    rdfs:isDefinedBy scor: ;
    vs:term_status "stable" ;
    dct:modified "2015-11-05"^^xsd:date ;
.

scor:hasMetricRS_102
    rdf:type owl:DatatypeProperty ;
    rdfs:subPropertyOf scor:hasResponsivenessMetric ;
    rdfs:domain [rdf:type owl:Class ;
        owl:unionOf (
        scor:DSPReceiveVerifyProductByCustomer
        scor:DMOPReceiveVerifyProductByCustomer
        scor:DSPReceiveVerifyProductByCustomer
        )] ;
    rdfs:label "Receive & Verify Product by Customer Cycle Time"@en;
    rdfs:comment "The average time associated with receiving and verifying an order at the customer site."@en;
    rdfs:isDefinedBy scor: ;
    vs:term_status "stable" ;
    dct:modified "2015-11-05"^^xsd:date ;
.

scor:hasMetricRS_103
    rdf:type owl:DatatypeProperty ;
    rdfs:subPropertyOf scor:hasResponsivenessMetric ;
    rdfs:domain [rdf:type owl:Class ;
        owl:unionOf (
        scor:DSPReceiveVerifyProductByCustomer
        scor:DMOPReceiveVerifyProductByCustomer
        scor:DSPReceiveVerifyProductByCustomer
        )] ;
    rdfs:label "Receive & Verify Product Cycle Time"@en;
    rdfs:comment "The average time associated with receiving and verifying an order."@en;
    rdfs:isDefinedBy scor: ;
    vs:term_status "stable" ;
    dct:modified "2015-11-05"^^xsd:date ;
.

scor:hasMetricRS_104
    rdf:type owl:DatatypeProperty ;
    rdfs:subPropertyOf scor:hasResponsivenessMetric ;
    rdfs:domain [rdf:type owl:Class ;
        owl:unionOf (
        scor:ReceiveDefectiveProduct
        )] ;
    rdfs:label "Receive Defective Product Cycle Time"@en;
    rdfs:comment "The average time associated with receiving defective product returns from the customer."@en;
    rdfs:isDefinedBy scor: ;
    vs:term_status "stable" ;
    dct:modified "2015-11-05"^^xsd:date ;
.

scor:hasMetricRS_105
    rdf:type owl:DatatypeProperty ;
    rdfs:subPropertyOf scor:hasResponsivenessMetric ;
    rdfs:domain [rdf:type owl:Class ;
        owl:unionOf (
        scor:ReceiveExcessProduct
        )] ;
    rdfs:label "Receive Excess Product Cycle Time"@en;
    rdfs:comment "The average time associated with receiving excess product returns from the customer."@en;
    rdfs:isDefinedBy scor: ;
    vs:term_status "stable" ;
    dct:modified "2015-11-05"^^xsd:date ;
.

scor:hasMetricRS_106
    rdf:type owl:DatatypeProperty ;
    rdfs:subPropertyOf scor:hasResponsivenessMetric ;
    rdfs:domain [rdf:type owl:Class ;
        owl:unionOf (
        scor:ReceiveMROProduct
        )] ;
    rdfs:label "Receive MRO Product Cycle Time"@en;
    rdfs:comment "The average time associated with receiving MRO product returns from the customer."@en;
    rdfs:isDefinedBy scor: ;
    vs:term_status "stable" ;
    dct:modified "2015-11-05"^^xsd:date ;
.

scor:hasMetricRS_107
    rdf:type owl:DatatypeProperty ;
    rdfs:subPropertyOf scor:hasResponsivenessMetric ;
    rdfs:domain [rdf:type owl:Class ;
        owl:unionOf (
        scor:ReceiveProductAtStore
        )] ;
    rdfs:label "Receive Product Cycle Time"@en;
    rdfs:comment "The average time associated with receiving a product."@en;
    rdfs:isDefinedBy scor: ;
    vs:term_status "stable" ;
    dct:modified "2015-11-05"^^xsd:date ;
.

scor:hasMetricRS_108
    rdf:type owl:DatatypeProperty ;
    rdfs:subPropertyOf scor:hasResponsivenessMetric ;
    rdfs:domain [rdf:type owl:Class ;
        owl:unionOf (
        scor:DSPReceiveProductFromSourceMake
        scor:DMOPReceiveProductFromSourceMake
        scor:DEOPReceiveProductFromSourceMake
        )] ;
    rdfs:label "Receive Product form Make/Source Cycle Time"@en;
    rdfs:comment "The average time associated with receiving a product from Make/Source."@en;
    rdfs:isDefinedBy scor: ;
    vs:term_status "stable" ;
    dct:modified "2015-11-05"^^xsd:date ;
.

scor:hasMetricRS_109
    rdf:type owl:DatatypeProperty ;
    rdfs:subPropertyOf scor:hasResponsivenessMetric ;
    rdfs:domain [rdf:type owl:Class ;
        owl:unionOf (
        scor:ReceiveProductAtStore
        )] ;
    rdfs:label "Receive Product at Store Cycle Time"@en;
    rdfs:comment "The average time associated with receiving a product at the customer store."@en;
    rdfs:isDefinedBy scor: ;
    vs:term_status "stable" ;
    dct:modified "2015-11-05"^^xsd:date ;
.

scor:hasMetricRS_110
    rdf:type owl:DatatypeProperty ;
    rdfs:subPropertyOf scor:hasResponsivenessMetric ;
    rdfs:domain [rdf:type owl:Class ;
        owl:unionOf (
        scor:DSPReceiveProductFromSourceMake
        scor:DMOPReceiveProductFromSourceMake
        scor:DEOPReceiveProductFromSourceMake
        )] ;
    rdfs:label "Receive Product from Source or Make Cycle Time"@en;
    rdfs:comment "The average time associated with receiving transfer of product to deliver processes from source or make."@en;
    rdfs:isDefinedBy scor: ;
    vs:term_status "stable" ;
    dct:modified "2015-11-05"^^xsd:date ;
.

scor:hasMetricRS_111
    rdf:type owl:DatatypeProperty ;
    rdfs:subPropertyOf scor:hasResponsivenessMetric ;
    rdfs:domain [rdf:type owl:Class ;
        owl:unionOf (
        scor:ReceiveConfigureEnterValidateOrder
        )] ;
    rdfs:label "Receive, Configure, Enter & Validate Order Cycle Time"@en;
    rdfs:comment "The average time associated with receiving and verifying and order at the customer site."@en;
    rdfs:isDefinedBy scor: ;
    vs:term_status "stable" ;
    dct:modified "2015-11-05"^^xsd:date ;
.

scor:hasMetricRS_112
    rdf:type owl:DatatypeProperty ;
    rdfs:subPropertyOf scor:hasResponsivenessMetric ;
    rdfs:domain [rdf:type owl:Class ;
        owl:unionOf (
        scor:ReceiveEnterValidateOrder
        )] ;
    rdfs:label "Receive, Enter & Validate Order Cycle Time"@en;
    rdfs:comment "The average time associated with receiving, entering and verifying an order at the customer site."@en;
    rdfs:isDefinedBy scor: ;
    vs:term_status "stable" ;
    dct:modified "2015-11-05"^^xsd:date ;
.

scor:hasMetricRS_113
    rdf:type owl:DatatypeProperty ;
    rdfs:subPropertyOf scor:hasResponsivenessMetric ;
    rdfs:domain [rdf:type owl:Class ;
        owl:unionOf (
        scor:SSPReceiveProduct
        scor:SMOPReceiveProduct
        scor:SEOPReceiveProduct
        )] ;
    rdfs:label "Receiving Product Cycle Time"@en;
    rdfs:comment "Total elapsed time from the time the product is received to time it is passed to next process."@en;
    rdfs:isDefinedBy scor: ;
    vs:term_status "stable" ;
    dct:modified "2015-11-05"^^xsd:date ;
.

scor:hasMetricRS_114
    rdf:type owl:DatatypeProperty ;
    rdfs:subPropertyOf scor:hasResponsivenessMetric ;
    rdfs:domain [rdf:type owl:Class ;
        owl:unionOf (
        scor:ReleaseProductToDeliver
        scor:ReleaseFinishedProductToDeliver
        scor:MEOReleaseProductToDeliver
        )] ;
    rdfs:label "Release Finished Product to Deliver Cycle Time"@en;
    rdfs:comment "The average time associated with releasing finished product to deliver."@en;
    rdfs:isDefinedBy scor: ;
    vs:term_status "stable" ;
    dct:modified "2015-11-05"^^xsd:date ;
.

scor:hasMetricRS_115
    rdf:type owl:DatatypeProperty ;
    rdfs:subPropertyOf scor:hasResponsivenessMetric ;
    rdfs:domain [rdf:type owl:Class ;
        owl:unionOf (
        scor:DMOPReserveInventoryDetermineDeliveryDate
        )] ;
    rdfs:label "Resever Inventory & Determine Data Cycle Time"@en;
    rdfs:comment "The average time associated with reserving inventory and determining a delivery date."@en;
    rdfs:isDefinedBy scor: ;
    vs:term_status "stable" ;
    dct:modified "2015-11-05"^^xsd:date ;
.

scor:hasMetricRS_116
    rdf:type owl:DatatypeProperty ;
    rdfs:subPropertyOf scor:hasResponsivenessMetric ;
    rdfs:domain [rdf:type owl:Class ;
        owl:unionOf (
        scor:DSPReserveInventoryDetermineDeliveryDate
        )] ;
    rdfs:label "Reserve Resources and Determine Delivery Date Cycle Time"@en;
    rdfs:comment "The average time associated with reserving resources and determining delivery date."@en;
    rdfs:isDefinedBy scor: ;
    vs:term_status "stable" ;
    dct:modified "2015-11-05"^^xsd:date ;
.

scor:hasMetricRS_117
    rdf:type owl:DatatypeProperty ;
    rdfs:subPropertyOf scor:hasResponsivenessMetric ;
    rdfs:domain [rdf:type owl:Class ;
        owl:unionOf (
        scor:DSPRouteShipments
        scor:DMOPRouteShipments
        scor:DEOPRouteShipments
        )] ;
    rdfs:label "Route Shipments Cycle Time"@en;
    rdfs:comment "The average time associated with routing shipments."@en;
    rdfs:isDefinedBy scor: ;
    vs:term_status "stable" ;
    dct:modified "2015-11-05"^^xsd:date ;
.

scor:hasMetricRS_118
    rdf:type owl:DatatypeProperty ;
    rdfs:subPropertyOf scor:hasResponsivenessMetric ;
    rdfs:domain [rdf:type owl:Class ;
        owl:unionOf (
        scor:ScheduleDefectiveReturnReceipt
        )] ;
    rdfs:label "Schedule Defective Return Receipt Cycle Time"@en;
    rdfs:comment "The average time associated with scheduling the receipt of the return of defective product."@en;
    rdfs:isDefinedBy scor: ;
    vs:term_status "stable" ;
    dct:modified "2015-11-05"^^xsd:date ;
.

scor:hasMetricRS_119
    rdf:type owl:DatatypeProperty ;
    rdfs:subPropertyOf scor:hasResponsivenessMetric ;
    rdfs:domain [rdf:type owl:Class ;
        owl:unionOf (
        scor:ScheduleExcessReturnReceipt
        )] ;
    rdfs:label "Schedule Excess Return Receipt Cycle Time"@en;
    rdfs:comment "The average time associated with scheduling the receipt of the return excess product."@en;
    rdfs:isDefinedBy scor: ;
    vs:term_status "stable" ;
    dct:modified "2015-11-05"^^xsd:date ;
.

scor:hasMetricRS_120
    rdf:type owl:DatatypeProperty ;
    rdfs:subPropertyOf scor:hasResponsivenessMetric ;
    rdfs:domain [rdf:type owl:Class ;
        owl:unionOf (
        scor:ScheduleInstallation
        )] ;
    rdfs:label "Schedule Installation Cycle Time"@en;
    rdfs:comment "The average time associated with scheduling the installation of the product."@en;
    rdfs:isDefinedBy scor: ;
    vs:term_status "stable" ;
    dct:modified "2015-11-05"^^xsd:date ;
.

scor:hasMetricRS_121
    rdf:type owl:DatatypeProperty ;
    rdfs:subPropertyOf scor:hasResponsivenessMetric ;
    rdfs:domain [rdf:type owl:Class ;
        owl:unionOf (
        scor:ScheduleMROReturnReceipt
        )] ;
    rdfs:label "Schedule MRO Return Receipt Cycle Time"@en;
    rdfs:comment "The average time associated with scheduling the receipt of the return MRO product."@en;
    rdfs:isDefinedBy scor: ;
    vs:term_status "stable" ;
    dct:modified "2015-11-05"^^xsd:date ;
.

scor:hasMetricRS_122
    rdf:type owl:DatatypeProperty ;
    rdfs:subPropertyOf scor:hasResponsivenessMetric ;
    rdfs:domain [rdf:type owl:Class ;
        owl:unionOf (
        scor:SSPScheduleProductDeliveries
        scor:SMOPScheduleProductDeliveries
        scor:SEOPScheduleProductDeliveries
        )] ;
    rdfs:label "Schedule Product Deliveries Cycle Time"@en;
    rdfs:comment "The average time associated with scheduling the shipment of the return MRO product."@en;
    rdfs:isDefinedBy scor: ;
    vs:term_status "stable" ;
    dct:modified "2015-11-05"^^xsd:date ;
.

scor:hasMetricRS_123
    rdf:type owl:DatatypeProperty ;
    rdfs:subPropertyOf scor:hasResponsivenessMetric ;
    rdfs:domain [rdf:type owl:Class ;
        owl:unionOf (
        scor:MSScheduleProductionActivities
        scor:MOScheduleProductionActivities
        scor:MEOScheduleProductionActivities
        )] ;
    rdfs:label "Schedule Production Activities Cycle Time."@en;
    rdfs:comment "The average time associated with scheudling production activities."@en;
    rdfs:isDefinedBy scor: ;
    vs:term_status "stable" ;
    dct:modified "2015-11-05"^^xsd:date ;
.

scor:hasMetricRS_124
    rdf:type owl:DatatypeProperty ;
    rdfs:subPropertyOf scor:hasResponsivenessMetric ;
    rdfs:domain [rdf:type owl:Class ;
        owl:unionOf (
        scor:DEOPSelectCarriersRateShipments
        )] ;
    rdfs:label "Select Carriers & Rate Shipments Cycle Time"@en;
    rdfs:comment "The average time associated with selecting carriers and rating shipments."@en;
    rdfs:isDefinedBy scor: ;
    vs:term_status "stable" ;
    dct:modified "2015-11-05"^^xsd:date ;
.

scor:hasMetricRS_125
    rdf:type owl:DatatypeProperty ;
    rdfs:subPropertyOf scor:hasResponsivenessMetric ;
    rdfs:domain [rdf:type owl:Class ;
        owl:unionOf (
        scor:SelectFinalSupplierNegotiate
        )] ;
    rdfs:label "Select Supplier and Negotiate Cycle Time"@en;
    rdfs:comment "The average time associated with selecting a supplier and negotiating."@en;
    rdfs:isDefinedBy scor: ;
    vs:term_status "stable" ;
    dct:modified "2015-11-05"^^xsd:date ;
.

scor:hasMetricRS_126
    rdf:type owl:DatatypeProperty ;
    rdfs:subPropertyOf scor:hasResponsivenessMetric ;
    rdfs:domain [rdf:type owl:Class ;
        owl:unionOf (
        scor:DSPShipProduct
        scor:DMOPShipProduct
        scor:DEOPShipProduct
        )] ;
    rdfs:label "Ship Product Cycle Time"@en;
    rdfs:comment "The average time associated with shipping the product."@en;
    rdfs:isDefinedBy scor: ;
    vs:term_status "stable" ;
    dct:modified "2015-11-05"^^xsd:date ;
.

scor:hasMetricRS_127
    rdf:type owl:DatatypeProperty ;
    rdfs:subPropertyOf scor:hasResponsivenessMetric ;
    rdfs:domain [rdf:type owl:Class ;
        owl:unionOf (
        scor:SourceReturnDefectiveProduct
        scor:SourceReturnExcessProduct
        )] ;
    rdfs:label "Source Return Cycle Time"@en;
    rdfs:comment "The average time associated with Sourcing Return."@en;
    rdfs:isDefinedBy scor: ;
    vs:term_status "stable" ;
    dct:modified "2015-11-05"^^xsd:date ;
.

scor:hasMetricRS_128
    rdf:type owl:DatatypeProperty ;
    rdfs:subPropertyOf scor:hasResponsivenessMetric ;
    rdfs:domain [rdf:type owl:Class ;
        owl:unionOf (
        scor:StageProduct
        scor:StageFinishedProduct
        scor:MEOStageFinishedProduct
        )] ;
    rdfs:label "Stage Finished Product Cycle Time"@en;
    rdfs:comment "The average time associated with staging the finished product."@en;
    rdfs:isDefinedBy scor: ;
    vs:term_status "stable" ;
    dct:modified "2015-11-05"^^xsd:date ;
.

scor:hasMetricRS_129
    rdf:type owl:DatatypeProperty ;
    rdfs:subPropertyOf scor:hasResponsivenessMetric ;
    rdfs:domain [rdf:type owl:Class ;
        owl:unionOf (
        scor:StockShelf
        )] ;
    rdfs:label "Stock Shelf Cycle Time"@en;
    rdfs:comment "The average time associated with stocking shelves."@en;
    rdfs:isDefinedBy scor: ;
    vs:term_status "stable" ;
    dct:modified "2015-11-05"^^xsd:date ;
.

#130-135 seems to be deprecated

scor:hasMetricRS_136
    rdf:type owl:DatatypeProperty ;
    rdfs:subPropertyOf scor:hasResponsivenessMetric ;
    rdfs:domain [rdf:type owl:Class ;
        owl:unionOf (
        scor:TransferDefectiveProduct
        )] ;
    rdfs:label "Transfer Defective Product Cycle Time"@en;
    rdfs:comment "The average time associated transfer until the product is moved to the next process. (Defective)"@en;
    rdfs:isDefinedBy scor: ;
    vs:term_status "stable" ;
    dct:modified "2015-11-05"^^xsd:date ;
.

scor:hasMetricRS_137
    rdf:type owl:DatatypeProperty ;
    rdfs:subPropertyOf scor:hasResponsivenessMetric ;
    rdfs:domain [rdf:type owl:Class ;
        owl:unionOf (
        scor:TransferExcessProduct
        )] ;
    rdfs:label "Transfer Excess Product Cycle Time"@en;
    rdfs:comment "The average time associated transfer until the product is moved to the next process. (Excess)"@en;
    rdfs:isDefinedBy scor: ;
    vs:term_status "stable" ;
    dct:modified "2015-11-05"^^xsd:date ;
.

scor:hasMetricRS_138
    rdf:type owl:DatatypeProperty ;
    rdfs:subPropertyOf scor:hasResponsivenessMetric ;
    rdfs:domain [rdf:type owl:Class ;
        owl:unionOf (
        scor:TransferMROProduct
        )] ;
    rdfs:label "Transfer MRO Product Cycle Time"@en;
    rdfs:comment "The average time associated transfer until the product is moved to the next process. (MRO)"@en;
    rdfs:isDefinedBy scor: ;
    vs:term_status "stable" ;
    dct:modified "2015-11-05"^^xsd:date ;
.

scor:hasMetricRS_139
    rdf:type owl:DatatypeProperty ;
    rdfs:subPropertyOf scor:hasResponsivenessMetric ;
    rdfs:domain [rdf:type owl:Class ;
        owl:unionOf (
        scor:SSPTransferProduct
        scor:SMOPTransferProduct
        scor:SEOPTransferProduct
        )] ;
    rdfs:label "Transfer Product Cycle Time"@en;
    rdfs:comment "The average time associated transfer until the product is moved to the next process."@en;
    rdfs:isDefinedBy scor: ;
    vs:term_status "stable" ;
    dct:modified "2015-11-05"^^xsd:date ;
.

scor:hasMetricRS_140
    rdf:type owl:DatatypeProperty ;
    rdfs:subPropertyOf scor:hasResponsivenessMetric ;
    rdfs:domain [rdf:type owl:Class ;
        owl:unionOf (
        scor:SSPVerifyProduct
        scor:SMOPVerifyProduct
        scor:SEOPVerifyProduct
        )] ;
    rdfs:label "Verify Product Cycle Time"@en;
    rdfs:comment "The average time associated transfer with verifying raw material products."@en;
    rdfs:isDefinedBy scor: ;
    vs:term_status "stable" ;
    dct:modified "2015-11-05"^^xsd:date ;
.

scor:hasMetricRS_141
    rdf:type owl:DatatypeProperty ;
    rdfs:subPropertyOf scor:hasResponsivenessMetric ;
    rdfs:domain [rdf:type owl:Class ;
        owl:unionOf (
        scor:MSWasteDisposal
        scor:MOWasteDisposal
        scor:MEOWasteDisposal
        )] ;
    rdfs:label "Waste accumulation Cycle Time"@en;
    rdfs:comment "The time required to collect and properly store production waste."@en;
    rdfs:isDefinedBy scor: ;
    vs:term_status "stable" ;
    dct:modified "2015-11-05"^^xsd:date ;
.

scor:hasMetricRS_142
    rdf:type owl:DatatypeProperty ;
    rdfs:subPropertyOf scor:hasResponsivenessMetric ;
    rdfs:domain [rdf:type owl:Class ;
        owl:unionOf (
        scor:MSPackage
        scor:MOPackage
        scor:MEOPackage
        )] ;
    rdfs:label "Package Cycle Time"@en;
    rdfs:comment "The average time associated transfer with packaging the product in the Make process."@en;
    rdfs:isDefinedBy scor: ;
    vs:term_status "stable" ;
    dct:modified "2015-11-05"^^xsd:date ;
.

######### Agility Metrics

scor:hasMetricAG_1
    rdf:type owl:DatatypeProperty ;
    rdfs:subPropertyOf scor:hasAgilityMetric ;
    rdfs:domain [rdf:type owl:Class ;
        owl:unionOf (
        scor:DeliverStockedProduct
        scor:DeliverMakeToOrderProduct
        scor:DeliverEngineerToOrderProduct
        )] ;
    rdfs:label "% of labor used in logistics, not used in direct activity"@en;
    rdfs:comment "Percent of labor used in logistics, not used in direct activity"@en;
    rdfs:isDefinedBy scor: ;
    vs:term_status "stable" ;
    dct:modified "2015-11-05"^^xsd:date ;
.

scor:hasMetricAG_2
    rdf:type owl:DatatypeProperty ;
    rdfs:subPropertyOf scor:hasAgilityMetric ;
    rdfs:domain [rdf:type owl:Class ;
        owl:unionOf (
        scor:MakeToStock
        scor:MakeToOrder
        scor:MakeEngineerToOrder
        )] ;
    rdfs:label "% of labor used in manufacturing, not used in direct activity"@en;
    rdfs:comment "Percent of labor used in manufacturing, not used in direct activity"@en;
    rdfs:isDefinedBy scor: ;
    vs:term_status "stable" ;
    dct:modified "2015-11-05"^^xsd:date ;
.

scor:hasMetricAG_3
    rdf:type owl:DatatypeProperty ;
    rdfs:subPropertyOf scor:hasAgilityMetric ;
    rdfs:domain [rdf:type owl:Class ;
        owl:unionOf (
        scor:DeliverReturnDefectiveProduct
        scor:DeliverReturnMROProduct
        scor:DeliverReturnExcessProduct
        )] ;
    rdfs:label "Additional deliver return volume"@en;
    rdfs:comment "Additional customer return volume"@en;
    rdfs:isDefinedBy scor: ;
    vs:term_status "stable" ;
    dct:modified "2015-11-05"^^xsd:date ;
.

scor:hasMetricAG_4
    rdf:type owl:DatatypeProperty ;
    rdfs:subPropertyOf scor:hasAgilityMetric ;
    rdfs:domain [rdf:type owl:Class ;
        owl:unionOf (
        scor:DeliverStockedProduct
        scor:DeliverMakeToOrderProduct
        scor:DeliverEngineerToOrderProduct
        )] ;
    rdfs:label "Additional Delivery volume"@en;
    rdfs:comment "Additional delivery volume"@en;
    rdfs:isDefinedBy scor: ;
    vs:term_status "stable" ;
    dct:modified "2015-11-05"^^xsd:date ;
.

#5-8 seem to be deprecated

scor:hasMetricAG_9
    rdf:type owl:DatatypeProperty ;
    rdfs:subPropertyOf scor:hasAgilityMetric ;
    rdfs:domain [rdf:type owl:Class ;
        owl:unionOf (
        scor:SourceStockedProduct
        scor:SourceMakeToOrderProduct
        scor:SourceEngineerToOrderProduct
        )] ;
    rdfs:label "Additional source volumes obtained in 30 days"@en;
    rdfs:comment "Additional source volume to be determined given ramped up resources"@en;
    rdfs:isDefinedBy scor: ;
    vs:term_status "stable" ;
    dct:modified "2015-11-05"^^xsd:date ;
.

#10-30 seem to be deprecated

scor:hasMetricAG_31
    rdf:type owl:DatatypeProperty ;
    rdfs:subPropertyOf scor:hasAgilityMetric ;
    rdfs:domain [rdf:type owl:Class ;
        owl:unionOf (
        scor:DeliverReturnDefectiveProduct
        scor:DeliverReturnMROProduct
        scor:DeliverReturnExcessProduct
        )] ;
    rdfs:label "Current Deliver Return Volume"@en;
    rdfs:comment "Current Return volume, number of orders returned"@en;
    rdfs:isDefinedBy scor: ;
    vs:term_status "stable" ;
    dct:modified "2015-11-05"^^xsd:date ;
.

scor:hasMetricAG_32
    rdf:type owl:DatatypeProperty ;
    rdfs:subPropertyOf scor:hasAgilityMetric ;
    rdfs:domain [rdf:type owl:Class ;
        owl:unionOf (
        scor:DeliverStockedProduct
        scor:DeliverMakeToOrderProduct
        scor:DeliverEngineerToOrderProduct
        scor:DeliverRetailProduct
        )] ;
    rdfs:label "Current Delivery Volume"@en;
    rdfs:comment "Number of orders shipped"@en;
    rdfs:isDefinedBy scor: ;
    vs:term_status "stable" ;
    dct:modified "2015-11-05"^^xsd:date ;
.

#33-37 seem to be deprecated

scor:hasMetricAG_38
    rdf:type owl:DatatypeProperty ;
    rdfs:subPropertyOf scor:hasAgilityMetric ;
    rdfs:domain [rdf:type owl:Class ;
        owl:unionOf (
        scor:MakeToStock
        scor:MakeToOrder
        scor:MakeEngineerToOrder
        )] ;
    rdfs:label "Current Make Volume"@en;
    rdfs:comment "Amount of each item which are manufactured"@en;
    rdfs:isDefinedBy scor: ;
    vs:term_status "stable" ;
    dct:modified "2015-11-05"^^xsd:date ;
.

#39 seem to be deprecated

scor:hasMetricAG_40
    rdf:type owl:DatatypeProperty ;
    rdfs:subPropertyOf scor:hasAgilityMetric ;
    rdfs:domain [rdf:type owl:Class ;
        owl:unionOf (
        scor:SourceStockedProduct
        scor:SourceMakeToOrderProduct
        scor:SourceEngineerToOrderProduct
        )] ;
    rdfs:label "Current Purchase Order Cycle Times"@en;
    rdfs:comment "Sum of time to place a purchase order and supplier lead time"@en;
    rdfs:isDefinedBy scor: ;
    vs:term_status "stable" ;
    dct:modified "2015-11-05"^^xsd:date ;
.

scor:hasMetricAG_41
    rdf:type owl:DatatypeProperty ;
    rdfs:subPropertyOf scor:hasAgilityMetric ;
    rdfs:domain [rdf:type owl:Class ;
        owl:unionOf (
        scor:SourceReturnDefectiveProduct
        )] ;
    rdfs:label "Current source return volume"@en;
    rdfs:comment "Current return volume, number of orders returned"@en;
    rdfs:isDefinedBy scor: ;
    vs:term_status "stable" ;
    dct:modified "2015-11-05"^^xsd:date ;
.

scor:hasMetricAG_42
    rdf:type owl:DatatypeProperty ;
    rdfs:subPropertyOf scor:hasAgilityMetric ;
    rdfs:domain [rdf:type owl:Class ;
        owl:unionOf (
        scor:SourceStockedProduct
        scor:SourceMakeToOrderProduct
        scor:SourceEngineerToOrderProduct
        )] ;
    rdfs:label "Current Source Volume"@en;
    rdfs:comment "Amount of each item which are purchased"@en;
    rdfs:isDefinedBy scor: ;
    vs:term_status "stable" ;
    dct:modified "2015-11-05"^^xsd:date ;
.
#43 seem to be deprecated

scor:hasMetricAG_44
    rdf:type owl:DatatypeProperty ;
    rdfs:subPropertyOf scor:hasAgilityMetric ;
    rdfs:domain [rdf:type owl:Class ;
        owl:unionOf (
        scor:DeliverReturnDefectiveProduct
        scor:DeliverReturnMROProduct
        scor:DeliverReturnExcessProduct
        )] ;
    rdfs:label "Customer return order cycle time reestablished and sustained in 30 days"@en;
    rdfs:comment "Customer return order cycle time reestablished and sustained for increased quantities returned from customer given 30 days, including customer return order processing cycle time, transit time, return processing and disposition cycle time, etc."@en;
    rdfs:isDefinedBy scor: ;
    vs:term_status "stable" ;
    dct:modified "2015-11-05"^^xsd:date ;
.

#45 seem to be deprecated

scor:hasMetricAG_46
    rdf:type owl:DatatypeProperty ;
    rdfs:subPropertyOf scor:hasAgilityMetric ;
    rdfs:domain [rdf:type owl:Class ;
        owl:unionOf (
        scor:SourceStockedProduct
        scor:SourceMakeToOrderProduct
        scor:SourceEngineerToOrderProduct
        )] ;
    rdfs:label "Demand sourcing-supplier constraints"@en;
    rdfs:comment "Percentage of orders with on time and accurate documentation supporting the order, including packing slips, bills of lading, invoices, etc. [Total number of orders delivered with correct and timely documentation] / [Total number of orders delivered] x 100%."@en;
    rdfs:isDefinedBy scor: ;
    vs:term_status "stable" ;
    dct:modified "2015-11-05"^^xsd:date ;
.


######### Cost Metrics

scor:hasMetricCO_1
    rdf:type owl:DatatypeProperty ;
    rdfs:subPropertyOf scor:hasCostMetric ;
    rdfs:domain [rdf:type owl:Class ;
        owl:unionOf (
        scor:PlanSupplyChain
        scor:PlanSource
        scor:PlanMake
        scor:PlanDeliver
        scor:PlanReturn
        scor:ManageSupplyChainHumanResources
        )] ;
    rdfs:label "Planning Labor Cost"@en;
    rdfs:comment "The costs associated with the personnel performing the tasks associated with supply and demand planning in support of operating the supply chain."@en;
    rdfs:isDefinedBy scor: ;
    vs:term_status "stable" ;
    dct:modified "2015-11-05"^^xsd:date ;
.

scor:hasMetricCO_2
    rdf:type owl:DatatypeProperty ;
    rdfs:subPropertyOf scor:hasCostMetric ;
    rdfs:domain [rdf:type owl:Class ;
        owl:unionOf (
        scor:PlanSupplyChain
        scor:PlanSource
        scor:PlanMake
        scor:PlanDeliver
        scor:PlanReturn
        scor:ManageDataAndInformation
        )] ;
    rdfs:label "Planning Automation Cost"@en;
    rdfs:comment "The costs associated with automation (software, hardware, maintenance and consumable materials) of supply chain processes."@en;
    rdfs:isDefinedBy scor: ;
    vs:term_status "stable" ;
    dct:modified "2015-11-05"^^xsd:date ;
.

scor:hasMetricCO_3
    rdf:type owl:DatatypeProperty ;
    rdfs:subPropertyOf scor:hasCostMetric ;
    rdfs:domain [rdf:type owl:Class ;
        owl:unionOf (
        scor:PlanSupplyChain
        scor:PlanSource
        scor:PlanMake
        scor:PlanDeliver
        scor:PlanReturn
        scor:ManageSupplyChainAssets
        )] ;
    rdfs:label "Planning Property, Plant, and Equipment Cost"@en;
    rdfs:comment "The costs associated with the (fixed) assets designated to support supply chain planning processes. PP&E costs include the cost of leases, rents, acquisition, depreciation, maintenance and disposition of land, buildings, and equipment and labor cost and expenses of internal and/or external maintenance and support staff."@en;
    rdfs:isDefinedBy scor: ;
    vs:term_status "stable" ;
    dct:modified "2015-11-05"^^xsd:date ;
.

scor:hasMetricCO_4
    rdf:type owl:DatatypeProperty ;
    rdfs:subPropertyOf scor:hasCostMetric ;
    rdfs:domain [rdf:type owl:Class ;
        owl:unionOf (
        scor:PlanSupplyChain
        scor:PlanSource
        scor:PlanMake
        scor:PlanDeliver
        scor:PlanReturn
        scor:ManageSupplyChainBusinessRules
        scor:ManagePerformance
        scor:ManageRegulatoryCompliance
        scor:ManageSupplyChainRisk
        )] ;
    rdfs:label "Planning GRC and Overhead Cost"@en;
    rdfs:comment "The governance, risk management, compliance and overhead costs allocated to supply chain planning processes. This may include cost of supporting organizations, e.g. Human Resources department, Legal department, Quality Department, as well as office supplies and other indirect cost."@en;
    rdfs:isDefinedBy scor: ;
    vs:term_status "stable" ;
    dct:modified "2015-11-05"^^xsd:date ;
.

scor:hasMetricCO_5
    rdf:type owl:DatatypeProperty ;
    rdfs:subPropertyOf scor:hasCostMetric ;
    rdfs:domain [rdf:type owl:Class ;
        owl:unionOf (
        scor:SourceStockedProduct
        scor:SourceMakeToOrderProduct
        scor:SourceEngineerToOrderProduct
        scor:GenerateStockingSchedule
        scor:ReceiveProductAtStore
        scor:PickProductFromBackroom
        scor:ManageSupplyChainHumanResources
        )] ;
    rdfs:label "Sourcing Labor Cost"@en;
    rdfs:comment "The labor costs associated with the personnel performing the ordering, receiving, processing and storing purchased materials."@en;
    rdfs:isDefinedBy scor: ;
    vs:term_status "stable" ;
    dct:modified "2015-11-05"^^xsd:date ;
.

scor:hasMetricCO_6
    rdf:type owl:DatatypeProperty ;
    rdfs:subPropertyOf scor:hasCostMetric ;
    rdfs:domain [rdf:type owl:Class ;
        owl:unionOf (
        scor:SourceStockedProduct
        scor:SourceMakeToOrderProduct
        scor:SourceEngineerToOrderProduct
        scor:ManageDataAndInformation
        )] ;
    rdfs:label "Sourcing Automation Cost"@en;
    rdfs:comment "The costs associated with the automation (software, hardware, maintenance and consumable materials) in support of the acquisition of materials and services."@en;
    rdfs:isDefinedBy scor: ;
    vs:term_status "stable" ;
    dct:modified "2015-11-05"^^xsd:date ;
.

scor:hasMetricCO_7
    rdf:type owl:DatatypeProperty ;
    rdfs:subPropertyOf scor:hasCostMetric ;
    rdfs:domain [rdf:type owl:Class ;
        owl:unionOf (
        scor:SourceStockedProduct
        scor:SourceMakeToOrderProduct
        scor:SourceEngineerToOrderProduct
        scor:ManageSupplyChainAssets
        )] ;
    rdfs:label "Sourcing Property, Plant and Equipment Cost"@en;
    rdfs:comment "The costs associated with the (fixed) assets designated to support the aquisition of materials, products, merchandise and services. PP&E costs include the cost of leases, rents, acquisition, depreciation, maintenance and disposition of land, buildings, and equipment and labor cost and expenses of internal and/or external maintenance and support staff."@en;
    rdfs:isDefinedBy scor: ;
    vs:term_status "stable" ;
    dct:modified "2015-11-05"^^xsd:date ;
.

scor:hasMetricCO_8
    rdf:type owl:DatatypeProperty ;
    rdfs:subPropertyOf scor:hasCostMetric ;
    rdfs:domain [rdf:type owl:Class ;
        owl:unionOf (
        scor:SourceStockedProduct
        scor:SourceMakeToOrderProduct
        scor:SourceEngineerToOrderProduct
        scor:GenerateStockingSchedule
        scor:ManageSupplyChainBusinessRules
        scor:ManagePerformance
        scor:ManageRegulatoryCompliance
        scor:ManageSupplyChainRisk
        )] ;
    rdfs:label "Sourcing GRC, Inventory and Overhead Cost"@en;
    rdfs:comment "The governnance, risk management, compliance, inventory and overhead costs allocated to aquisition processes (the ordering, receiving, inspecting, processing and storage of purchased materials, merchandise and services)."@en;    
    rdfs:isDefinedBy scor: ;
    vs:term_status "stable" ;
    dct:modified "2015-11-05"^^xsd:date ;
.

scor:hasMetricCO_9
    rdf:type owl:DatatypeProperty ;
    rdfs:subPropertyOf scor:hasCostMetric ;
    rdfs:domain [rdf:type owl:Class ;
        owl:unionOf (
        scor:SourceStockedProduct
        scor:SourceMakeToOrderProduct
        scor:SourceEngineerToOrderProduct
        scor:ManageSupplyChainContracts
        )] ;
    rdfs:label "Purchased Materials Cost"@en;
    rdfs:comment "The total cost of the materials, merchandise and services purchased to produce the final product or for resale. Purchased Materials Cost is reported at purchase price net of any discounts."@en;    
    rdfs:isDefinedBy scor: ;
    vs:term_status "stable" ;
    dct:modified "2015-11-05"^^xsd:date ;
.

scor:hasMetricCO_10
    rdf:type owl:DatatypeProperty ;
    rdfs:subPropertyOf scor:hasCostMetric ;
    rdfs:domain [rdf:type owl:Class ;
        owl:unionOf (
        scor:SourceStockedProduct
        scor:SourceMakeToOrderProduct
        scor:SourceEngineerToOrderProduct
        scor:ManageSupplyChainContracts
        scor:ManageSupplyChainNetworks
        )] ;
    rdfs:label "Material Transportation Cost"@en;
    rdfs:comment "The costs associated with the physical transportation of purchased materials to the location-of-use. Transportation costs include the transportation equipment ownership -- depreciation, equipment insurance, license and registration, financing -- and equipment operating costs (also known as the costs of driving): fuel, electricity, load insurance, maintenance and parking, tolls, and other trip specific costs."@en;     
    rdfs:isDefinedBy scor: ;
    vs:term_status "stable" ;
    dct:modified "2015-11-05"^^xsd:date ;
.

scor:hasMetricCO_11
    rdf:type owl:DatatypeProperty ;
    rdfs:subPropertyOf scor:hasCostMetric ;
    rdfs:domain [rdf:type owl:Class ;
        owl:unionOf (
        scor:SourceStockedProduct
        scor:SourceMakeToOrderProduct
        scor:SourceEngineerToOrderProduct
        scor:ManageSupplyChainContracts
        scor:ManageSupplyChainNetworks
        scor:ManageRegulatoryCompliance
        scor:ManageSupplyChainRisk
        )] ;
    rdfs:label "Material Customs, Duties, Taxes and Tariffs Cost"@en;
    rdfs:comment "The costs of import/export duties, taxes and tariffs, including the costs of third party services enabling customs, clearance."@en;    
    rdfs:isDefinedBy scor: ;
    vs:term_status "stable" ;
    dct:modified "2015-11-05"^^xsd:date ;
.

scor:hasMetricCO_12
    rdf:type owl:DatatypeProperty ;
    rdfs:subPropertyOf scor:hasCostMetric ;
    rdfs:domain [rdf:type owl:Class ;
        owl:unionOf (
        scor:SourceStockedProduct
        scor:SourceMakeToOrderProduct
        scor:SourceEngineerToOrderProduct
        scor:ManageSupplyChainBusinessRules
        scor:ManagePerformance
        scor:ManageSupplyChainNetworks
        scor:ManageRegulatoryCompliance
        scor:ManageSupplyChainRisk
        )] ;
    rdfs:label "Material Risk and Compliance Cost"@en;
    rdfs:comment "The costs associated with acquiring purchased materials (and services). Example costs included in Material Risk and Compliance Cost are: (1) Cost of theft, fraud, depreciation and shrinkage of in-transit goods (2) C-TPAT program costs (3) Carbon footprint mandate compliance costs (4) Cost of mitigation of potential risk of supply disruption (5) Cost of compliance to Health, Safety and Environmental legislation"@en;
    rdfs:isDefinedBy scor: ;
    vs:term_status "stable" ;
    dct:modified "2015-11-05"^^xsd:date ;
.

#13 seem to be deprecated

scor:hasMetricCO_14
    rdf:type owl:DatatypeProperty ;
    rdfs:subPropertyOf scor:hasCostMetric ;
    rdfs:domain [rdf:type owl:Class ;
        owl:unionOf (
        scor:MakeToStock
        scor:MakeToOrder
        scor:MakeEngineerToOrder
        scor:ManageSupplyChainHumanResources
        )] ;
    rdfs:label "Production (Direct) Labor Cost"@en;
    rdfs:comment "The total cost associated with the personnel performing the activities of Make (producing, manufacturing, re-manufacturing, refurbishment, MRO, repair, and/or recycling)."@en;
    rdfs:isDefinedBy scor: ;
    vs:term_status "stable" ;
    dct:modified "2015-11-05"^^xsd:date ;
.

scor:hasMetricCO_15
    rdf:type owl:DatatypeProperty ;
    rdfs:subPropertyOf scor:hasCostMetric ;
    rdfs:domain [rdf:type owl:Class ;
        owl:unionOf (
        scor:MakeToStock
        scor:MakeToOrder
        scor:MakeEngineerToOrder
        scor:ManageDataAndInformation
        )] ;
    rdfs:label "Production Automation Cost"@en;
    rdfs:comment "The costs associated with the automation (software, hardware, maintenance and consumable materials) of production processes."@en;    
    rdfs:isDefinedBy scor: ;
    vs:term_status "stable" ;
    dct:modified "2015-11-05"^^xsd:date ;
.

scor:hasMetricCO_16
    rdf:type owl:DatatypeProperty ;
    rdfs:subPropertyOf scor:hasCostMetric ;
    rdfs:domain [rdf:type owl:Class ;
        owl:unionOf (
        scor:MakeToStock
        scor:MakeToOrder
        scor:MakeEngineerToOrder
        scor:ManageSupplyChainAssets
        )] ;
    rdfs:label "Production Property, Plant, Equipment Cost"@en;
    rdfs:comment "The costs associated with the assets designated to support the production, manufacturing, assembly, remanufacturing, refurbishment, repair and overhaul of goods. PP&E costs include the cost of leases, rents, asquisition, depreciation, maintenance, and disposition of land, buildings, and eqipment and labor cost and expenses of internal maintenance and support staff."@en;    
    rdfs:isDefinedBy scor: ;
    vs:term_status "stable" ;
    dct:modified "2015-11-05"^^xsd:date ;
.

scor:hasMetricCO_17
    rdf:type owl:DatatypeProperty ;
    rdfs:subPropertyOf scor:hasCostMetric ;
    rdfs:domain [rdf:type owl:Class ;
        owl:unionOf (
        scor:MakeToStock
        scor:MakeToOrder
        scor:MakeEngineerToOrder
        scor:ManageSupplyChainBusinessRules
        scor:ManagePerformance
        scor:ManageRegulatoryCompliance
        scor:ManageSupplyChainRisk
        )] ;
    rdfs:label "Production GRC, Inventory and Overhead Cost"@en;
    rdfs:comment "The governance, risk management, compliance, inventory and overhead costs allocated to the production processes (manufacturing, re-manufacturing, refurbishment, repairs, maintenance, and overhaul)."@en;
    rdfs:isDefinedBy scor: ;
    vs:term_status "stable" ;
    dct:modified "2015-11-05"^^xsd:date ;
.

scor:hasMetricCO_18
    rdf:type owl:DatatypeProperty ;
    rdfs:subPropertyOf scor:hasCostMetric ;
    rdfs:domain [rdf:type owl:Class ;
        owl:unionOf (
        scor:DeliverStockedProduct
        scor:ProcessInquiryQuote
        scor:DSPConsolidateOrders
        scor:DSPBuildLoads
        scor:DSPRouteShipments
        scor:DSPSelectCarriersRateShipments
        scor:DSPInvoice
        scor:DeliverMakeToOrderProduct
        scor:DMOPInquiryQuote
        scor:DMOPReceiveVerifyProductByCustomer
        scor:DMOPReserveInventoryDetermineDeliveryDate
        scor:DMOPConsolidateOrders
        scor:DMOPBuildLoads
        scor:DMOPRouteShipments
        scor:DMOPSelectCarriersRateShipments
        scor:DMOPInvoice
        scor:ObtainRespondToRFPRFQ
        scor:NegotiateReceiveContract
        scor:EnterOrderCommitResourcesLaunchProgram
        scor:ScheduleInstallation
        scor:DEOPBuildLoads
        scor:DEOPRouteShipments
        scor:DEOPSelectCarriersRateShipments
        scor:DEOPInvoice
        scor:DeliverRetailProduct
        scor:Checkout
        scor:ManageSupplyChainHumanResources
        )] ;
    rdfs:label "Order Management Labor Cost"@en;
    rdfs:comment "The costs associated with the personnel performing the order management tasks of customer order entry, maintenance and scheduling of deliveries."@en;
    rdfs:isDefinedBy scor: ;
    vs:term_status "stable" ;
    dct:modified "2015-11-05"^^xsd:date ;
.

scor:hasMetricCO_19
    rdf:type owl:DatatypeProperty ;
    rdfs:subPropertyOf scor:hasCostMetric ;
    rdfs:domain [rdf:type owl:Class ;
        owl:unionOf (
        scor:DeliverStockedProduct
        scor:DeliverMakeToOrderProduct
        scor:DeliverEngineerToOrderProduct
        scor:DeliverRetailProduct
        scor:ManageDataAndInformation
        )] ;
    rdfs:label "Order Management Automation Cost"@en;
    rdfs:comment "The costs associated with the automation (software, hardware, maintenance and consumable materials) of order management processes."@en; 
    rdfs:isDefinedBy scor: ;
    vs:term_status "stable" ;
    dct:modified "2015-11-05"^^xsd:date ;
.

scor:hasMetricCO_20
    rdf:type owl:DatatypeProperty ;
    rdfs:subPropertyOf scor:hasCostMetric ;
    rdfs:domain [rdf:type owl:Class ;
        owl:unionOf (
        scor:DeliverStockedProduct
        scor:DeliverMakeToOrderProduct
        scor:DeliverEngineerToOrderProduct
        scor:DeliverRetailProduct
        scor:ManageSupplyChainAssets
        )] ;
    rdfs:label "Order Management Property, Plant and Equipment Cost"@en;
    rdfs:comment "The costs associated with the (fixed) assets designated to support order management processes. PP&E costs include the cost of leases, rents, aquisition, depreciation, maintenance and disposition of land, buildings and equipment and labor cost and expenses of internal and/or external maintenance and support staff."@en;
    rdfs:isDefinedBy scor: ;
    vs:term_status "stable" ;
    dct:modified "2015-11-05"^^xsd:date ;
.

scor:hasMetricCO_21
    rdf:type owl:DatatypeProperty ;
    rdfs:subPropertyOf scor:hasCostMetric ;
    rdfs:domain [rdf:type owl:Class ;
        owl:unionOf (
        scor:DeliverStockedProduct
        scor:DeliverMakeToOrderProduct
        scor:DeliverEngineerToOrderProduct
        scor:DeliverRetailProduct
        scor:ManageSupplyChainBusinessRules
        scor:ManagePerformance
        scor:ManageRegulatoryCompliance
        scor:ManageSupplyChainRisk
        )] ;
    rdfs:label "Order Management GRC, Inventory and Overhead Cost"@en;
    rdfs:comment "The governance, risk management, compliance, inventory and overhead costs allocated to order management processes (managing customer data, entry, maintenance, scheduling, prioritizion, and expedition of customer orders, invoicing and collections)."@en;
    rdfs:isDefinedBy scor: ;
    vs:term_status "stable" ;
    dct:modified "2015-11-05"^^xsd:date ;
.

scor:hasMetricCO_22
    rdf:type owl:DatatypeProperty ;
    rdfs:subPropertyOf scor:hasCostMetric ;
    rdfs:domain [rdf:type owl:Class ;
        owl:unionOf (
        scor:DeliverStockedProduct
        scor:DSPConsolidateOrders
        scor:DSPBuildLoads
        scor:DSPRouteShipments
        scor:DSPSelectCarriersRateShipments
        scor:DSPShipProduct
        scor:DeliverMakeToOrderProduct
        scor:DMOPConsolidateOrders
        scor:DMOPBuildLoads
        scor:DMOPSelectCarriersRateShipments
        scor:DMOPShipProduct
        scor:DeliverEngineerToOrderProduct
        scor:ScheduleInstallation
        scor:DEOPBuildLoads
        scor:DEOPRouteShipments
        scor:DEOPSelectCarriersRateShipments
        scor:DEOPShipProduct
        scor:DeliverRetailProduct
        scor:DeliverInstall
        scor:ReturnDefectiveProduct
        scor:ReturnMROPRoduct
        scor:ReturnExcessProduct
        scor:ManageSupplyChainContracts
        scor:ManageSupplyChainNetworks
        )] ;
    rdfs:label "Transportation Cost"@en;
    rdfs:comment "The costs associated with the physical transportation of goods between supply chain nodes."@en;
    rdfs:isDefinedBy scor: ;
    vs:term_status "stable" ;
    dct:modified "2015-11-05"^^xsd:date ;
.

scor:hasMetricCO_23
    rdf:type owl:DatatypeProperty ;
    rdfs:subPropertyOf scor:hasCostMetric ;
    rdfs:domain [rdf:type owl:Class ;
        owl:unionOf (
        scor:DeliverStockedProduct
        scor:DeliverMakeToOrderProduct
        scor:DeliverEngineerToOrderProduct
        scor:DeliverRetailProduct
        scor:ManageSupplyChainNetworks
        scor:ManageRegulatoryCompliance
        scor:ManageSupplyChainRisk
        )] ;
    rdfs:label "Fulfillment Customs, Duties, Taxes and Tariffs Cost"@en;
    rdfs:comment "The costs of import/export duties, taxes and tariffs, including the costs of third party services enabling customs, clearance. Internal personnel cost related to customs and duties are reported in the Order Management Labor Cost and should therefore not be reported in the Customs and Duties Cost."@en;    
    rdfs:isDefinedBy scor: ;
    vs:term_status "stable" ;
    dct:modified "2015-11-05"^^xsd:date ;
.

scor:hasMetricCO_24
    rdf:type owl:DatatypeProperty ;
    rdfs:subPropertyOf scor:hasCostMetric ;
    rdfs:domain [rdf:type owl:Class ;
        owl:unionOf (
        scor:DeliverStockedProduct
        scor:DSPReceiveProductFromSourceMake
        scor:DSPPickProduct
        scor:DSPPackProduct
        scor:LoadVehicleGenerateShippingDocuments
        scor:DSPShipProduct
        scor:DeliverMakeToOrderProduct
        scor:DMOPRouteShipments
        scor:DMOPReceiveProductFromSourceMake
        scor:DMOPPickProduct
        scor:DMOPPackProduct
        scor:DMOPLoadProductGenerateShippingDocs
        scor:DMOPShipProduct
        scor:DeliverEngineerToOrderProduct
        scor:DEOPReceiveProductFromSourceMake
        scor:DEOPPickProduct
        scor:DEOPPackProduct
        scor:DEOPLoadProductGenerateShippingDocs
        scor:DEOPShipProduct
        scor:DeliverRetailProduct
        scor:StockShelf
        scor:FillShoppingCart
        scor:DeliverInstall
        scor:ManageSupplyChainHumanResources
        )] ;
    rdfs:label "Fulfillment Labor Cost"@en;
    rdfs:comment "The costs associated with the personnel performing the order fulfillment tasks of picking, packing and shipping."@en;
    rdfs:isDefinedBy scor: ;
    vs:term_status "stable" ;
    dct:modified "2015-11-05"^^xsd:date ;
.

scor:hasMetricCO_25
    rdf:type owl:DatatypeProperty ;
    rdfs:subPropertyOf scor:hasCostMetric ;
    rdfs:domain [rdf:type owl:Class ;
        owl:unionOf (
        scor:DeliverStockedProduct
        scor:DeliverMakeToOrderProduct
        scor:DeliverEngineerToOrderProduct
        scor:DeliverRetailProduct
        scor:ManageDataAndInformation
        )] ;
    rdfs:label "Fulfillment Automation Cost"@en;
    rdfs:comment "The costs associated with the automation (software, hardware, maintenance and consumable materials) of phyiscal order fulfillment."@en; 
    rdfs:isDefinedBy scor: ;
    vs:term_status "stable" ;
    dct:modified "2015-11-05"^^xsd:date ;
.

scor:hasMetricCO_26
    rdf:type owl:DatatypeProperty ;
    rdfs:subPropertyOf scor:hasCostMetric ;
    rdfs:domain [rdf:type owl:Class ;
        owl:unionOf (
        scor:DeliverStockedProduct
        scor:DeliverMakeToOrderProduct
        scor:DeliverEngineerToOrderProduct
        scor:DeliverRetailProduct
        scor:ManageSupplyChainAssets
        )] ;
    rdfs:label "Fulfillment Property, Plant and Equipment Cost"@en;
    rdfs:comment "The costs associated with the (fixed) assets designated to support fulfillment of customer oders. PP&E costs include the cost of leases, rents, aquisition, depreciation, maintenance and disposition of land, buildings and equipment and labor cost and expenses of internal and/or external maintenance and support staff."@en;
    rdfs:isDefinedBy scor: ;
    vs:term_status "stable" ;
    dct:modified "2015-11-05"^^xsd:date ;
.

scor:hasMetricCO_27
    rdf:type owl:DatatypeProperty ;
    rdfs:subPropertyOf scor:hasCostMetric ;
    rdfs:domain [rdf:type owl:Class ;
        owl:unionOf (
        scor:DeliverStockedProduct
        scor:DeliverMakeToOrderProduct
        scor:DeliverEngineerToOrderProduct
        scor:DeliverRetailProduct
        scor:ManageSupplyChainBusinessRules
        scor:ManagePerformance
        scor:ManageRegulatoryCompliance
        scor:ManageSupplyChainRisk
        )] ;
    rdfs:label "Fulfillment GRC, Inventory and Overhead Cost"@en;
    rdfs:comment "The governance, risk management, compliance, inventory and overhead costs allocated to the fulfillment processes to customer orders (phyiscal handling of the product, such as storage, picking, packing and shipping)."@en;
    rdfs:isDefinedBy scor: ;
    vs:term_status "stable" ;
    dct:modified "2015-11-05"^^xsd:date ;
.

scor:hasMetricCO_28
    rdf:type owl:DatatypeProperty ;
    rdfs:subPropertyOf scor:hasCostMetric ;
    rdfs:domain [rdf:type owl:Class ;
        owl:unionOf (
        scor:DeliverReturnDefectiveProduct
        scor:AuthorizeDefectiveProductReturn
        scor:DeliverReturnExcessProduct
        scor:AuthorizeExcessProductReturn
        )] ;
    rdfs:label "Discounts and Refunds Cost"@en;
    rdfs:comment "The costs associated with the settlement of a return or defect claim. This may include the net cost of discounts offered for damaged goods, refunding of purchase price for returned goods."@en;
    rdfs:isDefinedBy scor: ;
    vs:term_status "stable" ;
    dct:modified "2015-11-05"^^xsd:date ;
.


scor:hasMetricCO_29
    rdf:type owl:DatatypeProperty ;
    rdfs:subPropertyOf scor:hasCostMetric ;
    rdfs:domain [rdf:type owl:Class ;
        owl:unionOf (
        scor:SourceReturnDefectiveProduct
        scor:DispositionDefectiveProduct
        scor:DeliverReturnDefectiveProduct
        scor:AuthorizeDefectiveProductReturn
        scor:DispositionMROProduct
        scor:SourceReturnExcessProduct
        scor:DispositionExcessProduct
        scor:DeliverReturnExcessProduct
        scor:AuthorizeExcessProductReturn
        )] ;
    rdfs:label "Disposition Cost"@en;
    rdfs:comment "The costs associated with the settlement of a return or defect claim. This may include the net cost of discounts offered for damaged goods, refunding of purchase price for returned goods."@en;
    rdfs:isDefinedBy scor: ;
    vs:term_status "stable" ;
    dct:modified "2015-11-05"^^xsd:date ;
.

scor:hasMetricCO_30
    rdf:type owl:DatatypeProperty ;
    rdfs:subPropertyOf scor:hasCostMetric ;
    rdfs:domain [rdf:type owl:Class ;
        owl:unionOf (
        scor:SourceReturnDefectiveProduct
        scor:ReturnMROPRoduct
        scor:SourceReturnExcessProduct
        scor:DeliverReturnExcessProduct
        )] ;
    rdfs:label "Return GRC, Inventory and Overhead Cost"@en;
    rdfs:comment "The governance, risk management, compliance, inventory and overhead costs allocated to return processes."@en;
    rdfs:isDefinedBy scor: ;
    vs:term_status "stable" ;
    dct:modified "2015-11-05"^^xsd:date ;
.

######### Asset Management Efficiency Metrics

#1 seems to be deprecated

scor:hasMetricAM_2
    rdf:type owl:DatatypeProperty ;
    rdfs:subPropertyOf scor:hasAssetManagemenEfficiencyMetric ;
    rdfs:domain [rdf:type owl:Class ;
        owl:unionOf (
        scor:IdentifySourcesOfSupply
        )] ;
    rdfs:label "% of material that has a valid"@en;
    rdfs:comment "% of the product content that has a supplier take- back program for recycling or reuse."@en;    
    rdfs:isDefinedBy scor: ;
    vs:term_status "stable" ;
    dct:modified "2015-11-05"^^xsd:date ;
.

scor:hasMetricAM_3
    rdf:type owl:DatatypeProperty ;
    rdfs:subPropertyOf scor:hasAssetManagemenEfficiencyMetric ;
    rdfs:domain [rdf:type owl:Class ;
        owl:unionOf (
        scor:IdentifySourcesOfSupply
        )] ;
    rdfs:label "% of materials that are recyclable/ reusable"@en;
    rdfs:comment "% of the product content that is recyclable or reusable"@en;
    rdfs:isDefinedBy scor: ;
    vs:term_status "stable" ;
    dct:modified "2015-11-05"^^xsd:date ;
.

scor:hasMetricAM_4
    rdf:type owl:DatatypeProperty ;
    rdfs:subPropertyOf scor:hasAssetManagemenEfficiencyMetric ;
    rdfs:domain [rdf:type owl:Class ;
        owl:unionOf (
        scor:MOPackage
        )] ;
    rdfs:label "% of packaging/shipping materials reused internally"@en;
    rdfs:comment "The percent of scrap from packaging that is immediately reused in the packaging process"@en;
    rdfs:isDefinedBy scor: ;
    vs:term_status "stable" ;
    dct:modified "2015-11-05"^^xsd:date ;
.

scor:hasMetricAM_5
    rdf:type owl:DatatypeProperty ;
    rdfs:subPropertyOf scor:hasAssetManagemenEfficiencyMetric ;
    rdfs:domain [rdf:type owl:Class ;
        owl:unionOf (
        scor:MSProduceTest
        scor:MOProduceTest
        scor:MEOProduceTest
        )] ;
    rdfs:label "% of production materials reused"@en;
    rdfs:comment "The percent of scrap from production that is immediately reused in the production process"@en;    
    rdfs:isDefinedBy scor: ;
    vs:term_status "stable" ;
    dct:modified "2015-11-05"^^xsd:date ;
.

scor:hasMetricAM_6
    rdf:type owl:DatatypeProperty ;
    rdfs:subPropertyOf scor:hasAssetManagemenEfficiencyMetric ;
    rdfs:domain [rdf:type owl:Class ;
        owl:unionOf (
        scor:MSProduceTest
        scor:MOProduceTest
        scor:MEOProduceTest
        )] ;
    rdfs:label "% of products consisting of previously used components"@en;
    rdfs:comment "the weight of recycled material in the product as a percent of total product weight"@en;  
    rdfs:isDefinedBy scor: ;
    vs:term_status "stable" ;
    dct:modified "2015-11-05"^^xsd:date ;
.

#7 seems to be deprecated

scor:hasMetricAM_8
    rdf:type owl:DatatypeProperty ;
    rdfs:subPropertyOf scor:hasAssetManagemenEfficiencyMetric ;
    rdfs:domain [rdf:type owl:Class ;
        owl:unionOf (
        scor:SourceReturnExcessProduct
        )] ;
    rdfs:label "Average age of Excess Inventory"@en;
    rdfs:comment "Average age of Excess Inventory in days"@en;
    rdfs:isDefinedBy scor: ;
    vs:term_status "stable" ;
    dct:modified "2015-11-05"^^xsd:date ;
.

scor:hasMetricAM_9
    rdf:type owl:DatatypeProperty ;
    rdfs:subPropertyOf scor:hasAssetManagemenEfficiencyMetric ;
    rdfs:domain [rdf:type owl:Class ;
        owl:unionOf (
        scor:MSScheduleProductionActivities
        scor:MSProduceTest
        scor:MSPackage
        scor:MOScheduleProductionActivities
        scor:MOProduceTest
        scor:MOPackage
        scor:MEOScheduleProductionActivities
        scor:MEOProduceTest
        scor:MEOPackage
        scor:ManageSupplyChainHumanResources
        scor:ManageSupplyChainAssets
        )] ;
    rdfs:label "Capacity Utilization"@en;
    rdfs:comment "A measure of how intensively a resource is being used to produce a good or service. Some factors that should be considered are internal manufacturing capacity, constraining processes,direct labor availability and key components/ materials availability."@en;  
    rdfs:isDefinedBy scor: ;
    vs:term_status "stable" ;
    dct:modified "2015-11-05"^^xsd:date ;
.

#10-11 seem to be deprecated

scor:hasMetricAM_12
    rdf:type owl:DatatypeProperty ;
    rdfs:subPropertyOf scor:hasAssetManagemenEfficiencyMetric ;
    rdfs:domain [rdf:type owl:Class ;
        owl:unionOf (
        scor:DeliverReturnDefectiveProduct
        scor:DeliverReturnMROProduct
        )] ;
    rdfs:label "Deliver Return Cycle Time"@en;
    rdfs:comment "The average time associated with returns."@en;
    rdfs:isDefinedBy scor: ;
    vs:term_status "stable" ;
    dct:modified "2015-11-05"^^xsd:date ;
.

#13 seem to be deprecated

scor:hasMetricAM_14
    rdf:type owl:DatatypeProperty ;
    rdfs:subPropertyOf scor:hasAssetManagemenEfficiencyMetric ;
    rdfs:domain [rdf:type owl:Class ;
        owl:unionOf (
        scor:MSProduceTest
        scor:MOProduceTest
        scor:MEOProduceTest
        )] ;
    rdfs:label "Hazardous materials used during production process as a % of all materials"@en;
    rdfs:comment "The % of material (by weight) issued for production that is classified as hazardous material"@en;
    rdfs:isDefinedBy scor: ;
    vs:term_status "stable" ;
    dct:modified "2015-11-05"^^xsd:date ;
.

scor:hasMetricAM_15
    rdf:type owl:DatatypeProperty ;
    rdfs:subPropertyOf scor:hasAssetManagemenEfficiencyMetric ;
    rdfs:domain [rdf:type owl:Class ;
        owl:unionOf (
        scor:MSWasteDisposal
        scor:MOWasteDisposal
        scor:MEOWasteDisposal
        )] ;
    rdfs:label "Hazardous waste as % of total waste"@en;
    rdfs:comment "The % of waste (by weight) generated from production that is classified as hazardous material"@en;
    rdfs:isDefinedBy scor: ;
    vs:term_status "stable" ;
    dct:modified "2015-11-05"^^xsd:date ;
.

scor:hasMetricAM_16
    rdf:type owl:DatatypeProperty ;
    rdfs:subPropertyOf scor:hasAssetManagemenEfficiencyMetric ;
    rdfs:domain [rdf:type owl:Class ;
        owl:unionOf (
        scor:SourceStockedProduct
        scor:SourceMakeToOrderProduct
        scor:SourceEngineerToOrderProduct
        )] ;
    rdfs:label "Inventory Days of Supply - Raw Material"@en;
    rdfs:comment "Value of raw materials / (COGS / 365) in days."@en;
    rdfs:isDefinedBy scor: ;
    vs:term_status "stable" ;
    dct:modified "2015-11-05"^^xsd:date ;
.

scor:hasMetricAM_17
    rdf:type owl:DatatypeProperty ;
    rdfs:subPropertyOf scor:hasAssetManagemenEfficiencyMetric ;
    rdfs:domain [rdf:type owl:Class ;
        owl:unionOf (
        scor:MakeToOrder
        scor:MakeEngineerToOrder
        scor:DeliverStockedProduct
        scor:DeliverMakeToOrderProduct
        scor:DeliverEngineerToOrderProduct
        )] ;
    rdfs:label "Inventory Days of Supply - WIP"@en;
    rdfs:comment "Total value of Work in Process / (COGS / 365) in days. WIP = Work In Process."@en;
    rdfs:isDefinedBy scor: ;
    vs:term_status "stable" ;
    dct:modified "2015-11-05"^^xsd:date ;
.

#18 seem to be deprecated

scor:hasMetricAM_19
    rdf:type owl:DatatypeProperty ;
    rdfs:subPropertyOf scor:hasAssetManagemenEfficiencyMetric ;
    rdfs:domain [rdf:type owl:Class ;
        owl:unionOf (
        scor:IssueMaterial
        scor:IssueSourcedInProcessProduct
        scor:MEOSourcedInProcessProduct
        )] ;
    rdfs:label "Packaging as % of total material"@en;
    rdfs:comment "The % by weight of packaging material to total raw material weight"@en;
    rdfs:isDefinedBy scor: ;
    vs:term_status "stable" ;
    dct:modified "2015-11-05"^^xsd:date ;
.

#20 seem to be deprecated

scor:hasMetricAM_21
    rdf:type owl:DatatypeProperty ;
    rdfs:subPropertyOf scor:hasAssetManagemenEfficiencyMetric ;
    rdfs:domain [rdf:type owl:Class ;
        owl:unionOf (
        scor:SourceReturnDefectiveProduct
        scor:ReturnDefectiveProduct
        scor:SourceReturnMROProduct
        )] ;
    rdfs:label "Rebuild or recycle rate"@en;
    rdfs:comment "Number of returned products that are rebuilt or recycled as a percent of the total number of products returned"@en;
    rdfs:isDefinedBy scor: ;
    vs:term_status "stable" ;
    dct:modified "2015-11-05"^^xsd:date ;
.

scor:hasMetricAM_22
    rdf:type owl:DatatypeProperty ;
    rdfs:subPropertyOf scor:hasAssetManagemenEfficiencyMetric ;
    rdfs:domain [rdf:type owl:Class ;
        owl:unionOf (
        scor:MakeToOrder
        scor:MakeToOrder
        scor:MakeEngineerToOrder
        )] ;
    rdfs:label "Recyclable waste as % of total waste"@en;
    rdfs:comment "The % of waste (by weight) generated from production that is recyclable."@en;
    rdfs:isDefinedBy scor: ;
    vs:term_status "stable" ;
    dct:modified "2015-11-05"^^xsd:date ;
.

#23-24 seem to be deprecated

scor:hasMetricAM_25
    rdf:type owl:DatatypeProperty ;
    rdfs:subPropertyOf scor:hasAssetManagemenEfficiencyMetric ;
    rdfs:domain [rdf:type owl:Class ;
        owl:unionOf (
        scor:DeliverReturnExcessProduct
        )] ;
    rdfs:label "Return for Recycle Rate"@en;
    rdfs:comment "Number of returns that are for recycling or re use as a per cent of the total number of products returned"@en;
    rdfs:isDefinedBy scor: ;
    vs:term_status "stable" ;
    dct:modified "2015-11-05"^^xsd:date ;
.

scor:hasMetricAM_26
    rdf:type owl:DatatypeProperty ;
    rdfs:subPropertyOf scor:hasAssetManagemenEfficiencyMetric ;
    rdfs:domain [rdf:type owl:Class ;
        owl:unionOf (
        scor:DeliverReturnDefectiveProduct
        )] ;
    rdfs:label "Return Rate"@en;
    rdfs:comment "Weight of products returned divided by the weight of product shipped"@en;
    rdfs:isDefinedBy scor: ;
    vs:term_status "stable" ;
    dct:modified "2015-11-05"^^xsd:date ;
.

#27 seem to be deprecated

scor:hasMetricAM_28
    rdf:type owl:DatatypeProperty ;
    rdfs:subPropertyOf scor:hasAssetManagemenEfficiencyMetric ;
    rdfs:domain [rdf:type owl:Class ;
        owl:unionOf (
        scor:SourceReturnDefectiveProduct
        scor:DeliverReturnDefectiveProduct
        )] ;
    rdfs:label "Percentage Defencitve Inventory"@en;
    rdfs:comment "The value of defective product inventory as a percentage of the value of total inventory (%) Calculation [Total Defective Product Inventory Value] / [Total Inventory Value] x 100%"@en;
    rdfs:isDefinedBy scor: ;
    vs:term_status "stable" ;
    dct:modified "2015-11-05"^^xsd:date ;
.

scor:hasMetricAM_29
    rdf:type owl:DatatypeProperty ;
    rdfs:subPropertyOf scor:hasAssetManagemenEfficiencyMetric ;
    rdfs:domain [rdf:type owl:Class ;
        owl:unionOf (
        scor:IdentifyDefectiveProductCondition
        scor:DispositionDefectiveProduct
        scor:DispositionMROProduct
        )] ;
    rdfs:label "Percentage Defective Inventory in Disposition"@en;
    rdfs:comment "The value of defective product awaiting a disposition decision as a percentage of the value of the total defective product inventory (%) Calculation [Value of Defective Inventory in Disposition Stage] / [Total Inventory Value] x 100%"@en;    
    rdfs:isDefinedBy scor: ;
    vs:term_status "stable" ;
    dct:modified "2015-11-05"^^xsd:date ;
.

scor:hasMetricAM_30
    rdf:type owl:DatatypeProperty ;
    rdfs:subPropertyOf scor:hasAssetManagemenEfficiencyMetric ;
    rdfs:domain [rdf:type owl:Class ;
        owl:unionOf (
        scor:RequestDefectiveProductReturnAuthorization
        )] ;
    rdfs:label "Percentage Defective Inventory in Return Authorization"@en;
    rdfs:comment "The value of defective product awaiting return authorization as a percentage of the total defectiv product inventory value (%) Calculation [Value of Defective Product Inventory in Request Return Authorization Stage] / [Total Defective Product Inventory Value] x 100%"@en;    rdfs:isDefinedBy scor: ;
    vs:term_status "stable" ;
    dct:modified "2015-11-05"^^xsd:date ;
.

scor:hasMetricAM_31
    rdf:type owl:DatatypeProperty ;
    rdfs:subPropertyOf scor:hasAssetManagemenEfficiencyMetric ;
    rdfs:domain [rdf:type owl:Class ;
        owl:unionOf (
        scor:ReturnDefectiveProduct
        )] ;
    rdfs:label "Percentage Defective Inventory in Return Transportation"@en;
    rdfs:comment "The value of defective product inventory in transportation as a percentage of total defective product inventory (%) Calculation [Value of Defective Product Inventory in Physical Return and Transportation Stage] / [Total Defective Product Inventory Value] x 100%"@en;    
    vs:term_status "stable" ;
    dct:modified "2015-11-05"^^xsd:date ;
.

scor:hasMetricAM_32
    rdf:type owl:DatatypeProperty ;
    rdfs:subPropertyOf scor:hasAssetManagemenEfficiencyMetric ;
    rdfs:domain [rdf:type owl:Class ;
        owl:unionOf (
        scor:ScheduleDefectiveProductShipment
        )] ;
    rdfs:label "Percentage Defective Product Inventory in Scheduling"@en;
    rdfs:comment "he value of defective product inventory awaiting scheduling as a percentage of the total defective product inventory value (%) Calculation [Value of Defective Product in Scheduling Stage] / [Total Defective Product Inventory Value] x 100%"@en;    
    vs:term_status "stable" ;
    dct:modified "2015-11-05"^^xsd:date ;
.

scor:hasMetricAM_33
    rdf:type owl:DatatypeProperty ;
    rdfs:subPropertyOf scor:hasAssetManagemenEfficiencyMetric ;
    rdfs:domain [rdf:type owl:Class ;
        owl:unionOf (
        scor:SourceReturnExcessProduct
        )] ;
    rdfs:label "Percentage Excess Inventory in Disposition"@en;
    rdfs:comment "Inventory Awaiting Return in the disposition decision stage. Calculation [Excess Inventory in Disposition Stage] / [Total Inventory Value] x 100%"@en;    
    vs:term_status "stable" ;
    dct:modified "2015-11-05"^^xsd:date ;
.

scor:hasMetricAM_34
    rdf:type owl:DatatypeProperty ;
    rdfs:subPropertyOf scor:hasAssetManagemenEfficiencyMetric ;
    rdfs:domain [rdf:type owl:Class ;
        owl:unionOf (
        scor:ReturnExcessProduct
        )] ;
    rdfs:label "Percentage Excess Inventory in Transportation"@en;
    rdfs:comment "Excess process in physcial return and transportation stage as a percentage of total excess product inventory (%) Calculation [Value of excess product inventory in physcial return and transportation stage] / [Total excess inventory value] x 100%"@en;    
    vs:term_status "stable" ;
    dct:modified "2015-11-05"^^xsd:date ;
.

scor:hasMetricAM_35
    rdf:type owl:DatatypeProperty ;
    rdfs:subPropertyOf scor:hasAssetManagemenEfficiencyMetric ;
    rdfs:domain [rdf:type owl:Class ;
        owl:unionOf (
        scor:RequestExcessProductReturnAuthorization
        )] ;
    rdfs:label "Percentage Excess Inventory in Request Return Authorization"@en;
    rdfs:comment "Inventory Awaiting Return Authorization (%) Calculation [Value of excess product in request return authorization stage] / [Value of total excess inventory] x 100%"@en;    
    vs:term_status "stable" ;
    dct:modified "2015-11-05"^^xsd:date ;
.

scor:hasMetricAM_36
    rdf:type owl:DatatypeProperty ;
    rdfs:subPropertyOf scor:hasAssetManagemenEfficiencyMetric ;
    rdfs:domain [rdf:type owl:Class ;
        owl:unionOf (
        scor:IdentifyExcessProductCondition
        )] ;
    rdfs:label "Percentage Excess Inventory in Identification"@en;
    rdfs:comment "Inventory awaiting return in the identification stage as a percentage of total excess inventory (%) Calculation [Value of Excess Inventory in Identification Stage] / [Total Inventory Value] x 100%"@en;    
    vs:term_status "stable" ;
    dct:modified "2015-11-05"^^xsd:date ;
.

scor:hasMetricAM_37
    rdf:type owl:DatatypeProperty ;
    rdfs:subPropertyOf scor:hasAssetManagemenEfficiencyMetric ;
    rdfs:domain [rdf:type owl:Class ;
        owl:unionOf (
        scor:SourceReturnExcessProduct
        scor:DeliverReturnExcessProduct
        )] ;
    rdfs:label "Percentage Excess Inventory"@en;
    vs:term_status "stable" ;
    dct:modified "2015-11-05"^^xsd:date ;
.

scor:hasMetricAM_38
    rdf:type owl:DatatypeProperty ;
    rdfs:subPropertyOf scor:hasAssetManagemenEfficiencyMetric ;
    rdfs:domain [rdf:type owl:Class ;
        owl:unionOf (
        scor:ScheduleExcessProductShipment
        )] ;
    rdfs:label "Percentage Excess Inventory in Scheduling"@en;
    rdfs:comment "Percentage of excess inventory awaiting scheduling the return (%) Calculation [Value of Excess Product Inventory in Scheduling Stage] / [Total Excess Product Inventory Value] x 100%"@en;    
    vs:term_status "stable" ;
    dct:modified "2015-11-05"^^xsd:date ;
.

scor:hasMetricAM_39
    rdf:type owl:DatatypeProperty ;
    rdfs:subPropertyOf scor:hasAssetManagemenEfficiencyMetric ;
    rdfs:domain [rdf:type owl:Class ;
        owl:unionOf (
        scor:DispositionMROProduct
        scor:DeliverReturnMROProduct
        )] ;
    rdfs:label "Percentage Unserviceable MRO Inventory in Disposition"@en;
    rdfs:comment "The value of unserviceable MRO Inventory in disposition stage as a percentage of total MRO inventory value (%) Calculation [Value of Unserviceable MRO Inventory in Disposition Stage] /[ Total MRO Inventory Value] x 100%"@en;    
    vs:term_status "stable" ;
    dct:modified "2015-11-05"^^xsd:date ;
.

scor:hasMetricAM_40
    rdf:type owl:DatatypeProperty ;
    rdfs:subPropertyOf scor:hasAssetManagemenEfficiencyMetric ;
    rdfs:domain [rdf:type owl:Class ;
        owl:unionOf (
        scor:ReturnMROPRoduct
        )] ;
    rdfs:label "Percentage Unserviceable MRO Inventory in Disposition"@en;
    rdfs:comment "The value of unserviceable MRO inventory in transportation as a percentage of the total MRO inventory value (%) Calculation [Value of Unserviceable MRO Inventory in Physical Return and Transportation Stage] / [Total MRO Inventory Value] x 100%"@en;    
    vs:term_status "stable" ;
    dct:modified "2015-11-05"^^xsd:date ;
.

scor:hasMetricAM_41
    rdf:type owl:DatatypeProperty ;
    rdfs:subPropertyOf scor:hasAssetManagemenEfficiencyMetric ;
    rdfs:domain [rdf:type owl:Class ;
        owl:unionOf (
        scor:RequestMROReturnAuthorization
        )] ;
    rdfs:label "Percentage Unserviceable MRO Inventory in Return Authorization"@en;
    rdfs:comment "The value of unserviceable MRO inventory awaiting return authorization as a percentage of the total MRO inventory value (%) Calculation [Value of Unserviceable MRO Inventory in Request Return Authorization Stage] / Total MRO Inventory Value] x 100%"@en;    
    vs:term_status "stable" ;
    dct:modified "2015-11-05"^^xsd:date ;
.

scor:hasMetricAM_42
    rdf:type owl:DatatypeProperty ;
    rdfs:subPropertyOf scor:hasAssetManagemenEfficiencyMetric ;
    rdfs:domain [rdf:type owl:Class ;
        owl:unionOf (
        scor:IdentifyMROProductCondition
        )] ;
    rdfs:label "Percentage Unserviceable MRO Inventory in Identification"@en;
    rdfs:comment "The value of unserviceable MRO Inventory awaiting identification as a percentage of total MRO inventory value (%) Calculation [Value of Unserviceable MRO Inventory in Identification Stage] / [Total MRO Inventory Value] x 100%"@en;    
    vs:term_status "stable" ;
    dct:modified "2015-11-05"^^xsd:date ;
.

scor:hasMetricAM_43
    rdf:type owl:DatatypeProperty ;
    rdfs:subPropertyOf scor:hasAssetManagemenEfficiencyMetric ;
    rdfs:domain [rdf:type owl:Class ;
        owl:unionOf (
        scor:ScheduleMROShipment
        )] ;
    rdfs:label "Percentage Unserviceable MRO Inventory in Scheduling"@en;
    rdfs:comment "The value of unserviceable MRO inventory awaiting scheduling as a percentage of the total MRO inventory value (%) Calculation [Value of Unserviceable MRO inventory in Scheduling Stage] / [Total MRO Inventory Value] x 100%"@en;    
    vs:term_status "stable" ;
    dct:modified "2015-11-05"^^xsd:date ;
.

#44 seem to be deprecated

scor:hasMetricAM_45
    rdf:type owl:DatatypeProperty ;
    rdfs:subPropertyOf scor:hasAssetManagemenEfficiencyMetric ;
    rdfs:domain [rdf:type owl:Class ;
        owl:unionOf (
        scor:DeliverStockedProduct
        scor:DeliverMakeToOrderProduct
        scor:DeliverEngineerToOrderProduct
        )] ;
    rdfs:label "Inventory Days of Supply - Finished Goods"@en;
    rdfs:comment "Finished goods inventory days of supply are calculated as gross finished goods inventory / (value of transfers / 365 days) in days."@en;    
    vs:term_status "stable" ;
    dct:modified "2015-11-05"^^xsd:date ;
.


#############################################################################################
#############################################################################################
#############################################################################################
#### Individuals

## Skills

scor:3WayReceivingMatch
    rdf:type scor:Skill ;
    rdfs:comment "Knowledge of the process of reconciling invoices with purchase orders and goods received notes in order to authorize payment of invoices"@en  ;
    rdfs:label "3-way Receiving Match"@en ;
    skos:notation "HS.0001"@en  ;
    rdfs:isDefinedBy scor: ;
    vs:term_status "stable" ;
    dct:modified "2015-11-05"^^xsd:date ;
 .

scor:Acceptancestable
    rdf:type scor:Skill ;
    rdfs:comment "Working knowledge of Functional and/or Quality Assurance stable of product to ensure it will perform in accordance with its intended contractual agreement for form, fit and function"@en  ;
    rdfs:label "Acceptance stable"@en ;
    skos:notation "HS.0002"@en  ;
    rdfs:isDefinedBy scor: ;
    vs:term_status "stable" ;
    dct:modified "2015-11-05"^^xsd:date ;
 .

scor:Accounting
    rdf:type scor:Skill ;
    rdfs:comment "The process of collecting, analyzing, and communicating financial information about a business entity to specified stakeholders"@en  ;
    rdfs:label "Accounting"@en ;
    skos:notation "HS.0003"@en  ;
    rdfs:isDefinedBy scor: ;
    vs:term_status "stable" ;
    dct:modified "2015-11-05"^^xsd:date ;
 .

scor:AdvertisingMethodologies
    rdf:type scor:Skill ;
    rdfs:comment "Knowledge of effective procurement or business development communication techniques to inform and/or solicit potential suppliers regarding product or service specifications"@en  ;
    rdfs:label "Advertising Methodologies"@en ;
    skos:notation "HS.0004"@en  ;
    rdfs:isDefinedBy scor: ;
    vs:term_status "stable" ;
    dct:modified "2015-11-05"^^xsd:date ;
 .

scor:AssemblyProcessDesign
    rdf:type scor:Skill ;
    rdfs:comment "The arrangement of workers, machines, and equipment in which the product being assembled passes consecutively from operation to operation until completed"@en  ;
    rdfs:label "Assembly Process Design"@en ;
    skos:notation "HS.0005"@en  ;
    rdfs:isDefinedBy scor: ;
    vs:term_status "stable" ;
    dct:modified "2015-11-05"^^xsd:date ;
 .

scor:AssetManagement
    rdf:type scor:Skill ;
    rdfs:comment "The process (which requires the use of spreadsheets or software) to identify, collect, maintain and track the companies assets"@en  ;
    rdfs:label "Asset Management"@en ;
    skos:notation "HS.0006"@en  ;
    rdfs:isDefinedBy scor: ;
    vs:term_status "stable" ;
    dct:modified "2015-11-05"^^xsd:date ;
 .

scor:AvailabilityManagement
    rdf:type scor:Skill ;
    rdfs:comment "The process of managing and allocating available resources and inventory (at various levels) based on business rules"@en  ;
    rdfs:label "Availability Management"@en ;
    skos:notation "HS.0007"@en  ;
    rdfs:isDefinedBy scor: ;
    vs:term_status "stable" ;
    dct:modified "2015-11-05"^^xsd:date ;
 .

scor:BarCodeHandlingRFID
    rdf:type scor:Skill ;
    rdfs:comment "Basic working knowledge of the concept of applying or incorporating onto/into a product an optical machine-readable representation of data (bar code) and /or using radio waves with radio-frequency identification tags (RFID) for the purpose of the identification and tracking of that product"@en  ;
    rdfs:label "Bar Code Handling/RFID"@en ;
    skos:notation "HS.0009"@en  ;
    rdfs:isDefinedBy scor: ;
    vs:term_status "stable" ;
    dct:modified "2015-11-05"^^xsd:date ;
 .

scor:BasicFinance
    rdf:type scor:Skill ;
    rdfs:comment "Working knowledge and ability to effectively interpret and communicate general financial accounting practices and principles which maintain company and regulatory compliance"@en  ;
    rdfs:label "Basic Finance"@en ;
    skos:notation "HS.0010"@en  ;
    rdfs:isDefinedBy scor: ;
    vs:term_status "stable" ;
    dct:modified "2015-11-05"^^xsd:date ;
 .

scor:BasicTransportationManagement
    rdf:type scor:Skill ;
    rdfs:comment "The management of transportation operations of all types, including tracking and managing every aspect of vehicle maintenance"@en  ;
    rdfs:label "Basic Transportation Management"@en ;
    skos:notation "HS.0011"@en  ;
    rdfs:isDefinedBy scor: ;
    vs:term_status "stable" ;
    dct:modified "2015-11-05"^^xsd:date ;
 .

scor:Benchmarking
    rdf:type scor:Skill ;
    rdfs:comment "Working knowledge of the process of capturing and comparing one's own business processes and performance metrics to industry peers and/or best practices from other industries"@en  ;
    rdfs:label "Benchmarking"@en ;
    skos:notation "HS.0012"@en  ;
    rdfs:isDefinedBy scor: ;
    vs:term_status "stable" ;
    dct:modified "2015-11-05"^^xsd:date ;
 .

scor:BlanketPurchaseOrderProcess
    rdf:type scor:Skill ;
    rdfs:comment "Working knowledge of the procurement process for soliciting, issuing and administering open-ended (period for performance) type purchase orders or contracts"@en  ;
    rdfs:label "Blanket purchase order process"@en ;
    skos:notation "HS.0013"@en  ;
    rdfs:isDefinedBy scor: ;
    vs:term_status "stable" ;
    dct:modified "2015-11-05"^^xsd:date ;
 .

scor:BuildScheduleEvaluation
    rdf:type scor:Skill ;
    rdfs:comment "Analyzing a product installation schedule against the constraints and requirements in order to ensure feasibility to effectively and efficiently complete the installation process"@en  ;
    rdfs:label "Build Schedule Evaluation"@en ;
    skos:notation "HS.0014"@en  ;
    rdfs:isDefinedBy scor: ;
    vs:term_status "stable" ;
    dct:modified "2015-11-05"^^xsd:date ;
 .

scor:CADCAM
    rdf:type scor:Skill ;
    rdfs:comment "The process to use computer technology to aid in the design, analysis, and manufacture of products"@en  ;
    rdfs:label "CAD/CAM"@en ;
    skos:notation "HS.0015"@en  ;
    rdfs:isDefinedBy scor: ;
    vs:term_status "stable" ;
    dct:modified "2015-11-05"^^xsd:date ;
 .

scor:CapacityPlanningManagement
    rdf:type scor:Skill ;
    rdfs:comment "The process of determining and managing the production capacity needed by an organization to meet changing demands for its products"@en  ;
    rdfs:label "Capacity Planning/Management"@en ;
    skos:notation "HS.0016"@en  ;
    rdfs:isDefinedBy scor: ;
    vs:term_status "stable" ;
    dct:modified "2015-11-05"^^xsd:date ;
 .

scor:CarrierSelection
    rdf:type scor:Skill ;
    rdfs:comment "Selection of a transportation mode and service provider in order to meet due dates, cost and service objectives"@en  ;
    rdfs:label "Carrier Selection"@en ;
    skos:notation "HS.0018"@en  ;
    rdfs:isDefinedBy scor: ;
    vs:term_status "stable" ;
    dct:modified "2015-11-05"^^xsd:date ;
 .

scor:ChangeNoticeDevelopment
    rdf:type scor:Skill ;
    rdfs:comment "Working knowledge of the procurement process and the ability to clearly disseminate specific contractual or technical requirements which have changed to Sourced contractors, suppliers or vendors"@en  ;
    rdfs:label "Change Notice Development"@en ;
    skos:notation "HS.0019"@en  ;
    rdfs:isDefinedBy scor: ;
    vs:term_status "stable" ;
    dct:modified "2015-11-05"^^xsd:date ;
 .

scor:CompetitiveBidding
    rdf:type scor:Skill ;
    rdfs:comment "Working knowledge of procurement process for requesting and receiving bids/quotes from competing contractors, suppliers, or vendors based on product part numbers, scope, specifications, terms and conditions"@en  ;
    rdfs:label "Competitive Bidding"@en ;
    skos:notation "HS.0020"@en  ;
    rdfs:isDefinedBy scor: ;
    vs:term_status "stable" ;
    dct:modified "2015-11-05"^^xsd:date ;
 .

scor:ConsignmentAgreementDevelopment
    rdf:type scor:Skill ;
    rdfs:comment "Working knowledge of Consignment Agreements which are when one party provides goods/services to another party for sale by that other party"@en  ;
    rdfs:label "Consignment Agreement Development"@en ;
    skos:notation "HS.0021"@en  ;
    rdfs:isDefinedBy scor: ;
    vs:term_status "stable" ;
    dct:modified "2015-11-05"^^xsd:date ;
 .

scor:ContractManagement
    rdf:type scor:Skill ;
    rdfs:comment "Experience in solicitation process, bid/proposal evaluation, contract award and post award administration, and closeout"@en  ;
    rdfs:label "Contract Management"@en ;
    skos:notation "HS.0022"@en  ;
    rdfs:isDefinedBy scor: ;
    vs:term_status "stable" ;
    dct:modified "2015-11-05"^^xsd:date ;
 .

scor:ControlsCompliance
    rdf:type scor:Skill ;
    rdfs:comment "Awareness of relevant regulations, laws and requirements, whether external or internal, and the ability to devise, implement and document the relevant and necessary controls in order to maintain compliance and successfully pass auditing requirements"@en  ;
    rdfs:label "Controls and Compliance"@en ;
    skos:notation "HS.0023"@en  ;
    rdfs:isDefinedBy scor: ;
    vs:term_status "stable" ;
    dct:modified "2015-11-05"^^xsd:date ;
 .

scor:CostPriceAnalysis
    rdf:type scor:Skill ;
    rdfs:comment "Basic financial understanding of analyzing the costs/prices associated with a bid/proposal/quotation for a sourced product for the purpose of attaining best cost/price and/or best value for that product"@en  ;
    rdfs:label "Cost/Price Analysis"@en ;
    skos:notation "HS.0024"@en  ;
    rdfs:isDefinedBy scor: ;
    vs:term_status "stable" ;
    dct:modified "2015-11-05"^^xsd:date ;
 .

scor:BusinessPolicyManagement
    rdf:type scor:Skill ;
    rdfs:comment "A documented set of basic principles and associated guidelines, formulated and enforced by the governing body or an assigned committee of an organization that direct and limit a company's decisions and actions in pursuit of its objectives"@en  ;
    rdfs:label "Business Rule/Policy Management"@en ;
    skos:notation "HS.0025"@en  ;
    rdfs:isDefinedBy scor: ;
    vs:term_status "stable" ;
    dct:modified "2015-11-05"^^xsd:date ;
 .

scor:CreditCollectionManagement
    rdf:type scor:Skill ;
    rdfs:comment "Set of activities to assess and rate the credit risk of a customer, identify/block non-creditworthy customers, manage outstanding balances, process credits, and investigate/pursue overdues"@en  ;
    rdfs:label "Credit/Collection Management"@en ;
    skos:notation "HS.0026"@en  ;
    rdfs:isDefinedBy scor: ;
    vs:term_status "stable" ;
    dct:modified "2015-11-05"^^xsd:date ;
 .

scor:HSCrossDocking
    rdf:type scor:Skill ;
    rdfs:comment "Basic knowledge of linking, staging and moving received sourced products with/to existing open orders minimizing the need for product inventory or storage"@en  ;
    rdfs:label "Cross Docking"@en ;
    skos:notation "HS.0027"@en  ;
    rdfs:isDefinedBy scor: ;
    vs:term_status "stable" ;
    dct:modified "2015-11-05"^^xsd:date ;
 .

scor:CustomerOrderManagement
    rdf:type scor:Skill ;
    rdfs:comment "The process or the work flow associated with the identification, receipt, acceptance, picking, packing, delivery and of the packed item(s) to a shipping carrier"@en  ;
    rdfs:label "Customer Order Management"@en ;
    skos:notation "HS.0028"@en  ;
    rdfs:isDefinedBy scor: ;
    vs:term_status "stable" ;
    dct:modified "2015-11-05"^^xsd:date ;
 .

scor:CustomerRelationshipManagement
    rdf:type scor:Skill ;
    rdfs:comment "Managing a company's relations and interactions with clients and sales prospects, possibly including the synchronization of business processes with the objective of identifying, attracting, and managing new and existing customers"@en  ;
    rdfs:label "Customer Relationship Management (CRM)"@en ;
    skos:notation "HS.0029"@en  ;
    rdfs:isDefinedBy scor: ;
    vs:term_status "stable" ;
    dct:modified "2015-11-05"^^xsd:date ;
 .

scor:CustomerRepair
    rdf:type scor:Skill ;
    rdfs:comment "The actions, tasks and responsibilities concerned with the decision to repair all mechanical/electrical out of order/broken products in line with the internal return rules"@en  ;
    rdfs:label "Customer Repair and Return Policy and Process"@en ;
    skos:notation "HS.0031"@en  ;
    rdfs:isDefinedBy scor: ;
    vs:term_status "stable" ;
    dct:modified "2015-11-05"^^xsd:date ;
 .

scor:CustomerSupplierCommunication
    rdf:type scor:Skill ;
    rdfs:comment "Process of transferring customer/supplier information by speech or writing"@en  ;
    rdfs:label "Customer/Supplier Communication"@en ;
    skos:notation "HS.0032"@en  ;
    rdfs:isDefinedBy scor: ;
    vs:term_status "stable" ;
    dct:modified "2015-11-05"^^xsd:date ;
 .

scor:DataManagement
    rdf:type scor:Skill ;
    rdfs:comment "Working knowledge of the processes required to develop, execute and sustain plans, policies, programs and practices that control, protect, deliver and enhance the value of data and information systems/assets"@en  ;
    rdfs:label "Data management"@en ;
    skos:notation "HS.0033"@en  ;
    rdfs:isDefinedBy scor: ;
    vs:term_status "stable" ;
    dct:modified "2015-11-05"^^xsd:date ;
 .

scor:DiscrepancyReportingResolution
    rdf:type scor:Skill ;
    rdfs:comment "Knowledge of techniques, systems, tools and human skills required to establish effective procedures to identify defective and missing product and then report onward, either internally or externally, ensuring closure on reports and improvements to avoid future repetition"@en  ;
    rdfs:label "Discrepancy Reporting and Resolution"@en ;
    skos:notation "HS.0034"@en  ;
    rdfs:isDefinedBy scor: ;
    vs:term_status "stable" ;
    dct:modified "2015-11-05"^^xsd:date ;
 .

scor:DeliveryBalancing
    rdf:type scor:Skill ;
    rdfs:comment "Delivery balancing is one part of Master Scheduling and involves the balancing of deliveries from suppliers against constrained criteria"@en  ;
    rdfs:label "Delivery Balancing"@en ;
    skos:notation "HS.0035"@en  ;
    rdfs:isDefinedBy scor: ;
    vs:term_status "stable" ;
    dct:modified "2015-11-05"^^xsd:date ;
 .

scor:DeliveryScheduling
    rdf:type scor:Skill ;
    rdfs:comment "Basic knowledge of scheduling and managing sourced product deliveries in order to meet the requirements of inventory replenishment or scheduled production plans"@en  ;
    rdfs:label "Delivery Scheduling"@en ;
    skos:notation "HS.0036"@en  ;
    rdfs:isDefinedBy scor: ;
    vs:term_status "stable" ;
    dct:modified "2015-11-05"^^xsd:date ;
 .

scor:HSDemandManagement
    rdf:type scor:Skill ;
    rdfs:comment "The manufacturing management process by which raw materials and production capacity are optimally allocated to meet demand"@en  ;
    rdfs:label "Demand Management (Skill)"@en ;
    skos:notation "HS.0037"@en  ;
    rdfs:isDefinedBy scor: ;
    vs:term_status "stable" ;
    dct:modified "2015-11-05"^^xsd:date ;
 .

scor:DesignEngineeringScheduleDevelopment
    rdf:type scor:Skill ;
    rdfs:comment "Analyzing the constraints and requirements of a product design cycle in order to evaluate and ensure the timely availability of the product design for building and installation of a product"@en  ;
    rdfs:label "Design/Engineering Schedule Development"@en ;
    skos:notation "HS.0038"@en  ;
    rdfs:isDefinedBy scor: ;
    vs:term_status "stable" ;
    dct:modified "2015-11-05"^^xsd:date ;
 .

scor:DrivingCertification
    rdf:type scor:Skill ;
    rdfs:comment "Ownership of the official, valid (not expired) document stating that the person is authorized and able to drive (a) class/es of vehicles"@en  ;
    rdfs:label "Driving Certification"@en ;
    skos:notation "HS.0039"@en  ;
    rdfs:isDefinedBy scor: ;
    vs:term_status "stable" ;
    dct:modified "2015-11-05"^^xsd:date ;
 .

scor:EHSregulations
    rdf:type scor:Skill ;
    rdfs:comment "The actions, tasks, and responsibilities concerned with the observance and application of the environment, health, and safety rules and standards"@en  ;
    rdfs:label "EHS regulations"@en ;
    skos:notation "HS.0041"@en  ;
    rdfs:isDefinedBy scor: ;
    vs:term_status "stable" ;
    dct:modified "2015-11-05"^^xsd:date ;
 .

scor:EnablingTechnology
    rdf:type scor:Skill ;
    rdfs:comment "Working awareness of relevant technology that could/can be used to improve the effectiveness or efficiency of operations within Source, but also widely across the Supply Chain or the enterprise"@en  ;
    rdfs:label "Enabling Technology"@en ;
    skos:notation "HS.0042"@en  ;
    rdfs:isDefinedBy scor: ;
    vs:term_status "stable" ;
    dct:modified "2015-11-05"^^xsd:date ;
 .

scor:Engineering
    rdf:type scor:Skill ;
    rdfs:comment "The discipline, art and profession of acquiring and applying technical, scientific, and mathematical knowledge to design and implement materials, structures, machines, devices, systems, and processes that safely realize a desired objective or invention"@en  ;
    rdfs:label "Engineering"@en ;
    skos:notation "HS.0043"@en  ;
    rdfs:isDefinedBy scor: ;
    vs:term_status "stable" ;
    dct:modified "2015-11-05"^^xsd:date ;
 .

scor:EnterpriseBusinessProcess
    rdf:type scor:Skill ;
    rdfs:comment "The end-to-end (cross-departmental, and often, cross-company) coordination of work activities that create and deliver ultimate value to customers"@en  ;
    rdfs:label "Enterprise Business Process"@en ;
    skos:notation "HS.0044"@en  ;
    rdfs:isDefinedBy scor: ;
    vs:term_status "stable" ;
    dct:modified "2015-11-05"^^xsd:date ;
 .

scor:EnvironmentalRequirements
    rdf:type scor:Skill ;
    rdfs:comment "Familiarity and understanding of internal and external goals, objectives, rules and laws pertaining to the operation of the Source function within the organization"@en  ;
    rdfs:label "Environmental Requirements"@en ;
    skos:notation "HS.0045"@en  ;
    rdfs:isDefinedBy scor: ;
    vs:term_status "stable" ;
    dct:modified "2015-11-05"^^xsd:date ;
 .

scor:ERPSystems
    rdf:type scor:Skill ;
    rdfs:comment "Working awareness of and conversant with installing and operating appropriate Enterprise Resource Planning (ERP) systems relevant to the organisation concerned"@en  ;
    rdfs:label "ERP Systems"@en ;
    skos:notation "HS.0046"@en  ;
    rdfs:isDefinedBy scor: ;
    vs:term_status "stable" ;
    dct:modified "2015-11-05"^^xsd:date ;
 .

scor:Forecasting
    rdf:type scor:Skill ;
    rdfs:comment "The process of predicting production requirements to meet estimated sales in a particular forecasting period"@en  ;
    rdfs:label "Forecasting"@en ;
    skos:notation "HS.0048"@en  ;
    rdfs:isDefinedBy scor: ;
    vs:term_status "stable" ;
    dct:modified "2015-11-05"^^xsd:date ;
 .

scor:IDDamageInspection
    rdf:type scor:Skill ;
    rdfs:comment "Working knowledge and ability to identify and inspect Sourced products for compliance with contractual part numbers, specifications, drawings, etc, including quality requirements and damage-free product receipt"@en  ;
    rdfs:label "ID and Damage Inspection"@en ;
    skos:notation "HS.0049"@en  ;
    rdfs:isDefinedBy scor: ;
    vs:term_status "stable" ;
    dct:modified "2015-11-05"^^xsd:date ;
 .

scor:ImportExportRegulations
    rdf:type scor:Skill ;
    rdfs:comment "The knowledge and understanding of the laws and regulations governing the import and export requirements of materials"@en  ;
    rdfs:label "Import/Export Regulations"@en ;
    skos:notation "HS.0050"@en  ;
    rdfs:isDefinedBy scor: ;
    vs:term_status "stable" ;
    dct:modified "2015-11-05"^^xsd:date ;
 .

scor:InstallationRequirements
    rdf:type scor:Skill ;
    rdfs:comment "The information, resources and skills requirements to effectively install purchased products as per customer requirements"@en  ;
    rdfs:label "Installation Requirements"@en ;
    skos:notation "HS.0051"@en  ;
    rdfs:isDefinedBy scor: ;
    vs:term_status "stable" ;
    dct:modified "2015-11-05"^^xsd:date ;
 .

scor:InstallationScheduling
    rdf:type scor:Skill ;
    rdfs:comment "The process of managing requirement and constraints associated with a installation schedule in order to effectively schedule product installation as per customer requirements"@en  ;
    rdfs:label "Installation Scheduling"@en ;
    skos:notation "HS.0052"@en  ;
    rdfs:isDefinedBy scor: ;
    vs:term_status "stable" ;
    dct:modified "2015-11-05"^^xsd:date ;
 .

scor:InstalledBaseManagement
    rdf:type scor:Skill ;
    rdfs:comment "Actions, tasks and responsibilities concerned with maintenance and update of info related to the number of units of the company products/platform actually installed and in use around the world"@en  ;
    rdfs:label "Installed base management"@en ;
    skos:notation "HS.0053"@en  ;
    rdfs:isDefinedBy scor: ;
    vs:term_status "stable" ;
    dct:modified "2015-11-05"^^xsd:date ;
 .

scor:IntellectualProperty
    rdf:type scor:Skill ;
    rdfs:comment "Conversant with and effectively manage Proprietary Data and Intellectual property on behalf of the organization"@en  ;
    rdfs:label "Intellectual Property/Proprietary Data"@en ;
    skos:notation "HS.0054"@en  ;
    rdfs:isDefinedBy scor: ;
    vs:term_status "stable" ;
    dct:modified "2015-11-05"^^xsd:date ;
 .

scor:InternationalTrade
    rdf:type scor:Skill ;
    rdfs:comment "The exchange of capital, goods, and services across international borders or territories"@en  ;
    rdfs:label "International Trade"@en ;
    skos:notation "HS.0055"@en  ;
    rdfs:isDefinedBy scor: ;
    vs:term_status "stable" ;
    dct:modified "2015-11-05"^^xsd:date ;
 .

scor:InterpretingSpecifications
    rdf:type scor:Skill ;
    rdfs:comment "Basic working knowledge and ability to read, interpret, understand, and effectively communicate technical specifications and/or drawings to support timely design and delivery of products meeting minimum requirements"@en  ;
    rdfs:label "Interpreting Specifications"@en ;
    skos:notation "HS.0056"@en  ;
    rdfs:isDefinedBy scor: ;
    vs:term_status "stable" ;
    dct:modified "2015-11-05"^^xsd:date ;
 .

scor:InventoryManagement
    rdf:type scor:Skill ;
    rdfs:comment "The formal management of the timing and quantities of goods to be ordered and stocked by an organization in order that demand can always be satisfied without excess expenditure"@en  ;
    rdfs:label "Inventory Management"@en ;
    skos:notation "HS.0058"@en  ;
    rdfs:isDefinedBy scor: ;
    vs:term_status "stable" ;
    dct:modified "2015-11-05"^^xsd:date ;
 .

scor:IssueProposalQuote
    rdf:type scor:Skill ;
    rdfs:comment "The compilation of all required specifications and details need to generate and communicate an RFP/Q"@en  ;
    rdfs:label "Issue Proposal/Quote"@en ;
    skos:notation "HS.0060"@en  ;
    rdfs:isDefinedBy scor: ;
    vs:term_status "stable" ;
    dct:modified "2015-11-05"^^xsd:date ;
 .

scor:ItemMaster
    rdf:type scor:Skill ;
    rdfs:comment "The ability to understand, interpret and effectively communicate a part master record (item master) or bill of materials (BOM) of parts lists that details description, unit of measure, dimensions, group/ family classification, production or sourcing data, quality requirements and/or restrictions"@en  ;
    rdfs:label "Item Master/BOM/BoL Interpretation"@en ;
    skos:notation "HS.0061"@en  ;
    rdfs:isDefinedBy scor: ;
    vs:term_status "stable" ;
    dct:modified "2015-11-05"^^xsd:date ;
 .

scor:KittingPacking
    rdf:type scor:Skill ;
    rdfs:comment "The process of aggregating and packing all elements belonging to a customer order"@en  ;
    rdfs:label "Kitting/Packing"@en ;
    skos:notation "HS.0062"@en  ;
    rdfs:isDefinedBy scor: ;
    vs:term_status "stable" ;
    dct:modified "2015-11-05"^^xsd:date ;
 .

scor:LaborCostsVerification
    rdf:type scor:Skill ;
    rdfs:comment "Capability of calculating, understanding, reporting on, and if necessary, be able to taking corrective action to control labour costs within one's area of responsibility against budgets or objectives that have been set"@en  ;
    rdfs:label "Labor Costs Verification"@en ;
    skos:notation "HS.0063"@en  ;
    rdfs:isDefinedBy scor: ;
    vs:term_status "stable" ;
    dct:modified "2015-11-05"^^xsd:date ;
 .

scor:LeadTimeValidation
    rdf:type scor:Skill ;
    rdfs:comment "The process of analyzing and validating feasibility of customer required lead-times"@en  ;
    rdfs:label "Lead-time validation"@en ;
    skos:notation "HS.0064"@en  ;
    rdfs:isDefinedBy scor: ;
    vs:term_status "stable" ;
    dct:modified "2015-11-05"^^xsd:date ;
 .

scor:LeanManufacturing
    rdf:type scor:Skill ;
    rdfs:comment "The process of identifying processes that impede the optimization of production"@en  ;
    rdfs:label "Lean Manufacturing"@en ;
    skos:notation "HS.0065"@en  ;
    rdfs:isDefinedBy scor: ;
    vs:term_status "stable" ;
    dct:modified "2015-11-05"^^xsd:date ;
 .

scor:LegislationStandards
    rdf:type scor:Skill ;
    rdfs:comment "Knowledge to manage conformance systems and actions for receiving product and relates to general legislation affecting the product being received as well as the specific standards or specifications that applies to the product"@en  ;
    rdfs:label "Legislation and Standards"@en ;
    skos:notation "HS.0066"@en  ;
    rdfs:isDefinedBy scor: ;
    vs:term_status "stable" ;
    dct:modified "2015-11-05"^^xsd:date ;
 .

scor:LinearProgramming
    rdf:type scor:Skill ;
    rdfs:comment "The branch of mathematics concerned with the minimization or maximization of a linear function of several variables and inequalities; used in many branches of industry to minimize costs or maximize production"@en  ;
    rdfs:label "Linear programming"@en ;
    skos:notation "HS.0067"@en  ;
    rdfs:isDefinedBy scor: ;
    vs:term_status "stable" ;
    dct:modified "2015-11-05"^^xsd:date ;
 .

scor:LoadBuilding
    rdf:type scor:Skill ;
    rdfs:comment "The process of order consolidation to meet service, cost, delivery and product specification requirements"@en  ;
    rdfs:label "Load Building"@en ;
    skos:notation "HS.0068"@en  ;
    rdfs:isDefinedBy scor: ;
    vs:term_status "stable" ;
    dct:modified "2015-11-05"^^xsd:date ;
 .

scor:LogisticsManagement
    rdf:type scor:Skill ;
    rdfs:comment "The process for planning, implementing, and controlling the flow and storage of goods, services, and related information between the point of origin and the point of consumption in order to meet customers’ requirements and thus add value for the customer"@en  ;
    rdfs:label "Logistics Management"@en ;
    skos:notation "HS.0069"@en  ;
    rdfs:isDefinedBy scor: ;
    vs:term_status "stable" ;
    dct:modified "2015-11-05"^^xsd:date ;
 .

scor:LogisticsNetworkModeling
    rdf:type scor:Skill ;
    rdfs:comment "The process of planning, implementing, and controlling the flow and storage of goods, services, and related information between the point of origin and the point of consumption in order to meet customers' requirements"@en  ;
    rdfs:label "Logistics network modeling"@en ;
    skos:notation "HS.0070"@en  ;
    rdfs:isDefinedBy scor: ;
    vs:term_status "stable" ;
    dct:modified "2015-11-05"^^xsd:date ;
 .

scor:LogisticsFreight
    rdf:type scor:Skill ;
    rdfs:comment "Working knowledge of the management and integration of information, sourced product/material, transportation, inventory, warehousing, material-handling, and packaging, and occasionally security, between the point of origin and the point of consumption in order to meet customer requirements"@en  ;
    rdfs:label "Logistics/Freight"@en ;
    skos:notation "HS.0071"@en  ;
    rdfs:isDefinedBy scor: ;
    vs:term_status "stable" ;
    dct:modified "2015-11-05"^^xsd:date ;
 .

scor:PerformanceManagement
    rdf:type scor:Skill ;
    rdfs:comment "A framework that identifies opportunities for performance improvement through use of performance measures such as standards and indicators"@en  ;
    rdfs:label "Performance Management"@en ;
    skos:notation "HS.0072"@en  ;
    rdfs:isDefinedBy scor: ;
    vs:term_status "stable" ;
    dct:modified "2015-11-05"^^xsd:date ;
 .

scor:ManufacturingResourceCommitment
    rdf:type scor:Skill ;
    rdfs:comment "The efficient and effective allocation of an organization's manufacturing resources and assets with the objective of meeting customer demands/requirements"@en  ;
    rdfs:label "Manufacturing Resource Commitment"@en ;
    skos:notation "HS.0073"@en  ;
    rdfs:isDefinedBy scor: ;
    vs:term_status "stable" ;
    dct:modified "2015-11-05"^^xsd:date ;
 .

scor:MasterScheduling
    rdf:type scor:Skill ;
    rdfs:comment "Knowledge of co-ordinating and keeping track of all the different components related to the Source activity"@en  ;
    rdfs:label "Master Scheduling"@en ;
    skos:notation "HS.0074"@en  ;
    rdfs:isDefinedBy scor: ;
    vs:term_status "stable" ;
    dct:modified "2015-11-05"^^xsd:date ;
 .

scor:MaterialHandlingEquipment
    rdf:type scor:Skill ;
    rdfs:comment "The ability to manipulate various types of material handling systems (e.g. forklifts, conveyors, palletizers, etc.) to pick, pack, and store orders and inventory"@en  ;
    rdfs:label "Material handling equipment usage"@en ;
    skos:notation "HS.0075"@en  ;
    rdfs:isDefinedBy scor: ;
    vs:term_status "stable" ;
    dct:modified "2015-11-05"^^xsd:date ;
 .

scor:MilestonePerformancePayments
    rdf:type scor:Skill ;
    rdfs:comment "Working knowledge of contractual requirements for the authorization of monetary payments for the successful completion of pre-defined development or performance milestones"@en  ;
    rdfs:label "Milestone/Performance Payments"@en ;
    skos:notation "HS.0076"@en  ;
    rdfs:isDefinedBy scor: ;
    vs:term_status "stable" ;
    dct:modified "2015-11-05"^^xsd:date ;
 .

scor:MPSMethodsTechniques
    rdf:type scor:Skill ;
    rdfs:comment "The techniques used in material requirements planning systems to develop a detailed plan for product manufacturing"@en  ;
    rdfs:label "MPS Methodologies and Techniques"@en ;
    skos:notation "HS.0077"@en  ;
    rdfs:isDefinedBy scor: ;
    vs:term_status "stable" ;
    dct:modified "2015-11-05"^^xsd:date ;
 .

scor:MROManagement
    rdf:type scor:Skill ;
    rdfs:comment "All actions which have the objective of retaining or restoring an item in or to a state in which it can perform its required function"@en  ;
    rdfs:label "MRO Management"@en ;
    skos:notation "HS.0078"@en  ;
    rdfs:isDefinedBy scor: ;
    vs:term_status "stable" ;
    dct:modified "2015-11-05"^^xsd:date ;
 .

scor:MRPSystems
    rdf:type scor:Skill ;
    rdfs:comment "The process of ensuring materials and products are available for production and delivery to customers, maintaining the lowest possible level of inventory and planning manufacturing activities, delivery schedules and purchasing activities"@en  ;
    rdfs:label "MRP Systems"@en ;
    skos:notation "HS.0079"@en  ;
    rdfs:isDefinedBy scor: ;
    vs:term_status "stable" ;
    dct:modified "2015-11-05"^^xsd:date ;
 .

scor:EnvironmentalInterpretation
    rdf:type scor:Skill ;
    rdfs:comment "Working knowledge and understanding of strict regulatory adherence to health and environmental requirements/restrictions associated with particular products as detailed on Material Safely Data Sheets (MSDS) or Certificates of Compliance CoC"@en  ;
    rdfs:label "Environmental Interpretation"@en ;
    skos:notation "HS.0080"@en  ;
    rdfs:isDefinedBy scor: ;
    vs:term_status "stable" ;
    dct:modified "2015-11-05"^^xsd:date ;
 .

scor:OfficeAutomationTools
    rdf:type scor:Skill ;
    rdfs:comment "Familiarity with relevant Office Automation Tools and be able to deploy against financial justification as appropriate taking account of project and change management requirements"@en  ;
    rdfs:label "Office automation tools"@en ;
    skos:notation "HS.0081"@en  ;
    rdfs:isDefinedBy scor: ;
    vs:term_status "stable" ;
    dct:modified "2015-11-05"^^xsd:date ;
 .

scor:Optimization
    rdf:type scor:Skill ;
    rdfs:comment "The process of improving various aspects of the business resulting in (such as) increased profits, improved product or greater customer satisfaction"@en  ;
    rdfs:label "Optimization"@en ;
    skos:notation "HS.0082"@en  ;
    rdfs:isDefinedBy scor: ;
    vs:term_status "stable" ;
    dct:modified "2015-11-05"^^xsd:date ;
 .

scor:OrderManagement
    rdf:type scor:Skill ;
    rdfs:comment "The process or the work flow associated with the identification, receipt, acceptance, picking, packing, delivery and of the packed item(s) to a shipping carrier"@en  ;
    rdfs:label "Order Management"@en ;
    skos:notation "HS.0083"@en  ;
    rdfs:isDefinedBy scor: ;
    vs:term_status "stable" ;
    dct:modified "2015-11-05"^^xsd:date ;
 .

scor:Outsourcing
    rdf:type scor:Skill ;
    rdfs:comment "A company that contracts with another company to provide services that might otherwise be performed by in-house employees"@en  ;
    rdfs:label "Outsourcing"@en ;
    skos:notation "HS.0085"@en  ;
    rdfs:isDefinedBy scor: ;
    vs:term_status "stable" ;
    dct:modified "2015-11-05"^^xsd:date ;
 .

scor:Packaging
    rdf:type scor:Skill ;
    rdfs:comment "The processes of coordinating a system of preparing goods for transport, warehousing, logistics, sale, and end use"@en  ;
    rdfs:label "Packaging"@en ;
    skos:notation "HS.0086"@en  ;
    rdfs:isDefinedBy scor: ;
    vs:term_status "stable" ;
    dct:modified "2015-11-05"^^xsd:date ;
 .

scor:PaymentProcessing
    rdf:type scor:Skill ;
    rdfs:comment "Working knowledge of the processes and policies required for contractual authorization of payments for sourced products and services"@en  ;
    rdfs:label "Payment Processing"@en ;
    skos:notation "HS.0087"@en  ;
    rdfs:isDefinedBy scor: ;
    vs:term_status "stable" ;
    dct:modified "2015-11-05"^^xsd:date ;
 .

scor:PhysicalCapability
    rdf:type scor:Skill ;
    rdfs:comment "The ability to complete a process through the use of dexterity, strength or other capacities"@en  ;
    rdfs:label "Physical Capability"@en ;
    skos:notation "HS.0088"@en  ;
    rdfs:isDefinedBy scor: ;
    vs:term_status "stable" ;
    dct:modified "2015-11-05"^^xsd:date ;
 .

scor:PhysicalDistributionSystems
    rdf:type scor:Skill ;
    rdfs:comment "The set of activities concerned with efficient movement of finished goods from the end of the production operation to the consumer"@en  ;
    rdfs:label "Physical Distribution Systems"@en ;
    skos:notation "HS.0089"@en  ;
    rdfs:isDefinedBy scor: ;
    vs:term_status "stable" ;
    dct:modified "2015-11-05"^^xsd:date ;
 .

scor:PickingProcess
    rdf:type scor:Skill ;
    rdfs:comment "The process of selecting and collecting SKUs and materials in a specified order and quantity with the objective of satisfying customers orders"@en  ;
    rdfs:label "Picking process / order batching"@en ;
    skos:notation "HS.0090"@en  ;
    rdfs:isDefinedBy scor: ;
    vs:term_status "stable" ;
    dct:modified "2015-11-05"^^xsd:date ;
 .

scor:PlanogramUsageStrategies
    rdf:type scor:Skill ;
    rdfs:comment "The process of using a planogram to diagram fixtures and products to illustrate how and where retail products should be displayed, usually on a store shelf in order to increase customer purchases"@en  ;
    rdfs:label "Planogram usage and strategies"@en ;
    skos:notation "HS.0091"@en  ;
    rdfs:isDefinedBy scor: ;
    vs:term_status "stable" ;
    dct:modified "2015-11-05"^^xsd:date ;
 .

scor:PricingManagement
    rdf:type scor:Skill ;
    rdfs:comment "The analysis and setting of prices (on a per unit or volume basis) to meet required characteristics, business rules and/or business performance requirements"@en  ;
    rdfs:label "Pricing Management"@en ;
    skos:notation "HS.0092"@en  ;
    rdfs:isDefinedBy scor: ;
    vs:term_status "stable" ;
    dct:modified "2015-11-05"^^xsd:date ;
 .

scor:Prioritization
    rdf:type scor:Skill ;
    rdfs:comment "The knowledge and ability to arrange process steps, jobs or orders in queue, or product receipts in the proper sequence in order to meet product/service production and deliveries as scheduled"@en  ;
    rdfs:label "Prioritization"@en ;
    skos:notation "HS.0093"@en  ;
    rdfs:isDefinedBy scor: ;
    vs:term_status "stable" ;
    dct:modified "2015-11-05"^^xsd:date ;
 .

scor:Procurement
    rdf:type scor:Skill ;
    rdfs:comment "Working knowledge of the process for acquiring goods and/or services at the best possible total cost of ownership, in the right quantity, quality, at the right time and in the right place, with all required documentation"@en  ;
    rdfs:label "Procurement"@en ;
    skos:notation "HS.0094"@en  ;
    rdfs:isDefinedBy scor: ;
    vs:term_status "stable" ;
    dct:modified "2015-11-05"^^xsd:date ;
 .

scor:ProductConfigurationValidation
    rdf:type scor:Skill ;
    rdfs:comment "The analysis of stated product and configuration specifications against required and feasible product's performance, functional, and physical requirements"@en  ;
    rdfs:label "Product and Configuration Validation"@en ;
    skos:notation "HS.0095"@en  ;
    rdfs:isDefinedBy scor: ;
    vs:term_status "stable" ;
    dct:modified "2015-11-05"^^xsd:date ;
 .

scor:ProductCheckoutProcess
    rdf:type scor:Skill ;
    rdfs:comment "The process of removing a product from inventory and exchanging funds for the value of the product in a retail supply chain"@en  ;
    rdfs:label "Product checkout process"@en ;
    skos:notation "HS.0096"@en  ;
    rdfs:isDefinedBy scor: ;
    vs:term_status "stable" ;
    dct:modified "2015-11-05"^^xsd:date ;
 .

scor:ProductDevelopment
    rdf:type scor:Skill ;
    rdfs:comment "Familiarity and awareness of the Product Development process and its key steps and the interaction with the Source activity"@en  ;
    rdfs:label "Product Development"@en ;
    skos:notation "HS.0097"@en  ;
    rdfs:isDefinedBy scor: ;
    vs:term_status "stable" ;
    dct:modified "2015-11-05"^^xsd:date ;
 .

scor:ProductInformationManagement
    rdf:type scor:Skill ;
    rdfs:comment "The use of software or other tools to capture and maintain information on products and/or services through their life cycle"@en  ;
    rdfs:label "Product Information Management"@en ;
    skos:notation "HS.0098"@en  ;
    rdfs:isDefinedBy scor: ;
    vs:term_status "stable" ;
    dct:modified "2015-11-05"^^xsd:date ;
 .

scor:Production
    rdf:type scor:Skill ;
    rdfs:comment "The process of using machines, tools, materials and labor to make things for use or sale"@en  ;
    rdfs:label "Production"@en ;
    skos:notation "HS.0099"@en  ;
    rdfs:isDefinedBy scor: ;
    vs:term_status "stable" ;
    dct:modified "2015-11-05"^^xsd:date ;
 .

scor:ProductionPlanning
    rdf:type scor:Skill ;
    rdfs:comment "Actions, tasks and responsibilities concerned with the planning, scheduling and releasing of production orders in order to satisfy demand while optimizing the available and planned resources/capacity"@en  ;
    rdfs:label "Production Planning"@en ;
    skos:notation "HS.0101"@en  ;
    rdfs:isDefinedBy scor: ;
    vs:term_status "stable" ;
    dct:modified "2015-11-05"^^xsd:date ;
 .


# Standart Practice Individuals
scor:ConsignmentInventory
    rdf:type scor:StandardPractice ;
    rdfs:comment "The organization of source processes where the ownership of materials transfers are based on a signal further down in the supply chain (for example Make or Deliver)."@en  ;
    rdfs:label "Consignment Inventory"@en ;
    skos:notation "BP.006"@en  ;
    rdfs:isDefinedBy scor: ;
    vs:term_status "stable" ;
    dct:modified "2015-11-05"^^xsd:date ;
 .

scor:SlowMovingInventoryMonitoring
    rdf:type scor:StandardPractice ;
    rdfs:comment "Slow-moving inventory is defined as the value of those SKUs whose stock level is higher than the total consumption within the last 12 months"@en  ;
    rdfs:label "Slow-moving Inventory Monitoring"@en ;
    skos:notation "BP.008"@en  ;
    rdfs:isDefinedBy scor: ;
    vs:term_status "stable" ;
    dct:modified "2015-11-05"^^xsd:date ;
 .

scor:Kanban
    rdf:type scor:StandardPractice ;
    rdfs:comment "A inventory replenishment technique where a material is replenished based on consumption"@en  ;
    rdfs:label "Kanban"@en ;
    skos:notation "BP.009"@en  ;
    rdfs:isDefinedBy scor: ;
    vs:term_status "stable" ;
    dct:modified "2015-11-05"^^xsd:date ;
 .

scor:MinMaxReplenishment
    rdf:type scor:StandardPractice ;
    rdfs:comment "A inventory replenishment practice where purchase requisitions or purchase orders are created when inventory for an item drops below the Minimum inventory level"@en  ;
    rdfs:label "Min-Max Replenishment"@en ;
    skos:notation "BP.010"@en  ;
    rdfs:isDefinedBy scor: ;
    vs:term_status "stable" ;
    dct:modified "2015-11-05"^^xsd:date ;
 .

scor:LotTracking
    rdf:type scor:StandardPractice ;
    rdfs:comment "The practice of storing information about the history and/or genealogy of a product or material"@en  ;
    rdfs:label "Lot Tracking"@en ;
    skos:notation "BP.012"@en  ;
    rdfs:isDefinedBy scor: ;
    vs:term_status "stable" ;
    dct:modified "2015-11-05"^^xsd:date ;
 .

scor:ItemRationalization
    rdf:type scor:StandardPractice ;
    rdfs:comment "Rationalization of inventory at the item/part/SKU number level"@en  ;
    rdfs:label "Item Rationalization"@en ;
    skos:notation "BP.013"@en  ;
    rdfs:isDefinedBy scor: ;
    vs:term_status "stable" ;
    dct:modified "2015-11-05"^^xsd:date ;
 .

scor:SafetyStockPlanning
    rdf:type scor:StandardPractice ;
    rdfs:comment "Meet desired customer service levels while maintaining a minimum amount of safety stock"@en  ;
    rdfs:label "Safety Stock Planning"@en ;
    skos:notation "BP.015"@en  ;
    rdfs:isDefinedBy scor: ;
    vs:term_status "stable" ;
    dct:modified "2015-11-05"^^xsd:date ;
 .

scor:DistributionPlanning
    rdf:type scor:StandardPractice ;
    rdfs:comment "Determine the best short-term strategy to meet demand and to replenish stocking locations"@en  ;
    rdfs:label "Distribution Planning"@en ;
    skos:notation "BP.017"@en  ;
    rdfs:isDefinedBy scor: ;
    vs:term_status "stable" ;
    dct:modified "2015-11-05"^^xsd:date ;
 .

scor:ABCInventoryClassificationSystem
    rdf:type scor:StandardPractice ;
    rdfs:comment "The ABC classification system is the Pareto analysis of a range of inventory items, into three or four inventory categories"@en  ;
    rdfs:label "ABC Inventory Classification System"@en ;
    skos:notation "BP.018"@en  ;
    rdfs:isDefinedBy scor: ;
    vs:term_status "stable" ;
    dct:modified "2015-11-05"^^xsd:date ;
 .

scor:DemandPlanning
    rdf:type scor:StandardPractice ;
    rdfs:comment "Demand Planning is the process used for developing an accurate and comprehensive material forecast"@en  ;
    rdfs:label "Demand Planning"@en ;
    skos:notation "BP.019"@en  ;
    rdfs:isDefinedBy scor: ;
    vs:term_status "stable" ;
    dct:modified "2015-11-05"^^xsd:date ;
 .

scor:SalesOperationsPlanning
    rdf:type scor:StandardPractice ;
    rdfs:comment "Mid to Long Term supply chain planning practice which seeks to compare the forecast sales plan to the company resources, and analyze where any imbalances to the plan might exist"@en  ;
    rdfs:label "Sales and Operations Planning"@en ;
    skos:notation "BP.021"@en  ;
    rdfs:isDefinedBy scor: ;
    vs:term_status "stable" ;
    dct:modified "2015-11-05"^^xsd:date ;
 .

scor:MRPI
    rdf:type scor:StandardPractice ;
    rdfs:comment "A 'plan' scheme of different inventory management practices has been adopted by a company in a mixed model manufacturing environment"@en  ;
    rdfs:label "MRP I"@en ;
    skos:notation "BP.022"@en  ;
    rdfs:isDefinedBy scor: ;
    vs:term_status "stable" ;
    dct:modified "2015-11-05"^^xsd:date ;
 .

scor:ImproveSOPprocess
    rdf:type scor:StandardPractice ;
    rdfs:comment "Establish disciplined monthly cross-functional process to increase accuracy of demand management, establish biz inventory policy, and agreement on demand and supply balancing"@en  ;
    rdfs:label "Improve S and OP process"@en ;
    skos:notation "BP.026"@en  ;
    rdfs:isDefinedBy scor: ;
    vs:term_status "stable" ;
    dct:modified "2015-11-05"^^xsd:date ;
 .

scor:StockKeepingUnit
    rdf:type scor:StandardPractice ;
    rdfs:comment "Inventory reduction practice to determine which SKUs that can be terminated t using SKU Cost of Sales Analysis"@en  ;
    rdfs:label "Stock keeping Unit (SKU) Rationalization/Cost of Sales Analysis"@en ;
    skos:notation "BP.031"@en  ;
    rdfs:isDefinedBy scor: ;
    vs:term_status "stable" ;
    dct:modified "2015-11-05"^^xsd:date ;
 .

scor:DelayInboundSupplierShipments
    rdf:type scor:StandardPractice ;
    rdfs:comment "Analyze and execute a delay in inbound supplier raw material shipments to reduce raw material costs at summer break, end-of-year or other scheduled plant closure"@en  ;
    rdfs:label "Delay Inbound Supplier Shipments"@en ;
    skos:notation "BP.045"@en  ;
    rdfs:isDefinedBy scor: ;
    vs:term_status "stable" ;
    dct:modified "2015-11-05"^^xsd:date ;
 .

scor:ExpediteOutboundCustomerShipments
    rdf:type scor:StandardPractice ;
    rdfs:comment "The practice of analyzing the cost of maintaining inventory vs. the cost of transportation for opportunities to optimize total cost"@en  ;
    rdfs:label "Expedite Outbound Customer Shipments"@en ;
    skos:notation "BP.046"@en  ;
    rdfs:isDefinedBy scor: ;
    vs:term_status "stable" ;
    dct:modified "2015-11-05"^^xsd:date ;
 .

scor:ReturnAuthorization
    rdf:type scor:StandardPractice ;
    rdfs:comment "The Return Authorization (Return Material Authorization/Return Merchandise Authorization/Goods Return Authorization) process provides the inputs into the reverse logistics plan"@en  ;
    rdfs:label "Return Authorization"@en ;
    skos:notation "BP.135"@en  ;
    rdfs:isDefinedBy scor: ;
    vs:term_status "stable" ;
    dct:modified "2015-11-05"^^xsd:date ;
 .

scor:OutsourcedReverseLogistics
    rdf:type scor:StandardPractice ;
    rdfs:comment "Rather than manage returns as part of a service organization or operations many companies turn to outsourced service providers including Contract Manufacturers, EMS providers and Third Party Logistics providers for returns management"@en  ;
    rdfs:label "Outsourced Reverse Logistics"@en ;
    skos:notation "BP.136"@en  ;
    rdfs:isDefinedBy scor: ;
    vs:term_status "stable" ;
    dct:modified "2015-11-05"^^xsd:date ;
 .

scor:PurchaseOrderManagement
    rdf:type scor:StandardPractice ;
    rdfs:comment "The practice of issuing a purchase order for a number of products which are required in the short to mid term"@en  ;
    rdfs:label "Purchase Order Management"@en ;
    skos:notation "BP.144"@en  ;
    rdfs:isDefinedBy scor: ;
    vs:term_status "stable" ;
    dct:modified "2015-11-05"^^xsd:date ;
 .

scor:BPCrossDocking
    rdf:type scor:StandardPractice ;
    rdfs:comment "the practice of unloading materials from an incoming vehicle and loading these materials directly onto outbound vehicles without putting away into the regular storage locations in a warehouse"@en  ;
    rdfs:label "Cross-Docking"@en ;
    skos:notation "BP.146"@en  ;
    rdfs:isDefinedBy scor: ;
    vs:term_status "stable" ;
    dct:modified "2015-11-05"^^xsd:date ;
 .

scor:WayDeliveryVerification
    rdf:type scor:StandardPractice ;
    rdfs:comment "The practice of checking received invoices from suppliers against the quantities received and against the associated Purchase Order, Contract or Vendor Schedule"@en  ;
    rdfs:label "3-Way Delivery Verification"@en ;
    skos:notation "BP.148"@en  ;
    rdfs:isDefinedBy scor: ;
    vs:term_status "stable" ;
    dct:modified "2015-11-05"^^xsd:date ;
 .

scor:RotableSparesPool
    rdf:type scor:StandardPractice ;
    rdfs:comment "An inventory of serviceable parts that can replace a customers broken part to increase their recovery time"@en  ;
    rdfs:label "Rotable Spares Pool"@en ;
    skos:notation "BP.168"@en  ;
    rdfs:isDefinedBy scor: ;
    vs:term_status "stable" ;
    dct:modified "2015-11-05"^^xsd:date ;
 .

scor:BeyondEconomicRepairManagement
    rdf:type scor:StandardPractice ;
    rdfs:comment "The practice of assessing items as they are removed for Maintenance, Repair and Overhaul to determine whether repair would cost more than buying a replacement part"@en  ;
    rdfs:label "Beyond Economic Repair (BER) Management"@en ;
    skos:notation "BP.169"@en  ;
    rdfs:isDefinedBy scor: ;
    vs:term_status "stable" ;
    dct:modified "2015-11-05"^^xsd:date ;
 .

# Emerging Practice Individuals


scor:DemandPlanningForecasting
    rdf:type scor:EmergingPractice ;
    rdfs:comment "Use state-of-the-art forecasting algorithms for product life-cycle planning and trade promotion planning."@en  ;
    rdfs:label "Demand Planning Forecasting"@en ;
    skos:notation "BP.014"@en ;
    rdfs:isDefinedBy scor: ;
    vs:term_status "stable" ;
    dct:modified "2015-11-05"^^xsd:date ;
 .

scor:SupplyNetworkPlanning
    rdf:type scor:EmergingPractice ;
    rdfs:comment "Simulate and implement comprehensive tactical planning and sourcing decisions based on a single, globally consistent model."@en  ;
    rdfs:label "Supply Network Planning"@en ;
    skos:notation "BP.016"@en  ;
    rdfs:isDefinedBy scor: ;
    vs:term_status "stable" ;
    dct:modified "2015-11-05"^^xsd:date ;
 .

scor:BPDemandManagement
    rdf:type scor:EmergingPractice ;
    rdfs:comment "Takes Demand Planning to the next level and integrates the plan up and down the supply chain as well as across the enterprise."@en ;
    rdfs:label "Demand Management (Emerging Practice)"@en ;
    skos:notation "BP.020"@en ;
    rdfs:isDefinedBy scor: ;
    vs:term_status "stable" ;
    dct:modified "2015-11-05"^^xsd:date ;
 .

scor:BusinessRuleManagement
    rdf:type scor:EmergingPractice ;
    rdfs:comment "Business rules are in a (human-readable) form that are used by, but not embedded in, supply chain systems"@en ;
    rdfs:label "Business Rule Management"@en ;
    skos:notation "BP.023"@en ;
    rdfs:isDefinedBy scor: ;
    vs:term_status "stable" ;
    dct:modified "2015-11-05"^^xsd:date ;
 .

scor:SupplyChainOptimization
    rdf:type scor:EmergingPractice ;
    rdfs:comment "A part of the enterprise strategic plan for leading edge companies"@en ;
    rdfs:label "Supply Chain Optimization"@en ;
    skos:notation "BP.024"@en  ;
    rdfs:isDefinedBy scor: ;
    vs:term_status "stable" ;
    dct:modified "2015-11-05"^^xsd:date ;
 .

scor:SelfServiceWarrantyClaimSubmittal
    rdf:type scor:EmergingPractice ;
    rdfs:comment "enables customers and service providers to submit warranty claims over the web, reducing internal validation and processing workload. "@en;
    rdfs:label "Self-Service Warranty Claim Submittal"@en ;
    skos:notation "BP.025"@en  ;
    rdfs:isDefinedBy scor: ;
    vs:term_status "stable" ;
    dct:modified "2015-11-05"^^xsd:date ;
 .

scor:BusinessRuleReview
    rdf:type scor:EmergingPractice ;
    rdfs:comment "Is performed by supply chain middle and upper level management of an organization."@en ;
    rdfs:label "Business Rule Review"@en ;
    skos:notation "BP.035"@en ;
    rdfs:isDefinedBy scor: ;
    vs:term_status "stable" ;
    dct:modified "2015-11-05"^^xsd:date ;
 .

scor:LeanPlanning
    rdf:type scor:EmergingPractice ;
    rdfs:comment "Creates real world project plans which robustly model the project from initiation to final delivery."@en  ;
    rdfs:label "Lean Planning"@en ;
    skos:notation "BP.049"@en  ;
    rdfs:isDefinedBy scor: ;
    vs:term_status "stable" ;
    dct:modified "2015-11-05"^^xsd:date ;
 .

scor:ReturnsReceivingRefurbishment
    rdf:type scor:EmergingPractice ;
    rdfs:comment "The practice of refurbishing materials during the receiving processes (i.e. Source processes) for returned materials."@en  ;
    rdfs:label "Returns Receiving Refurbishment"@en ;
    skos:notation "BP.073"@en  ;
    rdfs:isDefinedBy scor: ;
    vs:term_status "stable" ;
    dct:modified "2015-11-05"^^xsd:date ;
 .

scor:LoanerProgram
    rdf:type scor:EmergingPractice ;
    rdfs:comment "In order to minimize lost productivity, many companies offer a loaner program for their customers when they need to return a defective product."@en  ;
    rdfs:label "Loaner Program"@en ;
    skos:notation "BP.079"@en  ;
    rdfs:isDefinedBy scor: ;
    vs:term_status "stable" ;
    dct:modified "2015-11-05"^^xsd:date ;
 .

scor:MobileAccessOfInformation
    rdf:type scor:EmergingPractice ;
    rdfs:comment "Mobile access to information in supply chain means information on status metrics supply and demand are available in the internet smart phones and other similar mobile devices."@en  ;
    rdfs:label "Mobile Access of Information"@en ;
    skos:notation "BP.098"@en  ;
    rdfs:isDefinedBy scor: ;
    vs:term_status "stable" ;
    dct:modified "2015-11-05"^^xsd:date ;
 .

scor:ReturnPolicyConformanceIntegration
    rdf:type scor:EmergingPractice ;
    rdfs:comment "The practice of implementing standard procedures and enableing technology to ensure conformance to return policies."@en  ;
    rdfs:label "Return Policy Conformance Integration"@en ;
    skos:notation "BP.108"@en  ;
    rdfs:isDefinedBy scor: ;
    vs:term_status "stable" ;
    dct:modified "2015-11-05"^^xsd:date ;
 .

scor:CarcassPrepositioning
    rdf:type scor:EmergingPractice ;
    rdfs:comment "The practice of making disposition decisions for reparable parts/cores/carcasses early in the (Return Material Authorization) RMA process."@en ;
    rdfs:label "Carcass Prepositioning"@en ;
    skos:notation "BP.109"@en ;
    rdfs:isDefinedBy scor: ;
    vs:term_status "stable" ;
    dct:modified "2015-11-05"^^xsd:date ;
 .

scor:EmbedSpecializedServices
    rdf:type scor:EmergingPractice ;
    rdfs:comment "Add additional capability, processes and expertise by embedding specialized packaging, product completion and pack out services on-site from a 3rd party provider."@en  ;
    rdfs:label "Embed Specialized Services"@en ;
    skos:notation "BP.117"@en ;
    rdfs:isDefinedBy scor: ;
    vs:term_status "stable" ;
    dct:modified "2015-11-05"^^xsd:date ;
 .

scor:TransportationManagementOutsourcing
    rdf:type scor:EmergingPractice ;
    rdfs:comment "Outsourcing transportation creates an opportunity for small businesses to combine their transportation spend and get a lower overall tariff rate."@en  ;
    rdfs:label "Transportation Management Outsourcing"@en ;
    skos:notation "BP.118"@en  ;
    rdfs:isDefinedBy scor: ;
    vs:term_status "stable" ;
    dct:modified "2015-11-05"^^xsd:date ;
 .

scor:ThreeDPrintRapidProtoyping
    rdf:type scor:EmergingPractice ;
    rdfs:comment "3D printing is a phrase used to describe the process of creating three dimensional objects from digital file using a materials printer, in a manner similar to printing images on paper."@en  ;
    rdfs:label "3D Print Rapid Protoyping"@en ;
    skos:notation "BP.120"@en  ;
    rdfs:isDefinedBy scor: ;
    vs:term_status "stable" ;
    dct:modified "2015-11-05"^^xsd:date ;
 .

scor:DigitalPackagingOnDemand
    rdf:type scor:EmergingPractice ;
    rdfs:comment "The use of digital packaging printing to create custom product packaging unique to the customer and the product requirements."@en  ;
    rdfs:label "Digital Packaging on Demand"@en ;
    skos:notation "BP.121"@en ;
    rdfs:isDefinedBy scor: ;
    vs:term_status "stable" ;
    dct:modified "2015-11-05"^^xsd:date ;
 .

scor:CarcassDisassembly
    rdf:type scor:EmergingPractice ;
    rdfs:comment "Returned Maintenance, Repair, Operations (MRO) items are disassembled to the bill of material level and component parts are tested."@en ;
    rdfs:label "Carcass Disassembly"@en ;
    skos:notation "BP.137"@en ;
    rdfs:isDefinedBy scor: ;
    vs:term_status "stable" ;
    dct:modified "2015-11-05"^^xsd:date ;
 .

scor:BarCodingRFID
    rdf:type scor:EmergingPractice ;
    rdfs:comment "Bar coding is the practice of adding machine readable labels to packaging of goods, in order to increase reading speed and reducing reading errors."@en  ;
    rdfs:label "Bar Coding RFID"@en ;
    skos:notation "BP.153"@en  ;
    rdfs:isDefinedBy scor: ;
    vs:term_status "stable" ;
    dct:modified "2015-11-05"^^xsd:date ;
 .

scor:EnterpriseLevelSpendAnalysis
    rdf:type scor:EmergingPractice ;
    rdfs:comment "Spend analysis involved collection of data across procures to pay process in an enterprise and slicing and dicing these data into useful information."@en  ;
    rdfs:label "Enterprise Level Spend Analysis"@en ;
    skos:notation "BP.161"@en  ;
    rdfs:isDefinedBy scor: ;
    vs:term_status "stable" ;
    dct:modified "2015-11-05"^^xsd:date ;
 .

scor:LongTermSupplierAgreementPartnership
    rdf:type scor:EmergingPractice ;
    rdfs:comment "The Long Term Supplier Agreement/Partnership is a communication framework of buyer and supplier relationship."@en  ;
    rdfs:label "Long Term Supplier Agreement Partnership"@en ;
    skos:notation "BP.162"@en  ;
    rdfs:isDefinedBy scor: ;
    vs:term_status "stable" ;
    dct:modified "2015-11-05"^^xsd:date ;
 .

scor:MixedModeReverseMaterialIssue
    rdf:type scor:EmergingPractice ;
    rdfs:comment "Backflush is a concept where issuing of the material automatically happens once the finished product is ready."@en  ;
    rdfs:label "Mixed Mode Reverse Material Issue"@en ;
    skos:notation "BP.171"@en  ;
    rdfs:isDefinedBy scor: ;
    vs:term_status "stable" ;
    dct:modified "2015-11-05"^^xsd:date ;
 .

scor:ProductionSchedulingOptimizationUsingTech
    rdf:type scor:EmergingPractice ;
    rdfs:comment "Effective scheduling should not only include production related attributes (e.g. rated/demonstrated capacity asset loading sequencing changeover constraints etc.) but also other directly and indirectly related processes."@en  ;
    rdfs:label "Production Scheduling Optimization Using Tech"@en ;
    skos:notation "BP.172"@en  ;
    rdfs:isDefinedBy scor: ;
    vs:term_status "stable" ;
    dct:modified "2015-11-05"^^xsd:date ;
 .


# Best Practices individuals

scor:SCRiskManagement
    rdf:type scor:BestPractice ;
    rdfs:comment "the systematic identification, assessment and mitigation of potential disruptions in logistics networks"@en  ;
    rdfs:label "Supply Chain Risk Management"@en  ;
    skos:notation "BP.001"@en  ;
    rdfs:isDefinedBy scor: ;
    vs:term_status "stable" ;
    dct:modified "2015-11-05"^^xsd:date ;
 .

scor:RiskManagementStrategies
    rdf:type scor:BestPractice ;
    rdfs:comment "Risk management strategies are developed and communicated. Commonly used strategies are Risk Mitigation, Risk Avoidance, Risk Transfer and also Risk Acceptance"@en  ;
    rdfs:label "Risk Management Strategies"@en  ;
    skos:notation "BP.002"@en  ;
    rdfs:isDefinedBy scor: ;
    vs:term_status "stable" ;
    dct:modified "2015-11-05"^^xsd:date ;
 .

scor:SingleMinuteExchangeOfDie
    rdf:type scor:BestPractice ;
    rdfs:comment "The practice of reducing the time it takes to change a production line, equipment or machine from running one product to the next"@en  ;
    rdfs:label "Single-Minute Exchange of Die (SMED)"@en  ;
    skos:notation "BP.003"@en  ;
    rdfs:isDefinedBy scor: ;
    vs:term_status "stable" ;
    dct:modified "2015-11-05"^^xsd:date ;
 .

scor:NetworkPrioritizationForRiskIdentification
    rdf:type scor:BestPractice ;
    rdfs:comment "Network prioritization for risk identification is the process of prioritizing parts of a supply chain for risk analysis based on the overall risk potential in each portion of the supply chain"@en  ;
    rdfs:label "Network Prioritization for Risk Identification"@en  ;
    skos:notation "BP.004"@en  ;
    rdfs:isDefinedBy scor: ;
    vs:term_status "stable" ;
    dct:modified "2015-11-05"^^xsd:date ;
 .

scor:SelfInvoicing
    rdf:type scor:BestPractice ;
    rdfs:comment "The practice where a customer generates the invoices for the products or services it consumed from a supplier"@en  ;
    rdfs:label "Self-Invoicing"@en  ;
    skos:notation "BP.005"@en  ;
    rdfs:isDefinedBy scor: ;
    vs:term_status "stable" ;
    dct:modified "2015-11-05"^^xsd:date ;
 .

scor:BaselineInventoryMonitoring
    rdf:type scor:BestPractice ;
    rdfs:comment "To avoid overstock situations, we regularly review Baseline inventory levels. Baseline inventory is defined as the lowest stock level that a particular SKU actually had during the last 12 months."@en  ;
    rdfs:label "Baseline Inventory Monitoring"@en  ;
    skos:notation "BP.007"@en  ;
    rdfs:isDefinedBy scor: ;
    vs:term_status "stable" ;
    dct:modified "2015-11-05"^^xsd:date ;
 .

scor:ProductionLineSequencing
    rdf:type scor:BestPractice ;
    rdfs:comment "The practice where materials are ordered, shipped, received and/or staged in the same sequence as they will be consumed."@en  ;
    rdfs:label "Production Line Sequencing"@en  ;
    skos:notation "BP.011"@en  ;
    rdfs:isDefinedBy scor: ;
    vs:term_status "stable" ;
    dct:modified "2015-11-05"^^xsd:date ;
 .

scor:PullBasedInventoryReplenishment
    rdf:type scor:BestPractice ;
    rdfs:comment "Pull-based (Demand) replenishment is an approach that utilizes customer demand (`pull`) to replace and optimize inventory while reducing total net landed cost."@en  ;
    rdfs:label "Pull-Based Inventory Replenishment"@en  ;
    skos:notation "BP.027"@en  ;
    rdfs:isDefinedBy scor: ;
    vs:term_status "stable" ;
    dct:modified "2015-11-05"^^xsd:date ;
 .

scor:InventoryOptimization
    rdf:type scor:BestPractice ;
    rdfs:comment "Use of multi-echelon (simultaneous across all inventory stocking points in supply chain) stochastic (random variability) optimization."@en  ;
    rdfs:label "Inventory Optimization"@en  ;
    skos:notation "BP.028"@en  ;
    rdfs:isDefinedBy scor: ;
    vs:term_status "stable" ;
    dct:modified "2015-11-05"^^xsd:date ;
 .

scor:InventoryManagementBP029
    rdf:type scor:BestPractice ;
    rdfs:comment "Supply chains and supply networks both describe the flow and movement of materials & information, by linking organizations together to serve the end-customer."@en  ;
    rdfs:label "Inventory Management Using Supply Chain Network Optimization"@en  ;
    skos:notation "BP.029"@en  ;
    rdfs:isDefinedBy scor: ;
    vs:term_status "stable" ;
    dct:modified "2015-11-05"^^xsd:date ;
 .

scor:InventoryRecordAccuracy
    rdf:type scor:BestPractice ;
    rdfs:comment "Establish disciplined monthly process to ensure timely reporting of accurate inventory (physical inventory matches ERP inventory & identify sitting inventory not identified by a SKU) at the manufacturing and terminal locations."@en  ;
    rdfs:label "Inventory Record Accuracy"@en  ;
    skos:notation "BP.030"@en  ;
    rdfs:isDefinedBy scor: ;
    vs:term_status "stable" ;
    dct:modified "2015-11-05"^^xsd:date ;
 .

scor:ReduceSlowMovingInventory
    rdf:type scor:BestPractice ;
    rdfs:comment "Analyze and determine what inventory can be written off due to age, shelf-life, and/or lack of demand."@en  ;
    rdfs:label "Reduce / Write-off Slow Moving Inventory"@en  ;
    skos:notation "BP.032"@en  ;
    rdfs:isDefinedBy scor: ;
    vs:term_status "stable" ;
    dct:modified "2015-11-05"^^xsd:date ;
 .

scor:TraditionalDemandForecastingImprovement
    rdf:type scor:BestPractice ;
    rdfs:comment "Use of more sophisticated qualitative and quantitative forecasting processes and tools to improve customer demand forecast typically at SKU level."@en  ;
    rdfs:label "Traditional Demand Forecasting Improvement"@en  ;
    skos:notation "BP.033"@en  ;
    rdfs:isDefinedBy scor: ;
    vs:term_status "stable" ;
    dct:modified "2015-11-05"^^xsd:date ;
 .

scor:ExtendInventoryBP34
    rdf:type scor:BestPractice ;
    rdfs:comment "Collaborative inventory planning can be used as a way to extend supply chain planning with key customers."@en  ;
    rdfs:label "Extend Inventory Planning using Collaboration (Key Suppliers)"@en  ;
    skos:notation "BP.034"@en  ;
    rdfs:isDefinedBy scor: ;
    vs:term_status "stable" ;
    dct:modified "2015-11-05"^^xsd:date ;
 .

scor:ConsignmentInventoryWithSuppliers
    rdf:type scor:BestPractice ;
    rdfs:comment "Consignment inventory is a family of business models in which the buyer of a product provides certain information to a supplier of that product and the supplier takes full responsibility for maintaining an agreed of the material, usually at the buyer's consumption location (usually a store)."@en  ;
    rdfs:label "Consignment Inventory with Key Suppliers"@en  ;
    skos:notation "BP.036"@en  ;
    rdfs:isDefinedBy scor: ;
    vs:term_status "stable" ;
    dct:modified "2015-11-05"^^xsd:date ;
 .

scor:ManufacturingDirectDropShipment
    rdf:type scor:BestPractice ;
    rdfs:comment "The practice of shipping products and goods directly from the manufacturing plant to the customer (bypassing consolidation activities in warehouses and/or distribution centers)."@en  ;
    rdfs:label "Manufacturing Direct/Drop Shipment"@en  ;
    skos:notation "BP.037"@en  ;
    rdfs:isDefinedBy scor: ;
    vs:term_status "stable" ;
    dct:modified "2015-11-05"^^xsd:date ;
 .

scor:BatchSizeReduction
    rdf:type scor:BestPractice ;
    rdfs:comment "Use Lean principles to reduce size of manufacturing batch sizes to better match customer demand vs. asset utilization/quality issues."@en  ;
    rdfs:label "Batch Size Reduction"@en  ;
    skos:notation "BP.038"@en  ;
    rdfs:isDefinedBy scor: ;
    vs:term_status "stable" ;
    dct:modified "2015-11-05"^^xsd:date ;
 .

scor:RightSizeFrequencyOfProductionWheel
    rdf:type scor:BestPractice ;
    rdfs:comment "Use Lean principles to increase frequency/agility of production wheel, or production cycle in order to modify production planning and right-size finished goods and work-in-process inventory."@en  ;
    rdfs:label "Right Size Frequency of Production Wheel"@en  ;
    skos:notation "BP.039"@en  ;
    rdfs:isDefinedBy scor: ;
    vs:term_status "stable" ;
    dct:modified "2015-11-05"^^xsd:date ;
 .

scor:MTOOrderFulfillmentStrategy
    rdf:type scor:BestPractice ;
    rdfs:comment "Evaluate potential to change order fulfillment strategy from Make-To-Stock (MTS) to Make-To-Order (MTO) SKU by SKU to offset need to carry inventory due to infrequent demand or low demand."@en  ;
    rdfs:label "MTO Order Fulfillment Strategy"@en  ;
    skos:notation "BP.040"@en  ;
    rdfs:isDefinedBy scor: ;
    vs:term_status "stable" ;
    dct:modified "2015-11-05"^^xsd:date ;
 .

scor:TransportationOptimization
    rdf:type scor:BestPractice ;
    rdfs:comment "Evaluate potential to change inbound/outbound transportation mode to `faster` mode depending on freight terms (FOB, etc.) to accelerate transfer of inventory title to customer and/or better match demand/supply to optimize inventory balances."@en  ;
    rdfs:label "Transportation Optimization"@en  ;
    skos:notation "BP.041"@en  ;
    rdfs:isDefinedBy scor: ;
    vs:term_status "stable" ;
    dct:modified "2015-11-05"^^xsd:date ;
 .

scor:ReviewOfProcurementTermsConditions
    rdf:type scor:BestPractice ;
    rdfs:comment "Evaluate potential to change inbound/outbound transportation mode to `faster` mode depending on freight terms (FOB, etc.) to accelerate transfer of inventory title to customer and/or better match demand/supply to optimize inventory balances."@en  ;
    rdfs:label "Regular Review of Procurement Terms and Conditions"@en  ;
    skos:notation "BP.042"@en  ;
    rdfs:isDefinedBy scor: ;
    vs:term_status "stable" ;
    dct:modified "2015-11-05"^^xsd:date ;
 .

scor:ConsignmentInventoryReduction
    rdf:type scor:BestPractice ;
    rdfs:comment "Analyze potential to reduce consignment inventory commitments. These are typically included as part of the terms and conditions of customer contracts."@en  ;
    rdfs:label "Consignment Inventory Reduction"@en  ;
    skos:notation "BP.043"@en  ;
    rdfs:isDefinedBy scor: ;
    vs:term_status "stable" ;
    dct:modified "2015-11-05"^^xsd:date ;
 .

scor:InventoryFinancingEvaluation
    rdf:type scor:BestPractice ;
    rdfs:comment "Evaluate potential to use external finance company to `purchase inventory` while in-transit or in certain circumstances and sell back to the company prior to delivery to customer."@en  ;
    rdfs:label "Inventory Financing Evaluation"@en  ;
    skos:notation "BP.044"@en  ;
    rdfs:isDefinedBy scor: ;
    vs:term_status "stable" ;
    dct:modified "2015-11-05"^^xsd:date ;
 .

scor:FinishedGoodsInventoryPostponement
    rdf:type scor:BestPractice ;
    rdfs:comment "Provide process to determine and execute optimum placement and volume for Inventory in the Value Stream (Chain). Requires analysis of Value Stream and identification of opportunities for Demand Pooling of materials."@en  ;
    rdfs:label "Finished Goods Inventory Postponement"@en  ;
    skos:notation "BP.047"@en  ;
    rdfs:isDefinedBy scor: ;
    vs:term_status "stable" ;
    dct:modified "2015-11-05"^^xsd:date ;
 .

scor:InventoryIncentives
    rdf:type scor:BestPractice ;
    rdfs:comment "Balance cost/value of offering discounts for customers to move forward orders on specific finished good products in inventory."@en  ;
    rdfs:label "Inventory incentives / promotions for customers"@en  ;
    skos:notation "BP.048"@en  ;
    rdfs:isDefinedBy scor: ;
    vs:term_status "stable" ;
    dct:modified "2015-11-05"^^xsd:date ;
 .

scor:CustomerIncentives
    rdf:type scor:BestPractice ;
    rdfs:comment "Provide a one time improvement in finished good inventory; Requires analysis of value/cost trade-off to insure proper incentive."@en  ;
    rdfs:label "Customer Incentives/Promotions for Large Inventory Purchases"@en  ;
    skos:notation "BP.050"@en  ;
    rdfs:isDefinedBy scor: ;
    vs:term_status "stable" ;
    dct:modified "2015-11-05"^^xsd:date ;
 .

scor:EmbedInventoryManagementGoals
    rdf:type scor:BestPractice ;
    rdfs:comment "Develop method to embed and track specific inventory management goals for the business for all functions within the business due to cross-functional issues associated with inventory vs. service level."@en  ;
    rdfs:label "Embed Inventory Management Goals"@en  ;
    skos:notation "BP.051"@en  ;
    rdfs:isDefinedBy scor: ;
    vs:term_status "stable" ;
    dct:modified "2015-11-05"^^xsd:date ;
 .

scor:DesignForLogisticsManagement
    rdf:type scor:BestPractice ;
    rdfs:comment "Change new product development process to embed reuse and/or risk assessment around inventory management (e.g., include check off from supply chain of potential inventory management impact of proposed new product development). This could include mandatory end of lifecycle for another product, Commercial`s agreement to potential inventory/working capital exposure, etc."@en  ;
    rdfs:label "Design for Logistics (DFL) Management"@en  ;
    skos:notation "BP.052"@en  ;
    rdfs:isDefinedBy scor: ;
    vs:term_status "stable" ;
    dct:modified "2015-11-05"^^xsd:date ;
 .

scor:ManufacturingReliabilityImprovement
    rdf:type scor:BestPractice ;
    rdfs:comment "The practice includes use of reliability tools and implementation of work process roles within manufacturing to address manufacturing reliability."@en  ;
    rdfs:label "Manufacturing Reliability Improvement"@en  ;
    skos:notation "BP.053"@en  ;
    rdfs:isDefinedBy scor: ;
    vs:term_status "stable" ;
    dct:modified "2015-11-05"^^xsd:date ;
 .

scor:ManufacturingQualityImprovementsBP054
    rdf:type scor:BestPractice ;
    rdfs:comment "This consists of efforts to address manufacturing quality & improving manufacturing cost/capacity and service factor."@en  ;
    rdfs:label "Manufacturing Quality Improvements for Return Reduction"@en  ;
    skos:notation "BP.054"@en  ;
    rdfs:isDefinedBy scor: ;
    vs:term_status "stable" ;
    dct:modified "2015-11-05"^^xsd:date ;
 .

scor:FreightCarrierDeliveryBP55
    rdf:type scor:BestPractice ;
    rdfs:comment "The practice of formal freight carrier performance reviews to reduce the risk of landed cost budget variances."@en  ;
    rdfs:label "Freight Carrier Delivery Performance Evaluation"@en  ;
    skos:notation "BP.055"@en  ;
    rdfs:isDefinedBy scor: ;
    vs:term_status "stable" ;
    dct:modified "2015-11-05"^^xsd:date ;
 .

scor:SupplierRawMaterialBP56
    rdf:type scor:BestPractice ;
    rdfs:comment "Provide analysis of potential value that could be gained from raw material inventory reduction (in addition to traditional manufacturing quality/capacity and service factors)."@en  ;
    rdfs:label "Supplier Raw Material Quality Improvement"@en  ;
    skos:notation "BP.056"@en  ;
    rdfs:isDefinedBy scor: ;
    vs:term_status "stable" ;
    dct:modified "2015-11-05"^^xsd:date ;
 .

scor:InventoryManagementTraining
    rdf:type scor:BestPractice ;
    rdfs:comment "Develop a training curriculum and monitor key employee participation/completion in the areas of inventory management (particularly with schedulers, planners, SC managers) as well as exposure to  emerging best practices/technology (e.g., inventory optimization.)."@en  ;
    rdfs:label "Inventory Management Training"@en  ;
    skos:notation "BP.058"@en  ;
    rdfs:isDefinedBy scor: ;
    vs:term_status "stable" ;
    dct:modified "2015-11-05"^^xsd:date ;
 .

scor:EmployeeIncentivesInventoryBP59
    rdf:type scor:BestPractice ;
    rdfs:comment "Effective inventory management is the result of outstanding inventory control and inventory management."@en  ;
    rdfs:label "Employee Incentives for Effective Inventory Management"@en  ;
    skos:notation "BP.059"@en  ;
    rdfs:isDefinedBy scor: ;
    vs:term_status "stable" ;
    dct:modified "2015-11-05"^^xsd:date ;
 .

scor:OrderLeadTimeCorrectiveAction
    rdf:type scor:BestPractice ;
    rdfs:comment "Attaining acceptable delivery performance is the most significant manufacturing challenge faced by many organizations."@en  ;
    rdfs:label "Order Lead Time Corrective Action"@en  ;
    skos:notation "BP.060"@en  ;
    rdfs:isDefinedBy scor: ;
    vs:term_status "stable" ;
    dct:modified "2015-11-05"^^xsd:date ;
 .

scor:ReduceNonStrategicInventoryLevel
    rdf:type scor:BestPractice ;
    rdfs:comment "Unsold inventory is not `money in the bank`. A company should identify idle assets by analyzing production records, reviewing stock status reports to isolate inventory that is slow moving or out of balance, and sell/reduce the nonstrategic inventory."@en  ;
    rdfs:label "Reduce Non-Strategic Inventory Level"@en  ;
    skos:notation "BP.061"@en  ;
    rdfs:isDefinedBy scor: ;
    vs:term_status "stable" ;
    dct:modified "2015-11-05"^^xsd:date ;
 .

scor:MasterDataAccuracy
    rdf:type scor:BestPractice ;
    rdfs:comment "Re-validate existing Master Data (order lead times, replenishment times, transit times, etc.) to ensure it matches current operational capabilities and performance."@en  ;
    rdfs:label "Master Data Accuracy"@en  ;
    skos:notation "BP.061"@en  ;
    rdfs:isDefinedBy scor: ;
    vs:term_status "stable" ;
    dct:modified "2015-11-05"^^xsd:date ;
 .

scor:OptimizeSourcingDecisionsBP63
    rdf:type scor:BestPractice ;
    rdfs:comment "Assess potential to change sourcing decisions to local source point (likely the optimal source point) to reduce overall replenishment lead time."@en  ;
    rdfs:label "Optimize Sourcing Decisions to Local Source Point"@en  ;
    skos:notation "BP.063"@en  ;
    rdfs:isDefinedBy scor: ;
    vs:term_status "stable" ;
    dct:modified "2015-11-05"^^xsd:date ;
 .

scor:SafetyStockReduction
    rdf:type scor:BestPractice ;
    rdfs:comment "Pursue a more aggressive Reorder Point / safety stock target replenishment stance that places more risk on the chance of a stock out."@en  ;
    rdfs:label "Safety Stock Reduction"@en  ;
    skos:notation "BP.064"@en  ;
    rdfs:isDefinedBy scor: ;
    vs:term_status "stable" ;
    dct:modified "2015-11-05"^^xsd:date ;
 .

scor:SeasonalPackagingChange
    rdf:type scor:BestPractice ;
    rdfs:comment "What constitutes seasonal varies from organization to organization. From a requirements determination perspective however seasonal items may be classified as items that have less than six months of demand in the preceding 12 months."@en  ;
    rdfs:label "Seasonal Packaging Reduction/Removal"@en  ;
    skos:notation "BP.065"@en  ;
    rdfs:isDefinedBy scor: ;
    vs:term_status "stable" ;
    dct:modified "2015-11-05"^^xsd:date ;
 .

scor:ReduceReturnsInventoryBP66
    rdf:type scor:BestPractice ;
    rdfs:comment "Evaluate and establish a business returns policy (buyer`s remorse, defectives, warranty, overstock, Root Cause Investigation to determine & eliminate return cause, etc.) including determining its impact to overall inventory management."@en  ;
    rdfs:label "Returns Policy to Reduce Returns Inventory"@en  ;
    skos:notation "BP.066"@en  ;
    rdfs:isDefinedBy scor: ;
    vs:term_status "stable" ;
    dct:modified "2015-11-05"^^xsd:date ;
 .

scor:ReturnsInventoryReduction
    rdf:type scor:BestPractice ;
    rdfs:comment "Develop a process for efficiently receiving, processing and disposition of returned products."@en  ;
    rdfs:label "Returns Inventory Reduction"@en  ;
    skos:notation "BP.067"@en  ;
    rdfs:isDefinedBy scor: ;
    vs:term_status "stable" ;
    dct:modified "2015-11-05"^^xsd:date ;
 .

scor:SupplierDeliveryPerformanceAnalysis
    rdf:type scor:BestPractice ;
    rdfs:comment "Track and analyze the on time delivery performance for suppliers.."@en  ;
    rdfs:label "Supplier Delivery Performance Analysis"@en  ;
    skos:notation "BP.068"@en  ;
    rdfs:isDefinedBy scor: ;
    vs:term_status "stable" ;
    dct:modified "2015-11-05"^^xsd:date ;
 .

scor:RawMaterialsReceivingProcess
    rdf:type scor:BestPractice ;
    rdfs:comment "Develop process for efficiently receiving and processing raw materials from suppliers to minimize receipt of raw materials."@en  ;
    rdfs:label "Raw Materials Receiving Process"@en  ;
    skos:notation "BP.069"@en  ;
    rdfs:isDefinedBy scor: ;
    vs:term_status "stable" ;
    dct:modified "2015-11-05"^^xsd:date ;
 .

scor:PlanningInventoryTraining
    rdf:type scor:BestPractice ;
    rdfs:comment "Improve employee knowledge of inventory control to increase level of performance in inventory management."@en  ;
    rdfs:label "Planning/scheduling inventory training"@en  ;
    skos:notation "BP.070"@en  ;
    rdfs:isDefinedBy scor: ;
    vs:term_status "stable" ;
    dct:modified "2015-11-05"^^xsd:date ;
 .

scor:CostsInventoryStockingBP71
    rdf:type scor:BestPractice ;
    rdfs:comment "Balance the trade-off between logistics cost reduction and increased capital costs."@en  ;
    rdfs:label "Freight Costs and Inventory Stocking Optimization"@en  ;
    skos:notation "BP.071"@en  ;
    rdfs:isDefinedBy scor: ;
    vs:term_status "stable" ;
    dct:modified "2015-11-05"^^xsd:date ;
 .

scor:InboundRMAEnabledProcessing
    rdf:type scor:BestPractice ;
    rdfs:comment "This practice of requiring and enforcing a return shipment is accompanied by a company-issued Return Material (or Merchandise) Authorization (or Agreement) (RMA)."@en  ;
    rdfs:label "Inbound RMA-enabled Processing"@en  ;
    skos:notation "BP.072"@en  ;
    rdfs:isDefinedBy scor: ;
    vs:term_status "stable" ;
    dct:modified "2015-11-05"^^xsd:date ;
 .

scor:ProcessMetricsAlignment
    rdf:type scor:BestPractice ;
    rdfs:comment "Metric alignment refers to the organized and deliberate development of metrics across an organization. The process starts with organizational/business or supply chain metrics then decomposes to organizational processes at level-2, level-3, and further if desired."@en  ;
    rdfs:label "Process/Metrics Alignment"@en  ;
    skos:notation "BP.074"@en  ;
    rdfs:isDefinedBy scor: ;
    vs:term_status "stable" ;
    dct:modified "2015-11-05"^^xsd:date ;
 .

